<?xml version="1.0"?>
<rdf:RDF xmlns="http://www.semanticweb.org/cadex/ontologies/2020/1/untitled-ontology-71#"
     xml:base="http://www.semanticweb.org/cadex/ontologies/2020/1/untitled-ontology-71"
     xmlns:dc="http://purl.org/dc/elements/1.1/"
     xmlns:ns="http://creativecommons.org/ns#"
     xmlns:owl="http://www.w3.org/2002/07/owl#"
     xmlns:rdf="http://www.w3.org/1999/02/22-rdf-syntax-ns#"
     xmlns:xml="http://www.w3.org/XML/1998/namespace"
     xmlns:xsd="http://www.w3.org/2001/XMLSchema#"
     xmlns:rdfs="http://www.w3.org/2000/01/rdf-schema#"
     xmlns:untitled-ontology-71="http://www.semanticweb.org/cadex/ontologies/2020/1/untitled-ontology-71#">
    <owl:Ontology rdf:about="http://www.semanticweb.org/cadex/ontologies/2020/1/untitled-ontology-71">
        <ns:license>MIT</ns:license>
        <dc:title>The Creative Data Ontology</dc:title>
        <owl:versionInfo>5.4.23</owl:versionInfo>
    </owl:Ontology>
    


    <!-- 
    ///////////////////////////////////////////////////////////////////////////////////////
    //
    // Annotation properties
    //
    ///////////////////////////////////////////////////////////////////////////////////////
     -->

    


    <!-- http://creativecommons.org/ns#license -->

    <owl:AnnotationProperty rdf:about="http://creativecommons.org/ns#license"/>
    


    <!-- http://purl.org/dc/elements/1.1/title -->

    <owl:AnnotationProperty rdf:about="http://purl.org/dc/elements/1.1/title"/>
    


    <!-- 
    ///////////////////////////////////////////////////////////////////////////////////////
    //
    // Object Properties
    //
    ///////////////////////////////////////////////////////////////////////////////////////
     -->

    


    <!-- http://www.semanticweb.org/cadex/ontologies/2020/1/untitled-ontology-71#becomes -->

    <owl:ObjectProperty rdf:about="http://www.semanticweb.org/cadex/ontologies/2020/1/untitled-ontology-71#becomes">
        <rdfs:comment>This property groups sub-properties that represent a transformation from one type of entity to another.</rdfs:comment>
    </owl:ObjectProperty>
    


    <!-- http://www.semanticweb.org/cadex/ontologies/2020/1/untitled-ontology-71#becomesFile -->

    <owl:ObjectProperty rdf:about="http://www.semanticweb.org/cadex/ontologies/2020/1/untitled-ontology-71#becomesFile">
        <rdfs:subPropertyOf rdf:resource="http://www.semanticweb.org/cadex/ontologies/2020/1/untitled-ontology-71#becomes"/>
        <rdfs:domain rdf:resource="http://www.semanticweb.org/cadex/ontologies/2020/1/untitled-ontology-71#Asset"/>
        <rdfs:range rdf:resource="http://www.semanticweb.org/cadex/ontologies/2020/1/untitled-ontology-71#File"/>
        <rdfs:comment>This property encapsulates all the sub-properties that represents a transformation from a conceptual entity to a file on a computer.</rdfs:comment>
    </owl:ObjectProperty>
    


    <!-- http://www.semanticweb.org/cadex/ontologies/2020/1/untitled-ontology-71#by -->

    <owl:ObjectProperty rdf:about="http://www.semanticweb.org/cadex/ontologies/2020/1/untitled-ontology-71#by">
        <rdfs:comment>This property encapsulates all the sub-properties that describe how an entity has been interacted with by an instance of the Person class.</rdfs:comment>
    </owl:ObjectProperty>
    


    <!-- http://www.semanticweb.org/cadex/ontologies/2020/1/untitled-ontology-71#cameraIsPartOfRig -->

    <owl:ObjectProperty rdf:about="http://www.semanticweb.org/cadex/ontologies/2020/1/untitled-ontology-71#cameraIsPartOfRig">
        <rdfs:subPropertyOf rdf:resource="http://www.semanticweb.org/cadex/ontologies/2020/1/untitled-ontology-71#isPartOf"/>
        <rdfs:domain rdf:resource="http://www.semanticweb.org/cadex/ontologies/2020/1/untitled-ontology-71#Camera"/>
        <rdfs:range rdf:resource="http://www.semanticweb.org/cadex/ontologies/2020/1/untitled-ontology-71#Rig"/>
        <rdfs:comment>This property creates link from a camera which forms a part of or is involved in a rig.</rdfs:comment>
    </owl:ObjectProperty>
    


    <!-- http://www.semanticweb.org/cadex/ontologies/2020/1/untitled-ontology-71#cameraProducesCameraRoll -->

    <owl:ObjectProperty rdf:about="http://www.semanticweb.org/cadex/ontologies/2020/1/untitled-ontology-71#cameraProducesCameraRoll">
        <rdfs:subPropertyOf rdf:resource="http://www.semanticweb.org/cadex/ontologies/2020/1/untitled-ontology-71#produces"/>
        <owl:inverseOf rdf:resource="http://www.semanticweb.org/cadex/ontologies/2020/1/untitled-ontology-71#cameraRollIsFromCamera"/>
        <rdfs:domain rdf:resource="http://www.semanticweb.org/cadex/ontologies/2020/1/untitled-ontology-71#Camera"/>
        <rdfs:range rdf:resource="http://www.semanticweb.org/cadex/ontologies/2020/1/untitled-ontology-71#CameraRoll"/>
        <rdfs:comment>This property is a sub-property of produces and creates a relationship between a camera and the video roll that it creates.</rdfs:comment>
    </owl:ObjectProperty>
    


    <!-- http://www.semanticweb.org/cadex/ontologies/2020/1/untitled-ontology-71#cameraProducesSoundRoll -->

    <owl:ObjectProperty rdf:about="http://www.semanticweb.org/cadex/ontologies/2020/1/untitled-ontology-71#cameraProducesSoundRoll">
        <rdfs:subPropertyOf rdf:resource="http://www.semanticweb.org/cadex/ontologies/2020/1/untitled-ontology-71#produces"/>
        <rdfs:domain rdf:resource="http://www.semanticweb.org/cadex/ontologies/2020/1/untitled-ontology-71#Camera"/>
        <rdfs:range rdf:resource="http://www.semanticweb.org/cadex/ontologies/2020/1/untitled-ontology-71#SoundRoll"/>
        <rdfs:comment>This property is a sub-property of produces and creates a relationship between a camera and the audio roll that it creates.</rdfs:comment>
    </owl:ObjectProperty>
    


    <!-- http://www.semanticweb.org/cadex/ontologies/2020/1/untitled-ontology-71#cameraRollBecomesFolder -->

    <owl:ObjectProperty rdf:about="http://www.semanticweb.org/cadex/ontologies/2020/1/untitled-ontology-71#cameraRollBecomesFolder">
        <rdfs:subPropertyOf rdf:resource="http://www.semanticweb.org/cadex/ontologies/2020/1/untitled-ontology-71#becomes"/>
        <rdfs:domain rdf:resource="http://www.semanticweb.org/cadex/ontologies/2020/1/untitled-ontology-71#CameraRoll"/>
        <rdfs:range rdf:resource="http://www.semanticweb.org/cadex/ontologies/2020/1/untitled-ontology-71#Folder"/>
        <rdfs:comment>This property represents a transformation from an individual camera roll to a folder of files on a computer.</rdfs:comment>
    </owl:ObjectProperty>
    


    <!-- http://www.semanticweb.org/cadex/ontologies/2020/1/untitled-ontology-71#cameraRollContainsClip -->

    <owl:ObjectProperty rdf:about="http://www.semanticweb.org/cadex/ontologies/2020/1/untitled-ontology-71#cameraRollContainsClip">
        <rdfs:subPropertyOf rdf:resource="http://www.semanticweb.org/cadex/ontologies/2020/1/untitled-ontology-71#contains"/>
        <owl:inverseOf rdf:resource="http://www.semanticweb.org/cadex/ontologies/2020/1/untitled-ontology-71#clipIsFromCameraRoll"/>
        <rdfs:domain rdf:resource="http://www.semanticweb.org/cadex/ontologies/2020/1/untitled-ontology-71#CameraRoll"/>
        <rdfs:range rdf:resource="http://www.semanticweb.org/cadex/ontologies/2020/1/untitled-ontology-71#Clip"/>
        <rdfs:comment>This property creates a relationship between a roll and a clip to identify which roll a clip originated from.</rdfs:comment>
    </owl:ObjectProperty>
    


    <!-- http://www.semanticweb.org/cadex/ontologies/2020/1/untitled-ontology-71#cameraRollIsFromCamera -->

    <owl:ObjectProperty rdf:about="http://www.semanticweb.org/cadex/ontologies/2020/1/untitled-ontology-71#cameraRollIsFromCamera">
        <rdfs:subPropertyOf rdf:resource="http://www.semanticweb.org/cadex/ontologies/2020/1/untitled-ontology-71#isFrom"/>
        <rdfs:domain rdf:resource="http://www.semanticweb.org/cadex/ontologies/2020/1/untitled-ontology-71#CameraRoll"/>
        <rdfs:range rdf:resource="http://www.semanticweb.org/cadex/ontologies/2020/1/untitled-ontology-71#Camera"/>
        <rdfs:comment>This property creates link from a camera roll and the camera it originated from.</rdfs:comment>
    </owl:ObjectProperty>
    


    <!-- http://www.semanticweb.org/cadex/ontologies/2020/1/untitled-ontology-71#cameraUsesCrane -->

    <owl:ObjectProperty rdf:about="http://www.semanticweb.org/cadex/ontologies/2020/1/untitled-ontology-71#cameraUsesCrane">
        <rdfs:subPropertyOf rdf:resource="http://www.semanticweb.org/cadex/ontologies/2020/1/untitled-ontology-71#usesCrane"/>
        <rdfs:domain rdf:resource="http://www.semanticweb.org/cadex/ontologies/2020/1/untitled-ontology-71#Camera"/>
        <rdfs:range rdf:resource="http://www.semanticweb.org/cadex/ontologies/2020/1/untitled-ontology-71#Crane"/>
        <rdfs:comment>This property creates a relation between a crane and the camera that uses it.</rdfs:comment>
    </owl:ObjectProperty>
    


    <!-- http://www.semanticweb.org/cadex/ontologies/2020/1/untitled-ontology-71#cameraUsesLens -->

    <owl:ObjectProperty rdf:about="http://www.semanticweb.org/cadex/ontologies/2020/1/untitled-ontology-71#cameraUsesLens">
        <rdfs:subPropertyOf rdf:resource="http://www.semanticweb.org/cadex/ontologies/2020/1/untitled-ontology-71#usesLens"/>
        <rdfs:domain rdf:resource="http://www.semanticweb.org/cadex/ontologies/2020/1/untitled-ontology-71#Camera"/>
        <rdfs:range rdf:resource="http://www.semanticweb.org/cadex/ontologies/2020/1/untitled-ontology-71#Lens"/>
        <rdfs:comment>This property creates a relation between a lens and the camera that uses it.</rdfs:comment>
    </owl:ObjectProperty>
    


    <!-- http://www.semanticweb.org/cadex/ontologies/2020/1/untitled-ontology-71#castIsPartOfShoot -->

    <owl:ObjectProperty rdf:about="http://www.semanticweb.org/cadex/ontologies/2020/1/untitled-ontology-71#castIsPartOfShoot">
        <rdfs:subPropertyOf rdf:resource="http://www.semanticweb.org/cadex/ontologies/2020/1/untitled-ontology-71#isPartOf"/>
        <owl:inverseOf rdf:resource="http://www.semanticweb.org/cadex/ontologies/2020/1/untitled-ontology-71#shootUsesCast"/>
        <rdfs:domain rdf:resource="http://www.semanticweb.org/cadex/ontologies/2020/1/untitled-ontology-71#Cast"/>
        <rdfs:range rdf:resource="http://www.semanticweb.org/cadex/ontologies/2020/1/untitled-ontology-71#Shoot"/>
        <rdfs:comment>This property creates link from a cast member which forms a part of or is involved in a shoot.</rdfs:comment>
    </owl:ObjectProperty>
    


    <!-- http://www.semanticweb.org/cadex/ontologies/2020/1/untitled-ontology-71#castUsedIn -->

    <owl:ObjectProperty rdf:about="http://www.semanticweb.org/cadex/ontologies/2020/1/untitled-ontology-71#castUsedIn">
        <rdfs:subPropertyOf rdf:resource="http://www.semanticweb.org/cadex/ontologies/2020/1/untitled-ontology-71#usedIn"/>
        <rdfs:domain rdf:resource="http://www.semanticweb.org/cadex/ontologies/2020/1/untitled-ontology-71#Cast"/>
        <rdfs:comment>This property encapsulates all the sub-properties that describe the entity that a cast member is used in.</rdfs:comment>
    </owl:ObjectProperty>
    


    <!-- http://www.semanticweb.org/cadex/ontologies/2020/1/untitled-ontology-71#castUsedInProject -->

    <owl:ObjectProperty rdf:about="http://www.semanticweb.org/cadex/ontologies/2020/1/untitled-ontology-71#castUsedInProject">
        <rdfs:subPropertyOf rdf:resource="http://www.semanticweb.org/cadex/ontologies/2020/1/untitled-ontology-71#castUsedIn"/>
        <rdfs:domain rdf:resource="http://www.semanticweb.org/cadex/ontologies/2020/1/untitled-ontology-71#Cast"/>
        <rdfs:range rdf:resource="http://www.semanticweb.org/cadex/ontologies/2020/1/untitled-ontology-71#Project"/>
        <rdfs:comment>This property creates a link that describes a cast member is used in a project.</rdfs:comment>
    </owl:ObjectProperty>
    


    <!-- http://www.semanticweb.org/cadex/ontologies/2020/1/untitled-ontology-71#checkedBy -->

    <owl:ObjectProperty rdf:about="http://www.semanticweb.org/cadex/ontologies/2020/1/untitled-ontology-71#checkedBy">
        <rdfs:subPropertyOf rdf:resource="http://www.semanticweb.org/cadex/ontologies/2020/1/untitled-ontology-71#by"/>
        <rdfs:range rdf:resource="http://www.semanticweb.org/cadex/ontologies/2020/1/untitled-ontology-71#Staff"/>
        <rdfs:comment>This property encapsulates all the sub-properties that describe who an entity has been checked by.</rdfs:comment>
    </owl:ObjectProperty>
    


    <!-- http://www.semanticweb.org/cadex/ontologies/2020/1/untitled-ontology-71#clipHasFirstFrame -->

    <owl:ObjectProperty rdf:about="http://www.semanticweb.org/cadex/ontologies/2020/1/untitled-ontology-71#clipHasFirstFrame">
        <rdfs:subPropertyOf rdf:resource="http://www.semanticweb.org/cadex/ontologies/2020/1/untitled-ontology-71#hasFrame"/>
        <rdfs:domain rdf:resource="http://www.semanticweb.org/cadex/ontologies/2020/1/untitled-ontology-71#Clip"/>
        <rdfs:range rdf:resource="http://www.semanticweb.org/cadex/ontologies/2020/1/untitled-ontology-71#Frame"/>
        <rdfs:comment>This property creates link between a clip and its first frame.</rdfs:comment>
    </owl:ObjectProperty>
    


    <!-- http://www.semanticweb.org/cadex/ontologies/2020/1/untitled-ontology-71#clipHasIssue -->

    <owl:ObjectProperty rdf:about="http://www.semanticweb.org/cadex/ontologies/2020/1/untitled-ontology-71#clipHasIssue">
        <rdfs:subPropertyOf rdf:resource="http://www.semanticweb.org/cadex/ontologies/2020/1/untitled-ontology-71#hasIssue"/>
        <rdfs:domain rdf:resource="http://www.semanticweb.org/cadex/ontologies/2020/1/untitled-ontology-71#Clip"/>
        <rdfs:range rdf:resource="http://www.semanticweb.org/cadex/ontologies/2020/1/untitled-ontology-71#Issue"/>
        <rdfs:comment>This property creates link between a clip and its associated issue(s).</rdfs:comment>
    </owl:ObjectProperty>
    


    <!-- http://www.semanticweb.org/cadex/ontologies/2020/1/untitled-ontology-71#clipHasLastFrame -->

    <owl:ObjectProperty rdf:about="http://www.semanticweb.org/cadex/ontologies/2020/1/untitled-ontology-71#clipHasLastFrame">
        <rdfs:subPropertyOf rdf:resource="http://www.semanticweb.org/cadex/ontologies/2020/1/untitled-ontology-71#hasFrame"/>
        <rdfs:domain rdf:resource="http://www.semanticweb.org/cadex/ontologies/2020/1/untitled-ontology-71#Clip"/>
        <rdfs:range rdf:resource="http://www.semanticweb.org/cadex/ontologies/2020/1/untitled-ontology-71#Frame"/>
        <rdfs:comment>This property creates link between a clip and its last frame.</rdfs:comment>
    </owl:ObjectProperty>
    


    <!-- http://www.semanticweb.org/cadex/ontologies/2020/1/untitled-ontology-71#clipHasLoggingTag -->

    <owl:ObjectProperty rdf:about="http://www.semanticweb.org/cadex/ontologies/2020/1/untitled-ontology-71#clipHasLoggingTag">
        <rdfs:subPropertyOf rdf:resource="http://www.semanticweb.org/cadex/ontologies/2020/1/untitled-ontology-71#hasLoggingTag"/>
        <rdfs:domain rdf:resource="http://www.semanticweb.org/cadex/ontologies/2020/1/untitled-ontology-71#Clip"/>
        <rdfs:range rdf:resource="http://www.semanticweb.org/cadex/ontologies/2020/1/untitled-ontology-71#LoggingTag"/>
        <rdfs:comment>This property creates a relationship from clip to the logging tag(s) associated with it.</rdfs:comment>
    </owl:ObjectProperty>
    


    <!-- http://www.semanticweb.org/cadex/ontologies/2020/1/untitled-ontology-71#clipHasSoundRoll -->

    <owl:ObjectProperty rdf:about="http://www.semanticweb.org/cadex/ontologies/2020/1/untitled-ontology-71#clipHasSoundRoll">
        <rdfs:subPropertyOf rdf:resource="http://www.semanticweb.org/cadex/ontologies/2020/1/untitled-ontology-71#hasRoll"/>
        <rdfs:domain rdf:resource="http://www.semanticweb.org/cadex/ontologies/2020/1/untitled-ontology-71#Clip"/>
        <rdfs:range rdf:resource="http://www.semanticweb.org/cadex/ontologies/2020/1/untitled-ontology-71#SoundRoll"/>
        <rdfs:comment>This property creates link between a clip and its associated roll.</rdfs:comment>
    </owl:ObjectProperty>
    


    <!-- http://www.semanticweb.org/cadex/ontologies/2020/1/untitled-ontology-71#clipIsFromCameraRoll -->

    <owl:ObjectProperty rdf:about="http://www.semanticweb.org/cadex/ontologies/2020/1/untitled-ontology-71#clipIsFromCameraRoll">
        <rdfs:subPropertyOf rdf:resource="http://www.semanticweb.org/cadex/ontologies/2020/1/untitled-ontology-71#isFrom"/>
        <rdfs:domain rdf:resource="http://www.semanticweb.org/cadex/ontologies/2020/1/untitled-ontology-71#Clip"/>
        <rdfs:range rdf:resource="http://www.semanticweb.org/cadex/ontologies/2020/1/untitled-ontology-71#CameraRoll"/>
        <rdfs:comment>This property creates link from a clip and the camera roll it originated from.</rdfs:comment>
    </owl:ObjectProperty>
    


    <!-- http://www.semanticweb.org/cadex/ontologies/2020/1/untitled-ontology-71#clipIsFromTake -->

    <owl:ObjectProperty rdf:about="http://www.semanticweb.org/cadex/ontologies/2020/1/untitled-ontology-71#clipIsFromTake">
        <rdfs:subPropertyOf rdf:resource="http://www.semanticweb.org/cadex/ontologies/2020/1/untitled-ontology-71#isFrom"/>
        <rdfs:domain rdf:resource="http://www.semanticweb.org/cadex/ontologies/2020/1/untitled-ontology-71#Clip"/>
        <rdfs:range rdf:resource="http://www.semanticweb.org/cadex/ontologies/2020/1/untitled-ontology-71#Take"/>
        <rdfs:comment>This property creates link from a clip and the take it originated from.</rdfs:comment>
    </owl:ObjectProperty>
    


    <!-- http://www.semanticweb.org/cadex/ontologies/2020/1/untitled-ontology-71#clipUsesLUT -->

    <owl:ObjectProperty rdf:about="http://www.semanticweb.org/cadex/ontologies/2020/1/untitled-ontology-71#clipUsesLUT">
        <rdfs:subPropertyOf rdf:resource="http://www.semanticweb.org/cadex/ontologies/2020/1/untitled-ontology-71#usesLUT"/>
        <rdfs:domain rdf:resource="http://www.semanticweb.org/cadex/ontologies/2020/1/untitled-ontology-71#Clip"/>
        <rdfs:range rdf:resource="http://www.semanticweb.org/cadex/ontologies/2020/1/untitled-ontology-71#LUT"/>
        <rdfs:comment>This property creates a relation between a LUT and the clip that uses it.</rdfs:comment>
    </owl:ObjectProperty>
    


    <!-- http://www.semanticweb.org/cadex/ontologies/2020/1/untitled-ontology-71#clipUsesLens -->

    <owl:ObjectProperty rdf:about="http://www.semanticweb.org/cadex/ontologies/2020/1/untitled-ontology-71#clipUsesLens">
        <rdfs:subPropertyOf rdf:resource="http://www.semanticweb.org/cadex/ontologies/2020/1/untitled-ontology-71#usesLens"/>
        <owl:inverseOf rdf:resource="http://www.semanticweb.org/cadex/ontologies/2020/1/untitled-ontology-71#lensUsedInClip"/>
        <rdfs:domain rdf:resource="http://www.semanticweb.org/cadex/ontologies/2020/1/untitled-ontology-71#Clip"/>
        <rdfs:range rdf:resource="http://www.semanticweb.org/cadex/ontologies/2020/1/untitled-ontology-71#Lens"/>
        <rdfs:comment>This property creates a relation between a lens and the clip that uses it.</rdfs:comment>
    </owl:ObjectProperty>
    


    <!-- http://www.semanticweb.org/cadex/ontologies/2020/1/untitled-ontology-71#contains -->

    <owl:ObjectProperty rdf:about="http://www.semanticweb.org/cadex/ontologies/2020/1/untitled-ontology-71#contains">
        <rdfs:comment>This property creates a relationship between two entities whereby one is thought to be a container for another in the real world.</rdfs:comment>
    </owl:ObjectProperty>
    


    <!-- http://www.semanticweb.org/cadex/ontologies/2020/1/untitled-ontology-71#createdBy -->

    <owl:ObjectProperty rdf:about="http://www.semanticweb.org/cadex/ontologies/2020/1/untitled-ontology-71#createdBy">
        <rdfs:subPropertyOf rdf:resource="http://www.semanticweb.org/cadex/ontologies/2020/1/untitled-ontology-71#by"/>
        <rdfs:range rdf:resource="http://www.semanticweb.org/cadex/ontologies/2020/1/untitled-ontology-71#Staff"/>
        <rdfs:comment>This property encapsulates all the sub-properties that describe who an entity has been created by.</rdfs:comment>
    </owl:ObjectProperty>
    


    <!-- http://www.semanticweb.org/cadex/ontologies/2020/1/untitled-ontology-71#dataItemHasRecord -->

    <owl:ObjectProperty rdf:about="http://www.semanticweb.org/cadex/ontologies/2020/1/untitled-ontology-71#dataItemHasRecord">
        <rdfs:subPropertyOf rdf:resource="http://www.semanticweb.org/cadex/ontologies/2020/1/untitled-ontology-71#hasRecord"/>
        <rdfs:domain rdf:resource="http://www.semanticweb.org/cadex/ontologies/2020/1/untitled-ontology-71#DataItem"/>
        <rdfs:range rdf:resource="http://www.semanticweb.org/cadex/ontologies/2020/1/untitled-ontology-71#Record"/>
        <rdfs:comment>This property creates link between a data item and its record.</rdfs:comment>
    </owl:ObjectProperty>
    


    <!-- http://www.semanticweb.org/cadex/ontologies/2020/1/untitled-ontology-71#emailSentToClient -->

    <owl:ObjectProperty rdf:about="http://www.semanticweb.org/cadex/ontologies/2020/1/untitled-ontology-71#emailSentToClient">
        <rdfs:subPropertyOf rdf:resource="http://www.semanticweb.org/cadex/ontologies/2020/1/untitled-ontology-71#sentTo"/>
        <rdfs:domain rdf:resource="http://www.semanticweb.org/cadex/ontologies/2020/1/untitled-ontology-71#Email"/>
        <rdfs:range rdf:resource="http://www.semanticweb.org/cadex/ontologies/2020/1/untitled-ontology-71#Client"/>
        <rdfs:comment>This property represents a relationship between a client and an email sent to them, such as a receipt.</rdfs:comment>
    </owl:ObjectProperty>
    


    <!-- http://www.semanticweb.org/cadex/ontologies/2020/1/untitled-ontology-71#emailUsesHardDriveSnapshot -->

    <owl:ObjectProperty rdf:about="http://www.semanticweb.org/cadex/ontologies/2020/1/untitled-ontology-71#emailUsesHardDriveSnapshot">
        <rdfs:subPropertyOf rdf:resource="http://www.semanticweb.org/cadex/ontologies/2020/1/untitled-ontology-71#usesHardDriveSnapshot"/>
        <owl:inverseOf rdf:resource="http://www.semanticweb.org/cadex/ontologies/2020/1/untitled-ontology-71#hardDriveSnapshotIsPartOfEmail"/>
        <rdfs:domain rdf:resource="http://www.semanticweb.org/cadex/ontologies/2020/1/untitled-ontology-71#Email"/>
        <rdfs:range rdf:resource="http://www.semanticweb.org/cadex/ontologies/2020/1/untitled-ontology-71#HardDriveSnapshot"/>
        <rdfs:comment>This property creates link from an email to the hard drive snapshot attached to it.</rdfs:comment>
    </owl:ObjectProperty>
    


    <!-- http://www.semanticweb.org/cadex/ontologies/2020/1/untitled-ontology-71#equipmentHasAttachment -->

    <owl:ObjectProperty rdf:about="http://www.semanticweb.org/cadex/ontologies/2020/1/untitled-ontology-71#equipmentHasAttachment">
        <rdfs:subPropertyOf rdf:resource="http://www.semanticweb.org/cadex/ontologies/2020/1/untitled-ontology-71#hasEquipmentAttachment"/>
        <rdfs:domain rdf:resource="http://www.semanticweb.org/cadex/ontologies/2020/1/untitled-ontology-71#Equipment"/>
        <rdfs:range rdf:resource="http://www.semanticweb.org/cadex/ontologies/2020/1/untitled-ontology-71#EquipmentAttachment"/>
        <rdfs:comment>This property creates a relation between a piece of equipment and its attachments.</rdfs:comment>
    </owl:ObjectProperty>
    


    <!-- http://www.semanticweb.org/cadex/ontologies/2020/1/untitled-ontology-71#fixedBy -->

    <owl:ObjectProperty rdf:about="http://www.semanticweb.org/cadex/ontologies/2020/1/untitled-ontology-71#fixedBy">
        <rdfs:subPropertyOf rdf:resource="http://www.semanticweb.org/cadex/ontologies/2020/1/untitled-ontology-71#by"/>
        <rdfs:range rdf:resource="http://www.semanticweb.org/cadex/ontologies/2020/1/untitled-ontology-71#Staff"/>
        <rdfs:comment>This property encapsulates all the sub-properties that describe who an entity has been fixed by.</rdfs:comment>
    </owl:ObjectProperty>
    


    <!-- http://www.semanticweb.org/cadex/ontologies/2020/1/untitled-ontology-71#folderContainsFile -->

    <owl:ObjectProperty rdf:about="http://www.semanticweb.org/cadex/ontologies/2020/1/untitled-ontology-71#folderContainsFile">
        <rdfs:subPropertyOf rdf:resource="http://www.semanticweb.org/cadex/ontologies/2020/1/untitled-ontology-71#contains"/>
        <rdfs:domain rdf:resource="http://www.semanticweb.org/cadex/ontologies/2020/1/untitled-ontology-71#Folder"/>
        <rdfs:range rdf:resource="http://www.semanticweb.org/cadex/ontologies/2020/1/untitled-ontology-71#File"/>
        <rdfs:comment>This property creates a relationship between a file and a folder to identify where a file is stored on a computer.</rdfs:comment>
    </owl:ObjectProperty>
    


    <!-- http://www.semanticweb.org/cadex/ontologies/2020/1/untitled-ontology-71#frameIsPartOfClip -->

    <owl:ObjectProperty rdf:about="http://www.semanticweb.org/cadex/ontologies/2020/1/untitled-ontology-71#frameIsPartOfClip">
        <rdfs:subPropertyOf rdf:resource="http://www.semanticweb.org/cadex/ontologies/2020/1/untitled-ontology-71#isPartOf"/>
        <rdfs:domain rdf:resource="http://www.semanticweb.org/cadex/ontologies/2020/1/untitled-ontology-71#Frame"/>
        <rdfs:range rdf:resource="http://www.semanticweb.org/cadex/ontologies/2020/1/untitled-ontology-71#Clip"/>
        <rdfs:comment>This property creates link from a frame which forms a part of or is involved in a clip.</rdfs:comment>
    </owl:ObjectProperty>
    


    <!-- http://www.semanticweb.org/cadex/ontologies/2020/1/untitled-ontology-71#hardDriveSnapshotIsPartOfEmail -->

    <owl:ObjectProperty rdf:about="http://www.semanticweb.org/cadex/ontologies/2020/1/untitled-ontology-71#hardDriveSnapshotIsPartOfEmail">
        <rdfs:subPropertyOf rdf:resource="http://www.semanticweb.org/cadex/ontologies/2020/1/untitled-ontology-71#isPartOf"/>
        <rdfs:domain rdf:resource="http://www.semanticweb.org/cadex/ontologies/2020/1/untitled-ontology-71#HardDriveSnapshot"/>
        <rdfs:range rdf:resource="http://www.semanticweb.org/cadex/ontologies/2020/1/untitled-ontology-71#Email"/>
        <rdfs:comment>This property creates link from a hard drive snapshot to the email it is attached to.</rdfs:comment>
    </owl:ObjectProperty>
    


    <!-- http://www.semanticweb.org/cadex/ontologies/2020/1/untitled-ontology-71#hardDriveSnapshotSentToClient -->

    <owl:ObjectProperty rdf:about="http://www.semanticweb.org/cadex/ontologies/2020/1/untitled-ontology-71#hardDriveSnapshotSentToClient">
        <rdfs:subPropertyOf rdf:resource="http://www.semanticweb.org/cadex/ontologies/2020/1/untitled-ontology-71#sentTo"/>
        <rdfs:domain rdf:resource="http://www.semanticweb.org/cadex/ontologies/2020/1/untitled-ontology-71#HardDriveSnapshot"/>
        <rdfs:range rdf:resource="http://www.semanticweb.org/cadex/ontologies/2020/1/untitled-ontology-71#Client"/>
        <rdfs:comment>This property represents a relationship between a client and a hard drive snapshot sent to them as a receipt.</rdfs:comment>
    </owl:ObjectProperty>
    


    <!-- http://www.semanticweb.org/cadex/ontologies/2020/1/untitled-ontology-71#has -->

    <owl:ObjectProperty rdf:about="http://www.semanticweb.org/cadex/ontologies/2020/1/untitled-ontology-71#has">
        <rdfs:comment>This property encapsulates all the sub-properties that describe how an entity *owns* an instance of another class.</rdfs:comment>
    </owl:ObjectProperty>
    


    <!-- http://www.semanticweb.org/cadex/ontologies/2020/1/untitled-ontology-71#hasAsset -->

    <owl:ObjectProperty rdf:about="http://www.semanticweb.org/cadex/ontologies/2020/1/untitled-ontology-71#hasAsset">
        <rdfs:subPropertyOf rdf:resource="http://www.semanticweb.org/cadex/ontologies/2020/1/untitled-ontology-71#has"/>
        <rdfs:range rdf:resource="http://www.semanticweb.org/cadex/ontologies/2020/1/untitled-ontology-71#Asset"/>
        <rdfs:comment>This property encapsulates all the sub-properties that describe how an entity *owns* an asset.</rdfs:comment>
    </owl:ObjectProperty>
    


    <!-- http://www.semanticweb.org/cadex/ontologies/2020/1/untitled-ontology-71#hasClient -->

    <owl:ObjectProperty rdf:about="http://www.semanticweb.org/cadex/ontologies/2020/1/untitled-ontology-71#hasClient">
        <rdfs:subPropertyOf rdf:resource="http://www.semanticweb.org/cadex/ontologies/2020/1/untitled-ontology-71#has"/>
        <rdfs:range rdf:resource="http://www.semanticweb.org/cadex/ontologies/2020/1/untitled-ontology-71#Client"/>
        <rdfs:comment>This property encapsulates all the sub-properties that describe how an entity *owns* a client.</rdfs:comment>
    </owl:ObjectProperty>
    


    <!-- http://www.semanticweb.org/cadex/ontologies/2020/1/untitled-ontology-71#hasClipNote -->

    <owl:ObjectProperty rdf:about="http://www.semanticweb.org/cadex/ontologies/2020/1/untitled-ontology-71#hasClipNote">
        <rdfs:subPropertyOf rdf:resource="http://www.semanticweb.org/cadex/ontologies/2020/1/untitled-ontology-71#hasNote"/>
        <rdfs:domain rdf:resource="http://www.semanticweb.org/cadex/ontologies/2020/1/untitled-ontology-71#Clip"/>
        <rdfs:range rdf:resource="http://www.semanticweb.org/cadex/ontologies/2020/1/untitled-ontology-71#Note"/>
        <rdfs:comment>This property creates link between a clip and its associated note(s).</rdfs:comment>
    </owl:ObjectProperty>
    


    <!-- http://www.semanticweb.org/cadex/ontologies/2020/1/untitled-ontology-71#hasContactList -->

    <owl:ObjectProperty rdf:about="http://www.semanticweb.org/cadex/ontologies/2020/1/untitled-ontology-71#hasContactList">
        <rdfs:subPropertyOf rdf:resource="http://www.semanticweb.org/cadex/ontologies/2020/1/untitled-ontology-71#has"/>
        <rdfs:range rdf:resource="http://www.semanticweb.org/cadex/ontologies/2020/1/untitled-ontology-71#Staff"/>
        <rdfs:comment>This property encapsulates all the sub-properties that describe how an entity *owns* a contact list.</rdfs:comment>
    </owl:ObjectProperty>
    


    <!-- http://www.semanticweb.org/cadex/ontologies/2020/1/untitled-ontology-71#hasDeliverable -->

    <owl:ObjectProperty rdf:about="http://www.semanticweb.org/cadex/ontologies/2020/1/untitled-ontology-71#hasDeliverable">
        <rdfs:subPropertyOf rdf:resource="http://www.semanticweb.org/cadex/ontologies/2020/1/untitled-ontology-71#has"/>
        <rdfs:range rdf:resource="http://www.semanticweb.org/cadex/ontologies/2020/1/untitled-ontology-71#Deliverable"/>
        <rdfs:comment>This property encapsulates all the sub-properties that creates relationships from an entity to a deliverable associated with it</rdfs:comment>
    </owl:ObjectProperty>
    


    <!-- http://www.semanticweb.org/cadex/ontologies/2020/1/untitled-ontology-71#hasEquipment -->

    <owl:ObjectProperty rdf:about="http://www.semanticweb.org/cadex/ontologies/2020/1/untitled-ontology-71#hasEquipment">
        <rdfs:subPropertyOf rdf:resource="http://www.semanticweb.org/cadex/ontologies/2020/1/untitled-ontology-71#has"/>
        <rdfs:range rdf:resource="http://www.semanticweb.org/cadex/ontologies/2020/1/untitled-ontology-71#Equipment"/>
        <rdfs:comment>This property encapsulates all the sub-properties that describe how an entity has a piece of equipment.</rdfs:comment>
    </owl:ObjectProperty>
    


    <!-- http://www.semanticweb.org/cadex/ontologies/2020/1/untitled-ontology-71#hasEquipmentAttachment -->

    <owl:ObjectProperty rdf:about="http://www.semanticweb.org/cadex/ontologies/2020/1/untitled-ontology-71#hasEquipmentAttachment">
        <rdfs:subPropertyOf rdf:resource="http://www.semanticweb.org/cadex/ontologies/2020/1/untitled-ontology-71#has"/>
        <rdfs:comment>This property encapsulates all the sub-properties that describe how an entity has an equipment attachment.</rdfs:comment>
    </owl:ObjectProperty>
    


    <!-- http://www.semanticweb.org/cadex/ontologies/2020/1/untitled-ontology-71#hasEquipmentNote -->

    <owl:ObjectProperty rdf:about="http://www.semanticweb.org/cadex/ontologies/2020/1/untitled-ontology-71#hasEquipmentNote">
        <rdfs:subPropertyOf rdf:resource="http://www.semanticweb.org/cadex/ontologies/2020/1/untitled-ontology-71#hasNote"/>
        <rdfs:domain rdf:resource="http://www.semanticweb.org/cadex/ontologies/2020/1/untitled-ontology-71#Equipment"/>
        <rdfs:range rdf:resource="http://www.semanticweb.org/cadex/ontologies/2020/1/untitled-ontology-71#Note"/>
        <rdfs:comment>This property creates link between a piece of equipment and its associated note(s).</rdfs:comment>
    </owl:ObjectProperty>
    


    <!-- http://www.semanticweb.org/cadex/ontologies/2020/1/untitled-ontology-71#hasFile -->

    <owl:ObjectProperty rdf:about="http://www.semanticweb.org/cadex/ontologies/2020/1/untitled-ontology-71#hasFile">
        <rdfs:subPropertyOf rdf:resource="http://www.semanticweb.org/cadex/ontologies/2020/1/untitled-ontology-71#has"/>
        <rdfs:comment>This property encapsulates all the sub-properties that creates relationships from an entity to a file associated with it</rdfs:comment>
    </owl:ObjectProperty>
    


    <!-- http://www.semanticweb.org/cadex/ontologies/2020/1/untitled-ontology-71#hasFrame -->

    <owl:ObjectProperty rdf:about="http://www.semanticweb.org/cadex/ontologies/2020/1/untitled-ontology-71#hasFrame">
        <rdfs:subPropertyOf rdf:resource="http://www.semanticweb.org/cadex/ontologies/2020/1/untitled-ontology-71#has"/>
        <rdfs:range rdf:resource="http://www.semanticweb.org/cadex/ontologies/2020/1/untitled-ontology-71#Frame"/>
        <rdfs:comment>This property encapsulates all the sub-properties that creates relationships from an entity to a frame associated with it</rdfs:comment>
    </owl:ObjectProperty>
    


    <!-- http://www.semanticweb.org/cadex/ontologies/2020/1/untitled-ontology-71#hasIssue -->

    <owl:ObjectProperty rdf:about="http://www.semanticweb.org/cadex/ontologies/2020/1/untitled-ontology-71#hasIssue">
        <rdfs:subPropertyOf rdf:resource="http://www.semanticweb.org/cadex/ontologies/2020/1/untitled-ontology-71#has"/>
        <rdfs:range rdf:resource="http://www.semanticweb.org/cadex/ontologies/2020/1/untitled-ontology-71#Issue"/>
        <rdfs:comment>This property encapsulates all the sub-properties that creates relationships from an entity to an issue associated with it</rdfs:comment>
    </owl:ObjectProperty>
    


    <!-- http://www.semanticweb.org/cadex/ontologies/2020/1/untitled-ontology-71#hasLensGrid -->

    <owl:ObjectProperty rdf:about="http://www.semanticweb.org/cadex/ontologies/2020/1/untitled-ontology-71#hasLensGrid">
        <rdfs:subPropertyOf rdf:resource="http://www.semanticweb.org/cadex/ontologies/2020/1/untitled-ontology-71#has"/>
        <rdfs:comment>This property encapsulates all the sub-properties that describe how an entity *owns* a lens grid.</rdfs:comment>
    </owl:ObjectProperty>
    


    <!-- http://www.semanticweb.org/cadex/ontologies/2020/1/untitled-ontology-71#hasLensNote -->

    <owl:ObjectProperty rdf:about="http://www.semanticweb.org/cadex/ontologies/2020/1/untitled-ontology-71#hasLensNote">
        <rdfs:subPropertyOf rdf:resource="http://www.semanticweb.org/cadex/ontologies/2020/1/untitled-ontology-71#hasNote"/>
        <rdfs:domain rdf:resource="http://www.semanticweb.org/cadex/ontologies/2020/1/untitled-ontology-71#Lens"/>
        <rdfs:range rdf:resource="http://www.semanticweb.org/cadex/ontologies/2020/1/untitled-ontology-71#Note"/>
        <rdfs:comment>This property creates link between a lens and its associated note(s).</rdfs:comment>
    </owl:ObjectProperty>
    


    <!-- http://www.semanticweb.org/cadex/ontologies/2020/1/untitled-ontology-71#hasLocation -->

    <owl:ObjectProperty rdf:about="http://www.semanticweb.org/cadex/ontologies/2020/1/untitled-ontology-71#hasLocation">
        <rdfs:subPropertyOf rdf:resource="http://www.semanticweb.org/cadex/ontologies/2020/1/untitled-ontology-71#has"/>
        <rdfs:range rdf:resource="http://www.semanticweb.org/cadex/ontologies/2020/1/untitled-ontology-71#Location"/>
        <rdfs:comment>This property encapsulates all the sub-properties that creates relationships from an entity to an location associated with it</rdfs:comment>
    </owl:ObjectProperty>
    


    <!-- http://www.semanticweb.org/cadex/ontologies/2020/1/untitled-ontology-71#hasLoggingTag -->

    <owl:ObjectProperty rdf:about="http://www.semanticweb.org/cadex/ontologies/2020/1/untitled-ontology-71#hasLoggingTag">
        <rdfs:subPropertyOf rdf:resource="http://www.semanticweb.org/cadex/ontologies/2020/1/untitled-ontology-71#has"/>
        <rdfs:range rdf:resource="http://www.semanticweb.org/cadex/ontologies/2020/1/untitled-ontology-71#LoggingTag"/>
        <rdfs:comment>This property encapsulates all the sub-properties that creates relationships from an entity to a logging tag that can be used to search for it.</rdfs:comment>
    </owl:ObjectProperty>
    


    <!-- http://www.semanticweb.org/cadex/ontologies/2020/1/untitled-ontology-71#hasNote -->

    <owl:ObjectProperty rdf:about="http://www.semanticweb.org/cadex/ontologies/2020/1/untitled-ontology-71#hasNote">
        <rdfs:subPropertyOf rdf:resource="http://www.semanticweb.org/cadex/ontologies/2020/1/untitled-ontology-71#has"/>
        <rdfs:range rdf:resource="http://www.semanticweb.org/cadex/ontologies/2020/1/untitled-ontology-71#Note"/>
        <rdfs:comment>This property encapsulates all the sub-properties that creates relationships from an entity to a note made against it.</rdfs:comment>
    </owl:ObjectProperty>
    


    <!-- http://www.semanticweb.org/cadex/ontologies/2020/1/untitled-ontology-71#hasPreviousRecordVersion -->

    <owl:ObjectProperty rdf:about="http://www.semanticweb.org/cadex/ontologies/2020/1/untitled-ontology-71#hasPreviousRecordVersion">
        <rdfs:subPropertyOf rdf:resource="http://www.semanticweb.org/cadex/ontologies/2020/1/untitled-ontology-71#hasVersion"/>
        <rdf:type rdf:resource="http://www.w3.org/2002/07/owl#SymmetricProperty"/>
        <rdfs:domain rdf:resource="http://www.semanticweb.org/cadex/ontologies/2020/1/untitled-ontology-71#Record"/>
        <rdfs:range rdf:resource="http://www.semanticweb.org/cadex/ontologies/2020/1/untitled-ontology-71#Record"/>
        <rdfs:comment>This property links two versions of an entity record together to keep track of changes in metadata.</rdfs:comment>
    </owl:ObjectProperty>
    


    <!-- http://www.semanticweb.org/cadex/ontologies/2020/1/untitled-ontology-71#hasRecord -->

    <owl:ObjectProperty rdf:about="http://www.semanticweb.org/cadex/ontologies/2020/1/untitled-ontology-71#hasRecord">
        <rdfs:subPropertyOf rdf:resource="http://www.semanticweb.org/cadex/ontologies/2020/1/untitled-ontology-71#has"/>
        <rdfs:range rdf:resource="http://www.semanticweb.org/cadex/ontologies/2020/1/untitled-ontology-71#Record"/>
        <rdfs:comment>This property encapsulates all the sub-properties that describe how an entity has a record about it.</rdfs:comment>
    </owl:ObjectProperty>
    


    <!-- http://www.semanticweb.org/cadex/ontologies/2020/1/untitled-ontology-71#hasRental -->

    <owl:ObjectProperty rdf:about="http://www.semanticweb.org/cadex/ontologies/2020/1/untitled-ontology-71#hasRental">
        <rdfs:subPropertyOf rdf:resource="http://www.semanticweb.org/cadex/ontologies/2020/1/untitled-ontology-71#has"/>
        <rdfs:range rdf:resource="http://www.semanticweb.org/cadex/ontologies/2020/1/untitled-ontology-71#Rental"/>
        <rdfs:comment>This property encapsulates all the sub-properties that describe how an entity *owns* a rental.</rdfs:comment>
    </owl:ObjectProperty>
    


    <!-- http://www.semanticweb.org/cadex/ontologies/2020/1/untitled-ontology-71#hasRole -->

    <owl:ObjectProperty rdf:about="http://www.semanticweb.org/cadex/ontologies/2020/1/untitled-ontology-71#hasRole">
        <rdfs:subPropertyOf rdf:resource="http://www.semanticweb.org/cadex/ontologies/2020/1/untitled-ontology-71#has"/>
        <rdfs:range rdf:resource="http://www.semanticweb.org/cadex/ontologies/2020/1/untitled-ontology-71#Role"/>
        <rdfs:comment>This property encapsulates all the sub-properties that creates relationships from an entity to a role.</rdfs:comment>
    </owl:ObjectProperty>
    


    <!-- http://www.semanticweb.org/cadex/ontologies/2020/1/untitled-ontology-71#hasRoll -->

    <owl:ObjectProperty rdf:about="http://www.semanticweb.org/cadex/ontologies/2020/1/untitled-ontology-71#hasRoll">
        <rdfs:subPropertyOf rdf:resource="http://www.semanticweb.org/cadex/ontologies/2020/1/untitled-ontology-71#has"/>
        <rdfs:range rdf:resource="http://www.semanticweb.org/cadex/ontologies/2020/1/untitled-ontology-71#Roll"/>
        <rdfs:comment>This property encapsulates all the sub-properties that creates relationships from an entity to a roll associated with it.</rdfs:comment>
    </owl:ObjectProperty>
    


    <!-- http://www.semanticweb.org/cadex/ontologies/2020/1/untitled-ontology-71#hasScene -->

    <owl:ObjectProperty rdf:about="http://www.semanticweb.org/cadex/ontologies/2020/1/untitled-ontology-71#hasScene">
        <rdfs:subPropertyOf rdf:resource="http://www.semanticweb.org/cadex/ontologies/2020/1/untitled-ontology-71#has"/>
        <rdfs:range rdf:resource="http://www.semanticweb.org/cadex/ontologies/2020/1/untitled-ontology-71#Scene"/>
        <rdfs:comment>This property encapsulates all the sub-properties that creates relationships from an entity to a scene associated with it.</rdfs:comment>
    </owl:ObjectProperty>
    


    <!-- http://www.semanticweb.org/cadex/ontologies/2020/1/untitled-ontology-71#hasSceneContactList -->

    <owl:ObjectProperty rdf:about="http://www.semanticweb.org/cadex/ontologies/2020/1/untitled-ontology-71#hasSceneContactList">
        <rdfs:subPropertyOf rdf:resource="http://www.semanticweb.org/cadex/ontologies/2020/1/untitled-ontology-71#hasContactList"/>
        <rdfs:domain rdf:resource="http://www.semanticweb.org/cadex/ontologies/2020/1/untitled-ontology-71#Scene"/>
        <rdfs:range rdf:resource="http://www.semanticweb.org/cadex/ontologies/2020/1/untitled-ontology-71#Staff"/>
        <rdfs:comment>This property creates a relation between a scene and the staff on its contact list. The collection of all staff related to a scene in this way forms the contact list.</rdfs:comment>
    </owl:ObjectProperty>
    


    <!-- http://www.semanticweb.org/cadex/ontologies/2020/1/untitled-ontology-71#hasSceneNote -->

    <owl:ObjectProperty rdf:about="http://www.semanticweb.org/cadex/ontologies/2020/1/untitled-ontology-71#hasSceneNote">
        <rdfs:subPropertyOf rdf:resource="http://www.semanticweb.org/cadex/ontologies/2020/1/untitled-ontology-71#hasNote"/>
        <rdfs:domain rdf:resource="http://www.semanticweb.org/cadex/ontologies/2020/1/untitled-ontology-71#Scene"/>
        <rdfs:range rdf:resource="http://www.semanticweb.org/cadex/ontologies/2020/1/untitled-ontology-71#Note"/>
        <rdfs:comment>This property creates link between a scene and its associated note(s).</rdfs:comment>
    </owl:ObjectProperty>
    


    <!-- http://www.semanticweb.org/cadex/ontologies/2020/1/untitled-ontology-71#hasScriptBreakdown -->

    <owl:ObjectProperty rdf:about="http://www.semanticweb.org/cadex/ontologies/2020/1/untitled-ontology-71#hasScriptBreakdown">
        <rdfs:subPropertyOf rdf:resource="http://www.semanticweb.org/cadex/ontologies/2020/1/untitled-ontology-71#has"/>
        <rdfs:range rdf:resource="http://www.semanticweb.org/cadex/ontologies/2020/1/untitled-ontology-71#ScriptBreakdown"/>
        <rdfs:comment>This property encapsulates all the sub-properties that describe how an entity *owns* a script breakdown.</rdfs:comment>
    </owl:ObjectProperty>
    


    <!-- http://www.semanticweb.org/cadex/ontologies/2020/1/untitled-ontology-71#hasShoot -->

    <owl:ObjectProperty rdf:about="http://www.semanticweb.org/cadex/ontologies/2020/1/untitled-ontology-71#hasShoot">
        <rdfs:subPropertyOf rdf:resource="http://www.semanticweb.org/cadex/ontologies/2020/1/untitled-ontology-71#has"/>
        <rdfs:range rdf:resource="http://www.semanticweb.org/cadex/ontologies/2020/1/untitled-ontology-71#Shoot"/>
        <rdfs:comment>This property encapsulates all the sub-properties that describe how an entity *owns* a shoot.</rdfs:comment>
    </owl:ObjectProperty>
    


    <!-- http://www.semanticweb.org/cadex/ontologies/2020/1/untitled-ontology-71#hasShootDay -->

    <owl:ObjectProperty rdf:about="http://www.semanticweb.org/cadex/ontologies/2020/1/untitled-ontology-71#hasShootDay">
        <rdfs:subPropertyOf rdf:resource="http://www.semanticweb.org/cadex/ontologies/2020/1/untitled-ontology-71#has"/>
        <rdfs:comment>This property encapsulates all the sub-properties that describe how an entity *owns* a shoot day.</rdfs:comment>
    </owl:ObjectProperty>
    


    <!-- http://www.semanticweb.org/cadex/ontologies/2020/1/untitled-ontology-71#hasShootNote -->

    <owl:ObjectProperty rdf:about="http://www.semanticweb.org/cadex/ontologies/2020/1/untitled-ontology-71#hasShootNote">
        <rdfs:subPropertyOf rdf:resource="http://www.semanticweb.org/cadex/ontologies/2020/1/untitled-ontology-71#hasNote"/>
        <rdfs:domain rdf:resource="http://www.semanticweb.org/cadex/ontologies/2020/1/untitled-ontology-71#Shoot"/>
        <rdfs:range rdf:resource="http://www.semanticweb.org/cadex/ontologies/2020/1/untitled-ontology-71#Note"/>
        <rdfs:comment>This property creates link between a shoot and its associated note(s).</rdfs:comment>
    </owl:ObjectProperty>
    


    <!-- http://www.semanticweb.org/cadex/ontologies/2020/1/untitled-ontology-71#hasShootingSchedule -->

    <owl:ObjectProperty rdf:about="http://www.semanticweb.org/cadex/ontologies/2020/1/untitled-ontology-71#hasShootingSchedule">
        <rdfs:subPropertyOf rdf:resource="http://www.semanticweb.org/cadex/ontologies/2020/1/untitled-ontology-71#has"/>
        <rdfs:range rdf:resource="http://www.semanticweb.org/cadex/ontologies/2020/1/untitled-ontology-71#ShootingSchedule"/>
        <rdfs:comment>This property encapsulates all the sub-properties that describe how an entity *owns* a shooting schedule.</rdfs:comment>
    </owl:ObjectProperty>
    


    <!-- http://www.semanticweb.org/cadex/ontologies/2020/1/untitled-ontology-71#hasShot -->

    <owl:ObjectProperty rdf:about="http://www.semanticweb.org/cadex/ontologies/2020/1/untitled-ontology-71#hasShot">
        <rdfs:subPropertyOf rdf:resource="http://www.semanticweb.org/cadex/ontologies/2020/1/untitled-ontology-71#has"/>
        <rdfs:range rdf:resource="http://www.semanticweb.org/cadex/ontologies/2020/1/untitled-ontology-71#Shot"/>
        <rdfs:comment>This property encapsulates all the sub-properties that describe how an entity *owns* a shot.</rdfs:comment>
    </owl:ObjectProperty>
    


    <!-- http://www.semanticweb.org/cadex/ontologies/2020/1/untitled-ontology-71#hasSlate -->

    <owl:ObjectProperty rdf:about="http://www.semanticweb.org/cadex/ontologies/2020/1/untitled-ontology-71#hasSlate">
        <rdfs:subPropertyOf rdf:resource="http://www.semanticweb.org/cadex/ontologies/2020/1/untitled-ontology-71#has"/>
        <rdfs:range rdf:resource="http://www.semanticweb.org/cadex/ontologies/2020/1/untitled-ontology-71#Slate"/>
        <rdfs:comment>This property encapsulates all the sub-properties that creates relationships from an entity to a slate associated with it.</rdfs:comment>
    </owl:ObjectProperty>
    


    <!-- http://www.semanticweb.org/cadex/ontologies/2020/1/untitled-ontology-71#hasSlateDataOpNotes -->

    <owl:ObjectProperty rdf:about="http://www.semanticweb.org/cadex/ontologies/2020/1/untitled-ontology-71#hasSlateDataOpNotes">
        <rdfs:subPropertyOf rdf:resource="http://www.semanticweb.org/cadex/ontologies/2020/1/untitled-ontology-71#hasSlateNote"/>
        <rdfs:domain rdf:resource="http://www.semanticweb.org/cadex/ontologies/2020/1/untitled-ontology-71#Slate"/>
        <rdfs:range rdf:resource="http://www.semanticweb.org/cadex/ontologies/2020/1/untitled-ontology-71#Note"/>
        <rdfs:comment>This property creates link between a slate and its associated data op note(s).</rdfs:comment>
    </owl:ObjectProperty>
    


    <!-- http://www.semanticweb.org/cadex/ontologies/2020/1/untitled-ontology-71#hasSlateNote -->

    <owl:ObjectProperty rdf:about="http://www.semanticweb.org/cadex/ontologies/2020/1/untitled-ontology-71#hasSlateNote">
        <rdfs:subPropertyOf rdf:resource="http://www.semanticweb.org/cadex/ontologies/2020/1/untitled-ontology-71#hasNote"/>
        <rdfs:domain rdf:resource="http://www.semanticweb.org/cadex/ontologies/2020/1/untitled-ontology-71#Slate"/>
        <rdfs:range rdf:resource="http://www.semanticweb.org/cadex/ontologies/2020/1/untitled-ontology-71#Note"/>
        <rdfs:comment>This property creates link between a slate and its associated note(s).</rdfs:comment>
    </owl:ObjectProperty>
    


    <!-- http://www.semanticweb.org/cadex/ontologies/2020/1/untitled-ontology-71#hasStoryboard -->

    <owl:ObjectProperty rdf:about="http://www.semanticweb.org/cadex/ontologies/2020/1/untitled-ontology-71#hasStoryboard">
        <rdfs:subPropertyOf rdf:resource="http://www.semanticweb.org/cadex/ontologies/2020/1/untitled-ontology-71#has"/>
        <rdfs:range rdf:resource="http://www.semanticweb.org/cadex/ontologies/2020/1/untitled-ontology-71#Storyboard"/>
        <rdfs:comment>This property encapsulates all the sub-properties that describe how an entity *owns* a storyboard.</rdfs:comment>
    </owl:ObjectProperty>
    


    <!-- http://www.semanticweb.org/cadex/ontologies/2020/1/untitled-ontology-71#hasSupervisor -->

    <owl:ObjectProperty rdf:about="http://www.semanticweb.org/cadex/ontologies/2020/1/untitled-ontology-71#hasSupervisor">
        <rdfs:subPropertyOf rdf:resource="http://www.semanticweb.org/cadex/ontologies/2020/1/untitled-ontology-71#has"/>
        <rdfs:range rdf:resource="http://www.semanticweb.org/cadex/ontologies/2020/1/untitled-ontology-71#Staff"/>
        <rdfs:comment>This property encapsulates all the sub-properties that creates relationships from an entity to a staff member that supervises it.</rdfs:comment>
    </owl:ObjectProperty>
    


    <!-- http://www.semanticweb.org/cadex/ontologies/2020/1/untitled-ontology-71#hasTake -->

    <owl:ObjectProperty rdf:about="http://www.semanticweb.org/cadex/ontologies/2020/1/untitled-ontology-71#hasTake">
        <rdfs:subPropertyOf rdf:resource="http://www.semanticweb.org/cadex/ontologies/2020/1/untitled-ontology-71#has"/>
        <rdfs:range rdf:resource="http://www.semanticweb.org/cadex/ontologies/2020/1/untitled-ontology-71#Take"/>
        <rdfs:comment>This property encapsulates all the sub-properties that creates relationships from an entity to a take associated with it.</rdfs:comment>
    </owl:ObjectProperty>
    


    <!-- http://www.semanticweb.org/cadex/ontologies/2020/1/untitled-ontology-71#hasTask -->

    <owl:ObjectProperty rdf:about="http://www.semanticweb.org/cadex/ontologies/2020/1/untitled-ontology-71#hasTask">
        <rdfs:subPropertyOf rdf:resource="http://www.semanticweb.org/cadex/ontologies/2020/1/untitled-ontology-71#has"/>
        <rdfs:range rdf:resource="http://www.semanticweb.org/cadex/ontologies/2020/1/untitled-ontology-71#Task"/>
        <rdfs:comment>This property encapsulates all the sub-properties that creates relationships from an entity to a task associated with it.</rdfs:comment>
    </owl:ObjectProperty>
    


    <!-- http://www.semanticweb.org/cadex/ontologies/2020/1/untitled-ontology-71#hasUnit -->

    <owl:ObjectProperty rdf:about="http://www.semanticweb.org/cadex/ontologies/2020/1/untitled-ontology-71#hasUnit">
        <rdfs:subPropertyOf rdf:resource="http://www.semanticweb.org/cadex/ontologies/2020/1/untitled-ontology-71#has"/>
        <rdfs:range rdf:resource="http://www.semanticweb.org/cadex/ontologies/2020/1/untitled-ontology-71#Unit"/>
        <rdfs:comment>This property encapsulates all the sub-properties that creates relationships from an entity to a unit associated with it.</rdfs:comment>
    </owl:ObjectProperty>
    


    <!-- http://www.semanticweb.org/cadex/ontologies/2020/1/untitled-ontology-71#hasUnitNote -->

    <owl:ObjectProperty rdf:about="http://www.semanticweb.org/cadex/ontologies/2020/1/untitled-ontology-71#hasUnitNote">
        <rdfs:subPropertyOf rdf:resource="http://www.semanticweb.org/cadex/ontologies/2020/1/untitled-ontology-71#hasNote"/>
        <rdfs:domain rdf:resource="http://www.semanticweb.org/cadex/ontologies/2020/1/untitled-ontology-71#Unit"/>
        <rdfs:range rdf:resource="http://www.semanticweb.org/cadex/ontologies/2020/1/untitled-ontology-71#Note"/>
        <rdfs:comment>This property creates link between a unit and its associated note(s).</rdfs:comment>
    </owl:ObjectProperty>
    


    <!-- http://www.semanticweb.org/cadex/ontologies/2020/1/untitled-ontology-71#hasVersion -->

    <owl:ObjectProperty rdf:about="http://www.semanticweb.org/cadex/ontologies/2020/1/untitled-ontology-71#hasVersion">
        <rdfs:subPropertyOf rdf:resource="http://www.semanticweb.org/cadex/ontologies/2020/1/untitled-ontology-71#has"/>
        <rdfs:comment>This property encapsulates all the sub-properties that link two versions of the same entity together for the purposes of version control.</rdfs:comment>
    </owl:ObjectProperty>
    


    <!-- http://www.semanticweb.org/cadex/ontologies/2020/1/untitled-ontology-71#isAbout -->

    <owl:ObjectProperty rdf:about="http://www.semanticweb.org/cadex/ontologies/2020/1/untitled-ontology-71#isAbout">
        <rdfs:comment>This property encapsulates all the sub-properties that groups metadata about a real-world entity.</rdfs:comment>
    </owl:ObjectProperty>
    


    <!-- http://www.semanticweb.org/cadex/ontologies/2020/1/untitled-ontology-71#isFrom -->

    <owl:ObjectProperty rdf:about="http://www.semanticweb.org/cadex/ontologies/2020/1/untitled-ontology-71#isFrom">
        <rdfs:comment>This property creates link from an entity which originated from another entity.</rdfs:comment>
    </owl:ObjectProperty>
    


    <!-- http://www.semanticweb.org/cadex/ontologies/2020/1/untitled-ontology-71#isPartOf -->

    <owl:ObjectProperty rdf:about="http://www.semanticweb.org/cadex/ontologies/2020/1/untitled-ontology-71#isPartOf">
        <rdfs:comment>This property creates link from an entity which forms a part of or is involved in another entity.</rdfs:comment>
    </owl:ObjectProperty>
    


    <!-- http://www.semanticweb.org/cadex/ontologies/2020/1/untitled-ontology-71#issueCheckedBy -->

    <owl:ObjectProperty rdf:about="http://www.semanticweb.org/cadex/ontologies/2020/1/untitled-ontology-71#issueCheckedBy">
        <rdfs:subPropertyOf rdf:resource="http://www.semanticweb.org/cadex/ontologies/2020/1/untitled-ontology-71#checkedBy"/>
        <rdfs:domain rdf:resource="http://www.semanticweb.org/cadex/ontologies/2020/1/untitled-ontology-71#Issue"/>
        <rdfs:range rdf:resource="http://www.semanticweb.org/cadex/ontologies/2020/1/untitled-ontology-71#Staff"/>
        <rdfs:comment>This property creates a relation between an issue and the staff member that has checked it.</rdfs:comment>
    </owl:ObjectProperty>
    


    <!-- http://www.semanticweb.org/cadex/ontologies/2020/1/untitled-ontology-71#issueCreatedBy -->

    <owl:ObjectProperty rdf:about="http://www.semanticweb.org/cadex/ontologies/2020/1/untitled-ontology-71#issueCreatedBy">
        <rdfs:subPropertyOf rdf:resource="http://www.semanticweb.org/cadex/ontologies/2020/1/untitled-ontology-71#createdBy"/>
        <rdfs:domain rdf:resource="http://www.semanticweb.org/cadex/ontologies/2020/1/untitled-ontology-71#Issue"/>
        <rdfs:range rdf:resource="http://www.semanticweb.org/cadex/ontologies/2020/1/untitled-ontology-71#Staff"/>
        <rdfs:comment>This property creates a relation between an issue and the staff member that created it.</rdfs:comment>
    </owl:ObjectProperty>
    


    <!-- http://www.semanticweb.org/cadex/ontologies/2020/1/untitled-ontology-71#issueFixedBy -->

    <owl:ObjectProperty rdf:about="http://www.semanticweb.org/cadex/ontologies/2020/1/untitled-ontology-71#issueFixedBy">
        <rdfs:subPropertyOf rdf:resource="http://www.semanticweb.org/cadex/ontologies/2020/1/untitled-ontology-71#fixedBy"/>
        <rdfs:domain rdf:resource="http://www.semanticweb.org/cadex/ontologies/2020/1/untitled-ontology-71#Issue"/>
        <rdfs:range rdf:resource="http://www.semanticweb.org/cadex/ontologies/2020/1/untitled-ontology-71#Staff"/>
        <rdfs:comment>This property creates a relation between an issue and the staff member that fixed it.</rdfs:comment>
    </owl:ObjectProperty>
    


    <!-- http://www.semanticweb.org/cadex/ontologies/2020/1/untitled-ontology-71#lensCreatedBy -->

    <owl:ObjectProperty rdf:about="http://www.semanticweb.org/cadex/ontologies/2020/1/untitled-ontology-71#lensCreatedBy">
        <rdfs:subPropertyOf rdf:resource="http://www.semanticweb.org/cadex/ontologies/2020/1/untitled-ontology-71#createdBy"/>
        <rdfs:domain rdf:resource="http://www.semanticweb.org/cadex/ontologies/2020/1/untitled-ontology-71#Lens"/>
        <rdfs:range rdf:resource="http://www.semanticweb.org/cadex/ontologies/2020/1/untitled-ontology-71#Staff"/>
        <rdfs:comment>This property creates a relation between a lens and the staff member that created it.</rdfs:comment>
    </owl:ObjectProperty>
    


    <!-- http://www.semanticweb.org/cadex/ontologies/2020/1/untitled-ontology-71#lensHasLensGrid -->

    <owl:ObjectProperty rdf:about="http://www.semanticweb.org/cadex/ontologies/2020/1/untitled-ontology-71#lensHasLensGrid">
        <rdfs:subPropertyOf rdf:resource="http://www.semanticweb.org/cadex/ontologies/2020/1/untitled-ontology-71#hasLensGrid"/>
        <rdfs:domain rdf:resource="http://www.semanticweb.org/cadex/ontologies/2020/1/untitled-ontology-71#Lens"/>
        <rdfs:range rdf:resource="http://www.semanticweb.org/cadex/ontologies/2020/1/untitled-ontology-71#LensGrid"/>
        <rdfs:comment>This property creates a relation between a lens and its lens grid.</rdfs:comment>
    </owl:ObjectProperty>
    


    <!-- http://www.semanticweb.org/cadex/ontologies/2020/1/untitled-ontology-71#lensUpdatedBy -->

    <owl:ObjectProperty rdf:about="http://www.semanticweb.org/cadex/ontologies/2020/1/untitled-ontology-71#lensUpdatedBy">
        <rdfs:subPropertyOf rdf:resource="http://www.semanticweb.org/cadex/ontologies/2020/1/untitled-ontology-71#updatedBy"/>
        <rdfs:domain rdf:resource="http://www.semanticweb.org/cadex/ontologies/2020/1/untitled-ontology-71#Lens"/>
        <rdfs:range rdf:resource="http://www.semanticweb.org/cadex/ontologies/2020/1/untitled-ontology-71#Staff"/>
        <rdfs:comment>This property creates a relation between a lens and the staff member that updated it.</rdfs:comment>
    </owl:ObjectProperty>
    


    <!-- http://www.semanticweb.org/cadex/ontologies/2020/1/untitled-ontology-71#lensUsedIn -->

    <owl:ObjectProperty rdf:about="http://www.semanticweb.org/cadex/ontologies/2020/1/untitled-ontology-71#lensUsedIn">
        <rdfs:subPropertyOf rdf:resource="http://www.semanticweb.org/cadex/ontologies/2020/1/untitled-ontology-71#usedIn"/>
        <rdfs:domain rdf:resource="http://www.semanticweb.org/cadex/ontologies/2020/1/untitled-ontology-71#Lens"/>
        <rdfs:comment>This property encapsulates all the sub-properties that describe the entity that a lens is used in.</rdfs:comment>
    </owl:ObjectProperty>
    


    <!-- http://www.semanticweb.org/cadex/ontologies/2020/1/untitled-ontology-71#lensUsedInClip -->

    <owl:ObjectProperty rdf:about="http://www.semanticweb.org/cadex/ontologies/2020/1/untitled-ontology-71#lensUsedInClip">
        <rdfs:subPropertyOf rdf:resource="http://www.semanticweb.org/cadex/ontologies/2020/1/untitled-ontology-71#lensUsedIn"/>
        <rdfs:domain rdf:resource="http://www.semanticweb.org/cadex/ontologies/2020/1/untitled-ontology-71#Lens"/>
        <rdfs:range rdf:resource="http://www.semanticweb.org/cadex/ontologies/2020/1/untitled-ontology-71#Clip"/>
        <rdfs:comment>This property creates a link that describes how lens is used in a clip.</rdfs:comment>
    </owl:ObjectProperty>
    


    <!-- http://www.semanticweb.org/cadex/ontologies/2020/1/untitled-ontology-71#lensUsedInUnit -->

    <owl:ObjectProperty rdf:about="http://www.semanticweb.org/cadex/ontologies/2020/1/untitled-ontology-71#lensUsedInUnit">
        <rdfs:subPropertyOf rdf:resource="http://www.semanticweb.org/cadex/ontologies/2020/1/untitled-ontology-71#lensUsedIn"/>
        <rdfs:domain rdf:resource="http://www.semanticweb.org/cadex/ontologies/2020/1/untitled-ontology-71#Lens"/>
        <rdfs:range rdf:resource="http://www.semanticweb.org/cadex/ontologies/2020/1/untitled-ontology-71#Unit"/>
        <rdfs:comment>This property creates a link that describes how lens is used in a unit.</rdfs:comment>
    </owl:ObjectProperty>
    


    <!-- http://www.semanticweb.org/cadex/ontologies/2020/1/untitled-ontology-71#locationUsedIn -->

    <owl:ObjectProperty rdf:about="http://www.semanticweb.org/cadex/ontologies/2020/1/untitled-ontology-71#locationUsedIn">
        <rdfs:subPropertyOf rdf:resource="http://www.semanticweb.org/cadex/ontologies/2020/1/untitled-ontology-71#usedIn"/>
        <rdfs:domain rdf:resource="http://www.semanticweb.org/cadex/ontologies/2020/1/untitled-ontology-71#Location"/>
        <rdfs:comment>This property encapsulates all the sub-properties that describe the entity that a location is used in.</rdfs:comment>
    </owl:ObjectProperty>
    


    <!-- http://www.semanticweb.org/cadex/ontologies/2020/1/untitled-ontology-71#loggingTagCreatedBy -->

    <owl:ObjectProperty rdf:about="http://www.semanticweb.org/cadex/ontologies/2020/1/untitled-ontology-71#loggingTagCreatedBy">
        <rdfs:subPropertyOf rdf:resource="http://www.semanticweb.org/cadex/ontologies/2020/1/untitled-ontology-71#createdBy"/>
        <rdfs:domain rdf:resource="http://www.semanticweb.org/cadex/ontologies/2020/1/untitled-ontology-71#LoggingTag"/>
        <rdfs:range rdf:resource="http://www.semanticweb.org/cadex/ontologies/2020/1/untitled-ontology-71#Logger"/>
        <rdfs:comment>This property creates a relation between a logging tag and the logger that created it.</rdfs:comment>
    </owl:ObjectProperty>
    


    <!-- http://www.semanticweb.org/cadex/ontologies/2020/1/untitled-ontology-71#personHasRole -->

    <owl:ObjectProperty rdf:about="http://www.semanticweb.org/cadex/ontologies/2020/1/untitled-ontology-71#personHasRole">
        <rdfs:subPropertyOf rdf:resource="http://www.semanticweb.org/cadex/ontologies/2020/1/untitled-ontology-71#hasRole"/>
        <rdfs:domain rdf:resource="http://www.semanticweb.org/cadex/ontologies/2020/1/untitled-ontology-71#Person"/>
        <rdfs:range rdf:resource="http://www.semanticweb.org/cadex/ontologies/2020/1/untitled-ontology-71#Role"/>
        <rdfs:comment>This property creates link between a person and its associated role in the project.</rdfs:comment>
    </owl:ObjectProperty>
    


    <!-- http://www.semanticweb.org/cadex/ontologies/2020/1/untitled-ontology-71#produces -->

    <owl:ObjectProperty rdf:about="http://www.semanticweb.org/cadex/ontologies/2020/1/untitled-ontology-71#produces">
        <rdfs:comment>This property creates link between an entity and the output that it produces.</rdfs:comment>
    </owl:ObjectProperty>
    


    <!-- http://www.semanticweb.org/cadex/ontologies/2020/1/untitled-ontology-71#projectHasClient -->

    <owl:ObjectProperty rdf:about="http://www.semanticweb.org/cadex/ontologies/2020/1/untitled-ontology-71#projectHasClient">
        <rdfs:subPropertyOf rdf:resource="http://www.semanticweb.org/cadex/ontologies/2020/1/untitled-ontology-71#hasClient"/>
        <rdfs:domain rdf:resource="http://www.semanticweb.org/cadex/ontologies/2020/1/untitled-ontology-71#Project"/>
        <rdfs:range rdf:resource="http://www.semanticweb.org/cadex/ontologies/2020/1/untitled-ontology-71#Client"/>
        <rdfs:comment>This property creates a relation between a project and its clients.</rdfs:comment>
    </owl:ObjectProperty>
    


    <!-- http://www.semanticweb.org/cadex/ontologies/2020/1/untitled-ontology-71#projectHasDeliverable -->

    <owl:ObjectProperty rdf:about="http://www.semanticweb.org/cadex/ontologies/2020/1/untitled-ontology-71#projectHasDeliverable">
        <rdfs:subPropertyOf rdf:resource="http://www.semanticweb.org/cadex/ontologies/2020/1/untitled-ontology-71#hasDeliverable"/>
        <rdfs:domain rdf:resource="http://www.semanticweb.org/cadex/ontologies/2020/1/untitled-ontology-71#Project"/>
        <rdfs:range rdf:resource="http://www.semanticweb.org/cadex/ontologies/2020/1/untitled-ontology-71#Deliverable"/>
        <rdfs:comment>This property creates link between a project and its associated deliverable(s).</rdfs:comment>
    </owl:ObjectProperty>
    


    <!-- http://www.semanticweb.org/cadex/ontologies/2020/1/untitled-ontology-71#projectHasRental -->

    <owl:ObjectProperty rdf:about="http://www.semanticweb.org/cadex/ontologies/2020/1/untitled-ontology-71#projectHasRental">
        <rdfs:subPropertyOf rdf:resource="http://www.semanticweb.org/cadex/ontologies/2020/1/untitled-ontology-71#hasRental"/>
        <rdfs:domain rdf:resource="http://www.semanticweb.org/cadex/ontologies/2020/1/untitled-ontology-71#Project"/>
        <rdfs:range rdf:resource="http://www.semanticweb.org/cadex/ontologies/2020/1/untitled-ontology-71#Rental"/>
        <rdfs:comment>This property creates a relation between a project and its rentals.</rdfs:comment>
    </owl:ObjectProperty>
    


    <!-- http://www.semanticweb.org/cadex/ontologies/2020/1/untitled-ontology-71#projectHasShoot -->

    <owl:ObjectProperty rdf:about="http://www.semanticweb.org/cadex/ontologies/2020/1/untitled-ontology-71#projectHasShoot">
        <rdfs:subPropertyOf rdf:resource="http://www.semanticweb.org/cadex/ontologies/2020/1/untitled-ontology-71#hasShoot"/>
        <rdfs:domain rdf:resource="http://www.semanticweb.org/cadex/ontologies/2020/1/untitled-ontology-71#Project"/>
        <rdfs:range rdf:resource="http://www.semanticweb.org/cadex/ontologies/2020/1/untitled-ontology-71#Shoot"/>
        <rdfs:comment>This property creates a relation between a project and its shoots.</rdfs:comment>
    </owl:ObjectProperty>
    


    <!-- http://www.semanticweb.org/cadex/ontologies/2020/1/untitled-ontology-71#projectHasShootingSchedule -->

    <owl:ObjectProperty rdf:about="http://www.semanticweb.org/cadex/ontologies/2020/1/untitled-ontology-71#projectHasShootingSchedule">
        <rdfs:subPropertyOf rdf:resource="http://www.semanticweb.org/cadex/ontologies/2020/1/untitled-ontology-71#hasShootingSchedule"/>
        <rdfs:domain rdf:resource="http://www.semanticweb.org/cadex/ontologies/2020/1/untitled-ontology-71#Project"/>
        <rdfs:range rdf:resource="http://www.semanticweb.org/cadex/ontologies/2020/1/untitled-ontology-71#ShootingSchedule"/>
        <rdfs:comment>This property creates a relation between a project and its shooting schedule.</rdfs:comment>
    </owl:ObjectProperty>
    


    <!-- http://www.semanticweb.org/cadex/ontologies/2020/1/untitled-ontology-71#propUsedIn -->

    <owl:ObjectProperty rdf:about="http://www.semanticweb.org/cadex/ontologies/2020/1/untitled-ontology-71#propUsedIn">
        <rdfs:subPropertyOf rdf:resource="http://www.semanticweb.org/cadex/ontologies/2020/1/untitled-ontology-71#usedIn"/>
        <rdfs:comment>This property encapsulates all the sub-properties that describe the entity that a prop is used in.</rdfs:comment>
    </owl:ObjectProperty>
    


    <!-- http://www.semanticweb.org/cadex/ontologies/2020/1/untitled-ontology-71#propUsedInProject -->

    <owl:ObjectProperty rdf:about="http://www.semanticweb.org/cadex/ontologies/2020/1/untitled-ontology-71#propUsedInProject">
        <rdfs:subPropertyOf rdf:resource="http://www.semanticweb.org/cadex/ontologies/2020/1/untitled-ontology-71#propUsedIn"/>
        <rdfs:comment>This property creates a link that describes a prop is used in a project.</rdfs:comment>
    </owl:ObjectProperty>
    


    <!-- http://www.semanticweb.org/cadex/ontologies/2020/1/untitled-ontology-71#recordIsAboutDataItem -->

    <owl:ObjectProperty rdf:about="http://www.semanticweb.org/cadex/ontologies/2020/1/untitled-ontology-71#recordIsAboutDataItem">
        <rdfs:subPropertyOf rdf:resource="http://www.semanticweb.org/cadex/ontologies/2020/1/untitled-ontology-71#isAbout"/>
        <rdfs:domain rdf:resource="http://www.semanticweb.org/cadex/ontologies/2020/1/untitled-ontology-71#Record"/>
        <rdfs:range rdf:resource="http://www.semanticweb.org/cadex/ontologies/2020/1/untitled-ontology-71#DataItem"/>
        <rdfs:comment>This property creates link between a record and the data item it is about.</rdfs:comment>
    </owl:ObjectProperty>
    


    <!-- http://www.semanticweb.org/cadex/ontologies/2020/1/untitled-ontology-71#rentalContainsEquipment -->

    <owl:ObjectProperty rdf:about="http://www.semanticweb.org/cadex/ontologies/2020/1/untitled-ontology-71#rentalContainsEquipment">
        <rdfs:subPropertyOf rdf:resource="http://www.semanticweb.org/cadex/ontologies/2020/1/untitled-ontology-71#contains"/>
        <rdfs:domain rdf:resource="http://www.semanticweb.org/cadex/ontologies/2020/1/untitled-ontology-71#Rental"/>
        <rdfs:range rdf:resource="http://www.semanticweb.org/cadex/ontologies/2020/1/untitled-ontology-71#Equipment"/>
        <rdfs:comment>This property creates a relationship between a rental and a piece of equipment to identify which equipment are covered by a rental.</rdfs:comment>
    </owl:ObjectProperty>
    


    <!-- http://www.semanticweb.org/cadex/ontologies/2020/1/untitled-ontology-71#rigContainsCamera -->

    <owl:ObjectProperty rdf:about="http://www.semanticweb.org/cadex/ontologies/2020/1/untitled-ontology-71#rigContainsCamera">
        <rdfs:subPropertyOf rdf:resource="http://www.semanticweb.org/cadex/ontologies/2020/1/untitled-ontology-71#contains"/>
        <rdfs:domain rdf:resource="http://www.semanticweb.org/cadex/ontologies/2020/1/untitled-ontology-71#Rig"/>
        <rdfs:range rdf:resource="http://www.semanticweb.org/cadex/ontologies/2020/1/untitled-ontology-71#Camera"/>
        <rdfs:comment>This property creates a relationship between a rig and the camera(s) that form it.</rdfs:comment>
    </owl:ObjectProperty>
    


    <!-- http://www.semanticweb.org/cadex/ontologies/2020/1/untitled-ontology-71#sceneCreatedBy -->

    <owl:ObjectProperty rdf:about="http://www.semanticweb.org/cadex/ontologies/2020/1/untitled-ontology-71#sceneCreatedBy">
        <rdfs:subPropertyOf rdf:resource="http://www.semanticweb.org/cadex/ontologies/2020/1/untitled-ontology-71#createdBy"/>
        <rdfs:domain rdf:resource="http://www.semanticweb.org/cadex/ontologies/2020/1/untitled-ontology-71#Scene"/>
        <rdfs:range rdf:resource="http://www.semanticweb.org/cadex/ontologies/2020/1/untitled-ontology-71#Staff"/>
        <rdfs:comment>This property creates a relation between a scene and the staff member that created it.</rdfs:comment>
    </owl:ObjectProperty>
    


    <!-- http://www.semanticweb.org/cadex/ontologies/2020/1/untitled-ontology-71#sceneHasAsset -->

    <owl:ObjectProperty rdf:about="http://www.semanticweb.org/cadex/ontologies/2020/1/untitled-ontology-71#sceneHasAsset">
        <rdfs:subPropertyOf rdf:resource="http://www.semanticweb.org/cadex/ontologies/2020/1/untitled-ontology-71#hasAsset"/>
        <rdfs:domain rdf:resource="http://www.semanticweb.org/cadex/ontologies/2020/1/untitled-ontology-71#Scene"/>
        <rdfs:range rdf:resource="http://www.semanticweb.org/cadex/ontologies/2020/1/untitled-ontology-71#Asset"/>
        <rdfs:comment>This property creates a relation between a scene and its assets.</rdfs:comment>
    </owl:ObjectProperty>
    


    <!-- http://www.semanticweb.org/cadex/ontologies/2020/1/untitled-ontology-71#sceneHasShot -->

    <owl:ObjectProperty rdf:about="http://www.semanticweb.org/cadex/ontologies/2020/1/untitled-ontology-71#sceneHasShot">
        <rdfs:subPropertyOf rdf:resource="http://www.semanticweb.org/cadex/ontologies/2020/1/untitled-ontology-71#hasShot"/>
        <rdfs:domain rdf:resource="http://www.semanticweb.org/cadex/ontologies/2020/1/untitled-ontology-71#Scene"/>
        <rdfs:range rdf:resource="http://www.semanticweb.org/cadex/ontologies/2020/1/untitled-ontology-71#Shot"/>
        <rdfs:comment>This property creates a relation between a shot and its scene.</rdfs:comment>
    </owl:ObjectProperty>
    


    <!-- http://www.semanticweb.org/cadex/ontologies/2020/1/untitled-ontology-71#sceneHasTask -->

    <owl:ObjectProperty rdf:about="http://www.semanticweb.org/cadex/ontologies/2020/1/untitled-ontology-71#sceneHasTask">
        <rdfs:subPropertyOf rdf:resource="http://www.semanticweb.org/cadex/ontologies/2020/1/untitled-ontology-71#hasTask"/>
        <rdfs:domain rdf:resource="http://www.semanticweb.org/cadex/ontologies/2020/1/untitled-ontology-71#Scene"/>
        <rdfs:range rdf:resource="http://www.semanticweb.org/cadex/ontologies/2020/1/untitled-ontology-71#Task"/>
        <rdfs:comment>This property creates link between a scene and its associated tasks in the project.</rdfs:comment>
    </owl:ObjectProperty>
    


    <!-- http://www.semanticweb.org/cadex/ontologies/2020/1/untitled-ontology-71#sceneIsPartOfShootDay -->

    <owl:ObjectProperty rdf:about="http://www.semanticweb.org/cadex/ontologies/2020/1/untitled-ontology-71#sceneIsPartOfShootDay">
        <rdfs:subPropertyOf rdf:resource="http://www.semanticweb.org/cadex/ontologies/2020/1/untitled-ontology-71#isPartOf"/>
        <rdfs:domain rdf:resource="http://www.semanticweb.org/cadex/ontologies/2020/1/untitled-ontology-71#Scene"/>
        <rdfs:range rdf:resource="http://www.semanticweb.org/cadex/ontologies/2020/1/untitled-ontology-71#ShootDay"/>
        <rdfs:comment>This property creates link from a scene which forms a part of or is involved in a shoot.</rdfs:comment>
    </owl:ObjectProperty>
    


    <!-- http://www.semanticweb.org/cadex/ontologies/2020/1/untitled-ontology-71#sceneUpdatedBy -->

    <owl:ObjectProperty rdf:about="http://www.semanticweb.org/cadex/ontologies/2020/1/untitled-ontology-71#sceneUpdatedBy">
        <rdfs:subPropertyOf rdf:resource="http://www.semanticweb.org/cadex/ontologies/2020/1/untitled-ontology-71#updatedBy"/>
        <rdfs:domain rdf:resource="http://www.semanticweb.org/cadex/ontologies/2020/1/untitled-ontology-71#Scene"/>
        <rdfs:range rdf:resource="http://www.semanticweb.org/cadex/ontologies/2020/1/untitled-ontology-71#Staff"/>
        <rdfs:comment>This property creates a relation between a scene and the staff member that updated it.</rdfs:comment>
    </owl:ObjectProperty>
    


    <!-- http://www.semanticweb.org/cadex/ontologies/2020/1/untitled-ontology-71#scriptHasScene -->

    <owl:ObjectProperty rdf:about="http://www.semanticweb.org/cadex/ontologies/2020/1/untitled-ontology-71#scriptHasScene">
        <rdfs:subPropertyOf rdf:resource="http://www.semanticweb.org/cadex/ontologies/2020/1/untitled-ontology-71#hasScene"/>
        <rdfs:domain rdf:resource="http://www.semanticweb.org/cadex/ontologies/2020/1/untitled-ontology-71#Script"/>
        <rdfs:range rdf:resource="http://www.semanticweb.org/cadex/ontologies/2020/1/untitled-ontology-71#Scene"/>
        <rdfs:comment>This property creates link between a script and its associated scenes in the project.</rdfs:comment>
    </owl:ObjectProperty>
    


    <!-- http://www.semanticweb.org/cadex/ontologies/2020/1/untitled-ontology-71#scriptHasScriptBreakdown -->

    <owl:ObjectProperty rdf:about="http://www.semanticweb.org/cadex/ontologies/2020/1/untitled-ontology-71#scriptHasScriptBreakdown">
        <rdfs:subPropertyOf rdf:resource="http://www.semanticweb.org/cadex/ontologies/2020/1/untitled-ontology-71#hasScriptBreakdown"/>
        <rdfs:domain rdf:resource="http://www.semanticweb.org/cadex/ontologies/2020/1/untitled-ontology-71#Script"/>
        <rdfs:range rdf:resource="http://www.semanticweb.org/cadex/ontologies/2020/1/untitled-ontology-71#ScriptBreakdown"/>
        <rdfs:comment>This property creates a relation between a script and its breakdown.</rdfs:comment>
    </owl:ObjectProperty>
    


    <!-- http://www.semanticweb.org/cadex/ontologies/2020/1/untitled-ontology-71#scriptHasStoryboard -->

    <owl:ObjectProperty rdf:about="http://www.semanticweb.org/cadex/ontologies/2020/1/untitled-ontology-71#scriptHasStoryboard">
        <rdfs:subPropertyOf rdf:resource="http://www.semanticweb.org/cadex/ontologies/2020/1/untitled-ontology-71#hasStoryboard"/>
        <rdfs:domain rdf:resource="http://www.semanticweb.org/cadex/ontologies/2020/1/untitled-ontology-71#Script"/>
        <rdfs:range rdf:resource="http://www.semanticweb.org/cadex/ontologies/2020/1/untitled-ontology-71#Storyboard"/>
        <rdfs:comment>This property creates a relation between a script and its storyboard.</rdfs:comment>
    </owl:ObjectProperty>
    


    <!-- http://www.semanticweb.org/cadex/ontologies/2020/1/untitled-ontology-71#scriptTranslatedTo -->

    <owl:ObjectProperty rdf:about="http://www.semanticweb.org/cadex/ontologies/2020/1/untitled-ontology-71#scriptTranslatedTo">
        <rdfs:domain rdf:resource="http://www.semanticweb.org/cadex/ontologies/2020/1/untitled-ontology-71#Script"/>
        <rdfs:range rdf:resource="http://www.semanticweb.org/cadex/ontologies/2020/1/untitled-ontology-71#Script"/>
        <rdfs:comment>This property creates a relationship between two instances of a script, whereby one version is a translation of another.</rdfs:comment>
    </owl:ObjectProperty>
    


    <!-- http://www.semanticweb.org/cadex/ontologies/2020/1/untitled-ontology-71#scriptWrittenBy -->

    <owl:ObjectProperty rdf:about="http://www.semanticweb.org/cadex/ontologies/2020/1/untitled-ontology-71#scriptWrittenBy">
        <rdfs:subPropertyOf rdf:resource="http://www.semanticweb.org/cadex/ontologies/2020/1/untitled-ontology-71#writtenBy"/>
        <rdfs:domain rdf:resource="http://www.semanticweb.org/cadex/ontologies/2020/1/untitled-ontology-71#Script"/>
        <rdfs:range rdf:resource="http://www.semanticweb.org/cadex/ontologies/2020/1/untitled-ontology-71#Writer"/>
        <rdfs:comment>This property creates a relation between a script and the writer that wrote it.</rdfs:comment>
    </owl:ObjectProperty>
    


    <!-- http://www.semanticweb.org/cadex/ontologies/2020/1/untitled-ontology-71#sentTo -->

    <owl:ObjectProperty rdf:about="http://www.semanticweb.org/cadex/ontologies/2020/1/untitled-ontology-71#sentTo">
        <rdfs:comment>This property groups sub-properties that describes how an entity has been sent from one person to another.</rdfs:comment>
    </owl:ObjectProperty>
    


    <!-- http://www.semanticweb.org/cadex/ontologies/2020/1/untitled-ontology-71#shootCreatedBy -->

    <owl:ObjectProperty rdf:about="http://www.semanticweb.org/cadex/ontologies/2020/1/untitled-ontology-71#shootCreatedBy">
        <rdfs:subPropertyOf rdf:resource="http://www.semanticweb.org/cadex/ontologies/2020/1/untitled-ontology-71#createdBy"/>
        <rdfs:domain rdf:resource="http://www.semanticweb.org/cadex/ontologies/2020/1/untitled-ontology-71#Shoot"/>
        <rdfs:range rdf:resource="http://www.semanticweb.org/cadex/ontologies/2020/1/untitled-ontology-71#Staff"/>
        <rdfs:comment>This property creates a relation between a shoot and the staff member that created it.</rdfs:comment>
    </owl:ObjectProperty>
    


    <!-- http://www.semanticweb.org/cadex/ontologies/2020/1/untitled-ontology-71#shootDayHasScene -->

    <owl:ObjectProperty rdf:about="http://www.semanticweb.org/cadex/ontologies/2020/1/untitled-ontology-71#shootDayHasScene">
        <rdfs:subPropertyOf rdf:resource="http://www.semanticweb.org/cadex/ontologies/2020/1/untitled-ontology-71#hasScene"/>
        <rdfs:domain rdf:resource="http://www.semanticweb.org/cadex/ontologies/2020/1/untitled-ontology-71#ShootDay"/>
        <rdfs:range rdf:resource="http://www.semanticweb.org/cadex/ontologies/2020/1/untitled-ontology-71#Scene"/>
        <rdfs:comment>This property creates link between a shoot and its associated scene in the project.</rdfs:comment>
    </owl:ObjectProperty>
    


    <!-- http://www.semanticweb.org/cadex/ontologies/2020/1/untitled-ontology-71#shootDayIsPartOfShoot -->

    <owl:ObjectProperty rdf:about="http://www.semanticweb.org/cadex/ontologies/2020/1/untitled-ontology-71#shootDayIsPartOfShoot">
        <rdfs:subPropertyOf rdf:resource="http://www.semanticweb.org/cadex/ontologies/2020/1/untitled-ontology-71#isPartOf"/>
        <rdfs:domain rdf:resource="http://www.semanticweb.org/cadex/ontologies/2020/1/untitled-ontology-71#ShootDay"/>
        <rdfs:range rdf:resource="http://www.semanticweb.org/cadex/ontologies/2020/1/untitled-ontology-71#Shoot"/>
        <rdfs:comment>This property creates link from a shoot day which forms a part of or is involved in a shoot.</rdfs:comment>
    </owl:ObjectProperty>
    


    <!-- http://www.semanticweb.org/cadex/ontologies/2020/1/untitled-ontology-71#shootDayhasShootLocation -->

    <owl:ObjectProperty rdf:about="http://www.semanticweb.org/cadex/ontologies/2020/1/untitled-ontology-71#shootDayhasShootLocation">
        <rdfs:subPropertyOf rdf:resource="http://www.semanticweb.org/cadex/ontologies/2020/1/untitled-ontology-71#hasLocation"/>
        <owl:inverseOf rdf:resource="http://www.semanticweb.org/cadex/ontologies/2020/1/untitled-ontology-71#shootLocationUsedInShootDay"/>
        <rdfs:domain rdf:resource="http://www.semanticweb.org/cadex/ontologies/2020/1/untitled-ontology-71#ShootDay"/>
        <rdfs:range rdf:resource="http://www.semanticweb.org/cadex/ontologies/2020/1/untitled-ontology-71#Location"/>
        <rdfs:comment>This property creates a relationship from a shoot day to the shoot location associated with it.</rdfs:comment>
    </owl:ObjectProperty>
    


    <!-- http://www.semanticweb.org/cadex/ontologies/2020/1/untitled-ontology-71#shootHasShootDay -->

    <owl:ObjectProperty rdf:about="http://www.semanticweb.org/cadex/ontologies/2020/1/untitled-ontology-71#shootHasShootDay">
        <rdfs:subPropertyOf rdf:resource="http://www.semanticweb.org/cadex/ontologies/2020/1/untitled-ontology-71#hasShootDay"/>
        <rdfs:domain rdf:resource="http://www.semanticweb.org/cadex/ontologies/2020/1/untitled-ontology-71#Shoot"/>
        <rdfs:range rdf:resource="http://www.semanticweb.org/cadex/ontologies/2020/1/untitled-ontology-71#ShootDay"/>
        <rdfs:comment>This property creates a relation between a shoot and its shoot days.</rdfs:comment>
    </owl:ObjectProperty>
    


    <!-- http://www.semanticweb.org/cadex/ontologies/2020/1/untitled-ontology-71#shootIsPartOfProject -->

    <owl:ObjectProperty rdf:about="http://www.semanticweb.org/cadex/ontologies/2020/1/untitled-ontology-71#shootIsPartOfProject">
        <rdfs:subPropertyOf rdf:resource="http://www.semanticweb.org/cadex/ontologies/2020/1/untitled-ontology-71#isPartOf"/>
        <rdfs:domain rdf:resource="http://www.semanticweb.org/cadex/ontologies/2020/1/untitled-ontology-71#Shoot"/>
        <rdfs:range rdf:resource="http://www.semanticweb.org/cadex/ontologies/2020/1/untitled-ontology-71#Project"/>
        <rdfs:comment>This property creates link from a shoot which forms a part of or is involved in a project.</rdfs:comment>
    </owl:ObjectProperty>
    


    <!-- http://www.semanticweb.org/cadex/ontologies/2020/1/untitled-ontology-71#shootLocationUsedInShootDay -->

    <owl:ObjectProperty rdf:about="http://www.semanticweb.org/cadex/ontologies/2020/1/untitled-ontology-71#shootLocationUsedInShootDay">
        <rdfs:subPropertyOf rdf:resource="http://www.semanticweb.org/cadex/ontologies/2020/1/untitled-ontology-71#locationUsedIn"/>
        <rdfs:domain rdf:resource="http://www.semanticweb.org/cadex/ontologies/2020/1/untitled-ontology-71#Location"/>
        <rdfs:range rdf:resource="http://www.semanticweb.org/cadex/ontologies/2020/1/untitled-ontology-71#ShootDay"/>
        <rdfs:comment>This property creates a link that describes how a shoot location is used in a shoot day.</rdfs:comment>
    </owl:ObjectProperty>
    


    <!-- http://www.semanticweb.org/cadex/ontologies/2020/1/untitled-ontology-71#shootUpdatedBy -->

    <owl:ObjectProperty rdf:about="http://www.semanticweb.org/cadex/ontologies/2020/1/untitled-ontology-71#shootUpdatedBy">
        <rdfs:subPropertyOf rdf:resource="http://www.semanticweb.org/cadex/ontologies/2020/1/untitled-ontology-71#updatedBy"/>
        <rdfs:domain rdf:resource="http://www.semanticweb.org/cadex/ontologies/2020/1/untitled-ontology-71#Shoot"/>
        <rdfs:range rdf:resource="http://www.semanticweb.org/cadex/ontologies/2020/1/untitled-ontology-71#Staff"/>
        <rdfs:comment>This property creates a relation between a shoot and the staff member that updated it.</rdfs:comment>
    </owl:ObjectProperty>
    


    <!-- http://www.semanticweb.org/cadex/ontologies/2020/1/untitled-ontology-71#shootUsesCast -->

    <owl:ObjectProperty rdf:about="http://www.semanticweb.org/cadex/ontologies/2020/1/untitled-ontology-71#shootUsesCast">
        <rdfs:subPropertyOf rdf:resource="http://www.semanticweb.org/cadex/ontologies/2020/1/untitled-ontology-71#usesCast"/>
        <rdfs:domain rdf:resource="http://www.semanticweb.org/cadex/ontologies/2020/1/untitled-ontology-71#Shoot"/>
        <rdfs:range rdf:resource="http://www.semanticweb.org/cadex/ontologies/2020/1/untitled-ontology-71#Cast"/>
        <rdfs:comment>This property creates a relation between a cast member and the shoot that uses it.</rdfs:comment>
    </owl:ObjectProperty>
    


    <!-- http://www.semanticweb.org/cadex/ontologies/2020/1/untitled-ontology-71#shootUsesUnit -->

    <owl:ObjectProperty rdf:about="http://www.semanticweb.org/cadex/ontologies/2020/1/untitled-ontology-71#shootUsesUnit">
        <rdfs:subPropertyOf rdf:resource="http://www.semanticweb.org/cadex/ontologies/2020/1/untitled-ontology-71#usesUnit"/>
        <owl:inverseOf rdf:resource="http://www.semanticweb.org/cadex/ontologies/2020/1/untitled-ontology-71#unitIsPartOfShoot"/>
        <rdfs:domain rdf:resource="http://www.semanticweb.org/cadex/ontologies/2020/1/untitled-ontology-71#Shoot"/>
        <rdfs:range rdf:resource="http://www.semanticweb.org/cadex/ontologies/2020/1/untitled-ontology-71#Unit"/>
        <rdfs:comment>This property creates a relation between a unit and the shoot that uses it.</rdfs:comment>
    </owl:ObjectProperty>
    


    <!-- http://www.semanticweb.org/cadex/ontologies/2020/1/untitled-ontology-71#shotIsPartOfScene -->

    <owl:ObjectProperty rdf:about="http://www.semanticweb.org/cadex/ontologies/2020/1/untitled-ontology-71#shotIsPartOfScene">
        <rdfs:subPropertyOf rdf:resource="http://www.semanticweb.org/cadex/ontologies/2020/1/untitled-ontology-71#isPartOf"/>
        <rdfs:domain rdf:resource="http://www.semanticweb.org/cadex/ontologies/2020/1/untitled-ontology-71#Shot"/>
        <rdfs:range rdf:resource="http://www.semanticweb.org/cadex/ontologies/2020/1/untitled-ontology-71#Scene"/>
        <rdfs:comment>This property creates link from a shot which forms a part of or is involved in a scene.</rdfs:comment>
    </owl:ObjectProperty>
    


    <!-- http://www.semanticweb.org/cadex/ontologies/2020/1/untitled-ontology-71#shotProducesTake -->

    <owl:ObjectProperty rdf:about="http://www.semanticweb.org/cadex/ontologies/2020/1/untitled-ontology-71#shotProducesTake">
        <rdfs:subPropertyOf rdf:resource="http://www.semanticweb.org/cadex/ontologies/2020/1/untitled-ontology-71#produces"/>
        <rdfs:domain rdf:resource="http://www.semanticweb.org/cadex/ontologies/2020/1/untitled-ontology-71#Shot"/>
        <rdfs:range rdf:resource="http://www.semanticweb.org/cadex/ontologies/2020/1/untitled-ontology-71#Take"/>
        <rdfs:comment>This property is a sub-property of produces and creates a relationship between a shot and its outputted take.</rdfs:comment>
    </owl:ObjectProperty>
    


    <!-- http://www.semanticweb.org/cadex/ontologies/2020/1/untitled-ontology-71#slateCreatedBy -->

    <owl:ObjectProperty rdf:about="http://www.semanticweb.org/cadex/ontologies/2020/1/untitled-ontology-71#slateCreatedBy">
        <rdfs:subPropertyOf rdf:resource="http://www.semanticweb.org/cadex/ontologies/2020/1/untitled-ontology-71#createdBy"/>
        <rdfs:domain rdf:resource="http://www.semanticweb.org/cadex/ontologies/2020/1/untitled-ontology-71#Slate"/>
        <rdfs:range rdf:resource="http://www.semanticweb.org/cadex/ontologies/2020/1/untitled-ontology-71#Staff"/>
        <rdfs:comment>This property creates a relation between a slate and the staff member that created it.</rdfs:comment>
    </owl:ObjectProperty>
    


    <!-- http://www.semanticweb.org/cadex/ontologies/2020/1/untitled-ontology-71#slateHasEquipment -->

    <owl:ObjectProperty rdf:about="http://www.semanticweb.org/cadex/ontologies/2020/1/untitled-ontology-71#slateHasEquipment">
        <rdfs:subPropertyOf rdf:resource="http://www.semanticweb.org/cadex/ontologies/2020/1/untitled-ontology-71#hasEquipment"/>
        <rdfs:domain rdf:resource="http://www.semanticweb.org/cadex/ontologies/2020/1/untitled-ontology-71#Slate"/>
        <rdfs:range rdf:resource="http://www.semanticweb.org/cadex/ontologies/2020/1/untitled-ontology-71#Equipment"/>
        <rdfs:comment>This property creates link between a slate and its associated pieces of equipment.</rdfs:comment>
    </owl:ObjectProperty>
    


    <!-- http://www.semanticweb.org/cadex/ontologies/2020/1/untitled-ontology-71#slateHasFile -->

    <owl:ObjectProperty rdf:about="http://www.semanticweb.org/cadex/ontologies/2020/1/untitled-ontology-71#slateHasFile">
        <rdfs:subPropertyOf rdf:resource="http://www.semanticweb.org/cadex/ontologies/2020/1/untitled-ontology-71#hasFile"/>
        <rdfs:domain rdf:resource="http://www.semanticweb.org/cadex/ontologies/2020/1/untitled-ontology-71#Slate"/>
        <rdfs:range rdf:resource="http://www.semanticweb.org/cadex/ontologies/2020/1/untitled-ontology-71#File"/>
        <rdfs:comment>This property creates link between a slate and its associated file.</rdfs:comment>
    </owl:ObjectProperty>
    


    <!-- http://www.semanticweb.org/cadex/ontologies/2020/1/untitled-ontology-71#slateHasShootLocation -->

    <owl:ObjectProperty rdf:about="http://www.semanticweb.org/cadex/ontologies/2020/1/untitled-ontology-71#slateHasShootLocation">
        <rdfs:subPropertyOf rdf:resource="http://www.semanticweb.org/cadex/ontologies/2020/1/untitled-ontology-71#hasLocation"/>
        <rdfs:domain rdf:resource="http://www.semanticweb.org/cadex/ontologies/2020/1/untitled-ontology-71#Slate"/>
        <rdfs:range rdf:resource="http://www.semanticweb.org/cadex/ontologies/2020/1/untitled-ontology-71#Location"/>
        <rdfs:comment>This property creates a relationship from a slate to the shoot location associated with it.</rdfs:comment>
    </owl:ObjectProperty>
    


    <!-- http://www.semanticweb.org/cadex/ontologies/2020/1/untitled-ontology-71#slateHasTake -->

    <owl:ObjectProperty rdf:about="http://www.semanticweb.org/cadex/ontologies/2020/1/untitled-ontology-71#slateHasTake">
        <rdfs:subPropertyOf rdf:resource="http://www.semanticweb.org/cadex/ontologies/2020/1/untitled-ontology-71#hasTake"/>
        <rdfs:domain rdf:resource="http://www.semanticweb.org/cadex/ontologies/2020/1/untitled-ontology-71#Slate"/>
        <rdfs:range rdf:resource="http://www.semanticweb.org/cadex/ontologies/2020/1/untitled-ontology-71#Take"/>
        <rdfs:comment>This property creates link between a slate and its associated take in the project.</rdfs:comment>
    </owl:ObjectProperty>
    


    <!-- http://www.semanticweb.org/cadex/ontologies/2020/1/untitled-ontology-71#slateHasUnit -->

    <owl:ObjectProperty rdf:about="http://www.semanticweb.org/cadex/ontologies/2020/1/untitled-ontology-71#slateHasUnit">
        <rdfs:subPropertyOf rdf:resource="http://www.semanticweb.org/cadex/ontologies/2020/1/untitled-ontology-71#hasUnit"/>
        <rdfs:domain rdf:resource="http://www.semanticweb.org/cadex/ontologies/2020/1/untitled-ontology-71#Slate"/>
        <rdfs:range rdf:resource="http://www.semanticweb.org/cadex/ontologies/2020/1/untitled-ontology-71#Unit"/>
        <rdfs:comment>This property creates link between a slate and its associated unit(s) in the project.</rdfs:comment>
    </owl:ObjectProperty>
    


    <!-- http://www.semanticweb.org/cadex/ontologies/2020/1/untitled-ontology-71#slateUpdatedBy -->

    <owl:ObjectProperty rdf:about="http://www.semanticweb.org/cadex/ontologies/2020/1/untitled-ontology-71#slateUpdatedBy">
        <rdfs:subPropertyOf rdf:resource="http://www.semanticweb.org/cadex/ontologies/2020/1/untitled-ontology-71#updatedBy"/>
        <rdfs:domain rdf:resource="http://www.semanticweb.org/cadex/ontologies/2020/1/untitled-ontology-71#Slate"/>
        <rdfs:range rdf:resource="http://www.semanticweb.org/cadex/ontologies/2020/1/untitled-ontology-71#Staff"/>
        <rdfs:comment>This property creates a relation between a slate and the staff member that updated it.</rdfs:comment>
    </owl:ObjectProperty>
    


    <!-- http://www.semanticweb.org/cadex/ontologies/2020/1/untitled-ontology-71#slateUsesCamera -->

    <owl:ObjectProperty rdf:about="http://www.semanticweb.org/cadex/ontologies/2020/1/untitled-ontology-71#slateUsesCamera">
        <rdfs:subPropertyOf rdf:resource="http://www.semanticweb.org/cadex/ontologies/2020/1/untitled-ontology-71#usesCamera"/>
        <rdfs:domain rdf:resource="http://www.semanticweb.org/cadex/ontologies/2020/1/untitled-ontology-71#Slate"/>
        <rdfs:range rdf:resource="http://www.semanticweb.org/cadex/ontologies/2020/1/untitled-ontology-71#Camera"/>
        <rdfs:comment>This property creates a relation between a camera and the slate that uses it.</rdfs:comment>
    </owl:ObjectProperty>
    


    <!-- http://www.semanticweb.org/cadex/ontologies/2020/1/untitled-ontology-71#slateUsesDriftCamera -->

    <owl:ObjectProperty rdf:about="http://www.semanticweb.org/cadex/ontologies/2020/1/untitled-ontology-71#slateUsesDriftCamera">
        <rdfs:subPropertyOf rdf:resource="http://www.semanticweb.org/cadex/ontologies/2020/1/untitled-ontology-71#slateUsesCamera"/>
        <rdfs:domain rdf:resource="http://www.semanticweb.org/cadex/ontologies/2020/1/untitled-ontology-71#Slate"/>
        <rdfs:range rdf:resource="http://www.semanticweb.org/cadex/ontologies/2020/1/untitled-ontology-71#Camera"/>
        <rdfs:comment>This property creates a relation between a drift camera and the slate that uses it.</rdfs:comment>
    </owl:ObjectProperty>
    


    <!-- http://www.semanticweb.org/cadex/ontologies/2020/1/untitled-ontology-71#slateUsesLens -->

    <owl:ObjectProperty rdf:about="http://www.semanticweb.org/cadex/ontologies/2020/1/untitled-ontology-71#slateUsesLens">
        <rdfs:subPropertyOf rdf:resource="http://www.semanticweb.org/cadex/ontologies/2020/1/untitled-ontology-71#usesLens"/>
        <rdfs:domain rdf:resource="http://www.semanticweb.org/cadex/ontologies/2020/1/untitled-ontology-71#Slate"/>
        <rdfs:range rdf:resource="http://www.semanticweb.org/cadex/ontologies/2020/1/untitled-ontology-71#Lens"/>
        <rdfs:comment>This property creates a relation between a lens and the slate that uses it.</rdfs:comment>
    </owl:ObjectProperty>
    


    <!-- http://www.semanticweb.org/cadex/ontologies/2020/1/untitled-ontology-71#slateUsesWitnessCamera -->

    <owl:ObjectProperty rdf:about="http://www.semanticweb.org/cadex/ontologies/2020/1/untitled-ontology-71#slateUsesWitnessCamera">
        <rdfs:subPropertyOf rdf:resource="http://www.semanticweb.org/cadex/ontologies/2020/1/untitled-ontology-71#slateUsesCamera"/>
        <rdfs:domain rdf:resource="http://www.semanticweb.org/cadex/ontologies/2020/1/untitled-ontology-71#Slate"/>
        <rdfs:range rdf:resource="http://www.semanticweb.org/cadex/ontologies/2020/1/untitled-ontology-71#Camera"/>
        <rdfs:comment>This property creates a relation between a witness camera and the slate that uses it.</rdfs:comment>
    </owl:ObjectProperty>
    


    <!-- http://www.semanticweb.org/cadex/ontologies/2020/1/untitled-ontology-71#takeIsFromShot -->

    <owl:ObjectProperty rdf:about="http://www.semanticweb.org/cadex/ontologies/2020/1/untitled-ontology-71#takeIsFromShot">
        <rdfs:subPropertyOf rdf:resource="http://www.semanticweb.org/cadex/ontologies/2020/1/untitled-ontology-71#isFrom"/>
        <rdfs:domain rdf:resource="http://www.semanticweb.org/cadex/ontologies/2020/1/untitled-ontology-71#Take"/>
        <rdfs:range rdf:resource="http://www.semanticweb.org/cadex/ontologies/2020/1/untitled-ontology-71#Shot"/>
        <rdfs:comment>This property creates link from a take and the shot it originated from.</rdfs:comment>
    </owl:ObjectProperty>
    


    <!-- http://www.semanticweb.org/cadex/ontologies/2020/1/untitled-ontology-71#takeProducesClip -->

    <owl:ObjectProperty rdf:about="http://www.semanticweb.org/cadex/ontologies/2020/1/untitled-ontology-71#takeProducesClip">
        <rdfs:subPropertyOf rdf:resource="http://www.semanticweb.org/cadex/ontologies/2020/1/untitled-ontology-71#produces"/>
        <rdfs:domain rdf:resource="http://www.semanticweb.org/cadex/ontologies/2020/1/untitled-ontology-71#Take"/>
        <rdfs:range rdf:resource="http://www.semanticweb.org/cadex/ontologies/2020/1/untitled-ontology-71#Clip"/>
        <rdfs:comment>This property is a sub-property of produces and creates a relationship between a take and the clip it forms.</rdfs:comment>
    </owl:ObjectProperty>
    


    <!-- http://www.semanticweb.org/cadex/ontologies/2020/1/untitled-ontology-71#takeUsesCamera -->

    <owl:ObjectProperty rdf:about="http://www.semanticweb.org/cadex/ontologies/2020/1/untitled-ontology-71#takeUsesCamera">
        <rdfs:subPropertyOf rdf:resource="http://www.semanticweb.org/cadex/ontologies/2020/1/untitled-ontology-71#usesCamera"/>
        <rdfs:domain rdf:resource="http://www.semanticweb.org/cadex/ontologies/2020/1/untitled-ontology-71#Take"/>
        <rdfs:range rdf:resource="http://www.semanticweb.org/cadex/ontologies/2020/1/untitled-ontology-71#Camera"/>
        <rdfs:comment>This property creates a link that describes how takes uses a camera.</rdfs:comment>
    </owl:ObjectProperty>
    


    <!-- http://www.semanticweb.org/cadex/ontologies/2020/1/untitled-ontology-71#takeUsesFisheyeLens -->

    <owl:ObjectProperty rdf:about="http://www.semanticweb.org/cadex/ontologies/2020/1/untitled-ontology-71#takeUsesFisheyeLens">
        <rdfs:subPropertyOf rdf:resource="http://www.semanticweb.org/cadex/ontologies/2020/1/untitled-ontology-71#takeUsesLens"/>
        <rdfs:domain rdf:resource="http://www.semanticweb.org/cadex/ontologies/2020/1/untitled-ontology-71#Take"/>
        <rdfs:range rdf:resource="http://www.semanticweb.org/cadex/ontologies/2020/1/untitled-ontology-71#FisheyeLens"/>
        <rdfs:comment>This property creates a relation between a fisheye lens and the take that uses it.</rdfs:comment>
    </owl:ObjectProperty>
    


    <!-- http://www.semanticweb.org/cadex/ontologies/2020/1/untitled-ontology-71#takeUsesLens -->

    <owl:ObjectProperty rdf:about="http://www.semanticweb.org/cadex/ontologies/2020/1/untitled-ontology-71#takeUsesLens">
        <rdfs:subPropertyOf rdf:resource="http://www.semanticweb.org/cadex/ontologies/2020/1/untitled-ontology-71#usesLens"/>
        <rdfs:domain rdf:resource="http://www.semanticweb.org/cadex/ontologies/2020/1/untitled-ontology-71#Take"/>
        <rdfs:range rdf:resource="http://www.semanticweb.org/cadex/ontologies/2020/1/untitled-ontology-71#Lens"/>
        <rdfs:comment>This property creates a relation between a lens and the take that uses it.</rdfs:comment>
    </owl:ObjectProperty>
    


    <!-- http://www.semanticweb.org/cadex/ontologies/2020/1/untitled-ontology-71#takeUsesRectilinearLens -->

    <owl:ObjectProperty rdf:about="http://www.semanticweb.org/cadex/ontologies/2020/1/untitled-ontology-71#takeUsesRectilinearLens">
        <rdfs:subPropertyOf rdf:resource="http://www.semanticweb.org/cadex/ontologies/2020/1/untitled-ontology-71#takeUsesLens"/>
        <rdfs:domain rdf:resource="http://www.semanticweb.org/cadex/ontologies/2020/1/untitled-ontology-71#Take"/>
        <rdfs:range rdf:resource="http://www.semanticweb.org/cadex/ontologies/2020/1/untitled-ontology-71#RectilinearLens"/>
        <rdfs:comment>This property creates a relation between a rectilinear lens and the take that uses it.</rdfs:comment>
    </owl:ObjectProperty>
    


    <!-- http://www.semanticweb.org/cadex/ontologies/2020/1/untitled-ontology-71#takeUsesSlate -->

    <owl:ObjectProperty rdf:about="http://www.semanticweb.org/cadex/ontologies/2020/1/untitled-ontology-71#takeUsesSlate">
        <rdfs:subPropertyOf rdf:resource="http://www.semanticweb.org/cadex/ontologies/2020/1/untitled-ontology-71#usesSlate"/>
        <rdfs:domain rdf:resource="http://www.semanticweb.org/cadex/ontologies/2020/1/untitled-ontology-71#Take"/>
        <rdfs:range rdf:resource="http://www.semanticweb.org/cadex/ontologies/2020/1/untitled-ontology-71#Slate"/>
        <rdfs:comment>This property creates a relation between a slate and the take that uses it.</rdfs:comment>
    </owl:ObjectProperty>
    


    <!-- http://www.semanticweb.org/cadex/ontologies/2020/1/untitled-ontology-71#takeUsesStereoLeftEyeLens -->

    <owl:ObjectProperty rdf:about="http://www.semanticweb.org/cadex/ontologies/2020/1/untitled-ontology-71#takeUsesStereoLeftEyeLens">
        <rdfs:subPropertyOf rdf:resource="http://www.semanticweb.org/cadex/ontologies/2020/1/untitled-ontology-71#takeUsesLens"/>
        <rdfs:domain rdf:resource="http://www.semanticweb.org/cadex/ontologies/2020/1/untitled-ontology-71#Take"/>
        <rdfs:range rdf:resource="http://www.semanticweb.org/cadex/ontologies/2020/1/untitled-ontology-71#StereoLeftEyeLens"/>
        <rdfs:comment>This property creates a relation between a stereo left eye lens and the take that uses it.</rdfs:comment>
    </owl:ObjectProperty>
    


    <!-- http://www.semanticweb.org/cadex/ontologies/2020/1/untitled-ontology-71#takeUsesStereoRightEyeLens -->

    <owl:ObjectProperty rdf:about="http://www.semanticweb.org/cadex/ontologies/2020/1/untitled-ontology-71#takeUsesStereoRightEyeLens">
        <rdfs:subPropertyOf rdf:resource="http://www.semanticweb.org/cadex/ontologies/2020/1/untitled-ontology-71#takeUsesLens"/>
        <rdfs:domain rdf:resource="http://www.semanticweb.org/cadex/ontologies/2020/1/untitled-ontology-71#Take"/>
        <rdfs:range rdf:resource="http://www.semanticweb.org/cadex/ontologies/2020/1/untitled-ontology-71#StereoRightEyeLens"/>
        <rdfs:comment>This property creates a relation between a stereo right eye lens and the take that uses it.</rdfs:comment>
    </owl:ObjectProperty>
    


    <!-- http://www.semanticweb.org/cadex/ontologies/2020/1/untitled-ontology-71#unitCreatedBy -->

    <owl:ObjectProperty rdf:about="http://www.semanticweb.org/cadex/ontologies/2020/1/untitled-ontology-71#unitCreatedBy">
        <rdfs:subPropertyOf rdf:resource="http://www.semanticweb.org/cadex/ontologies/2020/1/untitled-ontology-71#createdBy"/>
        <rdfs:domain rdf:resource="http://www.semanticweb.org/cadex/ontologies/2020/1/untitled-ontology-71#Unit"/>
        <rdfs:range rdf:resource="http://www.semanticweb.org/cadex/ontologies/2020/1/untitled-ontology-71#Staff"/>
        <rdfs:comment>This property creates a relation between a unit and the staff member that created it.</rdfs:comment>
    </owl:ObjectProperty>
    


    <!-- http://www.semanticweb.org/cadex/ontologies/2020/1/untitled-ontology-71#unitHasFacilitySupervisor -->

    <owl:ObjectProperty rdf:about="http://www.semanticweb.org/cadex/ontologies/2020/1/untitled-ontology-71#unitHasFacilitySupervisor">
        <rdfs:subPropertyOf rdf:resource="http://www.semanticweb.org/cadex/ontologies/2020/1/untitled-ontology-71#hasSupervisor"/>
        <rdfs:domain rdf:resource="http://www.semanticweb.org/cadex/ontologies/2020/1/untitled-ontology-71#Unit"/>
        <rdfs:range rdf:resource="http://www.semanticweb.org/cadex/ontologies/2020/1/untitled-ontology-71#Staff"/>
        <rdfs:comment>This property creates a relationship from a unit to a staff member that supervises faciltiies.</rdfs:comment>
    </owl:ObjectProperty>
    


    <!-- http://www.semanticweb.org/cadex/ontologies/2020/1/untitled-ontology-71#unitHasSlate -->

    <owl:ObjectProperty rdf:about="http://www.semanticweb.org/cadex/ontologies/2020/1/untitled-ontology-71#unitHasSlate">
        <rdfs:subPropertyOf rdf:resource="http://www.semanticweb.org/cadex/ontologies/2020/1/untitled-ontology-71#hasSlate"/>
        <rdfs:domain rdf:resource="http://www.semanticweb.org/cadex/ontologies/2020/1/untitled-ontology-71#Unit"/>
        <rdfs:range rdf:resource="http://www.semanticweb.org/cadex/ontologies/2020/1/untitled-ontology-71#Slate"/>
        <rdfs:comment>This property creates link between a unit and its associated slate in the project.</rdfs:comment>
    </owl:ObjectProperty>
    


    <!-- http://www.semanticweb.org/cadex/ontologies/2020/1/untitled-ontology-71#unitHasVFXSupervisor -->

    <owl:ObjectProperty rdf:about="http://www.semanticweb.org/cadex/ontologies/2020/1/untitled-ontology-71#unitHasVFXSupervisor">
        <rdfs:subPropertyOf rdf:resource="http://www.semanticweb.org/cadex/ontologies/2020/1/untitled-ontology-71#hasSupervisor"/>
        <rdfs:domain rdf:resource="http://www.semanticweb.org/cadex/ontologies/2020/1/untitled-ontology-71#Unit"/>
        <rdfs:range rdf:resource="http://www.semanticweb.org/cadex/ontologies/2020/1/untitled-ontology-71#Staff"/>
        <rdfs:comment>This property creates a relationship from a unit to a staff member that supervises VFX.</rdfs:comment>
    </owl:ObjectProperty>
    


    <!-- http://www.semanticweb.org/cadex/ontologies/2020/1/untitled-ontology-71#unitIsPartOfShoot -->

    <owl:ObjectProperty rdf:about="http://www.semanticweb.org/cadex/ontologies/2020/1/untitled-ontology-71#unitIsPartOfShoot">
        <rdfs:subPropertyOf rdf:resource="http://www.semanticweb.org/cadex/ontologies/2020/1/untitled-ontology-71#isPartOf"/>
        <rdfs:domain rdf:resource="http://www.semanticweb.org/cadex/ontologies/2020/1/untitled-ontology-71#Unit"/>
        <rdfs:range rdf:resource="http://www.semanticweb.org/cadex/ontologies/2020/1/untitled-ontology-71#Shoot"/>
        <rdfs:comment>This property creates link from a unit which forms a part of or is involved in a shoot.</rdfs:comment>
    </owl:ObjectProperty>
    


    <!-- http://www.semanticweb.org/cadex/ontologies/2020/1/untitled-ontology-71#unitUpdatedBy -->

    <owl:ObjectProperty rdf:about="http://www.semanticweb.org/cadex/ontologies/2020/1/untitled-ontology-71#unitUpdatedBy">
        <rdfs:subPropertyOf rdf:resource="http://www.semanticweb.org/cadex/ontologies/2020/1/untitled-ontology-71#updatedBy"/>
        <rdfs:domain rdf:resource="http://www.semanticweb.org/cadex/ontologies/2020/1/untitled-ontology-71#Unit"/>
        <rdfs:range rdf:resource="http://www.semanticweb.org/cadex/ontologies/2020/1/untitled-ontology-71#Staff"/>
        <rdfs:comment>This property creates a relation between a unit and the staff member that updated it.</rdfs:comment>
    </owl:ObjectProperty>
    


    <!-- http://www.semanticweb.org/cadex/ontologies/2020/1/untitled-ontology-71#unitUsesLens -->

    <owl:ObjectProperty rdf:about="http://www.semanticweb.org/cadex/ontologies/2020/1/untitled-ontology-71#unitUsesLens">
        <rdfs:subPropertyOf rdf:resource="http://www.semanticweb.org/cadex/ontologies/2020/1/untitled-ontology-71#usesLens"/>
        <rdfs:domain rdf:resource="http://www.semanticweb.org/cadex/ontologies/2020/1/untitled-ontology-71#Unit"/>
        <rdfs:range rdf:resource="http://www.semanticweb.org/cadex/ontologies/2020/1/untitled-ontology-71#Lens"/>
        <rdfs:comment>This property creates a relation between a lens and the unit that uses it.</rdfs:comment>
    </owl:ObjectProperty>
    


    <!-- http://www.semanticweb.org/cadex/ontologies/2020/1/untitled-ontology-71#updatedBy -->

    <owl:ObjectProperty rdf:about="http://www.semanticweb.org/cadex/ontologies/2020/1/untitled-ontology-71#updatedBy">
        <rdfs:subPropertyOf rdf:resource="http://www.semanticweb.org/cadex/ontologies/2020/1/untitled-ontology-71#by"/>
        <rdfs:range rdf:resource="http://www.semanticweb.org/cadex/ontologies/2020/1/untitled-ontology-71#Staff"/>
        <rdfs:comment>This property encapsulates all the sub-properties that describe who an entity has been updated by.</rdfs:comment>
    </owl:ObjectProperty>
    


    <!-- http://www.semanticweb.org/cadex/ontologies/2020/1/untitled-ontology-71#usedIn -->

    <owl:ObjectProperty rdf:about="http://www.semanticweb.org/cadex/ontologies/2020/1/untitled-ontology-71#usedIn">
        <rdfs:comment>This property encapsulates all the sub-properties that describe how an entity is used in an instance of another class.</rdfs:comment>
    </owl:ObjectProperty>
    


    <!-- http://www.semanticweb.org/cadex/ontologies/2020/1/untitled-ontology-71#uses -->

    <owl:ObjectProperty rdf:about="http://www.semanticweb.org/cadex/ontologies/2020/1/untitled-ontology-71#uses">
        <rdfs:comment>This property encapsulates all the sub-properties that describe how an entity *uses* an instance of another class.</rdfs:comment>
    </owl:ObjectProperty>
    


    <!-- http://www.semanticweb.org/cadex/ontologies/2020/1/untitled-ontology-71#usesCamera -->

    <owl:ObjectProperty rdf:about="http://www.semanticweb.org/cadex/ontologies/2020/1/untitled-ontology-71#usesCamera">
        <rdfs:subPropertyOf rdf:resource="http://www.semanticweb.org/cadex/ontologies/2020/1/untitled-ontology-71#uses"/>
        <rdfs:range rdf:resource="http://www.semanticweb.org/cadex/ontologies/2020/1/untitled-ontology-71#Camera"/>
        <rdfs:comment>This property encapsulates all the sub-properties that describe how an entity *uses* a camera.</rdfs:comment>
    </owl:ObjectProperty>
    


    <!-- http://www.semanticweb.org/cadex/ontologies/2020/1/untitled-ontology-71#usesCast -->

    <owl:ObjectProperty rdf:about="http://www.semanticweb.org/cadex/ontologies/2020/1/untitled-ontology-71#usesCast">
        <rdfs:subPropertyOf rdf:resource="http://www.semanticweb.org/cadex/ontologies/2020/1/untitled-ontology-71#usesPersonWithRole"/>
        <rdfs:range rdf:resource="http://www.semanticweb.org/cadex/ontologies/2020/1/untitled-ontology-71#Cast"/>
        <rdfs:comment>This property encapsulates all the sub-properties that describe how an entity *uses* a cast member.</rdfs:comment>
    </owl:ObjectProperty>
    


    <!-- http://www.semanticweb.org/cadex/ontologies/2020/1/untitled-ontology-71#usesCrane -->

    <owl:ObjectProperty rdf:about="http://www.semanticweb.org/cadex/ontologies/2020/1/untitled-ontology-71#usesCrane">
        <rdfs:subPropertyOf rdf:resource="http://www.semanticweb.org/cadex/ontologies/2020/1/untitled-ontology-71#uses"/>
        <rdfs:range rdf:resource="http://www.semanticweb.org/cadex/ontologies/2020/1/untitled-ontology-71#Crane"/>
        <rdfs:comment>This property encapsulates all the sub-properties that describe how an entity *uses* a crane.</rdfs:comment>
    </owl:ObjectProperty>
    


    <!-- http://www.semanticweb.org/cadex/ontologies/2020/1/untitled-ontology-71#usesHardDriveSnapshot -->

    <owl:ObjectProperty rdf:about="http://www.semanticweb.org/cadex/ontologies/2020/1/untitled-ontology-71#usesHardDriveSnapshot">
        <rdfs:subPropertyOf rdf:resource="http://www.semanticweb.org/cadex/ontologies/2020/1/untitled-ontology-71#uses"/>
        <rdfs:range rdf:resource="http://www.semanticweb.org/cadex/ontologies/2020/1/untitled-ontology-71#HardDriveSnapshot"/>
        <rdfs:comment>This property encapsulates all the sub-properties that describe how an entity *uses* a hard drive snapshot.</rdfs:comment>
    </owl:ObjectProperty>
    


    <!-- http://www.semanticweb.org/cadex/ontologies/2020/1/untitled-ontology-71#usesLUT -->

    <owl:ObjectProperty rdf:about="http://www.semanticweb.org/cadex/ontologies/2020/1/untitled-ontology-71#usesLUT">
        <rdfs:subPropertyOf rdf:resource="http://www.semanticweb.org/cadex/ontologies/2020/1/untitled-ontology-71#uses"/>
        <rdfs:range rdf:resource="http://www.semanticweb.org/cadex/ontologies/2020/1/untitled-ontology-71#LUT"/>
        <rdfs:comment>This property encapsulates all the sub-properties that describe how an entity *uses* a LUT.</rdfs:comment>
    </owl:ObjectProperty>
    


    <!-- http://www.semanticweb.org/cadex/ontologies/2020/1/untitled-ontology-71#usesLens -->

    <owl:ObjectProperty rdf:about="http://www.semanticweb.org/cadex/ontologies/2020/1/untitled-ontology-71#usesLens">
        <rdfs:subPropertyOf rdf:resource="http://www.semanticweb.org/cadex/ontologies/2020/1/untitled-ontology-71#uses"/>
        <rdfs:range rdf:resource="http://www.semanticweb.org/cadex/ontologies/2020/1/untitled-ontology-71#Lens"/>
        <rdfs:comment>This property encapsulates all the sub-properties that describe how an entity *uses* a lens.</rdfs:comment>
    </owl:ObjectProperty>
    


    <!-- http://www.semanticweb.org/cadex/ontologies/2020/1/untitled-ontology-71#usesPersonWithRole -->

    <owl:ObjectProperty rdf:about="http://www.semanticweb.org/cadex/ontologies/2020/1/untitled-ontology-71#usesPersonWithRole">
        <rdfs:subPropertyOf rdf:resource="http://www.semanticweb.org/cadex/ontologies/2020/1/untitled-ontology-71#uses"/>
        <rdfs:range rdf:resource="http://www.semanticweb.org/cadex/ontologies/2020/1/untitled-ontology-71#Person"/>
        <rdfs:comment>This property encapsulates all the sub-properties that describe how an entity *uses* a person. The sub-properties of usesPerson are split into smaller property hierarchies for each type of subclass of a person.</rdfs:comment>
    </owl:ObjectProperty>
    


    <!-- http://www.semanticweb.org/cadex/ontologies/2020/1/untitled-ontology-71#usesSlate -->

    <owl:ObjectProperty rdf:about="http://www.semanticweb.org/cadex/ontologies/2020/1/untitled-ontology-71#usesSlate">
        <rdfs:subPropertyOf rdf:resource="http://www.semanticweb.org/cadex/ontologies/2020/1/untitled-ontology-71#uses"/>
        <rdfs:range rdf:resource="http://www.semanticweb.org/cadex/ontologies/2020/1/untitled-ontology-71#Slate"/>
        <rdfs:comment>This property encapsulates all the sub-properties that describe how an entity *uses* a slate.</rdfs:comment>
    </owl:ObjectProperty>
    


    <!-- http://www.semanticweb.org/cadex/ontologies/2020/1/untitled-ontology-71#usesUnit -->

    <owl:ObjectProperty rdf:about="http://www.semanticweb.org/cadex/ontologies/2020/1/untitled-ontology-71#usesUnit">
        <rdfs:subPropertyOf rdf:resource="http://www.semanticweb.org/cadex/ontologies/2020/1/untitled-ontology-71#uses"/>
        <rdfs:range rdf:resource="http://www.semanticweb.org/cadex/ontologies/2020/1/untitled-ontology-71#Unit"/>
        <rdfs:comment>This property encapsulates all the sub-properties that describe how an entity *uses* a unit.</rdfs:comment>
    </owl:ObjectProperty>
    


    <!-- http://www.semanticweb.org/cadex/ontologies/2020/1/untitled-ontology-71#writtenBy -->

    <owl:ObjectProperty rdf:about="http://www.semanticweb.org/cadex/ontologies/2020/1/untitled-ontology-71#writtenBy">
        <rdfs:subPropertyOf rdf:resource="http://www.semanticweb.org/cadex/ontologies/2020/1/untitled-ontology-71#by"/>
        <rdfs:range rdf:resource="http://www.semanticweb.org/cadex/ontologies/2020/1/untitled-ontology-71#Writer"/>
        <rdfs:comment>This property encapsulates all the sub-properties that describe who an entity has been written by.</rdfs:comment>
    </owl:ObjectProperty>
    


    <!-- 
    ///////////////////////////////////////////////////////////////////////////////////////
    //
    // Data properties
    //
    ///////////////////////////////////////////////////////////////////////////////////////
     -->

    


    <!-- http://www.semanticweb.org/cadex/ontologies/2020/1/untitled-ontology-71#clipUpdatedOn -->

    <owl:DatatypeProperty rdf:about="http://www.semanticweb.org/cadex/ontologies/2020/1/untitled-ontology-71#clipUpdatedOn">
        <rdfs:subPropertyOf rdf:resource="http://www.semanticweb.org/cadex/ontologies/2020/1/untitled-ontology-71#hasClipInfo"/>
        <rdfs:domain rdf:resource="http://www.semanticweb.org/cadex/ontologies/2020/1/untitled-ontology-71#Clip"/>
        <rdfs:range rdf:resource="http://www.w3.org/2001/XMLSchema#dateTimeStamp"/>
        <rdfs:comment>This property represents a metadata field that indicates the date and time a clip was last updated.</rdfs:comment>
    </owl:DatatypeProperty>
    


    <!-- http://www.semanticweb.org/cadex/ontologies/2020/1/untitled-ontology-71#fileCreatedOn -->

    <owl:DatatypeProperty rdf:about="http://www.semanticweb.org/cadex/ontologies/2020/1/untitled-ontology-71#fileCreatedOn">
        <rdfs:subPropertyOf rdf:resource="http://www.semanticweb.org/cadex/ontologies/2020/1/untitled-ontology-71#hasFileInfo"/>
        <rdfs:domain rdf:resource="http://www.semanticweb.org/cadex/ontologies/2020/1/untitled-ontology-71#File"/>
        <rdfs:range rdf:resource="http://www.w3.org/2001/XMLSchema#dateTimeStamp"/>
        <rdfs:comment>This property represents a metadata field that indicates the date and time a file was created.</rdfs:comment>
    </owl:DatatypeProperty>
    


    <!-- http://www.semanticweb.org/cadex/ontologies/2020/1/untitled-ontology-71#fileUpdatedOn -->

    <owl:DatatypeProperty rdf:about="http://www.semanticweb.org/cadex/ontologies/2020/1/untitled-ontology-71#fileUpdatedOn">
        <rdfs:subPropertyOf rdf:resource="http://www.semanticweb.org/cadex/ontologies/2020/1/untitled-ontology-71#hasFileInfo"/>
        <rdfs:domain rdf:resource="http://www.semanticweb.org/cadex/ontologies/2020/1/untitled-ontology-71#File"/>
        <rdfs:range rdf:resource="http://www.w3.org/2001/XMLSchema#dateTimeStamp"/>
        <rdfs:comment>This property represents a metadata field that indicates the date and time a file was last updated.</rdfs:comment>
    </owl:DatatypeProperty>
    


    <!-- http://www.semanticweb.org/cadex/ontologies/2020/1/untitled-ontology-71#hasAssetInfo -->

    <owl:DatatypeProperty rdf:about="http://www.semanticweb.org/cadex/ontologies/2020/1/untitled-ontology-71#hasAssetInfo">
        <rdfs:domain rdf:resource="http://www.semanticweb.org/cadex/ontologies/2020/1/untitled-ontology-71#Asset"/>
        <rdfs:comment>This is the parent of a set of properties that represent metadata fields describing an asset. This property should not be populated with a value because it does not itself represent a metadata field. Rather, it is used solely to organise the properties representing fields.</rdfs:comment>
    </owl:DatatypeProperty>
    


    <!-- http://www.semanticweb.org/cadex/ontologies/2020/1/untitled-ontology-71#hasCameraBodyID -->

    <owl:DatatypeProperty rdf:about="http://www.semanticweb.org/cadex/ontologies/2020/1/untitled-ontology-71#hasCameraBodyID">
        <rdfs:subPropertyOf rdf:resource="http://www.semanticweb.org/cadex/ontologies/2020/1/untitled-ontology-71#hasCameraInfo"/>
        <rdfs:domain rdf:resource="http://www.semanticweb.org/cadex/ontologies/2020/1/untitled-ontology-71#Camera"/>
        <rdfs:range rdf:resource="http://www.w3.org/2001/XMLSchema#string"/>
        <rdfs:comment>This property represents a metadata field that indicates the ID of a camera&apos;s body.</rdfs:comment>
    </owl:DatatypeProperty>
    


    <!-- http://www.semanticweb.org/cadex/ontologies/2020/1/untitled-ontology-71#hasCameraBrandName -->

    <owl:DatatypeProperty rdf:about="http://www.semanticweb.org/cadex/ontologies/2020/1/untitled-ontology-71#hasCameraBrandName">
        <rdfs:subPropertyOf rdf:resource="http://www.semanticweb.org/cadex/ontologies/2020/1/untitled-ontology-71#hasCameraInfo"/>
        <rdfs:domain rdf:resource="http://www.semanticweb.org/cadex/ontologies/2020/1/untitled-ontology-71#Camera"/>
        <rdfs:range rdf:resource="http://www.w3.org/2001/XMLSchema#string"/>
        <rdfs:comment>This property represents a metadata field that indicates the brand name of a camera.</rdfs:comment>
    </owl:DatatypeProperty>
    


    <!-- http://www.semanticweb.org/cadex/ontologies/2020/1/untitled-ontology-71#hasCameraHead -->

    <owl:DatatypeProperty rdf:about="http://www.semanticweb.org/cadex/ontologies/2020/1/untitled-ontology-71#hasCameraHead">
        <rdfs:subPropertyOf rdf:resource="http://www.semanticweb.org/cadex/ontologies/2020/1/untitled-ontology-71#hasSlateCameraInfo"/>
        <rdfs:domain rdf:resource="http://www.semanticweb.org/cadex/ontologies/2020/1/untitled-ontology-71#Slate"/>
        <rdfs:range rdf:resource="http://www.w3.org/2001/XMLSchema#string"/>
        <rdfs:comment>This property represents a metadata field that indicates the head of a slate&apos;s camera.</rdfs:comment>
    </owl:DatatypeProperty>
    


    <!-- http://www.semanticweb.org/cadex/ontologies/2020/1/untitled-ontology-71#hasCameraHeight -->

    <owl:DatatypeProperty rdf:about="http://www.semanticweb.org/cadex/ontologies/2020/1/untitled-ontology-71#hasCameraHeight">
        <rdfs:subPropertyOf rdf:resource="http://www.semanticweb.org/cadex/ontologies/2020/1/untitled-ontology-71#hasSlateCameraInfo"/>
        <rdfs:domain rdf:resource="http://www.semanticweb.org/cadex/ontologies/2020/1/untitled-ontology-71#Slate"/>
        <rdfs:range rdf:resource="http://www.w3.org/2001/XMLSchema#string"/>
        <rdfs:comment>This property represents a metadata field that indicates the height of a slate&apos;s camera.</rdfs:comment>
    </owl:DatatypeProperty>
    


    <!-- http://www.semanticweb.org/cadex/ontologies/2020/1/untitled-ontology-71#hasCameraInfo -->

    <owl:DatatypeProperty rdf:about="http://www.semanticweb.org/cadex/ontologies/2020/1/untitled-ontology-71#hasCameraInfo">
        <rdfs:domain rdf:resource="http://www.semanticweb.org/cadex/ontologies/2020/1/untitled-ontology-71#Camera"/>
        <rdfs:comment>This is the parent of a set of properties that represent metadata fields describing a camera. This property should not be populated with a value because it does not itself represent a metadata field. Rather, it is used solely to organise the properties representing fields.</rdfs:comment>
    </owl:DatatypeProperty>
    


    <!-- http://www.semanticweb.org/cadex/ontologies/2020/1/untitled-ontology-71#hasCameraModelName -->

    <owl:DatatypeProperty rdf:about="http://www.semanticweb.org/cadex/ontologies/2020/1/untitled-ontology-71#hasCameraModelName">
        <rdfs:subPropertyOf rdf:resource="http://www.semanticweb.org/cadex/ontologies/2020/1/untitled-ontology-71#hasCameraInfo"/>
        <rdfs:domain rdf:resource="http://www.semanticweb.org/cadex/ontologies/2020/1/untitled-ontology-71#Camera"/>
        <rdfs:range rdf:resource="http://www.w3.org/2001/XMLSchema#string"/>
        <rdfs:comment>This property represents a metadata field that indicates the model name of a camera.</rdfs:comment>
    </owl:DatatypeProperty>
    


    <!-- http://www.semanticweb.org/cadex/ontologies/2020/1/untitled-ontology-71#hasCameraMount -->

    <owl:DatatypeProperty rdf:about="http://www.semanticweb.org/cadex/ontologies/2020/1/untitled-ontology-71#hasCameraMount">
        <rdfs:subPropertyOf rdf:resource="http://www.semanticweb.org/cadex/ontologies/2020/1/untitled-ontology-71#hasSlateCameraInfo"/>
        <rdfs:domain rdf:resource="http://www.semanticweb.org/cadex/ontologies/2020/1/untitled-ontology-71#Slate"/>
        <rdfs:range rdf:resource="http://www.w3.org/2001/XMLSchema#string"/>
        <rdfs:comment>This property represents a metadata field that indicates the mount of a slate&apos;s camera.</rdfs:comment>
    </owl:DatatypeProperty>
    


    <!-- http://www.semanticweb.org/cadex/ontologies/2020/1/untitled-ontology-71#hasCameraMove -->

    <owl:DatatypeProperty rdf:about="http://www.semanticweb.org/cadex/ontologies/2020/1/untitled-ontology-71#hasCameraMove">
        <rdfs:subPropertyOf rdf:resource="http://www.semanticweb.org/cadex/ontologies/2020/1/untitled-ontology-71#hasSlateCameraInfo"/>
        <rdfs:domain rdf:resource="http://www.semanticweb.org/cadex/ontologies/2020/1/untitled-ontology-71#Slate"/>
        <rdfs:range rdf:resource="http://www.w3.org/2001/XMLSchema#string"/>
        <rdfs:comment>This property represents a metadata field that indicates the move of a slate&apos;s camera.</rdfs:comment>
    </owl:DatatypeProperty>
    


    <!-- http://www.semanticweb.org/cadex/ontologies/2020/1/untitled-ontology-71#hasCameraNav -->

    <owl:DatatypeProperty rdf:about="http://www.semanticweb.org/cadex/ontologies/2020/1/untitled-ontology-71#hasCameraNav">
        <rdfs:subPropertyOf rdf:resource="http://www.semanticweb.org/cadex/ontologies/2020/1/untitled-ontology-71#hasSlateCameraInfo"/>
        <rdfs:domain rdf:resource="http://www.semanticweb.org/cadex/ontologies/2020/1/untitled-ontology-71#Slate"/>
        <rdfs:range rdf:resource="http://www.w3.org/2001/XMLSchema#string"/>
        <rdfs:comment>This property represents a metadata field that indicates the navigation of a slate&apos;s camera.</rdfs:comment>
    </owl:DatatypeProperty>
    


    <!-- http://www.semanticweb.org/cadex/ontologies/2020/1/untitled-ontology-71#hasCameraReportNumber -->

    <owl:DatatypeProperty rdf:about="http://www.semanticweb.org/cadex/ontologies/2020/1/untitled-ontology-71#hasCameraReportNumber">
        <rdfs:subPropertyOf rdf:resource="http://www.semanticweb.org/cadex/ontologies/2020/1/untitled-ontology-71#hasSlateCameraInfo"/>
        <rdfs:domain rdf:resource="http://www.semanticweb.org/cadex/ontologies/2020/1/untitled-ontology-71#Slate"/>
        <rdfs:range rdf:resource="http://www.w3.org/2001/XMLSchema#int"/>
        <rdfs:comment>This property represents a metadata field that indicates the report number of a slate&apos;s camera.</rdfs:comment>
    </owl:DatatypeProperty>
    


    <!-- http://www.semanticweb.org/cadex/ontologies/2020/1/untitled-ontology-71#hasCameraRollInfo -->

    <owl:DatatypeProperty rdf:about="http://www.semanticweb.org/cadex/ontologies/2020/1/untitled-ontology-71#hasCameraRollInfo">
        <rdfs:subPropertyOf rdf:resource="http://www.semanticweb.org/cadex/ontologies/2020/1/untitled-ontology-71#hasRollInfo"/>
        <rdfs:domain rdf:resource="http://www.semanticweb.org/cadex/ontologies/2020/1/untitled-ontology-71#CameraRoll"/>
        <rdfs:comment>This is the parent of a set of properties that represent metadata fields describing a camera roll. This property should not be populated with a value because it does not itself represent a metadata field. Rather, it is used solely to organise the properties representing fields.</rdfs:comment>
    </owl:DatatypeProperty>
    


    <!-- http://www.semanticweb.org/cadex/ontologies/2020/1/untitled-ontology-71#hasCameraRollNumber -->

    <owl:DatatypeProperty rdf:about="http://www.semanticweb.org/cadex/ontologies/2020/1/untitled-ontology-71#hasCameraRollNumber">
        <rdfs:subPropertyOf rdf:resource="http://www.semanticweb.org/cadex/ontologies/2020/1/untitled-ontology-71#hasCameraRollInfo"/>
        <rdfs:domain rdf:resource="http://www.semanticweb.org/cadex/ontologies/2020/1/untitled-ontology-71#CameraRoll"/>
        <rdfs:range rdf:resource="http://www.w3.org/2001/XMLSchema#string"/>
        <rdfs:comment>This property represents a metadata field that indicates the roll number of a camera roll.</rdfs:comment>
    </owl:DatatypeProperty>
    


    <!-- http://www.semanticweb.org/cadex/ontologies/2020/1/untitled-ontology-71#hasCameraType -->

    <owl:DatatypeProperty rdf:about="http://www.semanticweb.org/cadex/ontologies/2020/1/untitled-ontology-71#hasCameraType">
        <rdfs:subPropertyOf rdf:resource="http://www.semanticweb.org/cadex/ontologies/2020/1/untitled-ontology-71#hasCameraInfo"/>
        <rdfs:domain rdf:resource="http://www.semanticweb.org/cadex/ontologies/2020/1/untitled-ontology-71#Camera"/>
        <rdfs:range rdf:resource="http://www.w3.org/2001/XMLSchema#string"/>
        <rdfs:comment>This property represents a metadata field that indicates the type of a camera.</rdfs:comment>
    </owl:DatatypeProperty>
    


    <!-- http://www.semanticweb.org/cadex/ontologies/2020/1/untitled-ontology-71#hasCastInfo -->

    <owl:DatatypeProperty rdf:about="http://www.semanticweb.org/cadex/ontologies/2020/1/untitled-ontology-71#hasCastInfo">
        <rdfs:subPropertyOf rdf:resource="http://www.semanticweb.org/cadex/ontologies/2020/1/untitled-ontology-71#hasPersonInfo"/>
        <rdfs:domain rdf:resource="http://www.semanticweb.org/cadex/ontologies/2020/1/untitled-ontology-71#Cast"/>
        <rdfs:comment>This is the parent of a set of properties that represent metadata fields describing a person with a role of cast. This property should not be populated with a value because it does not itself represent a metadata field. Rather, it is used solely to organise the properties representing fields.</rdfs:comment>
    </owl:DatatypeProperty>
    


    <!-- http://www.semanticweb.org/cadex/ontologies/2020/1/untitled-ontology-71#hasCastName -->

    <owl:DatatypeProperty rdf:about="http://www.semanticweb.org/cadex/ontologies/2020/1/untitled-ontology-71#hasCastName">
        <rdfs:subPropertyOf rdf:resource="http://www.semanticweb.org/cadex/ontologies/2020/1/untitled-ontology-71#hasCastInfo"/>
        <rdfs:domain rdf:resource="http://www.semanticweb.org/cadex/ontologies/2020/1/untitled-ontology-71#Cast"/>
        <rdfs:range rdf:resource="http://www.w3.org/2001/XMLSchema#string"/>
        <rdfs:comment>This property represents a metadata field that indicates the name of a cast member.</rdfs:comment>
    </owl:DatatypeProperty>
    


    <!-- http://www.semanticweb.org/cadex/ontologies/2020/1/untitled-ontology-71#hasClientAccountNumber -->

    <owl:DatatypeProperty rdf:about="http://www.semanticweb.org/cadex/ontologies/2020/1/untitled-ontology-71#hasClientAccountNumber">
        <rdfs:subPropertyOf rdf:resource="http://www.semanticweb.org/cadex/ontologies/2020/1/untitled-ontology-71#hasClientInfo"/>
        <rdfs:domain rdf:resource="http://www.semanticweb.org/cadex/ontologies/2020/1/untitled-ontology-71#Client"/>
        <rdfs:range rdf:resource="http://www.w3.org/2001/XMLSchema#string"/>
        <rdfs:comment>This property represents a metadata field that indicates the account number of a client.</rdfs:comment>
    </owl:DatatypeProperty>
    


    <!-- http://www.semanticweb.org/cadex/ontologies/2020/1/untitled-ontology-71#hasClientCompany -->

    <owl:DatatypeProperty rdf:about="http://www.semanticweb.org/cadex/ontologies/2020/1/untitled-ontology-71#hasClientCompany">
        <rdfs:subPropertyOf rdf:resource="http://www.semanticweb.org/cadex/ontologies/2020/1/untitled-ontology-71#hasClientInfo"/>
        <rdfs:domain rdf:resource="http://www.semanticweb.org/cadex/ontologies/2020/1/untitled-ontology-71#Client"/>
        <rdfs:range rdf:resource="http://www.w3.org/2001/XMLSchema#string"/>
        <rdfs:comment>This property represents a metadata field that indicates the compnay name of a client.</rdfs:comment>
    </owl:DatatypeProperty>
    


    <!-- http://www.semanticweb.org/cadex/ontologies/2020/1/untitled-ontology-71#hasClientEmailAddress -->

    <owl:DatatypeProperty rdf:about="http://www.semanticweb.org/cadex/ontologies/2020/1/untitled-ontology-71#hasClientEmailAddress">
        <rdfs:subPropertyOf rdf:resource="http://www.semanticweb.org/cadex/ontologies/2020/1/untitled-ontology-71#hasClientInfo"/>
        <rdfs:domain rdf:resource="http://www.semanticweb.org/cadex/ontologies/2020/1/untitled-ontology-71#Client"/>
        <rdfs:range rdf:resource="http://www.w3.org/2001/XMLSchema#string"/>
        <rdfs:comment>This property represents a metadata field that indicates the email address of a client.</rdfs:comment>
    </owl:DatatypeProperty>
    


    <!-- http://www.semanticweb.org/cadex/ontologies/2020/1/untitled-ontology-71#hasClientInfo -->

    <owl:DatatypeProperty rdf:about="http://www.semanticweb.org/cadex/ontologies/2020/1/untitled-ontology-71#hasClientInfo">
        <rdfs:subPropertyOf rdf:resource="http://www.semanticweb.org/cadex/ontologies/2020/1/untitled-ontology-71#hasPersonInfo"/>
        <rdfs:domain rdf:resource="http://www.semanticweb.org/cadex/ontologies/2020/1/untitled-ontology-71#Client"/>
        <rdfs:comment>This is the parent of a set of properties that represent metadata fields describing a person with a role of client. This property should not be populated with a value because it does not itself represent a metadata field. Rather, it is used solely to organise the properties representing fields.</rdfs:comment>
    </owl:DatatypeProperty>
    


    <!-- http://www.semanticweb.org/cadex/ontologies/2020/1/untitled-ontology-71#hasClientName -->

    <owl:DatatypeProperty rdf:about="http://www.semanticweb.org/cadex/ontologies/2020/1/untitled-ontology-71#hasClientName">
        <rdfs:subPropertyOf rdf:resource="http://www.semanticweb.org/cadex/ontologies/2020/1/untitled-ontology-71#hasClientInfo"/>
        <rdfs:domain rdf:resource="http://www.semanticweb.org/cadex/ontologies/2020/1/untitled-ontology-71#Client"/>
        <rdfs:range rdf:resource="http://www.w3.org/2001/XMLSchema#string"/>
        <rdfs:comment>This property represents a metadata field that indicates the name of a client.</rdfs:comment>
    </owl:DatatypeProperty>
    


    <!-- http://www.semanticweb.org/cadex/ontologies/2020/1/untitled-ontology-71#hasClientPostalAddress -->

    <owl:DatatypeProperty rdf:about="http://www.semanticweb.org/cadex/ontologies/2020/1/untitled-ontology-71#hasClientPostalAddress">
        <rdfs:subPropertyOf rdf:resource="http://www.semanticweb.org/cadex/ontologies/2020/1/untitled-ontology-71#hasClientInfo"/>
        <rdfs:domain rdf:resource="http://www.semanticweb.org/cadex/ontologies/2020/1/untitled-ontology-71#Client"/>
        <rdfs:range rdf:resource="http://www.w3.org/2001/XMLSchema#string"/>
        <rdfs:comment>This property represents a metadata field that indicates the postal address of a client.</rdfs:comment>
    </owl:DatatypeProperty>
    


    <!-- http://www.semanticweb.org/cadex/ontologies/2020/1/untitled-ontology-71#hasClipASCSAT -->

    <owl:DatatypeProperty rdf:about="http://www.semanticweb.org/cadex/ontologies/2020/1/untitled-ontology-71#hasClipASCSAT">
        <rdfs:subPropertyOf rdf:resource="http://www.semanticweb.org/cadex/ontologies/2020/1/untitled-ontology-71#hasClipInfo"/>
        <rdfs:domain rdf:resource="http://www.semanticweb.org/cadex/ontologies/2020/1/untitled-ontology-71#Clip"/>
        <rdfs:range rdf:resource="http://www.w3.org/2001/XMLSchema#float"/>
        <rdfs:comment>This property represents a metadata field that indicates the colour decision list (CDL) for the saturation of a clip.</rdfs:comment>
    </owl:DatatypeProperty>
    


    <!-- http://www.semanticweb.org/cadex/ontologies/2020/1/untitled-ontology-71#hasClipASCSOP -->

    <owl:DatatypeProperty rdf:about="http://www.semanticweb.org/cadex/ontologies/2020/1/untitled-ontology-71#hasClipASCSOP">
        <rdfs:subPropertyOf rdf:resource="http://www.semanticweb.org/cadex/ontologies/2020/1/untitled-ontology-71#hasClipInfo"/>
        <rdfs:domain rdf:resource="http://www.semanticweb.org/cadex/ontologies/2020/1/untitled-ontology-71#Clip"/>
        <rdfs:range rdf:resource="http://www.w3.org/2001/XMLSchema#string"/>
        <rdfs:comment>This property represents a metadata field that indicates the colour correction values for the lift, gamma, and gain of a clip.</rdfs:comment>
    </owl:DatatypeProperty>
    


    <!-- http://www.semanticweb.org/cadex/ontologies/2020/1/untitled-ontology-71#hasClipActiveHeight -->

    <owl:DatatypeProperty rdf:about="http://www.semanticweb.org/cadex/ontologies/2020/1/untitled-ontology-71#hasClipActiveHeight">
        <rdfs:subPropertyOf rdf:resource="http://www.semanticweb.org/cadex/ontologies/2020/1/untitled-ontology-71#hasClipInfo"/>
        <rdfs:domain rdf:resource="http://www.semanticweb.org/cadex/ontologies/2020/1/untitled-ontology-71#Clip"/>
        <rdfs:range rdf:resource="http://www.w3.org/2001/XMLSchema#int"/>
        <rdfs:comment>This property represents a metadata field that indicates the active height of a clip.</rdfs:comment>
    </owl:DatatypeProperty>
    


    <!-- http://www.semanticweb.org/cadex/ontologies/2020/1/untitled-ontology-71#hasClipActiveWidth -->

    <owl:DatatypeProperty rdf:about="http://www.semanticweb.org/cadex/ontologies/2020/1/untitled-ontology-71#hasClipActiveWidth">
        <rdfs:subPropertyOf rdf:resource="http://www.semanticweb.org/cadex/ontologies/2020/1/untitled-ontology-71#hasClipInfo"/>
        <rdfs:domain rdf:resource="http://www.semanticweb.org/cadex/ontologies/2020/1/untitled-ontology-71#Clip"/>
        <rdfs:range rdf:resource="http://www.w3.org/2001/XMLSchema#int"/>
        <rdfs:comment>This property represents a metadata field that indicates the active width of a clip.</rdfs:comment>
    </owl:DatatypeProperty>
    


    <!-- http://www.semanticweb.org/cadex/ontologies/2020/1/untitled-ontology-71#hasClipAudioBitDepth -->

    <owl:DatatypeProperty rdf:about="http://www.semanticweb.org/cadex/ontologies/2020/1/untitled-ontology-71#hasClipAudioBitDepth">
        <rdfs:subPropertyOf rdf:resource="http://www.semanticweb.org/cadex/ontologies/2020/1/untitled-ontology-71#hasClipAudioInfo"/>
        <rdfs:domain rdf:resource="http://www.semanticweb.org/cadex/ontologies/2020/1/untitled-ontology-71#Clip"/>
        <rdfs:range rdf:resource="http://www.w3.org/2001/XMLSchema#float"/>
        <rdfs:comment>This property represents a metadata field that indicates the bit depth of a clip&apos;s audio.</rdfs:comment>
    </owl:DatatypeProperty>
    


    <!-- http://www.semanticweb.org/cadex/ontologies/2020/1/untitled-ontology-71#hasClipAudioBitRate -->

    <owl:DatatypeProperty rdf:about="http://www.semanticweb.org/cadex/ontologies/2020/1/untitled-ontology-71#hasClipAudioBitRate">
        <rdfs:subPropertyOf rdf:resource="http://www.semanticweb.org/cadex/ontologies/2020/1/untitled-ontology-71#hasClipAudioInfo"/>
        <rdfs:domain rdf:resource="http://www.semanticweb.org/cadex/ontologies/2020/1/untitled-ontology-71#Clip"/>
        <rdfs:range rdf:resource="http://www.w3.org/2001/XMLSchema#float"/>
        <rdfs:comment>This property represents a metadata field that indicates the bit rate of a clip&apos;s audio.</rdfs:comment>
    </owl:DatatypeProperty>
    


    <!-- http://www.semanticweb.org/cadex/ontologies/2020/1/untitled-ontology-71#hasClipAudioCodec -->

    <owl:DatatypeProperty rdf:about="http://www.semanticweb.org/cadex/ontologies/2020/1/untitled-ontology-71#hasClipAudioCodec">
        <rdfs:subPropertyOf rdf:resource="http://www.semanticweb.org/cadex/ontologies/2020/1/untitled-ontology-71#hasClipAudioInfo"/>
        <rdfs:domain rdf:resource="http://www.semanticweb.org/cadex/ontologies/2020/1/untitled-ontology-71#Clip"/>
        <rdfs:range rdf:resource="http://www.w3.org/2001/XMLSchema#string"/>
        <rdfs:comment>This property represents a metadata field that indicates the codec of a clip&apos;s audio.</rdfs:comment>
    </owl:DatatypeProperty>
    


    <!-- http://www.semanticweb.org/cadex/ontologies/2020/1/untitled-ontology-71#hasClipAudioEndianness -->

    <owl:DatatypeProperty rdf:about="http://www.semanticweb.org/cadex/ontologies/2020/1/untitled-ontology-71#hasClipAudioEndianness">
        <rdfs:subPropertyOf rdf:resource="http://www.semanticweb.org/cadex/ontologies/2020/1/untitled-ontology-71#hasClipAudioInfo"/>
        <rdfs:domain rdf:resource="http://www.semanticweb.org/cadex/ontologies/2020/1/untitled-ontology-71#Clip"/>
        <rdfs:range rdf:resource="http://www.w3.org/2001/XMLSchema#string"/>
        <rdfs:comment>This property represents a metadata field that indicates the endianess of a clip&apos;s audio.</rdfs:comment>
    </owl:DatatypeProperty>
    


    <!-- http://www.semanticweb.org/cadex/ontologies/2020/1/untitled-ontology-71#hasClipAudioFormat -->

    <owl:DatatypeProperty rdf:about="http://www.semanticweb.org/cadex/ontologies/2020/1/untitled-ontology-71#hasClipAudioFormat">
        <rdfs:subPropertyOf rdf:resource="http://www.semanticweb.org/cadex/ontologies/2020/1/untitled-ontology-71#hasClipAudioInfo"/>
        <rdfs:domain rdf:resource="http://www.semanticweb.org/cadex/ontologies/2020/1/untitled-ontology-71#Clip"/>
        <rdfs:range rdf:resource="http://www.w3.org/2001/XMLSchema#string"/>
        <rdfs:comment>This property represents a metadata field that indicates the format of a clip&apos;s audio.</rdfs:comment>
    </owl:DatatypeProperty>
    


    <!-- http://www.semanticweb.org/cadex/ontologies/2020/1/untitled-ontology-71#hasClipAudioInfo -->

    <owl:DatatypeProperty rdf:about="http://www.semanticweb.org/cadex/ontologies/2020/1/untitled-ontology-71#hasClipAudioInfo">
        <rdfs:subPropertyOf rdf:resource="http://www.semanticweb.org/cadex/ontologies/2020/1/untitled-ontology-71#hasClipInfo"/>
        <rdfs:domain rdf:resource="http://www.semanticweb.org/cadex/ontologies/2020/1/untitled-ontology-71#Clip"/>
        <rdfs:comment>This is the parent of a set of properties that represent metadata fields describing the audio information of a clip. This property should not be populated with a value because it does not itself represent a metadata field. Rather, it is used solely to organise the properties representing fields.</rdfs:comment>
    </owl:DatatypeProperty>
    


    <!-- http://www.semanticweb.org/cadex/ontologies/2020/1/untitled-ontology-71#hasClipAudioMode -->

    <owl:DatatypeProperty rdf:about="http://www.semanticweb.org/cadex/ontologies/2020/1/untitled-ontology-71#hasClipAudioMode">
        <rdfs:subPropertyOf rdf:resource="http://www.semanticweb.org/cadex/ontologies/2020/1/untitled-ontology-71#hasClipAudioInfo"/>
        <rdfs:domain rdf:resource="http://www.semanticweb.org/cadex/ontologies/2020/1/untitled-ontology-71#Clip"/>
        <rdfs:range rdf:resource="http://www.w3.org/2001/XMLSchema#string"/>
        <rdfs:comment>This property represents a metadata field that indicates the mode of a clip&apos;s audio.</rdfs:comment>
    </owl:DatatypeProperty>
    


    <!-- http://www.semanticweb.org/cadex/ontologies/2020/1/untitled-ontology-71#hasClipAudioSamplingRate -->

    <owl:DatatypeProperty rdf:about="http://www.semanticweb.org/cadex/ontologies/2020/1/untitled-ontology-71#hasClipAudioSamplingRate">
        <rdfs:subPropertyOf rdf:resource="http://www.semanticweb.org/cadex/ontologies/2020/1/untitled-ontology-71#hasClipAudioInfo"/>
        <rdfs:domain rdf:resource="http://www.semanticweb.org/cadex/ontologies/2020/1/untitled-ontology-71#Clip"/>
        <rdfs:range rdf:resource="http://www.w3.org/2001/XMLSchema#float"/>
        <rdfs:comment>This property represents a metadata field that indicates the sampling rate of a clip&apos;s audio.</rdfs:comment>
    </owl:DatatypeProperty>
    


    <!-- http://www.semanticweb.org/cadex/ontologies/2020/1/untitled-ontology-71#hasClipBitRateMode -->

    <owl:DatatypeProperty rdf:about="http://www.semanticweb.org/cadex/ontologies/2020/1/untitled-ontology-71#hasClipBitRateMode">
        <rdfs:subPropertyOf rdf:resource="http://www.semanticweb.org/cadex/ontologies/2020/1/untitled-ontology-71#hasClipInfo"/>
        <rdfs:domain rdf:resource="http://www.semanticweb.org/cadex/ontologies/2020/1/untitled-ontology-71#Clip"/>
        <rdfs:range rdf:resource="http://www.w3.org/2001/XMLSchema#string"/>
        <rdfs:comment>This property represents a metadata field that indicates the bit rate mode of a clip.</rdfs:comment>
    </owl:DatatypeProperty>
    


    <!-- http://www.semanticweb.org/cadex/ontologies/2020/1/untitled-ontology-71#hasClipCameraFormat -->

    <owl:DatatypeProperty rdf:about="http://www.semanticweb.org/cadex/ontologies/2020/1/untitled-ontology-71#hasClipCameraFormat">
        <rdfs:subPropertyOf rdf:resource="http://www.semanticweb.org/cadex/ontologies/2020/1/untitled-ontology-71#hasClipInfo"/>
        <rdfs:domain rdf:resource="http://www.semanticweb.org/cadex/ontologies/2020/1/untitled-ontology-71#Clip"/>
        <rdfs:range rdf:resource="http://www.w3.org/2001/XMLSchema#string"/>
        <rdfs:comment>This property represents a metadata field that indicates the format of a clip&apos;s camera.</rdfs:comment>
    </owl:DatatypeProperty>
    


    <!-- http://www.semanticweb.org/cadex/ontologies/2020/1/untitled-ontology-71#hasClipCameraRole -->

    <owl:DatatypeProperty rdf:about="http://www.semanticweb.org/cadex/ontologies/2020/1/untitled-ontology-71#hasClipCameraRole">
        <rdfs:subPropertyOf rdf:resource="http://www.semanticweb.org/cadex/ontologies/2020/1/untitled-ontology-71#hasClipInfo"/>
        <rdfs:domain rdf:resource="http://www.semanticweb.org/cadex/ontologies/2020/1/untitled-ontology-71#Clip"/>
        <rdfs:range rdf:resource="http://www.w3.org/2001/XMLSchema#string"/>
        <rdfs:comment>This property represents a metadata field that indicates the role of a clip&apos;s camera.</rdfs:comment>
    </owl:DatatypeProperty>
    


    <!-- http://www.semanticweb.org/cadex/ontologies/2020/1/untitled-ontology-71#hasClipCameraTimecode -->

    <owl:DatatypeProperty rdf:about="http://www.semanticweb.org/cadex/ontologies/2020/1/untitled-ontology-71#hasClipCameraTimecode">
        <rdfs:subPropertyOf rdf:resource="http://www.semanticweb.org/cadex/ontologies/2020/1/untitled-ontology-71#hasClipInfo"/>
        <rdfs:domain rdf:resource="http://www.semanticweb.org/cadex/ontologies/2020/1/untitled-ontology-71#Clip"/>
        <rdfs:range rdf:resource="http://www.w3.org/2001/XMLSchema#string"/>
        <rdfs:comment>This property represents a metadata field that indicates the timecode of a clip&apos;s camera.</rdfs:comment>
    </owl:DatatypeProperty>
    


    <!-- http://www.semanticweb.org/cadex/ontologies/2020/1/untitled-ontology-71#hasClipChromaSubsampling -->

    <owl:DatatypeProperty rdf:about="http://www.semanticweb.org/cadex/ontologies/2020/1/untitled-ontology-71#hasClipChromaSubsampling">
        <rdfs:subPropertyOf rdf:resource="http://www.semanticweb.org/cadex/ontologies/2020/1/untitled-ontology-71#hasClipInfo"/>
        <rdfs:domain rdf:resource="http://www.semanticweb.org/cadex/ontologies/2020/1/untitled-ontology-71#Clip"/>
        <rdfs:range rdf:resource="http://www.w3.org/2001/XMLSchema#string"/>
        <rdfs:comment>This property represents a metadata field that indicates the chroma subsampling of a clip.</rdfs:comment>
    </owl:DatatypeProperty>
    


    <!-- http://www.semanticweb.org/cadex/ontologies/2020/1/untitled-ontology-71#hasClipColourSpace -->

    <owl:DatatypeProperty rdf:about="http://www.semanticweb.org/cadex/ontologies/2020/1/untitled-ontology-71#hasClipColourSpace">
        <rdfs:subPropertyOf rdf:resource="http://www.semanticweb.org/cadex/ontologies/2020/1/untitled-ontology-71#hasClipInfo"/>
        <rdfs:domain rdf:resource="http://www.semanticweb.org/cadex/ontologies/2020/1/untitled-ontology-71#Clip"/>
        <rdfs:range rdf:resource="http://www.w3.org/2001/XMLSchema#string"/>
        <rdfs:comment>This property represents a metadata field that indicates the colour space of a clip.</rdfs:comment>
    </owl:DatatypeProperty>
    


    <!-- http://www.semanticweb.org/cadex/ontologies/2020/1/untitled-ontology-71#hasClipComment -->

    <owl:DatatypeProperty rdf:about="http://www.semanticweb.org/cadex/ontologies/2020/1/untitled-ontology-71#hasClipComment">
        <rdfs:subPropertyOf rdf:resource="http://www.semanticweb.org/cadex/ontologies/2020/1/untitled-ontology-71#hasClipInfo"/>
        <rdfs:domain rdf:resource="http://www.semanticweb.org/cadex/ontologies/2020/1/untitled-ontology-71#Clip"/>
        <rdfs:range rdf:resource="http://www.w3.org/2001/XMLSchema#string"/>
        <rdfs:comment>This property represents a metadata field that attaches a comment to a clip.</rdfs:comment>
    </owl:DatatypeProperty>
    


    <!-- http://www.semanticweb.org/cadex/ontologies/2020/1/untitled-ontology-71#hasClipDisplayAspectRatio -->

    <owl:DatatypeProperty rdf:about="http://www.semanticweb.org/cadex/ontologies/2020/1/untitled-ontology-71#hasClipDisplayAspectRatio">
        <rdfs:subPropertyOf rdf:resource="http://www.semanticweb.org/cadex/ontologies/2020/1/untitled-ontology-71#hasClipInfo"/>
        <rdfs:domain rdf:resource="http://www.semanticweb.org/cadex/ontologies/2020/1/untitled-ontology-71#Clip"/>
        <rdfs:range rdf:resource="http://www.w3.org/2001/XMLSchema#string"/>
        <rdfs:comment>This property represents a metadata field that indicates the display aspect ratio of a clip.</rdfs:comment>
    </owl:DatatypeProperty>
    


    <!-- http://www.semanticweb.org/cadex/ontologies/2020/1/untitled-ontology-71#hasClipDuration -->

    <owl:DatatypeProperty rdf:about="http://www.semanticweb.org/cadex/ontologies/2020/1/untitled-ontology-71#hasClipDuration">
        <rdfs:subPropertyOf rdf:resource="http://www.semanticweb.org/cadex/ontologies/2020/1/untitled-ontology-71#hasClipInfo"/>
        <rdfs:domain rdf:resource="http://www.semanticweb.org/cadex/ontologies/2020/1/untitled-ontology-71#Clip"/>
        <rdfs:range rdf:resource="http://www.w3.org/2001/XMLSchema#string"/>
        <rdfs:comment>This property represents a metadata field that indicates the duration of a clip.</rdfs:comment>
    </owl:DatatypeProperty>
    


    <!-- http://www.semanticweb.org/cadex/ontologies/2020/1/untitled-ontology-71#hasClipEditName -->

    <owl:DatatypeProperty rdf:about="http://www.semanticweb.org/cadex/ontologies/2020/1/untitled-ontology-71#hasClipEditName">
        <rdfs:subPropertyOf rdf:resource="http://www.semanticweb.org/cadex/ontologies/2020/1/untitled-ontology-71#hasClipInfo"/>
        <rdfs:domain rdf:resource="http://www.semanticweb.org/cadex/ontologies/2020/1/untitled-ontology-71#Clip"/>
        <rdfs:range rdf:resource="http://www.w3.org/2001/XMLSchema#string"/>
        <rdfs:comment>This property represents a metadata field that indicates the edit name of a clip.</rdfs:comment>
    </owl:DatatypeProperty>
    


    <!-- http://www.semanticweb.org/cadex/ontologies/2020/1/untitled-ontology-71#hasClipEndTimecode -->

    <owl:DatatypeProperty rdf:about="http://www.semanticweb.org/cadex/ontologies/2020/1/untitled-ontology-71#hasClipEndTimecode">
        <rdfs:subPropertyOf rdf:resource="http://www.semanticweb.org/cadex/ontologies/2020/1/untitled-ontology-71#hasClipInfo"/>
        <rdfs:domain rdf:resource="http://www.semanticweb.org/cadex/ontologies/2020/1/untitled-ontology-71#Clip"/>
        <rdfs:range rdf:resource="http://www.w3.org/2001/XMLSchema#string"/>
        <rdfs:comment>This property represents a metadata field that indicates the end timecode of a clip.</rdfs:comment>
    </owl:DatatypeProperty>
    


    <!-- http://www.semanticweb.org/cadex/ontologies/2020/1/untitled-ontology-71#hasClipEvent -->

    <owl:DatatypeProperty rdf:about="http://www.semanticweb.org/cadex/ontologies/2020/1/untitled-ontology-71#hasClipEvent">
        <rdfs:subPropertyOf rdf:resource="http://www.semanticweb.org/cadex/ontologies/2020/1/untitled-ontology-71#hasClipInfo"/>
        <rdfs:domain rdf:resource="http://www.semanticweb.org/cadex/ontologies/2020/1/untitled-ontology-71#Clip"/>
        <rdfs:range rdf:resource="http://www.w3.org/2001/XMLSchema#int"/>
    </owl:DatatypeProperty>
    


    <!-- http://www.semanticweb.org/cadex/ontologies/2020/1/untitled-ontology-71#hasClipFix -->

    <owl:DatatypeProperty rdf:about="http://www.semanticweb.org/cadex/ontologies/2020/1/untitled-ontology-71#hasClipFix">
        <rdfs:subPropertyOf rdf:resource="http://www.semanticweb.org/cadex/ontologies/2020/1/untitled-ontology-71#hasClipInfo"/>
        <rdfs:domain rdf:resource="http://www.semanticweb.org/cadex/ontologies/2020/1/untitled-ontology-71#Clip"/>
        <rdfs:range rdf:resource="http://www.w3.org/2001/XMLSchema#boolean"/>
    </owl:DatatypeProperty>
    


    <!-- http://www.semanticweb.org/cadex/ontologies/2020/1/untitled-ontology-71#hasClipFormat -->

    <owl:DatatypeProperty rdf:about="http://www.semanticweb.org/cadex/ontologies/2020/1/untitled-ontology-71#hasClipFormat">
        <rdfs:subPropertyOf rdf:resource="http://www.semanticweb.org/cadex/ontologies/2020/1/untitled-ontology-71#hasClipInfo"/>
        <rdfs:domain rdf:resource="http://www.semanticweb.org/cadex/ontologies/2020/1/untitled-ontology-71#Clip"/>
        <rdfs:range rdf:resource="http://www.w3.org/2001/XMLSchema#string"/>
        <rdfs:comment>This property represents a metadata field that indicates the format of a clip.</rdfs:comment>
    </owl:DatatypeProperty>
    


    <!-- http://www.semanticweb.org/cadex/ontologies/2020/1/untitled-ontology-71#hasClipFrameCountEnd -->

    <owl:DatatypeProperty rdf:about="http://www.semanticweb.org/cadex/ontologies/2020/1/untitled-ontology-71#hasClipFrameCountEnd">
        <rdfs:subPropertyOf rdf:resource="http://www.semanticweb.org/cadex/ontologies/2020/1/untitled-ontology-71#hasClipInfo"/>
        <rdfs:domain rdf:resource="http://www.semanticweb.org/cadex/ontologies/2020/1/untitled-ontology-71#Clip"/>
        <rdfs:range rdf:resource="http://www.w3.org/2001/XMLSchema#int"/>
    </owl:DatatypeProperty>
    


    <!-- http://www.semanticweb.org/cadex/ontologies/2020/1/untitled-ontology-71#hasClipFrameCountStart -->

    <owl:DatatypeProperty rdf:about="http://www.semanticweb.org/cadex/ontologies/2020/1/untitled-ontology-71#hasClipFrameCountStart">
        <rdfs:subPropertyOf rdf:resource="http://www.semanticweb.org/cadex/ontologies/2020/1/untitled-ontology-71#hasClipInfo"/>
        <rdfs:domain rdf:resource="http://www.semanticweb.org/cadex/ontologies/2020/1/untitled-ontology-71#Clip"/>
        <rdfs:range rdf:resource="http://www.w3.org/2001/XMLSchema#int"/>
    </owl:DatatypeProperty>
    


    <!-- http://www.semanticweb.org/cadex/ontologies/2020/1/untitled-ontology-71#hasClipFrameRate -->

    <owl:DatatypeProperty rdf:about="http://www.semanticweb.org/cadex/ontologies/2020/1/untitled-ontology-71#hasClipFrameRate">
        <rdfs:subPropertyOf rdf:resource="http://www.semanticweb.org/cadex/ontologies/2020/1/untitled-ontology-71#hasClipInfo"/>
        <rdfs:domain rdf:resource="http://www.semanticweb.org/cadex/ontologies/2020/1/untitled-ontology-71#Clip"/>
        <rdfs:range rdf:resource="http://www.w3.org/2001/XMLSchema#float"/>
        <rdfs:comment>This property represents a metadata field that indicates the frame rate of a clip.</rdfs:comment>
    </owl:DatatypeProperty>
    


    <!-- http://www.semanticweb.org/cadex/ontologies/2020/1/untitled-ontology-71#hasClipFrameRateMode -->

    <owl:DatatypeProperty rdf:about="http://www.semanticweb.org/cadex/ontologies/2020/1/untitled-ontology-71#hasClipFrameRateMode">
        <rdfs:subPropertyOf rdf:resource="http://www.semanticweb.org/cadex/ontologies/2020/1/untitled-ontology-71#hasClipInfo"/>
        <rdfs:domain rdf:resource="http://www.semanticweb.org/cadex/ontologies/2020/1/untitled-ontology-71#Clip"/>
        <rdfs:range rdf:resource="http://www.w3.org/2001/XMLSchema#string"/>
        <rdfs:comment>This property represents a metadata field that indicates the frame rate mode of a clip.</rdfs:comment>
    </owl:DatatypeProperty>
    


    <!-- http://www.semanticweb.org/cadex/ontologies/2020/1/untitled-ontology-71#hasClipFramingType -->

    <owl:DatatypeProperty rdf:about="http://www.semanticweb.org/cadex/ontologies/2020/1/untitled-ontology-71#hasClipFramingType">
        <rdfs:subPropertyOf rdf:resource="http://www.semanticweb.org/cadex/ontologies/2020/1/untitled-ontology-71#hasClipInfo"/>
        <rdfs:domain rdf:resource="http://www.semanticweb.org/cadex/ontologies/2020/1/untitled-ontology-71#Clip"/>
        <rdfs:range rdf:resource="http://www.w3.org/2001/XMLSchema#string"/>
        <rdfs:comment>This property represents a metadata field that indicates the framing type of a clip.</rdfs:comment>
    </owl:DatatypeProperty>
    


    <!-- http://www.semanticweb.org/cadex/ontologies/2020/1/untitled-ontology-71#hasClipGPSTimeStamp -->

    <owl:DatatypeProperty rdf:about="http://www.semanticweb.org/cadex/ontologies/2020/1/untitled-ontology-71#hasClipGPSTimeStamp">
        <rdfs:subPropertyOf rdf:resource="http://www.semanticweb.org/cadex/ontologies/2020/1/untitled-ontology-71#hasClipInfo"/>
        <rdfs:domain rdf:resource="http://www.semanticweb.org/cadex/ontologies/2020/1/untitled-ontology-71#Clip"/>
        <rdfs:range rdf:resource="http://www.w3.org/2001/XMLSchema#dateTimeStamp"/>
        <rdfs:comment>This property represents a metadata field that indicates the GPS timestamp of a clip.</rdfs:comment>
    </owl:DatatypeProperty>
    


    <!-- http://www.semanticweb.org/cadex/ontologies/2020/1/untitled-ontology-71#hasClipHeight -->

    <owl:DatatypeProperty rdf:about="http://www.semanticweb.org/cadex/ontologies/2020/1/untitled-ontology-71#hasClipHeight">
        <rdfs:subPropertyOf rdf:resource="http://www.semanticweb.org/cadex/ontologies/2020/1/untitled-ontology-71#hasClipVideoInfo"/>
        <rdfs:domain rdf:resource="http://www.semanticweb.org/cadex/ontologies/2020/1/untitled-ontology-71#Clip"/>
        <rdfs:range rdf:resource="http://www.w3.org/2001/XMLSchema#int"/>
        <rdfs:comment>This property represents a metadata field that indicates the height of a clip&apos;s video.</rdfs:comment>
    </owl:DatatypeProperty>
    


    <!-- http://www.semanticweb.org/cadex/ontologies/2020/1/untitled-ontology-71#hasClipISO -->

    <owl:DatatypeProperty rdf:about="http://www.semanticweb.org/cadex/ontologies/2020/1/untitled-ontology-71#hasClipISO">
        <rdfs:subPropertyOf rdf:resource="http://www.semanticweb.org/cadex/ontologies/2020/1/untitled-ontology-71#hasClipInfo"/>
        <rdfs:domain rdf:resource="http://www.semanticweb.org/cadex/ontologies/2020/1/untitled-ontology-71#Clip"/>
        <rdfs:range rdf:resource="http://www.w3.org/2001/XMLSchema#int"/>
        <rdfs:comment>This property represents a metadata field that indicates the ISO of a clip.</rdfs:comment>
    </owl:DatatypeProperty>
    


    <!-- http://www.semanticweb.org/cadex/ontologies/2020/1/untitled-ontology-71#hasClipInfo -->

    <owl:DatatypeProperty rdf:about="http://www.semanticweb.org/cadex/ontologies/2020/1/untitled-ontology-71#hasClipInfo">
        <rdfs:subPropertyOf rdf:resource="http://www.semanticweb.org/cadex/ontologies/2020/1/untitled-ontology-71#hasAssetInfo"/>
        <rdfs:domain rdf:resource="http://www.semanticweb.org/cadex/ontologies/2020/1/untitled-ontology-71#Clip"/>
        <rdfs:comment>This is the parent of a set of properties that represent metadata fields describing a clip. This property should not be populated with a value because it does not itself represent a metadata field. Rather, it is used solely to organise the properties representing fields.</rdfs:comment>
    </owl:DatatypeProperty>
    


    <!-- http://www.semanticweb.org/cadex/ontologies/2020/1/untitled-ontology-71#hasClipInkDuration -->

    <owl:DatatypeProperty rdf:about="http://www.semanticweb.org/cadex/ontologies/2020/1/untitled-ontology-71#hasClipInkDuration">
        <rdfs:subPropertyOf rdf:resource="http://www.semanticweb.org/cadex/ontologies/2020/1/untitled-ontology-71#hasClipInfo"/>
        <rdfs:domain rdf:resource="http://www.semanticweb.org/cadex/ontologies/2020/1/untitled-ontology-71#Clip"/>
        <rdfs:range rdf:resource="http://www.w3.org/2001/XMLSchema#string"/>
    </owl:DatatypeProperty>
    


    <!-- http://www.semanticweb.org/cadex/ontologies/2020/1/untitled-ontology-71#hasClipInkNumber -->

    <owl:DatatypeProperty rdf:about="http://www.semanticweb.org/cadex/ontologies/2020/1/untitled-ontology-71#hasClipInkNumber">
        <rdfs:subPropertyOf rdf:resource="http://www.semanticweb.org/cadex/ontologies/2020/1/untitled-ontology-71#hasClipInfo"/>
        <rdfs:domain rdf:resource="http://www.semanticweb.org/cadex/ontologies/2020/1/untitled-ontology-71#Clip"/>
        <rdfs:range rdf:resource="http://www.w3.org/2001/XMLSchema#int"/>
    </owl:DatatypeProperty>
    


    <!-- http://www.semanticweb.org/cadex/ontologies/2020/1/untitled-ontology-71#hasClipInputFormat -->

    <owl:DatatypeProperty rdf:about="http://www.semanticweb.org/cadex/ontologies/2020/1/untitled-ontology-71#hasClipInputFormat">
        <rdfs:subPropertyOf rdf:resource="http://www.semanticweb.org/cadex/ontologies/2020/1/untitled-ontology-71#hasClipInfo"/>
        <rdfs:domain rdf:resource="http://www.semanticweb.org/cadex/ontologies/2020/1/untitled-ontology-71#Clip"/>
        <rdfs:range rdf:resource="http://www.w3.org/2001/XMLSchema#string"/>
        <rdfs:comment>This property represents a metadata field that indicates the input format of a clip.</rdfs:comment>
    </owl:DatatypeProperty>
    


    <!-- http://www.semanticweb.org/cadex/ontologies/2020/1/untitled-ontology-71#hasClipKNCopy -->

    <owl:DatatypeProperty rdf:about="http://www.semanticweb.org/cadex/ontologies/2020/1/untitled-ontology-71#hasClipKNCopy">
        <rdfs:subPropertyOf rdf:resource="http://www.semanticweb.org/cadex/ontologies/2020/1/untitled-ontology-71#hasClipInfo"/>
        <rdfs:domain rdf:resource="http://www.semanticweb.org/cadex/ontologies/2020/1/untitled-ontology-71#Clip"/>
        <rdfs:range rdf:resource="http://www.w3.org/2001/XMLSchema#string"/>
    </owl:DatatypeProperty>
    


    <!-- http://www.semanticweb.org/cadex/ontologies/2020/1/untitled-ontology-71#hasClipKNStart -->

    <owl:DatatypeProperty rdf:about="http://www.semanticweb.org/cadex/ontologies/2020/1/untitled-ontology-71#hasClipKNStart">
        <rdfs:subPropertyOf rdf:resource="http://www.semanticweb.org/cadex/ontologies/2020/1/untitled-ontology-71#hasClipInfo"/>
        <rdfs:domain rdf:resource="http://www.semanticweb.org/cadex/ontologies/2020/1/untitled-ontology-71#Clip"/>
        <rdfs:range rdf:resource="http://www.w3.org/2001/XMLSchema#string"/>
    </owl:DatatypeProperty>
    


    <!-- http://www.semanticweb.org/cadex/ontologies/2020/1/untitled-ontology-71#hasClipLTO -->

    <owl:DatatypeProperty rdf:about="http://www.semanticweb.org/cadex/ontologies/2020/1/untitled-ontology-71#hasClipLTO">
        <rdfs:subPropertyOf rdf:resource="http://www.semanticweb.org/cadex/ontologies/2020/1/untitled-ontology-71#hasClipInfo"/>
        <rdfs:domain rdf:resource="http://www.semanticweb.org/cadex/ontologies/2020/1/untitled-ontology-71#Clip"/>
        <rdfs:range rdf:resource="http://www.w3.org/2001/XMLSchema#string"/>
    </owl:DatatypeProperty>
    


    <!-- http://www.semanticweb.org/cadex/ontologies/2020/1/untitled-ontology-71#hasClipLabRoll -->

    <owl:DatatypeProperty rdf:about="http://www.semanticweb.org/cadex/ontologies/2020/1/untitled-ontology-71#hasClipLabRoll">
        <rdfs:subPropertyOf rdf:resource="http://www.semanticweb.org/cadex/ontologies/2020/1/untitled-ontology-71#hasClipInfo"/>
        <rdfs:domain rdf:resource="http://www.semanticweb.org/cadex/ontologies/2020/1/untitled-ontology-71#Clip"/>
        <rdfs:range rdf:resource="http://www.w3.org/2001/XMLSchema#string"/>
        <rdfs:comment>This property represents a metadata field that indicates the ID of a lab roll for a clip.</rdfs:comment>
    </owl:DatatypeProperty>
    


    <!-- http://www.semanticweb.org/cadex/ontologies/2020/1/untitled-ontology-71#hasClipLengthInFrames -->

    <owl:DatatypeProperty rdf:about="http://www.semanticweb.org/cadex/ontologies/2020/1/untitled-ontology-71#hasClipLengthInFrames">
        <rdfs:subPropertyOf rdf:resource="http://www.semanticweb.org/cadex/ontologies/2020/1/untitled-ontology-71#hasClipInfo"/>
        <rdfs:domain rdf:resource="http://www.semanticweb.org/cadex/ontologies/2020/1/untitled-ontology-71#Clip"/>
        <rdfs:range rdf:resource="http://www.w3.org/2001/XMLSchema#int"/>
        <rdfs:comment>This property represents a metadata field that indicates the length of a clip in frames.</rdfs:comment>
    </owl:DatatypeProperty>
    


    <!-- http://www.semanticweb.org/cadex/ontologies/2020/1/untitled-ontology-71#hasClipMarkIn -->

    <owl:DatatypeProperty rdf:about="http://www.semanticweb.org/cadex/ontologies/2020/1/untitled-ontology-71#hasClipMarkIn">
        <rdfs:subPropertyOf rdf:resource="http://www.semanticweb.org/cadex/ontologies/2020/1/untitled-ontology-71#hasClipInfo"/>
        <rdfs:domain rdf:resource="http://www.semanticweb.org/cadex/ontologies/2020/1/untitled-ontology-71#Clip"/>
        <rdfs:range rdf:resource="http://www.w3.org/2001/XMLSchema#string"/>
    </owl:DatatypeProperty>
    


    <!-- http://www.semanticweb.org/cadex/ontologies/2020/1/untitled-ontology-71#hasClipMasterName -->

    <owl:DatatypeProperty rdf:about="http://www.semanticweb.org/cadex/ontologies/2020/1/untitled-ontology-71#hasClipMasterName">
        <rdfs:subPropertyOf rdf:resource="http://www.semanticweb.org/cadex/ontologies/2020/1/untitled-ontology-71#hasClipInfo"/>
        <rdfs:domain rdf:resource="http://www.semanticweb.org/cadex/ontologies/2020/1/untitled-ontology-71#Clip"/>
        <rdfs:range rdf:resource="http://www.w3.org/2001/XMLSchema#string"/>
        <rdfs:comment>This property represents a metadata field that indicates the master name of a clip.</rdfs:comment>
    </owl:DatatypeProperty>
    


    <!-- http://www.semanticweb.org/cadex/ontologies/2020/1/untitled-ontology-71#hasClipNumberOfAudioStreams -->

    <owl:DatatypeProperty rdf:about="http://www.semanticweb.org/cadex/ontologies/2020/1/untitled-ontology-71#hasClipNumberOfAudioStreams">
        <rdfs:subPropertyOf rdf:resource="http://www.semanticweb.org/cadex/ontologies/2020/1/untitled-ontology-71#hasClipInfo"/>
        <rdfs:domain rdf:resource="http://www.semanticweb.org/cadex/ontologies/2020/1/untitled-ontology-71#Clip"/>
        <rdfs:range rdf:resource="http://www.w3.org/2001/XMLSchema#int"/>
        <rdfs:comment>This property represents a metadata field that indicates the number of audio streams in a clip.</rdfs:comment>
    </owl:DatatypeProperty>
    


    <!-- http://www.semanticweb.org/cadex/ontologies/2020/1/untitled-ontology-71#hasClipNumberOfVideoStreams -->

    <owl:DatatypeProperty rdf:about="http://www.semanticweb.org/cadex/ontologies/2020/1/untitled-ontology-71#hasClipNumberOfVideoStreams">
        <rdfs:subPropertyOf rdf:resource="http://www.semanticweb.org/cadex/ontologies/2020/1/untitled-ontology-71#hasClipInfo"/>
        <rdfs:domain rdf:resource="http://www.semanticweb.org/cadex/ontologies/2020/1/untitled-ontology-71#Clip"/>
        <rdfs:range rdf:resource="http://www.w3.org/2001/XMLSchema#int"/>
        <rdfs:comment>This property represents a metadata field that indicates the number of video streams in a clip.</rdfs:comment>
    </owl:DatatypeProperty>
    


    <!-- http://www.semanticweb.org/cadex/ontologies/2020/1/untitled-ontology-71#hasClipOutputFormat -->

    <owl:DatatypeProperty rdf:about="http://www.semanticweb.org/cadex/ontologies/2020/1/untitled-ontology-71#hasClipOutputFormat">
        <rdfs:subPropertyOf rdf:resource="http://www.semanticweb.org/cadex/ontologies/2020/1/untitled-ontology-71#hasClipInfo"/>
        <rdfs:domain rdf:resource="http://www.semanticweb.org/cadex/ontologies/2020/1/untitled-ontology-71#Clip"/>
        <rdfs:range rdf:resource="http://www.w3.org/2001/XMLSchema#string"/>
        <rdfs:comment>This property represents a metadata field that indicates the output format of a clip.</rdfs:comment>
    </owl:DatatypeProperty>
    


    <!-- http://www.semanticweb.org/cadex/ontologies/2020/1/untitled-ontology-71#hasClipOverallBitRate -->

    <owl:DatatypeProperty rdf:about="http://www.semanticweb.org/cadex/ontologies/2020/1/untitled-ontology-71#hasClipOverallBitRate">
        <rdfs:subPropertyOf rdf:resource="http://www.semanticweb.org/cadex/ontologies/2020/1/untitled-ontology-71#hasClipInfo"/>
        <rdfs:domain rdf:resource="http://www.semanticweb.org/cadex/ontologies/2020/1/untitled-ontology-71#Clip"/>
        <rdfs:range rdf:resource="http://www.w3.org/2001/XMLSchema#float"/>
        <rdfs:comment>This property represents a metadata field that indicates the overall bit rate of a clip.</rdfs:comment>
    </owl:DatatypeProperty>
    


    <!-- http://www.semanticweb.org/cadex/ontologies/2020/1/untitled-ontology-71#hasClipPixelAspectRatio -->

    <owl:DatatypeProperty rdf:about="http://www.semanticweb.org/cadex/ontologies/2020/1/untitled-ontology-71#hasClipPixelAspectRatio">
        <rdfs:subPropertyOf rdf:resource="http://www.semanticweb.org/cadex/ontologies/2020/1/untitled-ontology-71#hasClipInfo"/>
        <rdfs:domain rdf:resource="http://www.semanticweb.org/cadex/ontologies/2020/1/untitled-ontology-71#Clip"/>
        <rdfs:range rdf:resource="http://www.w3.org/2001/XMLSchema#string"/>
        <rdfs:comment>This property represents a metadata field that indicates the pixel aspect ratio of a clip.</rdfs:comment>
    </owl:DatatypeProperty>
    


    <!-- http://www.semanticweb.org/cadex/ontologies/2020/1/untitled-ontology-71#hasClipQualityCheck -->

    <owl:DatatypeProperty rdf:about="http://www.semanticweb.org/cadex/ontologies/2020/1/untitled-ontology-71#hasClipQualityCheck">
        <rdfs:subPropertyOf rdf:resource="http://www.semanticweb.org/cadex/ontologies/2020/1/untitled-ontology-71#hasClipInfo"/>
        <rdfs:domain rdf:resource="http://www.semanticweb.org/cadex/ontologies/2020/1/untitled-ontology-71#Clip"/>
        <rdfs:range rdf:resource="http://www.w3.org/2001/XMLSchema#boolean"/>
        <rdfs:comment>This property represents a metadata field that indicates whether a clip has passed through quality control checks.</rdfs:comment>
    </owl:DatatypeProperty>
    


    <!-- http://www.semanticweb.org/cadex/ontologies/2020/1/untitled-ontology-71#hasClipStartTimecode -->

    <owl:DatatypeProperty rdf:about="http://www.semanticweb.org/cadex/ontologies/2020/1/untitled-ontology-71#hasClipStartTimecode">
        <rdfs:subPropertyOf rdf:resource="http://www.semanticweb.org/cadex/ontologies/2020/1/untitled-ontology-71#hasClipInfo"/>
        <rdfs:domain rdf:resource="http://www.semanticweb.org/cadex/ontologies/2020/1/untitled-ontology-71#Clip"/>
        <rdfs:range rdf:resource="http://www.w3.org/2001/XMLSchema#string"/>
        <rdfs:comment>This property represents a metadata field that indicates the start timecode of a clip.</rdfs:comment>
    </owl:DatatypeProperty>
    


    <!-- http://www.semanticweb.org/cadex/ontologies/2020/1/untitled-ontology-71#hasClipTXSlate -->

    <owl:DatatypeProperty rdf:about="http://www.semanticweb.org/cadex/ontologies/2020/1/untitled-ontology-71#hasClipTXSlate">
        <rdfs:subPropertyOf rdf:resource="http://www.semanticweb.org/cadex/ontologies/2020/1/untitled-ontology-71#hasClipInfo"/>
        <rdfs:domain rdf:resource="http://www.semanticweb.org/cadex/ontologies/2020/1/untitled-ontology-71#Clip"/>
        <rdfs:range rdf:resource="http://www.w3.org/2001/XMLSchema#string"/>
    </owl:DatatypeProperty>
    


    <!-- http://www.semanticweb.org/cadex/ontologies/2020/1/untitled-ontology-71#hasClipTapeName -->

    <owl:DatatypeProperty rdf:about="http://www.semanticweb.org/cadex/ontologies/2020/1/untitled-ontology-71#hasClipTapeName">
        <rdfs:subPropertyOf rdf:resource="http://www.semanticweb.org/cadex/ontologies/2020/1/untitled-ontology-71#hasClipInfo"/>
        <rdfs:domain rdf:resource="http://www.semanticweb.org/cadex/ontologies/2020/1/untitled-ontology-71#Clip"/>
        <rdfs:range rdf:resource="http://www.w3.org/2001/XMLSchema#string"/>
        <rdfs:comment>This property represents a metadata field that indicates the name of the tape a clip resides on.</rdfs:comment>
    </owl:DatatypeProperty>
    


    <!-- http://www.semanticweb.org/cadex/ontologies/2020/1/untitled-ontology-71#hasClipTrack -->

    <owl:DatatypeProperty rdf:about="http://www.semanticweb.org/cadex/ontologies/2020/1/untitled-ontology-71#hasClipTrack">
        <rdfs:subPropertyOf rdf:resource="http://www.semanticweb.org/cadex/ontologies/2020/1/untitled-ontology-71#hasClipInfo"/>
        <rdfs:domain rdf:resource="http://www.semanticweb.org/cadex/ontologies/2020/1/untitled-ontology-71#Clip"/>
        <rdfs:range rdf:resource="http://www.w3.org/2001/XMLSchema#string"/>
    </owl:DatatypeProperty>
    


    <!-- http://www.semanticweb.org/cadex/ontologies/2020/1/untitled-ontology-71#hasClipUnitRole -->

    <owl:DatatypeProperty rdf:about="http://www.semanticweb.org/cadex/ontologies/2020/1/untitled-ontology-71#hasClipUnitRole">
        <rdfs:subPropertyOf rdf:resource="http://www.semanticweb.org/cadex/ontologies/2020/1/untitled-ontology-71#hasClipInfo"/>
        <rdfs:domain rdf:resource="http://www.semanticweb.org/cadex/ontologies/2020/1/untitled-ontology-71#Clip"/>
        <rdfs:range rdf:resource="http://www.w3.org/2001/XMLSchema#string"/>
        <rdfs:comment>This property represents a metadata field that indicates the role of a unit in a clip.</rdfs:comment>
    </owl:DatatypeProperty>
    


    <!-- http://www.semanticweb.org/cadex/ontologies/2020/1/untitled-ontology-71#hasClipVideoBitRate -->

    <owl:DatatypeProperty rdf:about="http://www.semanticweb.org/cadex/ontologies/2020/1/untitled-ontology-71#hasClipVideoBitRate">
        <rdfs:subPropertyOf rdf:resource="http://www.semanticweb.org/cadex/ontologies/2020/1/untitled-ontology-71#hasClipVideoInfo"/>
        <rdfs:domain rdf:resource="http://www.semanticweb.org/cadex/ontologies/2020/1/untitled-ontology-71#Clip"/>
        <rdfs:range rdf:resource="http://www.w3.org/2001/XMLSchema#float"/>
        <rdfs:comment>This property represents a metadata field that indicates the bit rate of a clip&apos;s video.</rdfs:comment>
    </owl:DatatypeProperty>
    


    <!-- http://www.semanticweb.org/cadex/ontologies/2020/1/untitled-ontology-71#hasClipVideoCodec -->

    <owl:DatatypeProperty rdf:about="http://www.semanticweb.org/cadex/ontologies/2020/1/untitled-ontology-71#hasClipVideoCodec">
        <rdfs:subPropertyOf rdf:resource="http://www.semanticweb.org/cadex/ontologies/2020/1/untitled-ontology-71#hasClipVideoInfo"/>
        <rdfs:domain rdf:resource="http://www.semanticweb.org/cadex/ontologies/2020/1/untitled-ontology-71#Clip"/>
        <rdfs:range rdf:resource="http://www.w3.org/2001/XMLSchema#string"/>
        <rdfs:comment>This property represents a metadata field that indicates the codec of a clip&apos;s video.</rdfs:comment>
    </owl:DatatypeProperty>
    


    <!-- http://www.semanticweb.org/cadex/ontologies/2020/1/untitled-ontology-71#hasClipVideoFormat -->

    <owl:DatatypeProperty rdf:about="http://www.semanticweb.org/cadex/ontologies/2020/1/untitled-ontology-71#hasClipVideoFormat">
        <rdfs:subPropertyOf rdf:resource="http://www.semanticweb.org/cadex/ontologies/2020/1/untitled-ontology-71#hasClipVideoInfo"/>
        <rdfs:domain rdf:resource="http://www.semanticweb.org/cadex/ontologies/2020/1/untitled-ontology-71#Clip"/>
        <rdfs:range rdf:resource="http://www.w3.org/2001/XMLSchema#string"/>
        <rdfs:comment>This property represents a metadata field that indicates the format of a clip&apos;s video.</rdfs:comment>
    </owl:DatatypeProperty>
    


    <!-- http://www.semanticweb.org/cadex/ontologies/2020/1/untitled-ontology-71#hasClipVideoFormatVersion -->

    <owl:DatatypeProperty rdf:about="http://www.semanticweb.org/cadex/ontologies/2020/1/untitled-ontology-71#hasClipVideoFormatVersion">
        <rdfs:subPropertyOf rdf:resource="http://www.semanticweb.org/cadex/ontologies/2020/1/untitled-ontology-71#hasClipVideoInfo"/>
        <rdfs:domain rdf:resource="http://www.semanticweb.org/cadex/ontologies/2020/1/untitled-ontology-71#Clip"/>
        <rdfs:range rdf:resource="http://www.w3.org/2001/XMLSchema#string"/>
        <rdfs:comment>This property represents a metadata field that indicates the format version of a clip&apos;s video.</rdfs:comment>
    </owl:DatatypeProperty>
    


    <!-- http://www.semanticweb.org/cadex/ontologies/2020/1/untitled-ontology-71#hasClipVideoInfo -->

    <owl:DatatypeProperty rdf:about="http://www.semanticweb.org/cadex/ontologies/2020/1/untitled-ontology-71#hasClipVideoInfo">
        <rdfs:subPropertyOf rdf:resource="http://www.semanticweb.org/cadex/ontologies/2020/1/untitled-ontology-71#hasClipInfo"/>
        <rdfs:domain rdf:resource="http://www.semanticweb.org/cadex/ontologies/2020/1/untitled-ontology-71#Clip"/>
        <rdfs:comment>This is the parent of a set of properties that represent metadata fields describing the video information of a clip. This property should not be populated with a value because it does not itself represent a metadata field. Rather, it is used solely to organise the properties representing fields.</rdfs:comment>
    </owl:DatatypeProperty>
    


    <!-- http://www.semanticweb.org/cadex/ontologies/2020/1/untitled-ontology-71#hasClipVideoMode -->

    <owl:DatatypeProperty rdf:about="http://www.semanticweb.org/cadex/ontologies/2020/1/untitled-ontology-71#hasClipVideoMode">
        <rdfs:subPropertyOf rdf:resource="http://www.semanticweb.org/cadex/ontologies/2020/1/untitled-ontology-71#hasClipVideoInfo"/>
        <rdfs:domain rdf:resource="http://www.semanticweb.org/cadex/ontologies/2020/1/untitled-ontology-71#Clip"/>
        <rdfs:range rdf:resource="http://www.w3.org/2001/XMLSchema#string"/>
        <rdfs:comment>This property represents a metadata field that indicates the mode of a clip&apos;s video.</rdfs:comment>
    </owl:DatatypeProperty>
    


    <!-- http://www.semanticweb.org/cadex/ontologies/2020/1/untitled-ontology-71#hasClipVideoProfile -->

    <owl:DatatypeProperty rdf:about="http://www.semanticweb.org/cadex/ontologies/2020/1/untitled-ontology-71#hasClipVideoProfile">
        <rdfs:subPropertyOf rdf:resource="http://www.semanticweb.org/cadex/ontologies/2020/1/untitled-ontology-71#hasClipVideoInfo"/>
        <rdfs:domain rdf:resource="http://www.semanticweb.org/cadex/ontologies/2020/1/untitled-ontology-71#Clip"/>
        <rdfs:range rdf:resource="http://www.w3.org/2001/XMLSchema#string"/>
        <rdfs:comment>This property represents a metadata field that indicates the profile of a clip&apos;s video.</rdfs:comment>
    </owl:DatatypeProperty>
    


    <!-- http://www.semanticweb.org/cadex/ontologies/2020/1/untitled-ontology-71#hasClipVideoResolution -->

    <owl:DatatypeProperty rdf:about="http://www.semanticweb.org/cadex/ontologies/2020/1/untitled-ontology-71#hasClipVideoResolution">
        <rdfs:subPropertyOf rdf:resource="http://www.semanticweb.org/cadex/ontologies/2020/1/untitled-ontology-71#hasClipVideoInfo"/>
        <rdfs:domain rdf:resource="http://www.semanticweb.org/cadex/ontologies/2020/1/untitled-ontology-71#Clip"/>
        <rdfs:range rdf:resource="http://www.w3.org/2001/XMLSchema#string"/>
        <rdfs:comment>This property represents a metadata field that indicates the resolution of a clip&apos;s video.</rdfs:comment>
    </owl:DatatypeProperty>
    


    <!-- http://www.semanticweb.org/cadex/ontologies/2020/1/untitled-ontology-71#hasClipWhiteBalance -->

    <owl:DatatypeProperty rdf:about="http://www.semanticweb.org/cadex/ontologies/2020/1/untitled-ontology-71#hasClipWhiteBalance">
        <rdfs:subPropertyOf rdf:resource="http://www.semanticweb.org/cadex/ontologies/2020/1/untitled-ontology-71#hasClipInfo"/>
        <rdfs:domain rdf:resource="http://www.semanticweb.org/cadex/ontologies/2020/1/untitled-ontology-71#Clip"/>
        <rdfs:range rdf:resource="http://www.w3.org/2001/XMLSchema#int"/>
        <rdfs:comment>This property represents a metadata field that indicates the white balance of a clip.</rdfs:comment>
    </owl:DatatypeProperty>
    


    <!-- http://www.semanticweb.org/cadex/ontologies/2020/1/untitled-ontology-71#hasClipWidth -->

    <owl:DatatypeProperty rdf:about="http://www.semanticweb.org/cadex/ontologies/2020/1/untitled-ontology-71#hasClipWidth">
        <rdfs:subPropertyOf rdf:resource="http://www.semanticweb.org/cadex/ontologies/2020/1/untitled-ontology-71#hasClipVideoInfo"/>
        <rdfs:domain rdf:resource="http://www.semanticweb.org/cadex/ontologies/2020/1/untitled-ontology-71#Clip"/>
        <rdfs:range rdf:resource="http://www.w3.org/2001/XMLSchema#int"/>
        <rdfs:comment>This property represents a metadata field that indicates the height of a clip&apos;s width.</rdfs:comment>
    </owl:DatatypeProperty>
    


    <!-- http://www.semanticweb.org/cadex/ontologies/2020/1/untitled-ontology-71#hasDeliverableAspectRatio -->

    <owl:DatatypeProperty rdf:about="http://www.semanticweb.org/cadex/ontologies/2020/1/untitled-ontology-71#hasDeliverableAspectRatio">
        <rdfs:subPropertyOf rdf:resource="http://www.semanticweb.org/cadex/ontologies/2020/1/untitled-ontology-71#hasDeliverableInfo"/>
        <rdfs:domain rdf:resource="http://www.semanticweb.org/cadex/ontologies/2020/1/untitled-ontology-71#Deliverable"/>
        <rdfs:range rdf:resource="http://www.w3.org/2001/XMLSchema#string"/>
        <rdfs:comment>This property represents a metadata field that indicates the aspect ratio of a deliverable.</rdfs:comment>
    </owl:DatatypeProperty>
    


    <!-- http://www.semanticweb.org/cadex/ontologies/2020/1/untitled-ontology-71#hasDeliverableAudioLanguage -->

    <owl:DatatypeProperty rdf:about="http://www.semanticweb.org/cadex/ontologies/2020/1/untitled-ontology-71#hasDeliverableAudioLanguage">
        <rdfs:subPropertyOf rdf:resource="http://www.semanticweb.org/cadex/ontologies/2020/1/untitled-ontology-71#hasDeliverableInfo"/>
        <rdfs:domain rdf:resource="http://www.semanticweb.org/cadex/ontologies/2020/1/untitled-ontology-71#Deliverable"/>
        <rdfs:range rdf:resource="http://www.w3.org/2001/XMLSchema#language"/>
        <rdfs:comment>This property represents a metadata field that indicates the audio language of a deliverable.</rdfs:comment>
    </owl:DatatypeProperty>
    


    <!-- http://www.semanticweb.org/cadex/ontologies/2020/1/untitled-ontology-71#hasDeliverableAudioLayout -->

    <owl:DatatypeProperty rdf:about="http://www.semanticweb.org/cadex/ontologies/2020/1/untitled-ontology-71#hasDeliverableAudioLayout">
        <rdfs:subPropertyOf rdf:resource="http://www.semanticweb.org/cadex/ontologies/2020/1/untitled-ontology-71#hasDeliverableInfo"/>
        <rdfs:domain rdf:resource="http://www.semanticweb.org/cadex/ontologies/2020/1/untitled-ontology-71#Deliverable"/>
        <rdfs:range rdf:resource="http://www.w3.org/2001/XMLSchema#string"/>
        <rdfs:comment>This property represents a metadata field that indicates the audio layout of a deliverable.</rdfs:comment>
    </owl:DatatypeProperty>
    


    <!-- http://www.semanticweb.org/cadex/ontologies/2020/1/untitled-ontology-71#hasDeliverableAudioType -->

    <owl:DatatypeProperty rdf:about="http://www.semanticweb.org/cadex/ontologies/2020/1/untitled-ontology-71#hasDeliverableAudioType">
        <rdfs:subPropertyOf rdf:resource="http://www.semanticweb.org/cadex/ontologies/2020/1/untitled-ontology-71#hasDeliverableInfo"/>
        <rdfs:domain rdf:resource="http://www.semanticweb.org/cadex/ontologies/2020/1/untitled-ontology-71#Deliverable"/>
        <rdfs:range rdf:resource="http://www.w3.org/2001/XMLSchema#string"/>
        <rdfs:comment>This property represents a metadata field that indicates the audio type of a deliverable.</rdfs:comment>
    </owl:DatatypeProperty>
    


    <!-- http://www.semanticweb.org/cadex/ontologies/2020/1/untitled-ontology-71#hasDeliverableAudioVersion -->

    <owl:DatatypeProperty rdf:about="http://www.semanticweb.org/cadex/ontologies/2020/1/untitled-ontology-71#hasDeliverableAudioVersion">
        <rdfs:subPropertyOf rdf:resource="http://www.semanticweb.org/cadex/ontologies/2020/1/untitled-ontology-71#hasDeliverableInfo"/>
        <rdfs:domain rdf:resource="http://www.semanticweb.org/cadex/ontologies/2020/1/untitled-ontology-71#Deliverable"/>
        <rdfs:range rdf:resource="http://www.w3.org/2001/XMLSchema#string"/>
        <rdfs:comment>This property represents a metadata field that indicates the audio version of a deliverable.</rdfs:comment>
    </owl:DatatypeProperty>
    


    <!-- http://www.semanticweb.org/cadex/ontologies/2020/1/untitled-ontology-71#hasDeliverableDescription -->

    <owl:DatatypeProperty rdf:about="http://www.semanticweb.org/cadex/ontologies/2020/1/untitled-ontology-71#hasDeliverableDescription">
        <rdfs:subPropertyOf rdf:resource="http://www.semanticweb.org/cadex/ontologies/2020/1/untitled-ontology-71#hasDeliverableInfo"/>
        <rdfs:domain rdf:resource="http://www.semanticweb.org/cadex/ontologies/2020/1/untitled-ontology-71#Deliverable"/>
        <rdfs:range rdf:resource="http://www.w3.org/2001/XMLSchema#string"/>
        <rdfs:comment>This property represents a metadata field that indicates the description of a deliverable. This field should be used to describe the differences in deliverable versions (e.g. &apos;Spanish audio&apos; or &apos;scenes of a sexual nature removed&apos;).</rdfs:comment>
    </owl:DatatypeProperty>
    


    <!-- http://www.semanticweb.org/cadex/ontologies/2020/1/untitled-ontology-71#hasDeliverableDubbingMixer -->

    <owl:DatatypeProperty rdf:about="http://www.semanticweb.org/cadex/ontologies/2020/1/untitled-ontology-71#hasDeliverableDubbingMixer">
        <rdfs:subPropertyOf rdf:resource="http://www.semanticweb.org/cadex/ontologies/2020/1/untitled-ontology-71#hasDeliverableInfo"/>
        <rdfs:domain rdf:resource="http://www.semanticweb.org/cadex/ontologies/2020/1/untitled-ontology-71#Deliverable"/>
        <rdfs:range rdf:resource="http://www.w3.org/2001/XMLSchema#string"/>
        <rdfs:comment>This property represents a metadata field that indicates the dubbing mixer of a deliverable.</rdfs:comment>
    </owl:DatatypeProperty>
    


    <!-- http://www.semanticweb.org/cadex/ontologies/2020/1/untitled-ontology-71#hasDeliverableDubbingStudio -->

    <owl:DatatypeProperty rdf:about="http://www.semanticweb.org/cadex/ontologies/2020/1/untitled-ontology-71#hasDeliverableDubbingStudio">
        <rdfs:subPropertyOf rdf:resource="http://www.semanticweb.org/cadex/ontologies/2020/1/untitled-ontology-71#hasDeliverableInfo"/>
        <rdfs:domain rdf:resource="http://www.semanticweb.org/cadex/ontologies/2020/1/untitled-ontology-71#Deliverable"/>
        <rdfs:range rdf:resource="http://www.w3.org/2001/XMLSchema#string"/>
        <rdfs:comment>This property represents a metadata field that indicates the dubbing studio of a deliverable.</rdfs:comment>
    </owl:DatatypeProperty>
    


    <!-- http://www.semanticweb.org/cadex/ontologies/2020/1/untitled-ontology-71#hasDeliverableFrameRate -->

    <owl:DatatypeProperty rdf:about="http://www.semanticweb.org/cadex/ontologies/2020/1/untitled-ontology-71#hasDeliverableFrameRate">
        <rdfs:subPropertyOf rdf:resource="http://www.semanticweb.org/cadex/ontologies/2020/1/untitled-ontology-71#hasDeliverableInfo"/>
        <rdfs:domain rdf:resource="http://www.semanticweb.org/cadex/ontologies/2020/1/untitled-ontology-71#Deliverable"/>
        <rdfs:range rdf:resource="http://www.w3.org/2001/XMLSchema#float"/>
        <rdfs:comment>This property represents a metadata field that indicates the frame rate of a deliverable.</rdfs:comment>
    </owl:DatatypeProperty>
    


    <!-- http://www.semanticweb.org/cadex/ontologies/2020/1/untitled-ontology-71#hasDeliverableInfo -->

    <owl:DatatypeProperty rdf:about="http://www.semanticweb.org/cadex/ontologies/2020/1/untitled-ontology-71#hasDeliverableInfo">
        <rdfs:domain rdf:resource="http://www.semanticweb.org/cadex/ontologies/2020/1/untitled-ontology-71#Deliverable"/>
        <rdfs:comment>This is the parent of a set of properties that represent metadata fields describing a deliverable. This property should not be populated with a value because it does not itself represent a metadata field. Rather, it is used solely to organise the properties representing fields.</rdfs:comment>
    </owl:DatatypeProperty>
    


    <!-- http://www.semanticweb.org/cadex/ontologies/2020/1/untitled-ontology-71#hasDeliverableLFOA -->

    <owl:DatatypeProperty rdf:about="http://www.semanticweb.org/cadex/ontologies/2020/1/untitled-ontology-71#hasDeliverableLFOA">
        <rdfs:subPropertyOf rdf:resource="http://www.semanticweb.org/cadex/ontologies/2020/1/untitled-ontology-71#hasDeliverableInfo"/>
        <rdfs:domain rdf:resource="http://www.semanticweb.org/cadex/ontologies/2020/1/untitled-ontology-71#Deliverable"/>
        <rdfs:range rdf:resource="http://www.w3.org/2001/XMLSchema#string"/>
    </owl:DatatypeProperty>
    


    <!-- http://www.semanticweb.org/cadex/ontologies/2020/1/untitled-ontology-71#hasDeliverableLength -->

    <owl:DatatypeProperty rdf:about="http://www.semanticweb.org/cadex/ontologies/2020/1/untitled-ontology-71#hasDeliverableLength">
        <rdfs:subPropertyOf rdf:resource="http://www.semanticweb.org/cadex/ontologies/2020/1/untitled-ontology-71#hasDeliverableInfo"/>
        <rdfs:domain rdf:resource="http://www.semanticweb.org/cadex/ontologies/2020/1/untitled-ontology-71#Deliverable"/>
        <rdfs:range rdf:resource="http://www.w3.org/2001/XMLSchema#string"/>
        <rdfs:comment>This property represents a metadata field that indicates the length of a deliverable.</rdfs:comment>
    </owl:DatatypeProperty>
    


    <!-- http://www.semanticweb.org/cadex/ontologies/2020/1/untitled-ontology-71#hasDeliverablePictureFileFormat -->

    <owl:DatatypeProperty rdf:about="http://www.semanticweb.org/cadex/ontologies/2020/1/untitled-ontology-71#hasDeliverablePictureFileFormat">
        <rdfs:subPropertyOf rdf:resource="http://www.semanticweb.org/cadex/ontologies/2020/1/untitled-ontology-71#hasDeliverableInfo"/>
        <rdfs:domain rdf:resource="http://www.semanticweb.org/cadex/ontologies/2020/1/untitled-ontology-71#Deliverable"/>
        <rdfs:range rdf:resource="http://www.w3.org/2001/XMLSchema#string"/>
        <rdfs:comment>This property represents a metadata field that indicates the file format of a deliverable&apos;s picture.</rdfs:comment>
    </owl:DatatypeProperty>
    


    <!-- http://www.semanticweb.org/cadex/ontologies/2020/1/untitled-ontology-71#hasDeliverablePictureResolution -->

    <owl:DatatypeProperty rdf:about="http://www.semanticweb.org/cadex/ontologies/2020/1/untitled-ontology-71#hasDeliverablePictureResolution">
        <rdfs:subPropertyOf rdf:resource="http://www.semanticweb.org/cadex/ontologies/2020/1/untitled-ontology-71#hasDeliverableInfo"/>
        <rdfs:domain rdf:resource="http://www.semanticweb.org/cadex/ontologies/2020/1/untitled-ontology-71#Deliverable"/>
        <rdfs:range rdf:resource="http://www.w3.org/2001/XMLSchema#string"/>
        <rdfs:comment>This property represents a metadata field that indicates the resolution of a deliverable&apos;s picture.</rdfs:comment>
    </owl:DatatypeProperty>
    


    <!-- http://www.semanticweb.org/cadex/ontologies/2020/1/untitled-ontology-71#hasDeliverablePictureVersion -->

    <owl:DatatypeProperty rdf:about="http://www.semanticweb.org/cadex/ontologies/2020/1/untitled-ontology-71#hasDeliverablePictureVersion">
        <rdfs:subPropertyOf rdf:resource="http://www.semanticweb.org/cadex/ontologies/2020/1/untitled-ontology-71#hasDeliverableInfo"/>
        <rdfs:domain rdf:resource="http://www.semanticweb.org/cadex/ontologies/2020/1/untitled-ontology-71#Deliverable"/>
        <rdfs:range rdf:resource="http://www.w3.org/2001/XMLSchema#string"/>
        <rdfs:comment>This property represents a metadata field that indicates the version of a deliverable&apos;s picture.</rdfs:comment>
    </owl:DatatypeProperty>
    


    <!-- http://www.semanticweb.org/cadex/ontologies/2020/1/untitled-ontology-71#hasDeliverableReelCount -->

    <owl:DatatypeProperty rdf:about="http://www.semanticweb.org/cadex/ontologies/2020/1/untitled-ontology-71#hasDeliverableReelCount">
        <rdfs:subPropertyOf rdf:resource="http://www.semanticweb.org/cadex/ontologies/2020/1/untitled-ontology-71#hasDeliverableInfo"/>
        <rdfs:domain rdf:resource="http://www.semanticweb.org/cadex/ontologies/2020/1/untitled-ontology-71#Deliverable"/>
        <rdfs:range rdf:resource="http://www.w3.org/2001/XMLSchema#int"/>
        <rdfs:comment>This property represents a metadata field that indicates the reel count of a deliverable.</rdfs:comment>
    </owl:DatatypeProperty>
    


    <!-- http://www.semanticweb.org/cadex/ontologies/2020/1/untitled-ontology-71#hasDeliverableReelNumber -->

    <owl:DatatypeProperty rdf:about="http://www.semanticweb.org/cadex/ontologies/2020/1/untitled-ontology-71#hasDeliverableReelNumber">
        <rdfs:subPropertyOf rdf:resource="http://www.semanticweb.org/cadex/ontologies/2020/1/untitled-ontology-71#hasDeliverableInfo"/>
        <rdfs:domain rdf:resource="http://www.semanticweb.org/cadex/ontologies/2020/1/untitled-ontology-71#Deliverable"/>
        <rdfs:range rdf:resource="http://www.w3.org/2001/XMLSchema#int"/>
        <rdfs:comment>This property represents a metadata field that indicates the reel number of a deliverable.</rdfs:comment>
    </owl:DatatypeProperty>
    


    <!-- http://www.semanticweb.org/cadex/ontologies/2020/1/untitled-ontology-71#hasDeliverableReleaseDate -->

    <owl:DatatypeProperty rdf:about="http://www.semanticweb.org/cadex/ontologies/2020/1/untitled-ontology-71#hasDeliverableReleaseDate">
        <rdfs:subPropertyOf rdf:resource="http://www.semanticweb.org/cadex/ontologies/2020/1/untitled-ontology-71#hasDeliverableInfo"/>
        <rdfs:domain rdf:resource="http://www.semanticweb.org/cadex/ontologies/2020/1/untitled-ontology-71#Deliverable"/>
        <rdfs:range rdf:resource="http://www.w3.org/2001/XMLSchema#dateTimeStamp"/>
        <rdfs:comment>This property represents a metadata field that indicates the release date of a deliverable.</rdfs:comment>
    </owl:DatatypeProperty>
    


    <!-- http://www.semanticweb.org/cadex/ontologies/2020/1/untitled-ontology-71#hasDeliverableSubtitleLanguage -->

    <owl:DatatypeProperty rdf:about="http://www.semanticweb.org/cadex/ontologies/2020/1/untitled-ontology-71#hasDeliverableSubtitleLanguage">
        <rdfs:subPropertyOf rdf:resource="http://www.semanticweb.org/cadex/ontologies/2020/1/untitled-ontology-71#hasDeliverableInfo"/>
        <rdfs:domain rdf:resource="http://www.semanticweb.org/cadex/ontologies/2020/1/untitled-ontology-71#Deliverable"/>
        <rdfs:range rdf:resource="http://www.w3.org/2001/XMLSchema#language"/>
        <rdfs:comment>This property represents a metadata field that indicates the subtitle language of a deliverable.</rdfs:comment>
    </owl:DatatypeProperty>
    


    <!-- http://www.semanticweb.org/cadex/ontologies/2020/1/untitled-ontology-71#hasFileAccessPermissions -->

    <owl:DatatypeProperty rdf:about="http://www.semanticweb.org/cadex/ontologies/2020/1/untitled-ontology-71#hasFileAccessPermissions">
        <rdfs:subPropertyOf rdf:resource="http://www.semanticweb.org/cadex/ontologies/2020/1/untitled-ontology-71#hasFileInfo"/>
        <rdfs:domain rdf:resource="http://www.semanticweb.org/cadex/ontologies/2020/1/untitled-ontology-71#File"/>
        <rdfs:range rdf:resource="http://www.w3.org/2001/XMLSchema#string"/>
        <rdfs:comment>This property represents a metadata field that indicates the access permissions of a file.</rdfs:comment>
    </owl:DatatypeProperty>
    


    <!-- http://www.semanticweb.org/cadex/ontologies/2020/1/untitled-ontology-71#hasFileChecksum -->

    <owl:DatatypeProperty rdf:about="http://www.semanticweb.org/cadex/ontologies/2020/1/untitled-ontology-71#hasFileChecksum">
        <rdfs:subPropertyOf rdf:resource="http://www.semanticweb.org/cadex/ontologies/2020/1/untitled-ontology-71#hasFileInfo"/>
        <rdfs:domain rdf:resource="http://www.semanticweb.org/cadex/ontologies/2020/1/untitled-ontology-71#File"/>
        <rdfs:range rdf:resource="http://www.w3.org/2001/XMLSchema#string"/>
        <rdfs:comment>This property represents a metadata field that indicates the checksum of a file.</rdfs:comment>
    </owl:DatatypeProperty>
    


    <!-- http://www.semanticweb.org/cadex/ontologies/2020/1/untitled-ontology-71#hasFileExtension -->

    <owl:DatatypeProperty rdf:about="http://www.semanticweb.org/cadex/ontologies/2020/1/untitled-ontology-71#hasFileExtension">
        <rdfs:subPropertyOf rdf:resource="http://www.semanticweb.org/cadex/ontologies/2020/1/untitled-ontology-71#hasFileInfo"/>
        <rdfs:domain rdf:resource="http://www.semanticweb.org/cadex/ontologies/2020/1/untitled-ontology-71#File"/>
        <rdfs:range rdf:resource="http://www.w3.org/2001/XMLSchema#string"/>
        <rdfs:comment>This property represents a metadata field that indicates the extension of a file.</rdfs:comment>
    </owl:DatatypeProperty>
    


    <!-- http://www.semanticweb.org/cadex/ontologies/2020/1/untitled-ontology-71#hasFileFieldDominance -->

    <owl:DatatypeProperty rdf:about="http://www.semanticweb.org/cadex/ontologies/2020/1/untitled-ontology-71#hasFileFieldDominance">
        <rdfs:subPropertyOf rdf:resource="http://www.semanticweb.org/cadex/ontologies/2020/1/untitled-ontology-71#hasFileInfo"/>
        <rdfs:domain rdf:resource="http://www.semanticweb.org/cadex/ontologies/2020/1/untitled-ontology-71#File"/>
        <rdfs:range rdf:resource="http://www.w3.org/2001/XMLSchema#string"/>
        <rdfs:comment>This property represents a metadata field that indicates the field dominance of a file.</rdfs:comment>
    </owl:DatatypeProperty>
    


    <!-- http://www.semanticweb.org/cadex/ontologies/2020/1/untitled-ontology-71#hasFileFormatProfile -->

    <owl:DatatypeProperty rdf:about="http://www.semanticweb.org/cadex/ontologies/2020/1/untitled-ontology-71#hasFileFormatProfile">
        <rdfs:subPropertyOf rdf:resource="http://www.semanticweb.org/cadex/ontologies/2020/1/untitled-ontology-71#hasFileInfo"/>
        <rdfs:domain rdf:resource="http://www.semanticweb.org/cadex/ontologies/2020/1/untitled-ontology-71#File"/>
        <rdfs:range rdf:resource="http://www.w3.org/2001/XMLSchema#string"/>
        <rdfs:comment>This property represents a metadata field that indicates the format profile of a file.</rdfs:comment>
    </owl:DatatypeProperty>
    


    <!-- http://www.semanticweb.org/cadex/ontologies/2020/1/untitled-ontology-71#hasFileInfo -->

    <owl:DatatypeProperty rdf:about="http://www.semanticweb.org/cadex/ontologies/2020/1/untitled-ontology-71#hasFileInfo">
        <rdfs:domain rdf:resource="http://www.semanticweb.org/cadex/ontologies/2020/1/untitled-ontology-71#File"/>
        <rdfs:comment>This is the parent of a set of properties that represent metadata fields describing a file. This property should not be populated with a value because it does not itself represent a metadata field. Rather, it is used solely to organise the properties representing fields.</rdfs:comment>
    </owl:DatatypeProperty>
    


    <!-- http://www.semanticweb.org/cadex/ontologies/2020/1/untitled-ontology-71#hasFileName -->

    <owl:DatatypeProperty rdf:about="http://www.semanticweb.org/cadex/ontologies/2020/1/untitled-ontology-71#hasFileName">
        <rdfs:subPropertyOf rdf:resource="http://www.semanticweb.org/cadex/ontologies/2020/1/untitled-ontology-71#hasFileInfo"/>
        <rdfs:domain rdf:resource="http://www.semanticweb.org/cadex/ontologies/2020/1/untitled-ontology-71#File"/>
        <rdfs:range rdf:resource="http://www.w3.org/2001/XMLSchema#string"/>
        <rdfs:comment>This property represents a metadata field that indicates the name of a file.</rdfs:comment>
    </owl:DatatypeProperty>
    


    <!-- http://www.semanticweb.org/cadex/ontologies/2020/1/untitled-ontology-71#hasFilePath -->

    <owl:DatatypeProperty rdf:about="http://www.semanticweb.org/cadex/ontologies/2020/1/untitled-ontology-71#hasFilePath">
        <rdfs:subPropertyOf rdf:resource="http://www.semanticweb.org/cadex/ontologies/2020/1/untitled-ontology-71#hasFileInfo"/>
        <rdfs:domain rdf:resource="http://www.semanticweb.org/cadex/ontologies/2020/1/untitled-ontology-71#File"/>
        <rdfs:range rdf:resource="http://www.w3.org/2001/XMLSchema#string"/>
        <rdfs:comment>This property represents a metadata field that indicates the path of a file.</rdfs:comment>
    </owl:DatatypeProperty>
    


    <!-- http://www.semanticweb.org/cadex/ontologies/2020/1/untitled-ontology-71#hasFileScanType -->

    <owl:DatatypeProperty rdf:about="http://www.semanticweb.org/cadex/ontologies/2020/1/untitled-ontology-71#hasFileScanType">
        <rdfs:subPropertyOf rdf:resource="http://www.semanticweb.org/cadex/ontologies/2020/1/untitled-ontology-71#hasFileInfo"/>
        <rdfs:domain rdf:resource="http://www.semanticweb.org/cadex/ontologies/2020/1/untitled-ontology-71#File"/>
        <rdfs:range rdf:resource="http://www.w3.org/2001/XMLSchema#string"/>
        <rdfs:comment>This property represents a metadata field that indicates the scan type of a file.</rdfs:comment>
    </owl:DatatypeProperty>
    


    <!-- http://www.semanticweb.org/cadex/ontologies/2020/1/untitled-ontology-71#hasFileSize -->

    <owl:DatatypeProperty rdf:about="http://www.semanticweb.org/cadex/ontologies/2020/1/untitled-ontology-71#hasFileSize">
        <rdfs:subPropertyOf rdf:resource="http://www.semanticweb.org/cadex/ontologies/2020/1/untitled-ontology-71#hasFileInfo"/>
        <rdfs:domain rdf:resource="http://www.semanticweb.org/cadex/ontologies/2020/1/untitled-ontology-71#File"/>
        <rdfs:range rdf:resource="http://www.w3.org/2001/XMLSchema#int"/>
        <rdfs:comment>This property represents a metadata field that indicates the size of a file.</rdfs:comment>
    </owl:DatatypeProperty>
    


    <!-- http://www.semanticweb.org/cadex/ontologies/2020/1/untitled-ontology-71#hasFileWritingApplication -->

    <owl:DatatypeProperty rdf:about="http://www.semanticweb.org/cadex/ontologies/2020/1/untitled-ontology-71#hasFileWritingApplication">
        <rdfs:subPropertyOf rdf:resource="http://www.semanticweb.org/cadex/ontologies/2020/1/untitled-ontology-71#hasFileInfo"/>
        <rdfs:domain rdf:resource="http://www.semanticweb.org/cadex/ontologies/2020/1/untitled-ontology-71#File"/>
        <rdfs:range rdf:resource="http://www.w3.org/2001/XMLSchema#string"/>
        <rdfs:comment>This property represents a metadata field that indicates the writing application of a file.</rdfs:comment>
    </owl:DatatypeProperty>
    


    <!-- http://www.semanticweb.org/cadex/ontologies/2020/1/untitled-ontology-71#hasIssueCheckDate -->

    <owl:DatatypeProperty rdf:about="http://www.semanticweb.org/cadex/ontologies/2020/1/untitled-ontology-71#hasIssueCheckDate">
        <rdfs:subPropertyOf rdf:resource="http://www.semanticweb.org/cadex/ontologies/2020/1/untitled-ontology-71#hasIssueInfo"/>
        <rdfs:domain rdf:resource="http://www.semanticweb.org/cadex/ontologies/2020/1/untitled-ontology-71#Issue"/>
        <rdfs:range rdf:resource="http://www.w3.org/2001/XMLSchema#dateTimeStamp"/>
        <rdfs:comment>This property represents a metadata field that indicates the check date of an issue.</rdfs:comment>
    </owl:DatatypeProperty>
    


    <!-- http://www.semanticweb.org/cadex/ontologies/2020/1/untitled-ontology-71#hasIssueDate -->

    <owl:DatatypeProperty rdf:about="http://www.semanticweb.org/cadex/ontologies/2020/1/untitled-ontology-71#hasIssueDate">
        <rdfs:subPropertyOf rdf:resource="http://www.semanticweb.org/cadex/ontologies/2020/1/untitled-ontology-71#hasIssueInfo"/>
        <rdfs:domain rdf:resource="http://www.semanticweb.org/cadex/ontologies/2020/1/untitled-ontology-71#Issue"/>
        <rdfs:range rdf:resource="http://www.w3.org/2001/XMLSchema#dateTimeStamp"/>
        <rdfs:comment>This property represents a metadata field that indicates the date of an issue.</rdfs:comment>
    </owl:DatatypeProperty>
    


    <!-- http://www.semanticweb.org/cadex/ontologies/2020/1/untitled-ontology-71#hasIssueDescription -->

    <owl:DatatypeProperty rdf:about="http://www.semanticweb.org/cadex/ontologies/2020/1/untitled-ontology-71#hasIssueDescription">
        <rdfs:subPropertyOf rdf:resource="http://www.semanticweb.org/cadex/ontologies/2020/1/untitled-ontology-71#hasIssueInfo"/>
        <rdfs:domain rdf:resource="http://www.semanticweb.org/cadex/ontologies/2020/1/untitled-ontology-71#Issue"/>
        <rdfs:range rdf:resource="http://www.w3.org/2001/XMLSchema#string"/>
        <rdfs:comment>This property represents a metadata field that indicates the description of an issue.</rdfs:comment>
    </owl:DatatypeProperty>
    


    <!-- http://www.semanticweb.org/cadex/ontologies/2020/1/untitled-ontology-71#hasIssueFixDate -->

    <owl:DatatypeProperty rdf:about="http://www.semanticweb.org/cadex/ontologies/2020/1/untitled-ontology-71#hasIssueFixDate">
        <rdfs:subPropertyOf rdf:resource="http://www.semanticweb.org/cadex/ontologies/2020/1/untitled-ontology-71#hasIssueInfo"/>
        <rdfs:domain rdf:resource="http://www.semanticweb.org/cadex/ontologies/2020/1/untitled-ontology-71#Issue"/>
        <rdfs:range rdf:resource="http://www.w3.org/2001/XMLSchema#dateTimeStamp"/>
        <rdfs:comment>This property represents a metadata field that indicates the fix date of an issue.</rdfs:comment>
    </owl:DatatypeProperty>
    


    <!-- http://www.semanticweb.org/cadex/ontologies/2020/1/untitled-ontology-71#hasIssueInfo -->

    <owl:DatatypeProperty rdf:about="http://www.semanticweb.org/cadex/ontologies/2020/1/untitled-ontology-71#hasIssueInfo">
        <rdfs:domain rdf:resource="http://www.semanticweb.org/cadex/ontologies/2020/1/untitled-ontology-71#Issue"/>
        <rdfs:comment>This is the parent of a set of properties that represent metadata fields describing an issue. This property should not be populated with a value because it does not itself represent a metadata field. Rather, it is used solely to organise the properties representing fields.</rdfs:comment>
    </owl:DatatypeProperty>
    


    <!-- http://www.semanticweb.org/cadex/ontologies/2020/1/untitled-ontology-71#hasIssueMissingLines -->

    <owl:DatatypeProperty rdf:about="http://www.semanticweb.org/cadex/ontologies/2020/1/untitled-ontology-71#hasIssueMissingLines">
        <rdfs:subPropertyOf rdf:resource="http://www.semanticweb.org/cadex/ontologies/2020/1/untitled-ontology-71#hasIssueInfo"/>
        <rdfs:domain rdf:resource="http://www.semanticweb.org/cadex/ontologies/2020/1/untitled-ontology-71#Issue"/>
        <rdfs:range rdf:resource="http://www.w3.org/2001/XMLSchema#boolean"/>
    </owl:DatatypeProperty>
    


    <!-- http://www.semanticweb.org/cadex/ontologies/2020/1/untitled-ontology-71#hasIssueMixerResponse -->

    <owl:DatatypeProperty rdf:about="http://www.semanticweb.org/cadex/ontologies/2020/1/untitled-ontology-71#hasIssueMixerResponse">
        <rdfs:subPropertyOf rdf:resource="http://www.semanticweb.org/cadex/ontologies/2020/1/untitled-ontology-71#hasIssueInfo"/>
        <rdfs:domain rdf:resource="http://www.semanticweb.org/cadex/ontologies/2020/1/untitled-ontology-71#Issue"/>
        <rdfs:range>
            <rdfs:Datatype>
                <owl:oneOf>
                    <rdf:Description>
                        <rdf:type rdf:resource="http://www.w3.org/1999/02/22-rdf-syntax-ns#List"/>
                        <rdf:first>Fixed</rdf:first>
                        <rdf:rest>
                            <rdf:Description>
                                <rdf:type rdf:resource="http://www.w3.org/1999/02/22-rdf-syntax-ns#List"/>
                                <rdf:first>No Fix Needed</rdf:first>
                                <rdf:rest rdf:resource="http://www.w3.org/1999/02/22-rdf-syntax-ns#nil"/>
                            </rdf:Description>
                        </rdf:rest>
                    </rdf:Description>
                </owl:oneOf>
            </rdfs:Datatype>
        </rdfs:range>
        <rdfs:comment>This property represents a metadata field that indicates the response of a mixer to an issue.</rdfs:comment>
    </owl:DatatypeProperty>
    


    <!-- http://www.semanticweb.org/cadex/ontologies/2020/1/untitled-ontology-71#hasIssueTimecodeIn -->

    <owl:DatatypeProperty rdf:about="http://www.semanticweb.org/cadex/ontologies/2020/1/untitled-ontology-71#hasIssueTimecodeIn">
        <rdfs:subPropertyOf rdf:resource="http://www.semanticweb.org/cadex/ontologies/2020/1/untitled-ontology-71#hasIssueInfo"/>
        <rdfs:domain rdf:resource="http://www.semanticweb.org/cadex/ontologies/2020/1/untitled-ontology-71#Issue"/>
        <rdfs:range rdf:resource="http://www.w3.org/2001/XMLSchema#string"/>
    </owl:DatatypeProperty>
    


    <!-- http://www.semanticweb.org/cadex/ontologies/2020/1/untitled-ontology-71#hasIssueTimecodeOut -->

    <owl:DatatypeProperty rdf:about="http://www.semanticweb.org/cadex/ontologies/2020/1/untitled-ontology-71#hasIssueTimecodeOut">
        <rdfs:subPropertyOf rdf:resource="http://www.semanticweb.org/cadex/ontologies/2020/1/untitled-ontology-71#hasIssueInfo"/>
        <rdfs:domain rdf:resource="http://www.semanticweb.org/cadex/ontologies/2020/1/untitled-ontology-71#Issue"/>
        <rdfs:range rdf:resource="http://www.w3.org/2001/XMLSchema#string"/>
    </owl:DatatypeProperty>
    


    <!-- http://www.semanticweb.org/cadex/ontologies/2020/1/untitled-ontology-71#hasIssueType -->

    <owl:DatatypeProperty rdf:about="http://www.semanticweb.org/cadex/ontologies/2020/1/untitled-ontology-71#hasIssueType">
        <rdfs:subPropertyOf rdf:resource="http://www.semanticweb.org/cadex/ontologies/2020/1/untitled-ontology-71#hasIssueInfo"/>
        <rdfs:domain rdf:resource="http://www.semanticweb.org/cadex/ontologies/2020/1/untitled-ontology-71#Issue"/>
        <rdfs:range rdf:resource="http://www.w3.org/2001/XMLSchema#string"/>
        <rdfs:comment>This property represents a metadata field that indicates the type of an issue.</rdfs:comment>
    </owl:DatatypeProperty>
    


    <!-- http://www.semanticweb.org/cadex/ontologies/2020/1/untitled-ontology-71#hasLensComment -->

    <owl:DatatypeProperty rdf:about="http://www.semanticweb.org/cadex/ontologies/2020/1/untitled-ontology-71#hasLensComment">
        <rdfs:subPropertyOf rdf:resource="http://www.semanticweb.org/cadex/ontologies/2020/1/untitled-ontology-71#hasLensInfo"/>
        <rdfs:domain rdf:resource="http://www.semanticweb.org/cadex/ontologies/2020/1/untitled-ontology-71#Lens"/>
        <rdfs:range rdf:resource="http://www.w3.org/2001/XMLSchema#string"/>
        <rdfs:comment>This property represents a metadata field that indicates the comments made about a lens.</rdfs:comment>
    </owl:DatatypeProperty>
    


    <!-- http://www.semanticweb.org/cadex/ontologies/2020/1/untitled-ontology-71#hasLensDescription -->

    <owl:DatatypeProperty rdf:about="http://www.semanticweb.org/cadex/ontologies/2020/1/untitled-ontology-71#hasLensDescription">
        <rdfs:subPropertyOf rdf:resource="http://www.semanticweb.org/cadex/ontologies/2020/1/untitled-ontology-71#hasLensInfo"/>
        <rdfs:domain rdf:resource="http://www.semanticweb.org/cadex/ontologies/2020/1/untitled-ontology-71#Lens"/>
        <rdfs:range rdf:resource="http://www.w3.org/2001/XMLSchema#string"/>
        <rdfs:comment>This property represents a metadata field that indicates the description of a lens.</rdfs:comment>
    </owl:DatatypeProperty>
    


    <!-- http://www.semanticweb.org/cadex/ontologies/2020/1/untitled-ontology-71#hasLensFilmstripThumbnail -->

    <owl:DatatypeProperty rdf:about="http://www.semanticweb.org/cadex/ontologies/2020/1/untitled-ontology-71#hasLensFilmstripThumbnail">
        <rdfs:subPropertyOf rdf:resource="http://www.semanticweb.org/cadex/ontologies/2020/1/untitled-ontology-71#hasLensInfo"/>
        <rdfs:domain rdf:resource="http://www.semanticweb.org/cadex/ontologies/2020/1/untitled-ontology-71#Lens"/>
    </owl:DatatypeProperty>
    


    <!-- http://www.semanticweb.org/cadex/ontologies/2020/1/untitled-ontology-71#hasLensGridAngle -->

    <owl:DatatypeProperty rdf:about="http://www.semanticweb.org/cadex/ontologies/2020/1/untitled-ontology-71#hasLensGridAngle">
        <rdfs:subPropertyOf rdf:resource="http://www.semanticweb.org/cadex/ontologies/2020/1/untitled-ontology-71#hasLensGridInfo"/>
        <rdfs:domain rdf:resource="http://www.semanticweb.org/cadex/ontologies/2020/1/untitled-ontology-71#Lens"/>
        <rdfs:range rdf:resource="http://www.w3.org/2001/XMLSchema#string"/>
        <rdfs:comment>This property represents a metadata field that indicates the angle of a lens grid.</rdfs:comment>
    </owl:DatatypeProperty>
    


    <!-- http://www.semanticweb.org/cadex/ontologies/2020/1/untitled-ontology-71#hasLensGridCameraRoll -->

    <owl:DatatypeProperty rdf:about="http://www.semanticweb.org/cadex/ontologies/2020/1/untitled-ontology-71#hasLensGridCameraRoll">
        <rdfs:subPropertyOf rdf:resource="http://www.semanticweb.org/cadex/ontologies/2020/1/untitled-ontology-71#hasLensGridInfo"/>
        <rdfs:domain rdf:resource="http://www.semanticweb.org/cadex/ontologies/2020/1/untitled-ontology-71#Lens"/>
        <rdfs:range rdf:resource="http://www.w3.org/2001/XMLSchema#string"/>
        <rdfs:comment>This property represents a metadata field that indicates the camera roll of a lens grid.</rdfs:comment>
    </owl:DatatypeProperty>
    


    <!-- http://www.semanticweb.org/cadex/ontologies/2020/1/untitled-ontology-71#hasLensGridDistance -->

    <owl:DatatypeProperty rdf:about="http://www.semanticweb.org/cadex/ontologies/2020/1/untitled-ontology-71#hasLensGridDistance">
        <rdfs:subPropertyOf rdf:resource="http://www.semanticweb.org/cadex/ontologies/2020/1/untitled-ontology-71#hasLensGridInfo"/>
        <rdfs:domain rdf:resource="http://www.semanticweb.org/cadex/ontologies/2020/1/untitled-ontology-71#Lens"/>
        <rdfs:range rdf:resource="http://www.w3.org/2001/XMLSchema#string"/>
        <rdfs:comment>This property represents a metadata field that indicates the distance of a lens grid.</rdfs:comment>
    </owl:DatatypeProperty>
    


    <!-- http://www.semanticweb.org/cadex/ontologies/2020/1/untitled-ontology-71#hasLensGridInfo -->

    <owl:DatatypeProperty rdf:about="http://www.semanticweb.org/cadex/ontologies/2020/1/untitled-ontology-71#hasLensGridInfo">
        <rdfs:subPropertyOf rdf:resource="http://www.semanticweb.org/cadex/ontologies/2020/1/untitled-ontology-71#hasAssetInfo"/>
        <rdfs:comment>This is the parent of a set of properties that represent metadata fields describing a lens grid. This property should not be populated with a value because it does not itself represent a metadata field. Rather, it is used solely to organise the properties representing fields.</rdfs:comment>
    </owl:DatatypeProperty>
    


    <!-- http://www.semanticweb.org/cadex/ontologies/2020/1/untitled-ontology-71#hasLensGridTStop -->

    <owl:DatatypeProperty rdf:about="http://www.semanticweb.org/cadex/ontologies/2020/1/untitled-ontology-71#hasLensGridTStop">
        <rdfs:subPropertyOf rdf:resource="http://www.semanticweb.org/cadex/ontologies/2020/1/untitled-ontology-71#hasLensGridInfo"/>
        <rdfs:domain rdf:resource="http://www.semanticweb.org/cadex/ontologies/2020/1/untitled-ontology-71#Lens"/>
        <rdfs:range rdf:resource="http://www.w3.org/2001/XMLSchema#string"/>
        <rdfs:comment>This property represents a metadata field that indicates the T stop of a lens grid.</rdfs:comment>
    </owl:DatatypeProperty>
    


    <!-- http://www.semanticweb.org/cadex/ontologies/2020/1/untitled-ontology-71#hasLensGridTake -->

    <owl:DatatypeProperty rdf:about="http://www.semanticweb.org/cadex/ontologies/2020/1/untitled-ontology-71#hasLensGridTake">
        <rdfs:subPropertyOf rdf:resource="http://www.semanticweb.org/cadex/ontologies/2020/1/untitled-ontology-71#hasLensGridInfo"/>
        <rdfs:domain rdf:resource="http://www.semanticweb.org/cadex/ontologies/2020/1/untitled-ontology-71#Lens"/>
        <rdfs:range rdf:resource="http://www.w3.org/2001/XMLSchema#string"/>
        <rdfs:comment>This property represents a metadata field that indicates the take of a lens grid.</rdfs:comment>
    </owl:DatatypeProperty>
    


    <!-- http://www.semanticweb.org/cadex/ontologies/2020/1/untitled-ontology-71#hasLensGroup -->

    <owl:DatatypeProperty rdf:about="http://www.semanticweb.org/cadex/ontologies/2020/1/untitled-ontology-71#hasLensGroup">
        <rdfs:subPropertyOf rdf:resource="http://www.semanticweb.org/cadex/ontologies/2020/1/untitled-ontology-71#hasLensInfo"/>
        <rdfs:domain rdf:resource="http://www.semanticweb.org/cadex/ontologies/2020/1/untitled-ontology-71#Lens"/>
        <rdfs:range rdf:resource="http://www.w3.org/2001/XMLSchema#string"/>
        <rdfs:comment>This property represents a metadata field that indicates the group of a lens.</rdfs:comment>
    </owl:DatatypeProperty>
    


    <!-- http://www.semanticweb.org/cadex/ontologies/2020/1/untitled-ontology-71#hasLensHeroScanCount -->

    <owl:DatatypeProperty rdf:about="http://www.semanticweb.org/cadex/ontologies/2020/1/untitled-ontology-71#hasLensHeroScanCount">
        <rdfs:subPropertyOf rdf:resource="http://www.semanticweb.org/cadex/ontologies/2020/1/untitled-ontology-71#hasLensInfo"/>
        <rdfs:domain rdf:resource="http://www.semanticweb.org/cadex/ontologies/2020/1/untitled-ontology-71#Lens"/>
        <rdfs:range rdf:resource="http://www.w3.org/2001/XMLSchema#int"/>
        <rdfs:comment>This property represents a metadata field that indicates the hero scan count of a lens.</rdfs:comment>
    </owl:DatatypeProperty>
    


    <!-- http://www.semanticweb.org/cadex/ontologies/2020/1/untitled-ontology-71#hasLensInfo -->

    <owl:DatatypeProperty rdf:about="http://www.semanticweb.org/cadex/ontologies/2020/1/untitled-ontology-71#hasLensInfo">
        <rdfs:domain rdf:resource="http://www.semanticweb.org/cadex/ontologies/2020/1/untitled-ontology-71#Lens"/>
        <rdfs:comment>This is the parent of a set of properties that represent metadata fields describing a lens. This property should not be populated with a value because it does not itself represent a metadata field. Rather, it is used solely to organise the properties representing fields.</rdfs:comment>
    </owl:DatatypeProperty>
    


    <!-- http://www.semanticweb.org/cadex/ontologies/2020/1/untitled-ontology-71#hasLensName -->

    <owl:DatatypeProperty rdf:about="http://www.semanticweb.org/cadex/ontologies/2020/1/untitled-ontology-71#hasLensName">
        <rdfs:subPropertyOf rdf:resource="http://www.semanticweb.org/cadex/ontologies/2020/1/untitled-ontology-71#hasLensInfo"/>
        <rdfs:domain rdf:resource="http://www.semanticweb.org/cadex/ontologies/2020/1/untitled-ontology-71#Lens"/>
        <rdfs:range rdf:resource="http://www.w3.org/2001/XMLSchema#string"/>
        <rdfs:comment>This property represents a metadata field that indicates the name of a lens.</rdfs:comment>
    </owl:DatatypeProperty>
    


    <!-- http://www.semanticweb.org/cadex/ontologies/2020/1/untitled-ontology-71#hasLensNameAlternative -->

    <owl:DatatypeProperty rdf:about="http://www.semanticweb.org/cadex/ontologies/2020/1/untitled-ontology-71#hasLensNameAlternative">
        <rdfs:subPropertyOf rdf:resource="http://www.semanticweb.org/cadex/ontologies/2020/1/untitled-ontology-71#hasLensInfo"/>
        <rdfs:domain rdf:resource="http://www.semanticweb.org/cadex/ontologies/2020/1/untitled-ontology-71#Lens"/>
        <rdfs:range rdf:resource="http://www.w3.org/2001/XMLSchema#string"/>
        <rdfs:comment>This property represents a metadata field that indicates the alternative name of a lens.</rdfs:comment>
    </owl:DatatypeProperty>
    


    <!-- http://www.semanticweb.org/cadex/ontologies/2020/1/untitled-ontology-71#hasLensReel -->

    <owl:DatatypeProperty rdf:about="http://www.semanticweb.org/cadex/ontologies/2020/1/untitled-ontology-71#hasLensReel">
        <rdfs:subPropertyOf rdf:resource="http://www.semanticweb.org/cadex/ontologies/2020/1/untitled-ontology-71#hasLensInfo"/>
        <rdfs:domain rdf:resource="http://www.semanticweb.org/cadex/ontologies/2020/1/untitled-ontology-71#Lens"/>
        <rdfs:range rdf:resource="http://www.w3.org/2001/XMLSchema#string"/>
        <rdfs:comment>This property represents a metadata field that indicates the reel of a lens.</rdfs:comment>
    </owl:DatatypeProperty>
    


    <!-- http://www.semanticweb.org/cadex/ontologies/2020/1/untitled-ontology-71#hasLensSerialNumber -->

    <owl:DatatypeProperty rdf:about="http://www.semanticweb.org/cadex/ontologies/2020/1/untitled-ontology-71#hasLensSerialNumber">
        <rdfs:subPropertyOf rdf:resource="http://www.semanticweb.org/cadex/ontologies/2020/1/untitled-ontology-71#hasLensInfo"/>
        <rdfs:domain rdf:resource="http://www.semanticweb.org/cadex/ontologies/2020/1/untitled-ontology-71#Lens"/>
        <rdfs:range rdf:resource="http://www.w3.org/2001/XMLSchema#string"/>
        <rdfs:comment>This property represents a metadata field that indicates the serial number of a lens.</rdfs:comment>
    </owl:DatatypeProperty>
    


    <!-- http://www.semanticweb.org/cadex/ontologies/2020/1/untitled-ontology-71#hasLensStatus -->

    <owl:DatatypeProperty rdf:about="http://www.semanticweb.org/cadex/ontologies/2020/1/untitled-ontology-71#hasLensStatus">
        <rdfs:subPropertyOf rdf:resource="http://www.semanticweb.org/cadex/ontologies/2020/1/untitled-ontology-71#hasLensInfo"/>
        <rdfs:domain rdf:resource="http://www.semanticweb.org/cadex/ontologies/2020/1/untitled-ontology-71#Lens"/>
        <rdfs:range rdf:resource="http://www.w3.org/2001/XMLSchema#string"/>
        <rdfs:comment>This property represents a metadata field that indicates the status of a lens.</rdfs:comment>
    </owl:DatatypeProperty>
    


    <!-- http://www.semanticweb.org/cadex/ontologies/2020/1/untitled-ontology-71#hasLensTag -->

    <owl:DatatypeProperty rdf:about="http://www.semanticweb.org/cadex/ontologies/2020/1/untitled-ontology-71#hasLensTag">
        <rdfs:subPropertyOf rdf:resource="http://www.semanticweb.org/cadex/ontologies/2020/1/untitled-ontology-71#hasLensInfo"/>
        <rdfs:domain rdf:resource="http://www.semanticweb.org/cadex/ontologies/2020/1/untitled-ontology-71#Lens"/>
        <rdfs:range rdf:resource="http://www.w3.org/2001/XMLSchema#string"/>
        <rdfs:comment>This property represents a metadata field that indicates the tag assigned to a lens.</rdfs:comment>
    </owl:DatatypeProperty>
    


    <!-- http://www.semanticweb.org/cadex/ontologies/2020/1/untitled-ontology-71#hasLensThumbnail -->

    <owl:DatatypeProperty rdf:about="http://www.semanticweb.org/cadex/ontologies/2020/1/untitled-ontology-71#hasLensThumbnail">
        <rdfs:subPropertyOf rdf:resource="http://www.semanticweb.org/cadex/ontologies/2020/1/untitled-ontology-71#hasLensInfo"/>
        <rdfs:domain rdf:resource="http://www.semanticweb.org/cadex/ontologies/2020/1/untitled-ontology-71#Lens"/>
    </owl:DatatypeProperty>
    


    <!-- http://www.semanticweb.org/cadex/ontologies/2020/1/untitled-ontology-71#hasLensType -->

    <owl:DatatypeProperty rdf:about="http://www.semanticweb.org/cadex/ontologies/2020/1/untitled-ontology-71#hasLensType">
        <rdfs:subPropertyOf rdf:resource="http://www.semanticweb.org/cadex/ontologies/2020/1/untitled-ontology-71#hasLensInfo"/>
        <rdfs:domain rdf:resource="http://www.semanticweb.org/cadex/ontologies/2020/1/untitled-ontology-71#Lens"/>
        <rdfs:range rdf:resource="http://www.w3.org/2001/XMLSchema#string"/>
        <rdfs:comment>This property represents a metadata field that indicates the type of a lens.</rdfs:comment>
    </owl:DatatypeProperty>
    


    <!-- http://www.semanticweb.org/cadex/ontologies/2020/1/untitled-ontology-71#hasLocationAddress -->

    <owl:DatatypeProperty rdf:about="http://www.semanticweb.org/cadex/ontologies/2020/1/untitled-ontology-71#hasLocationAddress">
        <rdfs:subPropertyOf rdf:resource="http://www.semanticweb.org/cadex/ontologies/2020/1/untitled-ontology-71#hasLocationInfo"/>
        <rdfs:domain rdf:resource="http://www.semanticweb.org/cadex/ontologies/2020/1/untitled-ontology-71#Location"/>
        <rdfs:range rdf:resource="http://www.w3.org/2001/XMLSchema#string"/>
        <rdfs:comment>This property represents a metadata field that indicates the address of a location.</rdfs:comment>
    </owl:DatatypeProperty>
    


    <!-- http://www.semanticweb.org/cadex/ontologies/2020/1/untitled-ontology-71#hasLocationAltitude -->

    <owl:DatatypeProperty rdf:about="http://www.semanticweb.org/cadex/ontologies/2020/1/untitled-ontology-71#hasLocationAltitude">
        <rdfs:subPropertyOf rdf:resource="http://www.semanticweb.org/cadex/ontologies/2020/1/untitled-ontology-71#hasLocationInfo"/>
        <rdfs:domain rdf:resource="http://www.semanticweb.org/cadex/ontologies/2020/1/untitled-ontology-71#Location"/>
        <rdfs:range rdf:resource="http://www.w3.org/2001/XMLSchema#string"/>
        <rdfs:comment>This property represents a metadata field that indicates the altitude of a location.</rdfs:comment>
    </owl:DatatypeProperty>
    


    <!-- http://www.semanticweb.org/cadex/ontologies/2020/1/untitled-ontology-71#hasLocationInfo -->

    <owl:DatatypeProperty rdf:about="http://www.semanticweb.org/cadex/ontologies/2020/1/untitled-ontology-71#hasLocationInfo">
        <rdfs:domain rdf:resource="http://www.semanticweb.org/cadex/ontologies/2020/1/untitled-ontology-71#Location"/>
        <rdfs:comment>This is the parent of a set of properties that represent metadata fields describing a location. This property should not be populated with a value because it does not itself represent a metadata field. Rather, it is used solely to organise the properties representing fields.</rdfs:comment>
    </owl:DatatypeProperty>
    


    <!-- http://www.semanticweb.org/cadex/ontologies/2020/1/untitled-ontology-71#hasLocationLatitude -->

    <owl:DatatypeProperty rdf:about="http://www.semanticweb.org/cadex/ontologies/2020/1/untitled-ontology-71#hasLocationLatitude">
        <rdfs:subPropertyOf rdf:resource="http://www.semanticweb.org/cadex/ontologies/2020/1/untitled-ontology-71#hasLocationInfo"/>
        <rdfs:domain rdf:resource="http://www.semanticweb.org/cadex/ontologies/2020/1/untitled-ontology-71#Location"/>
        <rdfs:range rdf:resource="http://www.w3.org/2001/XMLSchema#string"/>
        <rdfs:comment>This property represents a metadata field that indicates the latitude of a location.</rdfs:comment>
    </owl:DatatypeProperty>
    


    <!-- http://www.semanticweb.org/cadex/ontologies/2020/1/untitled-ontology-71#hasLocationLatitudeReference -->

    <owl:DatatypeProperty rdf:about="http://www.semanticweb.org/cadex/ontologies/2020/1/untitled-ontology-71#hasLocationLatitudeReference">
        <rdfs:subPropertyOf rdf:resource="http://www.semanticweb.org/cadex/ontologies/2020/1/untitled-ontology-71#hasLocationInfo"/>
        <rdfs:domain rdf:resource="http://www.semanticweb.org/cadex/ontologies/2020/1/untitled-ontology-71#Location"/>
        <rdfs:range>
            <rdfs:Datatype>
                <owl:oneOf>
                    <rdf:Description>
                        <rdf:type rdf:resource="http://www.w3.org/1999/02/22-rdf-syntax-ns#List"/>
                        <rdf:first>N</rdf:first>
                        <rdf:rest>
                            <rdf:Description>
                                <rdf:type rdf:resource="http://www.w3.org/1999/02/22-rdf-syntax-ns#List"/>
                                <rdf:first>S</rdf:first>
                                <rdf:rest rdf:resource="http://www.w3.org/1999/02/22-rdf-syntax-ns#nil"/>
                            </rdf:Description>
                        </rdf:rest>
                    </rdf:Description>
                </owl:oneOf>
            </rdfs:Datatype>
        </rdfs:range>
        <rdfs:comment>This property represents a metadata field that indicates the latitude reference of a location.</rdfs:comment>
    </owl:DatatypeProperty>
    


    <!-- http://www.semanticweb.org/cadex/ontologies/2020/1/untitled-ontology-71#hasLocationLongitude -->

    <owl:DatatypeProperty rdf:about="http://www.semanticweb.org/cadex/ontologies/2020/1/untitled-ontology-71#hasLocationLongitude">
        <rdfs:subPropertyOf rdf:resource="http://www.semanticweb.org/cadex/ontologies/2020/1/untitled-ontology-71#hasLocationInfo"/>
        <rdfs:domain rdf:resource="http://www.semanticweb.org/cadex/ontologies/2020/1/untitled-ontology-71#Location"/>
        <rdfs:range rdf:resource="http://www.w3.org/2001/XMLSchema#string"/>
        <rdfs:comment>This property represents a metadata field that indicates the longitude of a location.</rdfs:comment>
    </owl:DatatypeProperty>
    


    <!-- http://www.semanticweb.org/cadex/ontologies/2020/1/untitled-ontology-71#hasLocationLongitudeReference -->

    <owl:DatatypeProperty rdf:about="http://www.semanticweb.org/cadex/ontologies/2020/1/untitled-ontology-71#hasLocationLongitudeReference">
        <rdfs:subPropertyOf rdf:resource="http://www.semanticweb.org/cadex/ontologies/2020/1/untitled-ontology-71#hasLocationInfo"/>
        <rdfs:domain rdf:resource="http://www.semanticweb.org/cadex/ontologies/2020/1/untitled-ontology-71#Location"/>
        <rdfs:range rdf:resource="http://www.w3.org/2001/XMLSchema#string"/>
        <rdfs:comment>This property represents a metadata field that indicates the longitude reference of a location.</rdfs:comment>
    </owl:DatatypeProperty>
    


    <!-- http://www.semanticweb.org/cadex/ontologies/2020/1/untitled-ontology-71#hasLocationName -->

    <owl:DatatypeProperty rdf:about="http://www.semanticweb.org/cadex/ontologies/2020/1/untitled-ontology-71#hasLocationName">
        <rdfs:subPropertyOf rdf:resource="http://www.semanticweb.org/cadex/ontologies/2020/1/untitled-ontology-71#hasLocationInfo"/>
        <rdfs:domain rdf:resource="http://www.semanticweb.org/cadex/ontologies/2020/1/untitled-ontology-71#Location"/>
        <rdfs:range rdf:resource="http://www.w3.org/2001/XMLSchema#string"/>
        <rdfs:comment>This property represents a metadata field that indicates the name of a location.</rdfs:comment>
    </owl:DatatypeProperty>
    


    <!-- http://www.semanticweb.org/cadex/ontologies/2020/1/untitled-ontology-71#hasLoggingTagInfo -->

    <owl:DatatypeProperty rdf:about="http://www.semanticweb.org/cadex/ontologies/2020/1/untitled-ontology-71#hasLoggingTagInfo">
        <rdfs:comment>This is the parent of a set of properties that represent metadata fields describing a logging tag. This property should not be populated with a value because it does not itself represent a metadata field. Rather, it is used solely to organise the properties representing fields.</rdfs:comment>
    </owl:DatatypeProperty>
    


    <!-- http://www.semanticweb.org/cadex/ontologies/2020/1/untitled-ontology-71#hasLoggingTagName -->

    <owl:DatatypeProperty rdf:about="http://www.semanticweb.org/cadex/ontologies/2020/1/untitled-ontology-71#hasLoggingTagName">
        <rdfs:subPropertyOf rdf:resource="http://www.semanticweb.org/cadex/ontologies/2020/1/untitled-ontology-71#hasLoggingTagInfo"/>
        <rdfs:domain rdf:resource="http://www.semanticweb.org/cadex/ontologies/2020/1/untitled-ontology-71#LoggingTag"/>
        <rdfs:range rdf:resource="http://www.w3.org/2001/XMLSchema#string"/>
        <rdfs:comment>This property represents a metadata field that indicates the name of a logging tag.</rdfs:comment>
    </owl:DatatypeProperty>
    


    <!-- http://www.semanticweb.org/cadex/ontologies/2020/1/untitled-ontology-71#hasLoggingTagTimecodeInClip -->

    <owl:DatatypeProperty rdf:about="http://www.semanticweb.org/cadex/ontologies/2020/1/untitled-ontology-71#hasLoggingTagTimecodeInClip">
        <rdfs:subPropertyOf rdf:resource="http://www.semanticweb.org/cadex/ontologies/2020/1/untitled-ontology-71#hasLoggingTagInfo"/>
        <rdfs:domain rdf:resource="http://www.semanticweb.org/cadex/ontologies/2020/1/untitled-ontology-71#LoggingTag"/>
        <rdfs:range rdf:resource="http://www.w3.org/2001/XMLSchema#string"/>
        <rdfs:comment>This property represents a metadata field that indicates the timecode of a clip that a logging tag is applied to.</rdfs:comment>
    </owl:DatatypeProperty>
    


    <!-- http://www.semanticweb.org/cadex/ontologies/2020/1/untitled-ontology-71#hasLoggingTagTimestamp -->

    <owl:DatatypeProperty rdf:about="http://www.semanticweb.org/cadex/ontologies/2020/1/untitled-ontology-71#hasLoggingTagTimestamp">
        <rdfs:subPropertyOf rdf:resource="http://www.semanticweb.org/cadex/ontologies/2020/1/untitled-ontology-71#hasLoggingTagInfo"/>
        <rdfs:domain rdf:resource="http://www.semanticweb.org/cadex/ontologies/2020/1/untitled-ontology-71#LoggingTag"/>
        <rdfs:range rdf:resource="http://www.w3.org/2001/XMLSchema#dateTimeStamp"/>
        <rdfs:comment>This property represents a metadata field that indicates the date and time that a logging tag was linked to a clip.</rdfs:comment>
    </owl:DatatypeProperty>
    


    <!-- http://www.semanticweb.org/cadex/ontologies/2020/1/untitled-ontology-71#hasLoggingTagType -->

    <owl:DatatypeProperty rdf:about="http://www.semanticweb.org/cadex/ontologies/2020/1/untitled-ontology-71#hasLoggingTagType">
        <rdfs:subPropertyOf rdf:resource="http://www.semanticweb.org/cadex/ontologies/2020/1/untitled-ontology-71#hasLoggingTagInfo"/>
        <rdfs:domain rdf:resource="http://www.semanticweb.org/cadex/ontologies/2020/1/untitled-ontology-71#LoggingTag"/>
        <rdfs:range>
            <rdfs:Datatype>
                <owl:oneOf>
                    <rdf:Description>
                        <rdf:type rdf:resource="http://www.w3.org/1999/02/22-rdf-syntax-ns#List"/>
                        <rdf:first>Action</rdf:first>
                        <rdf:rest>
                            <rdf:Description>
                                <rdf:type rdf:resource="http://www.w3.org/1999/02/22-rdf-syntax-ns#List"/>
                                <rdf:first>Emotion</rdf:first>
                                <rdf:rest>
                                    <rdf:Description>
                                        <rdf:type rdf:resource="http://www.w3.org/1999/02/22-rdf-syntax-ns#List"/>
                                        <rdf:first>Legal</rdf:first>
                                        <rdf:rest>
                                            <rdf:Description>
                                                <rdf:type rdf:resource="http://www.w3.org/1999/02/22-rdf-syntax-ns#List"/>
                                                <rdf:first>Location</rdf:first>
                                                <rdf:rest>
                                                    <rdf:Description>
                                                        <rdf:type rdf:resource="http://www.w3.org/1999/02/22-rdf-syntax-ns#List"/>
                                                        <rdf:first>Object</rdf:first>
                                                        <rdf:rest>
                                                            <rdf:Description>
                                                                <rdf:type rdf:resource="http://www.w3.org/1999/02/22-rdf-syntax-ns#List"/>
                                                                <rdf:first>Other</rdf:first>
                                                                <rdf:rest>
                                                                    <rdf:Description>
                                                                        <rdf:type rdf:resource="http://www.w3.org/1999/02/22-rdf-syntax-ns#List"/>
                                                                        <rdf:first>Person</rdf:first>
                                                                        <rdf:rest rdf:resource="http://www.w3.org/1999/02/22-rdf-syntax-ns#nil"/>
                                                                    </rdf:Description>
                                                                </rdf:rest>
                                                            </rdf:Description>
                                                        </rdf:rest>
                                                    </rdf:Description>
                                                </rdf:rest>
                                            </rdf:Description>
                                        </rdf:rest>
                                    </rdf:Description>
                                </rdf:rest>
                            </rdf:Description>
                        </rdf:rest>
                    </rdf:Description>
                </owl:oneOf>
            </rdfs:Datatype>
        </rdfs:range>
        <rdfs:comment>This property represents a metadata field that indicates the type of a logging tag.</rdfs:comment>
    </owl:DatatypeProperty>
    


    <!-- http://www.semanticweb.org/cadex/ontologies/2020/1/untitled-ontology-71#hasNoteInfo -->

    <owl:DatatypeProperty rdf:about="http://www.semanticweb.org/cadex/ontologies/2020/1/untitled-ontology-71#hasNoteInfo">
        <rdfs:comment>This is the parent of a set of properties that represent metadata fields describing a note. This property should not be populated with a value because it does not itself represent a metadata field. Rather, it is used solely to organise the properties representing fields.</rdfs:comment>
    </owl:DatatypeProperty>
    


    <!-- http://www.semanticweb.org/cadex/ontologies/2020/1/untitled-ontology-71#hasNoteStatus -->

    <owl:DatatypeProperty rdf:about="http://www.semanticweb.org/cadex/ontologies/2020/1/untitled-ontology-71#hasNoteStatus">
        <rdfs:subPropertyOf rdf:resource="http://www.semanticweb.org/cadex/ontologies/2020/1/untitled-ontology-71#hasNoteInfo"/>
        <rdfs:domain rdf:resource="http://www.semanticweb.org/cadex/ontologies/2020/1/untitled-ontology-71#Note"/>
        <rdfs:range>
            <rdfs:Datatype>
                <owl:oneOf>
                    <rdf:Description>
                        <rdf:type rdf:resource="http://www.w3.org/1999/02/22-rdf-syntax-ns#List"/>
                        <rdf:first>Complete</rdf:first>
                        <rdf:rest>
                            <rdf:Description>
                                <rdf:type rdf:resource="http://www.w3.org/1999/02/22-rdf-syntax-ns#List"/>
                                <rdf:first>Open</rdf:first>
                                <rdf:rest rdf:resource="http://www.w3.org/1999/02/22-rdf-syntax-ns#nil"/>
                            </rdf:Description>
                        </rdf:rest>
                    </rdf:Description>
                </owl:oneOf>
            </rdfs:Datatype>
        </rdfs:range>
        <rdfs:comment>This property represents a metadata field that indicates the status of a note.</rdfs:comment>
    </owl:DatatypeProperty>
    


    <!-- http://www.semanticweb.org/cadex/ontologies/2020/1/untitled-ontology-71#hasPersonInfo -->

    <owl:DatatypeProperty rdf:about="http://www.semanticweb.org/cadex/ontologies/2020/1/untitled-ontology-71#hasPersonInfo">
        <rdfs:domain rdf:resource="http://www.semanticweb.org/cadex/ontologies/2020/1/untitled-ontology-71#Person"/>
        <rdfs:comment>This is the parent of a set of properties that represent metadata fields describing a person. This property should not be populated with a value because it does not itself represent a metadata field. Rather, it is used solely to organise the properties representing fields.</rdfs:comment>
    </owl:DatatypeProperty>
    


    <!-- http://www.semanticweb.org/cadex/ontologies/2020/1/untitled-ontology-71#hasProjectEpisodeTitle -->

    <owl:DatatypeProperty rdf:about="http://www.semanticweb.org/cadex/ontologies/2020/1/untitled-ontology-71#hasProjectEpisodeTitle">
        <rdfs:subPropertyOf rdf:resource="http://www.semanticweb.org/cadex/ontologies/2020/1/untitled-ontology-71#hasProjectInfo"/>
        <rdfs:domain rdf:resource="http://www.semanticweb.org/cadex/ontologies/2020/1/untitled-ontology-71#Project"/>
        <rdfs:range rdf:resource="http://www.w3.org/2001/XMLSchema#string"/>
        <rdfs:comment>This property represents a metadata field that indicates the episode title of a project.</rdfs:comment>
    </owl:DatatypeProperty>
    


    <!-- http://www.semanticweb.org/cadex/ontologies/2020/1/untitled-ontology-71#hasProjectGenre -->

    <owl:DatatypeProperty rdf:about="http://www.semanticweb.org/cadex/ontologies/2020/1/untitled-ontology-71#hasProjectGenre">
        <rdfs:subPropertyOf rdf:resource="http://www.semanticweb.org/cadex/ontologies/2020/1/untitled-ontology-71#hasProjectInfo"/>
        <rdfs:domain rdf:resource="http://www.semanticweb.org/cadex/ontologies/2020/1/untitled-ontology-71#Project"/>
        <rdfs:range rdf:resource="http://www.w3.org/2001/XMLSchema#string"/>
        <rdfs:comment>This property represents a metadata field that indicates the genre of a project.</rdfs:comment>
    </owl:DatatypeProperty>
    


    <!-- http://www.semanticweb.org/cadex/ontologies/2020/1/untitled-ontology-71#hasProjectInfo -->

    <owl:DatatypeProperty rdf:about="http://www.semanticweb.org/cadex/ontologies/2020/1/untitled-ontology-71#hasProjectInfo">
        <rdfs:domain rdf:resource="http://www.semanticweb.org/cadex/ontologies/2020/1/untitled-ontology-71#Project"/>
        <rdfs:comment>This is the parent of a set of properties that represent metadata fields describing a project. This property should not be populated with a value because it does not itself represent a metadata field. Rather, it is used solely to organise the properties representing fields.</rdfs:comment>
    </owl:DatatypeProperty>
    


    <!-- http://www.semanticweb.org/cadex/ontologies/2020/1/untitled-ontology-71#hasProjectName -->

    <owl:DatatypeProperty rdf:about="http://www.semanticweb.org/cadex/ontologies/2020/1/untitled-ontology-71#hasProjectName">
        <rdfs:subPropertyOf rdf:resource="http://www.semanticweb.org/cadex/ontologies/2020/1/untitled-ontology-71#hasProjectInfo"/>
        <rdfs:domain rdf:resource="http://www.semanticweb.org/cadex/ontologies/2020/1/untitled-ontology-71#Project"/>
        <rdfs:range rdf:resource="http://www.w3.org/2001/XMLSchema#string"/>
        <rdfs:comment>This property represents a metadata field that indicates the name of a project.</rdfs:comment>
    </owl:DatatypeProperty>
    


    <!-- http://www.semanticweb.org/cadex/ontologies/2020/1/untitled-ontology-71#hasProjectReelCount -->

    <owl:DatatypeProperty rdf:about="http://www.semanticweb.org/cadex/ontologies/2020/1/untitled-ontology-71#hasProjectReelCount">
        <rdfs:subPropertyOf rdf:resource="http://www.semanticweb.org/cadex/ontologies/2020/1/untitled-ontology-71#hasProjectInfo"/>
        <rdfs:domain rdf:resource="http://www.semanticweb.org/cadex/ontologies/2020/1/untitled-ontology-71#Project"/>
        <rdfs:range rdf:resource="http://www.w3.org/2001/XMLSchema#int"/>
        <rdfs:comment>This property represents a metadata field that indicates the reel count of a project.</rdfs:comment>
    </owl:DatatypeProperty>
    


    <!-- http://www.semanticweb.org/cadex/ontologies/2020/1/untitled-ontology-71#hasProjectSeriesNumber -->

    <owl:DatatypeProperty rdf:about="http://www.semanticweb.org/cadex/ontologies/2020/1/untitled-ontology-71#hasProjectSeriesNumber">
        <rdfs:subPropertyOf rdf:resource="http://www.semanticweb.org/cadex/ontologies/2020/1/untitled-ontology-71#hasProjectInfo"/>
        <rdfs:domain rdf:resource="http://www.semanticweb.org/cadex/ontologies/2020/1/untitled-ontology-71#Project"/>
        <rdfs:range rdf:resource="http://www.w3.org/2001/XMLSchema#int"/>
        <rdfs:comment>This property represents a metadata field that indicates the series number of a project.</rdfs:comment>
    </owl:DatatypeProperty>
    


    <!-- http://www.semanticweb.org/cadex/ontologies/2020/1/untitled-ontology-71#hasProjectTitle -->

    <owl:DatatypeProperty rdf:about="http://www.semanticweb.org/cadex/ontologies/2020/1/untitled-ontology-71#hasProjectTitle">
        <rdfs:subPropertyOf rdf:resource="http://www.semanticweb.org/cadex/ontologies/2020/1/untitled-ontology-71#hasProjectInfo"/>
        <rdfs:domain rdf:resource="http://www.semanticweb.org/cadex/ontologies/2020/1/untitled-ontology-71#Project"/>
        <rdfs:range rdf:resource="http://www.w3.org/2001/XMLSchema#string"/>
        <rdfs:comment>This property represents a metadata field that indicates the title of a project.</rdfs:comment>
    </owl:DatatypeProperty>
    


    <!-- http://www.semanticweb.org/cadex/ontologies/2020/1/untitled-ontology-71#hasPropID -->

    <owl:DatatypeProperty rdf:about="http://www.semanticweb.org/cadex/ontologies/2020/1/untitled-ontology-71#hasPropID">
        <rdfs:subPropertyOf rdf:resource="http://www.semanticweb.org/cadex/ontologies/2020/1/untitled-ontology-71#hasPropInfo"/>
        <rdfs:domain rdf:resource="http://www.semanticweb.org/cadex/ontologies/2020/1/untitled-ontology-71#Prop"/>
        <rdfs:range rdf:resource="http://www.w3.org/2001/XMLSchema#string"/>
        <rdfs:comment>This property represents a metadata field that indicates the ID of a prop.</rdfs:comment>
    </owl:DatatypeProperty>
    


    <!-- http://www.semanticweb.org/cadex/ontologies/2020/1/untitled-ontology-71#hasPropInfo -->

    <owl:DatatypeProperty rdf:about="http://www.semanticweb.org/cadex/ontologies/2020/1/untitled-ontology-71#hasPropInfo">
        <rdfs:domain rdf:resource="http://www.semanticweb.org/cadex/ontologies/2020/1/untitled-ontology-71#Prop"/>
        <rdfs:comment>This is the parent of a set of properties that represent metadata fields describing a prop. This property should not be populated with a value because it does not itself represent a metadata field. Rather, it is used solely to organise the properties representing fields.</rdfs:comment>
    </owl:DatatypeProperty>
    


    <!-- http://www.semanticweb.org/cadex/ontologies/2020/1/untitled-ontology-71#hasPropName -->

    <owl:DatatypeProperty rdf:about="http://www.semanticweb.org/cadex/ontologies/2020/1/untitled-ontology-71#hasPropName">
        <rdfs:subPropertyOf rdf:resource="http://www.semanticweb.org/cadex/ontologies/2020/1/untitled-ontology-71#hasPropInfo"/>
        <rdfs:domain rdf:resource="http://www.semanticweb.org/cadex/ontologies/2020/1/untitled-ontology-71#Prop"/>
        <rdfs:range rdf:resource="http://www.w3.org/2001/XMLSchema#string"/>
        <rdfs:comment>This property represents a metadata field that indicates the name of a prop.</rdfs:comment>
    </owl:DatatypeProperty>
    


    <!-- http://www.semanticweb.org/cadex/ontologies/2020/1/untitled-ontology-71#hasRecordInfo -->

    <owl:DatatypeProperty rdf:about="http://www.semanticweb.org/cadex/ontologies/2020/1/untitled-ontology-71#hasRecordInfo">
        <rdfs:comment>This is the parent of a set of properties that represent metadata fields describing a record. This property should not be populated with a value because it does not itself represent a metadata field. Rather, it is used solely to organise the properties representing fields.</rdfs:comment>
    </owl:DatatypeProperty>
    


    <!-- http://www.semanticweb.org/cadex/ontologies/2020/1/untitled-ontology-71#hasRentalEndDate -->

    <owl:DatatypeProperty rdf:about="http://www.semanticweb.org/cadex/ontologies/2020/1/untitled-ontology-71#hasRentalEndDate">
        <rdfs:subPropertyOf rdf:resource="http://www.semanticweb.org/cadex/ontologies/2020/1/untitled-ontology-71#hasRentalInfo"/>
        <rdfs:domain rdf:resource="http://www.semanticweb.org/cadex/ontologies/2020/1/untitled-ontology-71#Rental"/>
        <rdfs:range rdf:resource="http://www.w3.org/2001/XMLSchema#dateTimeStamp"/>
        <rdfs:comment>This property represents a metadata field that indicates the end date of a rental.</rdfs:comment>
    </owl:DatatypeProperty>
    


    <!-- http://www.semanticweb.org/cadex/ontologies/2020/1/untitled-ontology-71#hasRentalInfo -->

    <owl:DatatypeProperty rdf:about="http://www.semanticweb.org/cadex/ontologies/2020/1/untitled-ontology-71#hasRentalInfo">
        <rdfs:domain rdf:resource="http://www.semanticweb.org/cadex/ontologies/2020/1/untitled-ontology-71#Rental"/>
        <rdfs:comment>This is the parent of a set of properties that represent metadata fields describing a rental. This property should not be populated with a value because it does not itself represent a metadata field. Rather, it is used solely to organise the properties representing fields.</rdfs:comment>
    </owl:DatatypeProperty>
    


    <!-- http://www.semanticweb.org/cadex/ontologies/2020/1/untitled-ontology-71#hasRentalStartDate -->

    <owl:DatatypeProperty rdf:about="http://www.semanticweb.org/cadex/ontologies/2020/1/untitled-ontology-71#hasRentalStartDate">
        <rdfs:subPropertyOf rdf:resource="http://www.semanticweb.org/cadex/ontologies/2020/1/untitled-ontology-71#hasRentalInfo"/>
        <rdfs:domain rdf:resource="http://www.semanticweb.org/cadex/ontologies/2020/1/untitled-ontology-71#Rental"/>
        <rdfs:range rdf:resource="http://www.w3.org/2001/XMLSchema#dateTimeStamp"/>
        <rdfs:comment>This property represents a metadata field that indicates the start date of a rental.</rdfs:comment>
    </owl:DatatypeProperty>
    


    <!-- http://www.semanticweb.org/cadex/ontologies/2020/1/untitled-ontology-71#hasRollInfo -->

    <owl:DatatypeProperty rdf:about="http://www.semanticweb.org/cadex/ontologies/2020/1/untitled-ontology-71#hasRollInfo">
        <rdfs:domain rdf:resource="http://www.semanticweb.org/cadex/ontologies/2020/1/untitled-ontology-71#Roll"/>
        <rdfs:comment>This is the parent of a set of properties that represent metadata fields describing a roll. This property should not be populated with a value because it does not itself represent a metadata field. Rather, it is used solely to organise the properties representing fields.</rdfs:comment>
    </owl:DatatypeProperty>
    


    <!-- http://www.semanticweb.org/cadex/ontologies/2020/1/untitled-ontology-71#hasSceneCode -->

    <owl:DatatypeProperty rdf:about="http://www.semanticweb.org/cadex/ontologies/2020/1/untitled-ontology-71#hasSceneCode">
        <rdfs:subPropertyOf rdf:resource="http://www.semanticweb.org/cadex/ontologies/2020/1/untitled-ontology-71#hasSceneInfo"/>
        <rdfs:domain rdf:resource="http://www.semanticweb.org/cadex/ontologies/2020/1/untitled-ontology-71#Scene"/>
        <rdfs:range rdf:resource="http://www.w3.org/2001/XMLSchema#string"/>
        <rdfs:comment>This property represents a metadata field that indicates the code of a scene.</rdfs:comment>
    </owl:DatatypeProperty>
    


    <!-- http://www.semanticweb.org/cadex/ontologies/2020/1/untitled-ontology-71#hasSceneCuts -->

    <owl:DatatypeProperty rdf:about="http://www.semanticweb.org/cadex/ontologies/2020/1/untitled-ontology-71#hasSceneCuts">
        <rdfs:subPropertyOf rdf:resource="http://www.semanticweb.org/cadex/ontologies/2020/1/untitled-ontology-71#hasSceneInfo"/>
        <rdfs:domain rdf:resource="http://www.semanticweb.org/cadex/ontologies/2020/1/untitled-ontology-71#Scene"/>
        <rdfs:range rdf:resource="http://www.w3.org/2001/XMLSchema#string"/>
        <rdfs:comment>This property represents a metadata field that indicates the cuts of a scene.</rdfs:comment>
    </owl:DatatypeProperty>
    


    <!-- http://www.semanticweb.org/cadex/ontologies/2020/1/untitled-ontology-71#hasSceneDeliveries -->

    <owl:DatatypeProperty rdf:about="http://www.semanticweb.org/cadex/ontologies/2020/1/untitled-ontology-71#hasSceneDeliveries">
        <rdfs:subPropertyOf rdf:resource="http://www.semanticweb.org/cadex/ontologies/2020/1/untitled-ontology-71#hasSceneInfo"/>
        <rdfs:domain rdf:resource="http://www.semanticweb.org/cadex/ontologies/2020/1/untitled-ontology-71#Scene"/>
        <rdfs:range rdf:resource="http://www.w3.org/2001/XMLSchema#string"/>
        <rdfs:comment>This property represents a metadata field that indicates the deliveries of a scene.</rdfs:comment>
    </owl:DatatypeProperty>
    


    <!-- http://www.semanticweb.org/cadex/ontologies/2020/1/untitled-ontology-71#hasSceneDescription -->

    <owl:DatatypeProperty rdf:about="http://www.semanticweb.org/cadex/ontologies/2020/1/untitled-ontology-71#hasSceneDescription">
        <rdfs:subPropertyOf rdf:resource="http://www.semanticweb.org/cadex/ontologies/2020/1/untitled-ontology-71#hasSceneInfo"/>
        <rdfs:domain rdf:resource="http://www.semanticweb.org/cadex/ontologies/2020/1/untitled-ontology-71#Scene"/>
        <rdfs:range rdf:resource="http://www.w3.org/2001/XMLSchema#string"/>
        <rdfs:comment>This property represents a metadata field that indicates the description of a scene.</rdfs:comment>
    </owl:DatatypeProperty>
    


    <!-- http://www.semanticweb.org/cadex/ontologies/2020/1/untitled-ontology-71#hasSceneFilmstripThumbnail -->

    <owl:DatatypeProperty rdf:about="http://www.semanticweb.org/cadex/ontologies/2020/1/untitled-ontology-71#hasSceneFilmstripThumbnail">
        <rdfs:subPropertyOf rdf:resource="http://www.semanticweb.org/cadex/ontologies/2020/1/untitled-ontology-71#hasSceneInfo"/>
        <rdfs:domain rdf:resource="http://www.semanticweb.org/cadex/ontologies/2020/1/untitled-ontology-71#Scene"/>
    </owl:DatatypeProperty>
    


    <!-- http://www.semanticweb.org/cadex/ontologies/2020/1/untitled-ontology-71#hasSceneInfo -->

    <owl:DatatypeProperty rdf:about="http://www.semanticweb.org/cadex/ontologies/2020/1/untitled-ontology-71#hasSceneInfo">
        <rdfs:domain rdf:resource="http://www.semanticweb.org/cadex/ontologies/2020/1/untitled-ontology-71#Scene"/>
        <rdfs:comment>This is the parent of a set of properties that represent metadata fields describing a scene. This property should not be populated with a value because it does not itself represent a metadata field. Rather, it is used solely to organise the properties representing fields.</rdfs:comment>
    </owl:DatatypeProperty>
    


    <!-- http://www.semanticweb.org/cadex/ontologies/2020/1/untitled-ontology-71#hasSceneLaunches -->

    <owl:DatatypeProperty rdf:about="http://www.semanticweb.org/cadex/ontologies/2020/1/untitled-ontology-71#hasSceneLaunches">
        <rdfs:subPropertyOf rdf:resource="http://www.semanticweb.org/cadex/ontologies/2020/1/untitled-ontology-71#hasSceneInfo"/>
        <rdfs:domain rdf:resource="http://www.semanticweb.org/cadex/ontologies/2020/1/untitled-ontology-71#Scene"/>
        <rdfs:range rdf:resource="http://www.w3.org/2001/XMLSchema#string"/>
        <rdfs:comment>This property represents a metadata field that indicates the launchs of a scene.</rdfs:comment>
    </owl:DatatypeProperty>
    


    <!-- http://www.semanticweb.org/cadex/ontologies/2020/1/untitled-ontology-71#hasSceneName -->

    <owl:DatatypeProperty rdf:about="http://www.semanticweb.org/cadex/ontologies/2020/1/untitled-ontology-71#hasSceneName">
        <rdfs:subPropertyOf rdf:resource="http://www.semanticweb.org/cadex/ontologies/2020/1/untitled-ontology-71#hasSceneInfo"/>
        <rdfs:domain rdf:resource="http://www.semanticweb.org/cadex/ontologies/2020/1/untitled-ontology-71#Scene"/>
        <rdfs:range rdf:resource="http://www.w3.org/2001/XMLSchema#string"/>
        <rdfs:comment>This property represents a metadata field that indicates the name of a scene.</rdfs:comment>
    </owl:DatatypeProperty>
    


    <!-- http://www.semanticweb.org/cadex/ontologies/2020/1/untitled-ontology-71#hasSceneNameAlternative -->

    <owl:DatatypeProperty rdf:about="http://www.semanticweb.org/cadex/ontologies/2020/1/untitled-ontology-71#hasSceneNameAlternative">
        <rdfs:subPropertyOf rdf:resource="http://www.semanticweb.org/cadex/ontologies/2020/1/untitled-ontology-71#hasSceneInfo"/>
        <rdfs:domain rdf:resource="http://www.semanticweb.org/cadex/ontologies/2020/1/untitled-ontology-71#Scene"/>
        <rdfs:range rdf:resource="http://www.w3.org/2001/XMLSchema#string"/>
        <rdfs:comment>This property represents a metadata field that indicates the alternative name of a scene.</rdfs:comment>
    </owl:DatatypeProperty>
    


    <!-- http://www.semanticweb.org/cadex/ontologies/2020/1/untitled-ontology-71#hasSceneNumber -->

    <owl:DatatypeProperty rdf:about="http://www.semanticweb.org/cadex/ontologies/2020/1/untitled-ontology-71#hasSceneNumber">
        <rdfs:subPropertyOf rdf:resource="http://www.semanticweb.org/cadex/ontologies/2020/1/untitled-ontology-71#hasSceneInfo"/>
        <rdfs:domain rdf:resource="http://www.semanticweb.org/cadex/ontologies/2020/1/untitled-ontology-71#Scene"/>
        <rdfs:range rdf:resource="http://www.w3.org/2001/XMLSchema#int"/>
        <rdfs:comment>This property represents a metadata field that indicates the numerical ID of a scene.</rdfs:comment>
    </owl:DatatypeProperty>
    


    <!-- http://www.semanticweb.org/cadex/ontologies/2020/1/untitled-ontology-71#hasSceneScriptLocation -->

    <owl:DatatypeProperty rdf:about="http://www.semanticweb.org/cadex/ontologies/2020/1/untitled-ontology-71#hasSceneScriptLocation">
        <rdfs:subPropertyOf rdf:resource="http://www.semanticweb.org/cadex/ontologies/2020/1/untitled-ontology-71#hasSceneInfo"/>
        <rdfs:domain rdf:resource="http://www.semanticweb.org/cadex/ontologies/2020/1/untitled-ontology-71#Scene"/>
        <rdfs:range rdf:resource="http://www.w3.org/2001/XMLSchema#string"/>
        <rdfs:comment>This property represents a metadata field that indicates the location of the scene in a script.</rdfs:comment>
    </owl:DatatypeProperty>
    


    <!-- http://www.semanticweb.org/cadex/ontologies/2020/1/untitled-ontology-71#hasSceneSequenceLink -->

    <owl:DatatypeProperty rdf:about="http://www.semanticweb.org/cadex/ontologies/2020/1/untitled-ontology-71#hasSceneSequenceLink">
        <rdfs:subPropertyOf rdf:resource="http://www.semanticweb.org/cadex/ontologies/2020/1/untitled-ontology-71#hasSceneInfo"/>
        <rdfs:domain rdf:resource="http://www.semanticweb.org/cadex/ontologies/2020/1/untitled-ontology-71#Scene"/>
        <rdfs:range rdf:resource="http://www.w3.org/2001/XMLSchema#string"/>
        <rdfs:comment>This property represents a metadata field that indicates the sequence link of a scene.</rdfs:comment>
    </owl:DatatypeProperty>
    


    <!-- http://www.semanticweb.org/cadex/ontologies/2020/1/untitled-ontology-71#hasSceneSequencePrefix -->

    <owl:DatatypeProperty rdf:about="http://www.semanticweb.org/cadex/ontologies/2020/1/untitled-ontology-71#hasSceneSequencePrefix">
        <rdfs:subPropertyOf rdf:resource="http://www.semanticweb.org/cadex/ontologies/2020/1/untitled-ontology-71#hasSceneInfo"/>
        <rdfs:domain rdf:resource="http://www.semanticweb.org/cadex/ontologies/2020/1/untitled-ontology-71#Scene"/>
        <rdfs:range rdf:resource="http://www.w3.org/2001/XMLSchema#string"/>
        <rdfs:comment>This property represents a metadata field that indicates the sequence prefix of a scene.</rdfs:comment>
    </owl:DatatypeProperty>
    


    <!-- http://www.semanticweb.org/cadex/ontologies/2020/1/untitled-ontology-71#hasSceneStatus -->

    <owl:DatatypeProperty rdf:about="http://www.semanticweb.org/cadex/ontologies/2020/1/untitled-ontology-71#hasSceneStatus">
        <rdfs:subPropertyOf rdf:resource="http://www.semanticweb.org/cadex/ontologies/2020/1/untitled-ontology-71#hasSceneInfo"/>
        <rdfs:domain rdf:resource="http://www.semanticweb.org/cadex/ontologies/2020/1/untitled-ontology-71#Scene"/>
        <rdfs:range rdf:resource="http://www.w3.org/2001/XMLSchema#string"/>
        <rdfs:comment>This property represents a metadata field that indicates the status of a scene.</rdfs:comment>
    </owl:DatatypeProperty>
    


    <!-- http://www.semanticweb.org/cadex/ontologies/2020/1/untitled-ontology-71#hasSceneTag -->

    <owl:DatatypeProperty rdf:about="http://www.semanticweb.org/cadex/ontologies/2020/1/untitled-ontology-71#hasSceneTag">
        <rdfs:subPropertyOf rdf:resource="http://www.semanticweb.org/cadex/ontologies/2020/1/untitled-ontology-71#hasSceneInfo"/>
        <rdfs:domain rdf:resource="http://www.semanticweb.org/cadex/ontologies/2020/1/untitled-ontology-71#Scene"/>
        <rdfs:range rdf:resource="http://www.w3.org/2001/XMLSchema#string"/>
        <rdfs:comment>This property represents a metadata field that indicates the tags assigned to a scene.</rdfs:comment>
    </owl:DatatypeProperty>
    


    <!-- http://www.semanticweb.org/cadex/ontologies/2020/1/untitled-ontology-71#hasSceneThumbnail -->

    <owl:DatatypeProperty rdf:about="http://www.semanticweb.org/cadex/ontologies/2020/1/untitled-ontology-71#hasSceneThumbnail">
        <rdfs:subPropertyOf rdf:resource="http://www.semanticweb.org/cadex/ontologies/2020/1/untitled-ontology-71#hasSceneInfo"/>
        <rdfs:domain rdf:resource="http://www.semanticweb.org/cadex/ontologies/2020/1/untitled-ontology-71#Scene"/>
    </owl:DatatypeProperty>
    


    <!-- http://www.semanticweb.org/cadex/ontologies/2020/1/untitled-ontology-71#hasSceneType -->

    <owl:DatatypeProperty rdf:about="http://www.semanticweb.org/cadex/ontologies/2020/1/untitled-ontology-71#hasSceneType">
        <rdfs:subPropertyOf rdf:resource="http://www.semanticweb.org/cadex/ontologies/2020/1/untitled-ontology-71#hasSceneInfo"/>
        <rdfs:domain rdf:resource="http://www.semanticweb.org/cadex/ontologies/2020/1/untitled-ontology-71#Scene"/>
        <rdfs:range rdf:resource="http://www.w3.org/2001/XMLSchema#string"/>
        <rdfs:comment>This property represents a metadata field that indicates the type of a scene.</rdfs:comment>
    </owl:DatatypeProperty>
    


    <!-- http://www.semanticweb.org/cadex/ontologies/2020/1/untitled-ontology-71#hasSceneVersionLink -->

    <owl:DatatypeProperty rdf:about="http://www.semanticweb.org/cadex/ontologies/2020/1/untitled-ontology-71#hasSceneVersionLink">
        <rdfs:subPropertyOf rdf:resource="http://www.semanticweb.org/cadex/ontologies/2020/1/untitled-ontology-71#hasSceneInfo"/>
        <rdfs:domain rdf:resource="http://www.semanticweb.org/cadex/ontologies/2020/1/untitled-ontology-71#Scene"/>
        <rdfs:range rdf:resource="http://www.w3.org/2001/XMLSchema#string"/>
        <rdfs:comment>This property represents a metadata field that indicates the version link of a scene.</rdfs:comment>
    </owl:DatatypeProperty>
    


    <!-- http://www.semanticweb.org/cadex/ontologies/2020/1/untitled-ontology-71#hasShootCode -->

    <owl:DatatypeProperty rdf:about="http://www.semanticweb.org/cadex/ontologies/2020/1/untitled-ontology-71#hasShootCode">
        <rdfs:subPropertyOf rdf:resource="http://www.semanticweb.org/cadex/ontologies/2020/1/untitled-ontology-71#hasShootInfo"/>
        <rdfs:domain rdf:resource="http://www.semanticweb.org/cadex/ontologies/2020/1/untitled-ontology-71#Shoot"/>
        <rdfs:range rdf:resource="http://www.w3.org/2001/XMLSchema#string"/>
        <rdfs:comment>This property represents a metadata field that indicates the code of a shoot.</rdfs:comment>
    </owl:DatatypeProperty>
    


    <!-- http://www.semanticweb.org/cadex/ontologies/2020/1/untitled-ontology-71#hasShootDayDate -->

    <owl:DatatypeProperty rdf:about="http://www.semanticweb.org/cadex/ontologies/2020/1/untitled-ontology-71#hasShootDayDate">
        <rdfs:subPropertyOf rdf:resource="http://www.semanticweb.org/cadex/ontologies/2020/1/untitled-ontology-71#hasShootDayInfo"/>
        <rdfs:domain rdf:resource="http://www.semanticweb.org/cadex/ontologies/2020/1/untitled-ontology-71#ShootDay"/>
        <rdfs:range rdf:resource="http://www.w3.org/2001/XMLSchema#dateTimeStamp"/>
        <rdfs:comment>This property represents a metadata field that indicates the date of a shoot day.</rdfs:comment>
    </owl:DatatypeProperty>
    


    <!-- http://www.semanticweb.org/cadex/ontologies/2020/1/untitled-ontology-71#hasShootDayInfo -->

    <owl:DatatypeProperty rdf:about="http://www.semanticweb.org/cadex/ontologies/2020/1/untitled-ontology-71#hasShootDayInfo">
        <rdfs:subPropertyOf rdf:resource="http://www.w3.org/2002/07/owl#topDataProperty"/>
        <rdfs:comment>This is the parent of a set of properties that represent metadata fields describing a shoot day. This property should not be populated with a value because it does not itself represent a metadata field. Rather, it is used solely to organise the properties representing fields.</rdfs:comment>
    </owl:DatatypeProperty>
    


    <!-- http://www.semanticweb.org/cadex/ontologies/2020/1/untitled-ontology-71#hasShootDayNumber -->

    <owl:DatatypeProperty rdf:about="http://www.semanticweb.org/cadex/ontologies/2020/1/untitled-ontology-71#hasShootDayNumber">
        <rdfs:subPropertyOf rdf:resource="http://www.semanticweb.org/cadex/ontologies/2020/1/untitled-ontology-71#hasShootDayInfo"/>
        <rdfs:domain rdf:resource="http://www.semanticweb.org/cadex/ontologies/2020/1/untitled-ontology-71#ShootDay"/>
        <rdfs:range rdf:resource="http://www.w3.org/2001/XMLSchema#int"/>
        <rdfs:comment>This property represents a metadata field that indicates the number of a shoot day (e.g. the 5th day of a shoot).</rdfs:comment>
    </owl:DatatypeProperty>
    


    <!-- http://www.semanticweb.org/cadex/ontologies/2020/1/untitled-ontology-71#hasShootDayTimeZone -->

    <owl:DatatypeProperty rdf:about="http://www.semanticweb.org/cadex/ontologies/2020/1/untitled-ontology-71#hasShootDayTimeZone">
        <rdfs:subPropertyOf rdf:resource="http://www.semanticweb.org/cadex/ontologies/2020/1/untitled-ontology-71#hasShootDayInfo"/>
        <rdfs:domain rdf:resource="http://www.semanticweb.org/cadex/ontologies/2020/1/untitled-ontology-71#ShootDay"/>
        <rdfs:range rdf:resource="http://www.w3.org/2001/XMLSchema#string"/>
        <rdfs:comment>This property represents a metadata field that indicates the time zone of a shoot day.</rdfs:comment>
    </owl:DatatypeProperty>
    


    <!-- http://www.semanticweb.org/cadex/ontologies/2020/1/untitled-ontology-71#hasShootDeliveries -->

    <owl:DatatypeProperty rdf:about="http://www.semanticweb.org/cadex/ontologies/2020/1/untitled-ontology-71#hasShootDeliveries">
        <rdfs:subPropertyOf rdf:resource="http://www.semanticweb.org/cadex/ontologies/2020/1/untitled-ontology-71#hasShootInfo"/>
        <rdfs:domain rdf:resource="http://www.semanticweb.org/cadex/ontologies/2020/1/untitled-ontology-71#Shoot"/>
        <rdfs:range rdf:resource="http://www.w3.org/2001/XMLSchema#string"/>
        <rdfs:comment>This property represents a metadata field that indicates the code of a shoot.</rdfs:comment>
    </owl:DatatypeProperty>
    


    <!-- http://www.semanticweb.org/cadex/ontologies/2020/1/untitled-ontology-71#hasShootDescription -->

    <owl:DatatypeProperty rdf:about="http://www.semanticweb.org/cadex/ontologies/2020/1/untitled-ontology-71#hasShootDescription">
        <rdfs:subPropertyOf rdf:resource="http://www.semanticweb.org/cadex/ontologies/2020/1/untitled-ontology-71#hasShootInfo"/>
        <rdfs:domain rdf:resource="http://www.semanticweb.org/cadex/ontologies/2020/1/untitled-ontology-71#Shoot"/>
        <rdfs:range rdf:resource="http://www.w3.org/2001/XMLSchema#string"/>
        <rdfs:comment>This property represents a metadata field that indicates the description of a shoot.</rdfs:comment>
    </owl:DatatypeProperty>
    


    <!-- http://www.semanticweb.org/cadex/ontologies/2020/1/untitled-ontology-71#hasShootEnvironment -->

    <owl:DatatypeProperty rdf:about="http://www.semanticweb.org/cadex/ontologies/2020/1/untitled-ontology-71#hasShootEnvironment">
        <rdfs:subPropertyOf rdf:resource="http://www.semanticweb.org/cadex/ontologies/2020/1/untitled-ontology-71#hasShootInfo"/>
        <rdfs:domain rdf:resource="http://www.semanticweb.org/cadex/ontologies/2020/1/untitled-ontology-71#Shoot"/>
        <rdfs:range rdf:resource="http://www.w3.org/2001/XMLSchema#string"/>
        <rdfs:comment>This property represents a metadata field that indicates the environment of a shoot.</rdfs:comment>
    </owl:DatatypeProperty>
    


    <!-- http://www.semanticweb.org/cadex/ontologies/2020/1/untitled-ontology-71#hasShootFilmstripThumbnail -->

    <owl:DatatypeProperty rdf:about="http://www.semanticweb.org/cadex/ontologies/2020/1/untitled-ontology-71#hasShootFilmstripThumbnail">
        <rdfs:subPropertyOf rdf:resource="http://www.semanticweb.org/cadex/ontologies/2020/1/untitled-ontology-71#hasShootInfo"/>
        <rdfs:domain rdf:resource="http://www.semanticweb.org/cadex/ontologies/2020/1/untitled-ontology-71#Shoot"/>
    </owl:DatatypeProperty>
    


    <!-- http://www.semanticweb.org/cadex/ontologies/2020/1/untitled-ontology-71#hasShootInfo -->

    <owl:DatatypeProperty rdf:about="http://www.semanticweb.org/cadex/ontologies/2020/1/untitled-ontology-71#hasShootInfo">
        <rdfs:domain rdf:resource="http://www.semanticweb.org/cadex/ontologies/2020/1/untitled-ontology-71#Shoot"/>
        <rdfs:comment>This is the parent of a set of properties that represent metadata fields describing a shoot. This property should not be populated with a value because it does not itself represent a metadata field. Rather, it is used solely to organise the properties representing fields.</rdfs:comment>
    </owl:DatatypeProperty>
    


    <!-- http://www.semanticweb.org/cadex/ontologies/2020/1/untitled-ontology-71#hasShootLocationDescription -->

    <owl:DatatypeProperty rdf:about="http://www.semanticweb.org/cadex/ontologies/2020/1/untitled-ontology-71#hasShootLocationDescription">
        <rdfs:subPropertyOf rdf:resource="http://www.semanticweb.org/cadex/ontologies/2020/1/untitled-ontology-71#hasShootInfo"/>
        <rdfs:domain rdf:resource="http://www.semanticweb.org/cadex/ontologies/2020/1/untitled-ontology-71#Shoot"/>
        <rdfs:range rdf:resource="http://www.w3.org/2001/XMLSchema#string"/>
        <rdfs:comment>This property represents a metadata field that indicates the shoot-specific description of the shoot&apos;s location.</rdfs:comment>
    </owl:DatatypeProperty>
    


    <!-- http://www.semanticweb.org/cadex/ontologies/2020/1/untitled-ontology-71#hasShootNameAlternative -->

    <owl:DatatypeProperty rdf:about="http://www.semanticweb.org/cadex/ontologies/2020/1/untitled-ontology-71#hasShootNameAlternative">
        <rdfs:subPropertyOf rdf:resource="http://www.semanticweb.org/cadex/ontologies/2020/1/untitled-ontology-71#hasShootInfo"/>
        <rdfs:domain rdf:resource="http://www.semanticweb.org/cadex/ontologies/2020/1/untitled-ontology-71#Shoot"/>
        <rdfs:range rdf:resource="http://www.w3.org/2001/XMLSchema#string"/>
        <rdfs:comment>This property represents a metadata field that indicates the alternative name of a shoot.</rdfs:comment>
    </owl:DatatypeProperty>
    


    <!-- http://www.semanticweb.org/cadex/ontologies/2020/1/untitled-ontology-71#hasShootScriptLocation -->

    <owl:DatatypeProperty rdf:about="http://www.semanticweb.org/cadex/ontologies/2020/1/untitled-ontology-71#hasShootScriptLocation">
        <rdfs:subPropertyOf rdf:resource="http://www.semanticweb.org/cadex/ontologies/2020/1/untitled-ontology-71#hasShootInfo"/>
        <rdfs:domain rdf:resource="http://www.semanticweb.org/cadex/ontologies/2020/1/untitled-ontology-71#Shoot"/>
        <rdfs:range rdf:resource="http://www.w3.org/2001/XMLSchema#string"/>
        <rdfs:comment>This property represents a metadata field that indicates the location of the shoot in a script.</rdfs:comment>
    </owl:DatatypeProperty>
    


    <!-- http://www.semanticweb.org/cadex/ontologies/2020/1/untitled-ontology-71#hasShootSequence -->

    <owl:DatatypeProperty rdf:about="http://www.semanticweb.org/cadex/ontologies/2020/1/untitled-ontology-71#hasShootSequence">
        <rdfs:subPropertyOf rdf:resource="http://www.semanticweb.org/cadex/ontologies/2020/1/untitled-ontology-71#hasShootInfo"/>
        <rdfs:domain rdf:resource="http://www.semanticweb.org/cadex/ontologies/2020/1/untitled-ontology-71#Shoot"/>
        <rdfs:range rdf:resource="http://www.w3.org/2001/XMLSchema#string"/>
        <rdfs:comment>This property represents a metadata field that indicates the sequence of a shoot.</rdfs:comment>
    </owl:DatatypeProperty>
    


    <!-- http://www.semanticweb.org/cadex/ontologies/2020/1/untitled-ontology-71#hasShootStatus -->

    <owl:DatatypeProperty rdf:about="http://www.semanticweb.org/cadex/ontologies/2020/1/untitled-ontology-71#hasShootStatus">
        <rdfs:subPropertyOf rdf:resource="http://www.semanticweb.org/cadex/ontologies/2020/1/untitled-ontology-71#hasShootInfo"/>
        <rdfs:domain rdf:resource="http://www.semanticweb.org/cadex/ontologies/2020/1/untitled-ontology-71#Shoot"/>
        <rdfs:range rdf:resource="http://www.w3.org/2001/XMLSchema#string"/>
        <rdfs:comment>This property represents a metadata field that indicates the status of a shoot.</rdfs:comment>
    </owl:DatatypeProperty>
    


    <!-- http://www.semanticweb.org/cadex/ontologies/2020/1/untitled-ontology-71#hasShootTag -->

    <owl:DatatypeProperty rdf:about="http://www.semanticweb.org/cadex/ontologies/2020/1/untitled-ontology-71#hasShootTag">
        <rdfs:subPropertyOf rdf:resource="http://www.semanticweb.org/cadex/ontologies/2020/1/untitled-ontology-71#hasShootInfo"/>
        <rdfs:domain rdf:resource="http://www.semanticweb.org/cadex/ontologies/2020/1/untitled-ontology-71#Shoot"/>
        <rdfs:range rdf:resource="http://www.w3.org/2001/XMLSchema#string"/>
        <rdfs:comment>This property represents a metadata field that indicates the tags assigned to a shoot.</rdfs:comment>
    </owl:DatatypeProperty>
    


    <!-- http://www.semanticweb.org/cadex/ontologies/2020/1/untitled-ontology-71#hasShootThumbnail -->

    <owl:DatatypeProperty rdf:about="http://www.semanticweb.org/cadex/ontologies/2020/1/untitled-ontology-71#hasShootThumbnail">
        <rdfs:subPropertyOf rdf:resource="http://www.semanticweb.org/cadex/ontologies/2020/1/untitled-ontology-71#hasShootInfo"/>
        <rdfs:domain rdf:resource="http://www.semanticweb.org/cadex/ontologies/2020/1/untitled-ontology-71#Shoot"/>
    </owl:DatatypeProperty>
    


    <!-- http://www.semanticweb.org/cadex/ontologies/2020/1/untitled-ontology-71#hasShotInfo -->

    <owl:DatatypeProperty rdf:about="http://www.semanticweb.org/cadex/ontologies/2020/1/untitled-ontology-71#hasShotInfo">
        <rdfs:domain rdf:resource="http://www.semanticweb.org/cadex/ontologies/2020/1/untitled-ontology-71#Shot"/>
        <rdfs:comment>This is the parent of a set of properties that represent metadata fields describing a shot. This property should not be populated with a value because it does not itself represent a metadata field. Rather, it is used solely to organise the properties representing fields.</rdfs:comment>
    </owl:DatatypeProperty>
    


    <!-- http://www.semanticweb.org/cadex/ontologies/2020/1/untitled-ontology-71#hasShotNumber -->

    <owl:DatatypeProperty rdf:about="http://www.semanticweb.org/cadex/ontologies/2020/1/untitled-ontology-71#hasShotNumber">
        <rdfs:subPropertyOf rdf:resource="http://www.semanticweb.org/cadex/ontologies/2020/1/untitled-ontology-71#hasShotInfo"/>
        <rdfs:domain rdf:resource="http://www.semanticweb.org/cadex/ontologies/2020/1/untitled-ontology-71#Shot"/>
        <rdfs:range rdf:resource="http://www.w3.org/2001/XMLSchema#int"/>
        <rdfs:comment>This property represents a metadata field that indicates the numerical ID of a shot.</rdfs:comment>
    </owl:DatatypeProperty>
    


    <!-- http://www.semanticweb.org/cadex/ontologies/2020/1/untitled-ontology-71#hasSlateAspectRatio -->

    <owl:DatatypeProperty rdf:about="http://www.semanticweb.org/cadex/ontologies/2020/1/untitled-ontology-71#hasSlateAspectRatio">
        <rdfs:subPropertyOf rdf:resource="http://www.semanticweb.org/cadex/ontologies/2020/1/untitled-ontology-71#hasSlateInfo"/>
        <rdfs:domain rdf:resource="http://www.semanticweb.org/cadex/ontologies/2020/1/untitled-ontology-71#Slate"/>
        <rdfs:range rdf:resource="http://www.w3.org/2001/XMLSchema#string"/>
        <rdfs:comment>This property represents a metadata field that indicates the aspect ratio of a slate.</rdfs:comment>
    </owl:DatatypeProperty>
    


    <!-- http://www.semanticweb.org/cadex/ontologies/2020/1/untitled-ontology-71#hasSlateCameraInfo -->

    <owl:DatatypeProperty rdf:about="http://www.semanticweb.org/cadex/ontologies/2020/1/untitled-ontology-71#hasSlateCameraInfo">
        <rdfs:subPropertyOf rdf:resource="http://www.semanticweb.org/cadex/ontologies/2020/1/untitled-ontology-71#hasSlateInfo"/>
        <rdfs:domain rdf:resource="http://www.semanticweb.org/cadex/ontologies/2020/1/untitled-ontology-71#Slate"/>
        <rdfs:comment>This is the parent of a set of properties that represent metadata fields describing slate-specific information about a camera. This property should not be populated with a value because it does not itself represent a metadata field. Rather, it is used solely to organise the properties representing fields.</rdfs:comment>
    </owl:DatatypeProperty>
    


    <!-- http://www.semanticweb.org/cadex/ontologies/2020/1/untitled-ontology-71#hasSlateDataOp -->

    <owl:DatatypeProperty rdf:about="http://www.semanticweb.org/cadex/ontologies/2020/1/untitled-ontology-71#hasSlateDataOp">
        <rdfs:subPropertyOf rdf:resource="http://www.semanticweb.org/cadex/ontologies/2020/1/untitled-ontology-71#hasSlateInfo"/>
        <rdfs:domain rdf:resource="http://www.semanticweb.org/cadex/ontologies/2020/1/untitled-ontology-71#Slate"/>
        <rdfs:range rdf:resource="http://www.w3.org/2001/XMLSchema#string"/>
        <rdfs:comment>This property represents a metadata field that indicates the data op of a slate.</rdfs:comment>
    </owl:DatatypeProperty>
    


    <!-- http://www.semanticweb.org/cadex/ontologies/2020/1/untitled-ontology-71#hasSlateDataOpChecklist -->

    <owl:DatatypeProperty rdf:about="http://www.semanticweb.org/cadex/ontologies/2020/1/untitled-ontology-71#hasSlateDataOpChecklist">
        <rdfs:subPropertyOf rdf:resource="http://www.semanticweb.org/cadex/ontologies/2020/1/untitled-ontology-71#hasSlateInfo"/>
        <rdfs:domain rdf:resource="http://www.semanticweb.org/cadex/ontologies/2020/1/untitled-ontology-71#Slate"/>
        <rdfs:range rdf:resource="http://www.w3.org/2001/XMLSchema#string"/>
        <rdfs:comment>This property represents a metadata field that indicates the data op checklist of a slate.</rdfs:comment>
    </owl:DatatypeProperty>
    


    <!-- http://www.semanticweb.org/cadex/ontologies/2020/1/untitled-ontology-71#hasSlateDeliveries -->

    <owl:DatatypeProperty rdf:about="http://www.semanticweb.org/cadex/ontologies/2020/1/untitled-ontology-71#hasSlateDeliveries">
        <rdfs:subPropertyOf rdf:resource="http://www.semanticweb.org/cadex/ontologies/2020/1/untitled-ontology-71#hasSlateInfo"/>
        <rdfs:domain rdf:resource="http://www.semanticweb.org/cadex/ontologies/2020/1/untitled-ontology-71#Slate"/>
        <rdfs:range rdf:resource="http://www.w3.org/2001/XMLSchema#string"/>
        <rdfs:comment>This property represents a metadata field that indicates the deliveries of a slate.</rdfs:comment>
    </owl:DatatypeProperty>
    


    <!-- http://www.semanticweb.org/cadex/ontologies/2020/1/untitled-ontology-71#hasSlateDescription -->

    <owl:DatatypeProperty rdf:about="http://www.semanticweb.org/cadex/ontologies/2020/1/untitled-ontology-71#hasSlateDescription">
        <rdfs:subPropertyOf rdf:resource="http://www.semanticweb.org/cadex/ontologies/2020/1/untitled-ontology-71#hasSlateInfo"/>
        <rdfs:domain rdf:resource="http://www.semanticweb.org/cadex/ontologies/2020/1/untitled-ontology-71#Slate"/>
        <rdfs:range rdf:resource="http://www.w3.org/2001/XMLSchema#string"/>
        <rdfs:comment>This property represents a metadata field that indicates the description of a slate.</rdfs:comment>
    </owl:DatatypeProperty>
    


    <!-- http://www.semanticweb.org/cadex/ontologies/2020/1/untitled-ontology-71#hasSlateDuration -->

    <owl:DatatypeProperty rdf:about="http://www.semanticweb.org/cadex/ontologies/2020/1/untitled-ontology-71#hasSlateDuration">
        <rdfs:subPropertyOf rdf:resource="http://www.semanticweb.org/cadex/ontologies/2020/1/untitled-ontology-71#hasSlateInfo"/>
        <rdfs:domain rdf:resource="http://www.semanticweb.org/cadex/ontologies/2020/1/untitled-ontology-71#Slate"/>
        <rdfs:range rdf:resource="http://www.w3.org/2001/XMLSchema#string"/>
        <rdfs:comment>This property represents a metadata field that indicates the duration of a slate.</rdfs:comment>
    </owl:DatatypeProperty>
    


    <!-- http://www.semanticweb.org/cadex/ontologies/2020/1/untitled-ontology-71#hasSlateElement -->

    <owl:DatatypeProperty rdf:about="http://www.semanticweb.org/cadex/ontologies/2020/1/untitled-ontology-71#hasSlateElement">
        <rdfs:subPropertyOf rdf:resource="http://www.semanticweb.org/cadex/ontologies/2020/1/untitled-ontology-71#hasSlateInfo"/>
        <rdfs:domain rdf:resource="http://www.semanticweb.org/cadex/ontologies/2020/1/untitled-ontology-71#Slate"/>
        <rdfs:range rdf:resource="http://www.w3.org/2001/XMLSchema#string"/>
        <rdfs:comment>This property represents a metadata field that indicates the element of a slate.</rdfs:comment>
    </owl:DatatypeProperty>
    


    <!-- http://www.semanticweb.org/cadex/ontologies/2020/1/untitled-ontology-71#hasSlateFilmstripThumbnail -->

    <owl:DatatypeProperty rdf:about="http://www.semanticweb.org/cadex/ontologies/2020/1/untitled-ontology-71#hasSlateFilmstripThumbnail">
        <rdfs:subPropertyOf rdf:resource="http://www.semanticweb.org/cadex/ontologies/2020/1/untitled-ontology-71#hasSlateInfo"/>
        <rdfs:domain rdf:resource="http://www.semanticweb.org/cadex/ontologies/2020/1/untitled-ontology-71#Slate"/>
    </owl:DatatypeProperty>
    


    <!-- http://www.semanticweb.org/cadex/ontologies/2020/1/untitled-ontology-71#hasSlateFocusUnit -->

    <owl:DatatypeProperty rdf:about="http://www.semanticweb.org/cadex/ontologies/2020/1/untitled-ontology-71#hasSlateFocusUnit">
        <rdfs:subPropertyOf rdf:resource="http://www.semanticweb.org/cadex/ontologies/2020/1/untitled-ontology-71#hasSlateInfo"/>
        <rdfs:domain rdf:resource="http://www.semanticweb.org/cadex/ontologies/2020/1/untitled-ontology-71#Slate"/>
        <rdfs:range rdf:resource="http://www.w3.org/2001/XMLSchema#string"/>
        <rdfs:comment>This property represents a metadata field that indicates the focus unit of a slate.</rdfs:comment>
    </owl:DatatypeProperty>
    


    <!-- http://www.semanticweb.org/cadex/ontologies/2020/1/untitled-ontology-71#hasSlateFullCameraList -->

    <owl:DatatypeProperty rdf:about="http://www.semanticweb.org/cadex/ontologies/2020/1/untitled-ontology-71#hasSlateFullCameraList">
        <rdfs:subPropertyOf rdf:resource="http://www.semanticweb.org/cadex/ontologies/2020/1/untitled-ontology-71#hasSlateInfo"/>
        <rdfs:domain rdf:resource="http://www.semanticweb.org/cadex/ontologies/2020/1/untitled-ontology-71#Slate"/>
        <rdfs:range rdf:resource="http://www.w3.org/2001/XMLSchema#string"/>
        <rdfs:comment>This property represents a metadata field that indicates the full camera list of a slate.</rdfs:comment>
    </owl:DatatypeProperty>
    


    <!-- http://www.semanticweb.org/cadex/ontologies/2020/1/untitled-ontology-71#hasSlateHDRI -->

    <owl:DatatypeProperty rdf:about="http://www.semanticweb.org/cadex/ontologies/2020/1/untitled-ontology-71#hasSlateHDRI">
        <rdfs:subPropertyOf rdf:resource="http://www.semanticweb.org/cadex/ontologies/2020/1/untitled-ontology-71#hasSlateInfo"/>
        <rdfs:domain rdf:resource="http://www.semanticweb.org/cadex/ontologies/2020/1/untitled-ontology-71#Slate"/>
        <rdfs:range rdf:resource="http://www.w3.org/2001/XMLSchema#string"/>
        <rdfs:comment>This property represents a metadata field that indicates the HDRI of a slate.</rdfs:comment>
    </owl:DatatypeProperty>
    


    <!-- http://www.semanticweb.org/cadex/ontologies/2020/1/untitled-ontology-71#hasSlateHeightUnit -->

    <owl:DatatypeProperty rdf:about="http://www.semanticweb.org/cadex/ontologies/2020/1/untitled-ontology-71#hasSlateHeightUnit">
        <rdfs:subPropertyOf rdf:resource="http://www.semanticweb.org/cadex/ontologies/2020/1/untitled-ontology-71#hasSlateInfo"/>
        <rdfs:domain rdf:resource="http://www.semanticweb.org/cadex/ontologies/2020/1/untitled-ontology-71#Slate"/>
        <rdfs:range rdf:resource="http://www.w3.org/2001/XMLSchema#string"/>
        <rdfs:comment>This property represents a metadata field that indicates the height unit of a slate.</rdfs:comment>
    </owl:DatatypeProperty>
    


    <!-- http://www.semanticweb.org/cadex/ontologies/2020/1/untitled-ontology-71#hasSlateISO -->

    <owl:DatatypeProperty rdf:about="http://www.semanticweb.org/cadex/ontologies/2020/1/untitled-ontology-71#hasSlateISO">
        <rdfs:subPropertyOf rdf:resource="http://www.semanticweb.org/cadex/ontologies/2020/1/untitled-ontology-71#hasSlateInfo"/>
        <rdfs:domain rdf:resource="http://www.semanticweb.org/cadex/ontologies/2020/1/untitled-ontology-71#Slate"/>
        <rdfs:range rdf:resource="http://www.w3.org/2001/XMLSchema#string"/>
        <rdfs:comment>This property represents a metadata field that indicates the ISO of a slate.</rdfs:comment>
    </owl:DatatypeProperty>
    


    <!-- http://www.semanticweb.org/cadex/ontologies/2020/1/untitled-ontology-71#hasSlateInfo -->

    <owl:DatatypeProperty rdf:about="http://www.semanticweb.org/cadex/ontologies/2020/1/untitled-ontology-71#hasSlateInfo">
        <rdfs:domain rdf:resource="http://www.semanticweb.org/cadex/ontologies/2020/1/untitled-ontology-71#Slate"/>
        <rdfs:comment>This is the parent of a set of properties that represent metadata fields describing a slate. This property should not be populated with a value because it does not itself represent a metadata field. Rather, it is used solely to organise the properties representing fields.</rdfs:comment>
    </owl:DatatypeProperty>
    


    <!-- http://www.semanticweb.org/cadex/ontologies/2020/1/untitled-ontology-71#hasSlateKeyMeasure -->

    <owl:DatatypeProperty rdf:about="http://www.semanticweb.org/cadex/ontologies/2020/1/untitled-ontology-71#hasSlateKeyMeasure">
        <rdfs:subPropertyOf rdf:resource="http://www.semanticweb.org/cadex/ontologies/2020/1/untitled-ontology-71#hasSlateInfo"/>
        <rdfs:domain rdf:resource="http://www.semanticweb.org/cadex/ontologies/2020/1/untitled-ontology-71#Slate"/>
        <rdfs:range rdf:resource="http://www.w3.org/2001/XMLSchema#string"/>
        <rdfs:comment>This property represents a metadata field that indicates the key measure of a slate.</rdfs:comment>
    </owl:DatatypeProperty>
    


    <!-- http://www.semanticweb.org/cadex/ontologies/2020/1/untitled-ontology-71#hasSlateName -->

    <owl:DatatypeProperty rdf:about="http://www.semanticweb.org/cadex/ontologies/2020/1/untitled-ontology-71#hasSlateName">
        <rdfs:subPropertyOf rdf:resource="http://www.semanticweb.org/cadex/ontologies/2020/1/untitled-ontology-71#hasSlateInfo"/>
        <rdfs:domain rdf:resource="http://www.semanticweb.org/cadex/ontologies/2020/1/untitled-ontology-71#Slate"/>
        <rdfs:range rdf:resource="http://www.w3.org/2001/XMLSchema#string"/>
        <rdfs:comment>This property represents a metadata field that indicates the name of a slate.</rdfs:comment>
    </owl:DatatypeProperty>
    


    <!-- http://www.semanticweb.org/cadex/ontologies/2020/1/untitled-ontology-71#hasSlateNameAlternative -->

    <owl:DatatypeProperty rdf:about="http://www.semanticweb.org/cadex/ontologies/2020/1/untitled-ontology-71#hasSlateNameAlternative">
        <rdfs:subPropertyOf rdf:resource="http://www.semanticweb.org/cadex/ontologies/2020/1/untitled-ontology-71#hasSlateInfo"/>
        <rdfs:domain rdf:resource="http://www.semanticweb.org/cadex/ontologies/2020/1/untitled-ontology-71#Slate"/>
        <rdfs:range rdf:resource="http://www.w3.org/2001/XMLSchema#string"/>
        <rdfs:comment>This property represents a metadata field that indicates the alternative name of a slate.</rdfs:comment>
    </owl:DatatypeProperty>
    


    <!-- http://www.semanticweb.org/cadex/ontologies/2020/1/untitled-ontology-71#hasSlatePlanning -->

    <owl:DatatypeProperty rdf:about="http://www.semanticweb.org/cadex/ontologies/2020/1/untitled-ontology-71#hasSlatePlanning">
        <rdfs:subPropertyOf rdf:resource="http://www.semanticweb.org/cadex/ontologies/2020/1/untitled-ontology-71#hasSlateInfo"/>
        <rdfs:domain rdf:resource="http://www.semanticweb.org/cadex/ontologies/2020/1/untitled-ontology-71#Slate"/>
        <rdfs:range rdf:resource="http://www.w3.org/2001/XMLSchema#string"/>
        <rdfs:comment>This property represents a metadata field that indicates the planning of a slate.</rdfs:comment>
    </owl:DatatypeProperty>
    


    <!-- http://www.semanticweb.org/cadex/ontologies/2020/1/untitled-ontology-71#hasSlatePrevis -->

    <owl:DatatypeProperty rdf:about="http://www.semanticweb.org/cadex/ontologies/2020/1/untitled-ontology-71#hasSlatePrevis">
        <rdfs:subPropertyOf rdf:resource="http://www.semanticweb.org/cadex/ontologies/2020/1/untitled-ontology-71#hasSlateInfo"/>
        <rdfs:domain rdf:resource="http://www.semanticweb.org/cadex/ontologies/2020/1/untitled-ontology-71#Slate"/>
        <rdfs:range rdf:resource="http://www.w3.org/2001/XMLSchema#string"/>
        <rdfs:comment>This property represents a metadata field that indicates the previs of a slate.</rdfs:comment>
    </owl:DatatypeProperty>
    


    <!-- http://www.semanticweb.org/cadex/ontologies/2020/1/untitled-ontology-71#hasSlateStatus -->

    <owl:DatatypeProperty rdf:about="http://www.semanticweb.org/cadex/ontologies/2020/1/untitled-ontology-71#hasSlateStatus">
        <rdfs:subPropertyOf rdf:resource="http://www.semanticweb.org/cadex/ontologies/2020/1/untitled-ontology-71#hasSlateInfo"/>
        <rdfs:domain rdf:resource="http://www.semanticweb.org/cadex/ontologies/2020/1/untitled-ontology-71#Slate"/>
        <rdfs:range rdf:resource="http://www.w3.org/2001/XMLSchema#string"/>
        <rdfs:comment>This property represents a metadata field that indicates the status of a slate.</rdfs:comment>
    </owl:DatatypeProperty>
    


    <!-- http://www.semanticweb.org/cadex/ontologies/2020/1/untitled-ontology-71#hasSlateStereoConvergence -->

    <owl:DatatypeProperty rdf:about="http://www.semanticweb.org/cadex/ontologies/2020/1/untitled-ontology-71#hasSlateStereoConvergence">
        <rdfs:subPropertyOf rdf:resource="http://www.semanticweb.org/cadex/ontologies/2020/1/untitled-ontology-71#hasSlateStereoInfo"/>
        <rdfs:domain rdf:resource="http://www.semanticweb.org/cadex/ontologies/2020/1/untitled-ontology-71#Slate"/>
        <rdfs:range rdf:resource="http://www.w3.org/2001/XMLSchema#string"/>
        <rdfs:comment>This property represents a metadata field that indicates the stereo convergence of a slate.</rdfs:comment>
    </owl:DatatypeProperty>
    


    <!-- http://www.semanticweb.org/cadex/ontologies/2020/1/untitled-ontology-71#hasSlateStereoIO -->

    <owl:DatatypeProperty rdf:about="http://www.semanticweb.org/cadex/ontologies/2020/1/untitled-ontology-71#hasSlateStereoIO">
        <rdfs:subPropertyOf rdf:resource="http://www.semanticweb.org/cadex/ontologies/2020/1/untitled-ontology-71#hasSlateStereoInfo"/>
        <rdfs:domain rdf:resource="http://www.semanticweb.org/cadex/ontologies/2020/1/untitled-ontology-71#Slate"/>
        <rdfs:range rdf:resource="http://www.w3.org/2001/XMLSchema#string"/>
        <rdfs:comment>This property represents a metadata field that indicates the stereo IO of a slate.</rdfs:comment>
    </owl:DatatypeProperty>
    


    <!-- http://www.semanticweb.org/cadex/ontologies/2020/1/untitled-ontology-71#hasSlateStereoInfo -->

    <owl:DatatypeProperty rdf:about="http://www.semanticweb.org/cadex/ontologies/2020/1/untitled-ontology-71#hasSlateStereoInfo">
        <rdfs:subPropertyOf rdf:resource="http://www.semanticweb.org/cadex/ontologies/2020/1/untitled-ontology-71#hasSlateInfo"/>
        <rdfs:domain rdf:resource="http://www.semanticweb.org/cadex/ontologies/2020/1/untitled-ontology-71#Slate"/>
        <rdfs:comment>This is the parent of a set of properties that represent metadata fields describing stereo information about a slate. This property should not be populated with a value because it does not itself represent a metadata field. Rather, it is used solely to organise the properties representing fields.</rdfs:comment>
    </owl:DatatypeProperty>
    


    <!-- http://www.semanticweb.org/cadex/ontologies/2020/1/untitled-ontology-71#hasSlateStereoType -->

    <owl:DatatypeProperty rdf:about="http://www.semanticweb.org/cadex/ontologies/2020/1/untitled-ontology-71#hasSlateStereoType">
        <rdfs:subPropertyOf rdf:resource="http://www.semanticweb.org/cadex/ontologies/2020/1/untitled-ontology-71#hasSlateStereoInfo"/>
        <rdfs:domain rdf:resource="http://www.semanticweb.org/cadex/ontologies/2020/1/untitled-ontology-71#Slate"/>
        <rdfs:range rdf:resource="http://www.w3.org/2001/XMLSchema#string"/>
        <rdfs:comment>This property represents a metadata field that indicates the stereo type of a slate.</rdfs:comment>
    </owl:DatatypeProperty>
    


    <!-- http://www.semanticweb.org/cadex/ontologies/2020/1/untitled-ontology-71#hasSlateStereoUnderOverSlung -->

    <owl:DatatypeProperty rdf:about="http://www.semanticweb.org/cadex/ontologies/2020/1/untitled-ontology-71#hasSlateStereoUnderOverSlung">
        <rdfs:subPropertyOf rdf:resource="http://www.semanticweb.org/cadex/ontologies/2020/1/untitled-ontology-71#hasSlateStereoInfo"/>
        <rdfs:domain rdf:resource="http://www.semanticweb.org/cadex/ontologies/2020/1/untitled-ontology-71#Slate"/>
        <rdfs:range rdf:resource="http://www.w3.org/2001/XMLSchema#string"/>
        <rdfs:comment>This property represents a metadata field that indicates the stereo under/over slung of a slate.</rdfs:comment>
    </owl:DatatypeProperty>
    


    <!-- http://www.semanticweb.org/cadex/ontologies/2020/1/untitled-ontology-71#hasSlateStock -->

    <owl:DatatypeProperty rdf:about="http://www.semanticweb.org/cadex/ontologies/2020/1/untitled-ontology-71#hasSlateStock">
        <rdfs:subPropertyOf rdf:resource="http://www.semanticweb.org/cadex/ontologies/2020/1/untitled-ontology-71#hasSlateInfo"/>
        <rdfs:domain rdf:resource="http://www.semanticweb.org/cadex/ontologies/2020/1/untitled-ontology-71#Slate"/>
        <rdfs:range rdf:resource="http://www.w3.org/2001/XMLSchema#string"/>
        <rdfs:comment>This property represents a metadata field that indicates the stock of a slate.</rdfs:comment>
    </owl:DatatypeProperty>
    


    <!-- http://www.semanticweb.org/cadex/ontologies/2020/1/untitled-ontology-71#hasSlateStoryboard -->

    <owl:DatatypeProperty rdf:about="http://www.semanticweb.org/cadex/ontologies/2020/1/untitled-ontology-71#hasSlateStoryboard">
        <rdfs:subPropertyOf rdf:resource="http://www.semanticweb.org/cadex/ontologies/2020/1/untitled-ontology-71#hasSlateInfo"/>
        <rdfs:domain rdf:resource="http://www.semanticweb.org/cadex/ontologies/2020/1/untitled-ontology-71#Slate"/>
        <rdfs:range rdf:resource="http://www.w3.org/2001/XMLSchema#string"/>
        <rdfs:comment>This property represents a metadata field that indicates the storyboard of a slate.</rdfs:comment>
    </owl:DatatypeProperty>
    


    <!-- http://www.semanticweb.org/cadex/ontologies/2020/1/untitled-ontology-71#hasSlateSunPosition -->

    <owl:DatatypeProperty rdf:about="http://www.semanticweb.org/cadex/ontologies/2020/1/untitled-ontology-71#hasSlateSunPosition">
        <rdfs:subPropertyOf rdf:resource="http://www.semanticweb.org/cadex/ontologies/2020/1/untitled-ontology-71#hasSlateInfo"/>
        <rdfs:domain rdf:resource="http://www.semanticweb.org/cadex/ontologies/2020/1/untitled-ontology-71#Slate"/>
        <rdfs:range rdf:resource="http://www.w3.org/2001/XMLSchema#string"/>
        <rdfs:comment>This property represents a metadata field that indicates the sun position in a slate.</rdfs:comment>
    </owl:DatatypeProperty>
    


    <!-- http://www.semanticweb.org/cadex/ontologies/2020/1/untitled-ontology-71#hasSlateTag -->

    <owl:DatatypeProperty rdf:about="http://www.semanticweb.org/cadex/ontologies/2020/1/untitled-ontology-71#hasSlateTag">
        <rdfs:subPropertyOf rdf:resource="http://www.semanticweb.org/cadex/ontologies/2020/1/untitled-ontology-71#hasSlateInfo"/>
        <rdfs:domain rdf:resource="http://www.semanticweb.org/cadex/ontologies/2020/1/untitled-ontology-71#Slate"/>
        <rdfs:range rdf:resource="http://www.w3.org/2001/XMLSchema#string"/>
        <rdfs:comment>This property represents a metadata field that indicates the tag of a slate.</rdfs:comment>
    </owl:DatatypeProperty>
    


    <!-- http://www.semanticweb.org/cadex/ontologies/2020/1/untitled-ontology-71#hasSlateTakeCopies -->

    <owl:DatatypeProperty rdf:about="http://www.semanticweb.org/cadex/ontologies/2020/1/untitled-ontology-71#hasSlateTakeCopies">
        <rdfs:subPropertyOf rdf:resource="http://www.semanticweb.org/cadex/ontologies/2020/1/untitled-ontology-71#hasSlateInfo"/>
        <rdfs:domain rdf:resource="http://www.semanticweb.org/cadex/ontologies/2020/1/untitled-ontology-71#Slate"/>
        <rdfs:range rdf:resource="http://www.w3.org/2001/XMLSchema#string"/>
        <rdfs:comment>This property represents a metadata field that indicates the take copies of a slate.</rdfs:comment>
    </owl:DatatypeProperty>
    


    <!-- http://www.semanticweb.org/cadex/ontologies/2020/1/untitled-ontology-71#hasSlateThumbnail -->

    <owl:DatatypeProperty rdf:about="http://www.semanticweb.org/cadex/ontologies/2020/1/untitled-ontology-71#hasSlateThumbnail">
        <rdfs:subPropertyOf rdf:resource="http://www.semanticweb.org/cadex/ontologies/2020/1/untitled-ontology-71#hasSlateInfo"/>
        <rdfs:domain rdf:resource="http://www.semanticweb.org/cadex/ontologies/2020/1/untitled-ontology-71#Slate"/>
    </owl:DatatypeProperty>
    


    <!-- http://www.semanticweb.org/cadex/ontologies/2020/1/untitled-ontology-71#hasSlateTime -->

    <owl:DatatypeProperty rdf:about="http://www.semanticweb.org/cadex/ontologies/2020/1/untitled-ontology-71#hasSlateTime">
        <rdfs:subPropertyOf rdf:resource="http://www.semanticweb.org/cadex/ontologies/2020/1/untitled-ontology-71#hasSlateInfo"/>
        <rdfs:domain rdf:resource="http://www.semanticweb.org/cadex/ontologies/2020/1/untitled-ontology-71#Slate"/>
        <rdfs:range rdf:resource="http://www.w3.org/2001/XMLSchema#dateTimeStamp"/>
        <rdfs:comment>This property represents a metadata field that indicates the time on a slate.</rdfs:comment>
    </owl:DatatypeProperty>
    


    <!-- http://www.semanticweb.org/cadex/ontologies/2020/1/untitled-ontology-71#hasSlateTimecodeIn -->

    <owl:DatatypeProperty rdf:about="http://www.semanticweb.org/cadex/ontologies/2020/1/untitled-ontology-71#hasSlateTimecodeIn">
        <rdfs:subPropertyOf rdf:resource="http://www.semanticweb.org/cadex/ontologies/2020/1/untitled-ontology-71#hasSlateInfo"/>
        <rdfs:domain rdf:resource="http://www.semanticweb.org/cadex/ontologies/2020/1/untitled-ontology-71#Slate"/>
        <rdfs:range rdf:resource="http://www.w3.org/2001/XMLSchema#string"/>
        <rdfs:comment>This property represents a metadata field that indicates the starting timecode on a slate.</rdfs:comment>
    </owl:DatatypeProperty>
    


    <!-- http://www.semanticweb.org/cadex/ontologies/2020/1/untitled-ontology-71#hasSlateTimecodeOut -->

    <owl:DatatypeProperty rdf:about="http://www.semanticweb.org/cadex/ontologies/2020/1/untitled-ontology-71#hasSlateTimecodeOut">
        <rdfs:subPropertyOf rdf:resource="http://www.semanticweb.org/cadex/ontologies/2020/1/untitled-ontology-71#hasSlateInfo"/>
        <rdfs:domain rdf:resource="http://www.semanticweb.org/cadex/ontologies/2020/1/untitled-ontology-71#Slate"/>
        <rdfs:range rdf:resource="http://www.w3.org/2001/XMLSchema#string"/>
        <rdfs:comment>This property represents a metadata field that indicates the ending timecode on a slate.</rdfs:comment>
    </owl:DatatypeProperty>
    


    <!-- http://www.semanticweb.org/cadex/ontologies/2020/1/untitled-ontology-71#hasSlateVFXDescription -->

    <owl:DatatypeProperty rdf:about="http://www.semanticweb.org/cadex/ontologies/2020/1/untitled-ontology-71#hasSlateVFXDescription">
        <rdfs:subPropertyOf rdf:resource="http://www.semanticweb.org/cadex/ontologies/2020/1/untitled-ontology-71#hasSlateDescription"/>
        <rdfs:domain rdf:resource="http://www.semanticweb.org/cadex/ontologies/2020/1/untitled-ontology-71#Slate"/>
        <rdfs:range rdf:resource="http://www.w3.org/2001/XMLSchema#string"/>
        <rdfs:comment>This property represents a metadata field that indicates the VFX-specific description of a slate.</rdfs:comment>
    </owl:DatatypeProperty>
    


    <!-- http://www.semanticweb.org/cadex/ontologies/2020/1/untitled-ontology-71#hasSlateVersionLink -->

    <owl:DatatypeProperty rdf:about="http://www.semanticweb.org/cadex/ontologies/2020/1/untitled-ontology-71#hasSlateVersionLink">
        <rdfs:subPropertyOf rdf:resource="http://www.semanticweb.org/cadex/ontologies/2020/1/untitled-ontology-71#hasSlateInfo"/>
        <rdfs:domain rdf:resource="http://www.semanticweb.org/cadex/ontologies/2020/1/untitled-ontology-71#Slate"/>
        <rdfs:range rdf:resource="http://www.w3.org/2001/XMLSchema#string"/>
        <rdfs:comment>This property represents a metadata field that indicates the version link of a slate.</rdfs:comment>
    </owl:DatatypeProperty>
    


    <!-- http://www.semanticweb.org/cadex/ontologies/2020/1/untitled-ontology-71#hasSlateWeather -->

    <owl:DatatypeProperty rdf:about="http://www.semanticweb.org/cadex/ontologies/2020/1/untitled-ontology-71#hasSlateWeather">
        <rdfs:subPropertyOf rdf:resource="http://www.semanticweb.org/cadex/ontologies/2020/1/untitled-ontology-71#hasSlateInfo"/>
        <rdfs:domain rdf:resource="http://www.semanticweb.org/cadex/ontologies/2020/1/untitled-ontology-71#Slate"/>
        <rdfs:range rdf:resource="http://www.w3.org/2001/XMLSchema#string"/>
        <rdfs:comment>This property represents a metadata field that indicates the weather of a slate.</rdfs:comment>
    </owl:DatatypeProperty>
    


    <!-- http://www.semanticweb.org/cadex/ontologies/2020/1/untitled-ontology-71#hasSoundRollInfo -->

    <owl:DatatypeProperty rdf:about="http://www.semanticweb.org/cadex/ontologies/2020/1/untitled-ontology-71#hasSoundRollInfo">
        <rdfs:subPropertyOf rdf:resource="http://www.semanticweb.org/cadex/ontologies/2020/1/untitled-ontology-71#hasRollInfo"/>
        <rdfs:domain rdf:resource="http://www.semanticweb.org/cadex/ontologies/2020/1/untitled-ontology-71#SoundRoll"/>
        <rdfs:comment>This is the parent of a set of properties that represent metadata fields describing a sound roll. This property should not be populated with a value because it does not itself represent a metadata field. Rather, it is used solely to organise the properties representing fields.</rdfs:comment>
    </owl:DatatypeProperty>
    


    <!-- http://www.semanticweb.org/cadex/ontologies/2020/1/untitled-ontology-71#hasSoundRollNumber -->

    <owl:DatatypeProperty rdf:about="http://www.semanticweb.org/cadex/ontologies/2020/1/untitled-ontology-71#hasSoundRollNumber">
        <rdfs:subPropertyOf rdf:resource="http://www.semanticweb.org/cadex/ontologies/2020/1/untitled-ontology-71#hasSoundRollInfo"/>
        <rdfs:domain rdf:resource="http://www.semanticweb.org/cadex/ontologies/2020/1/untitled-ontology-71#SoundRoll"/>
        <rdfs:range rdf:resource="http://www.w3.org/2001/XMLSchema#int"/>
        <rdfs:comment>This property represents a metadata field that indicates the roll number of a sound roll.</rdfs:comment>
    </owl:DatatypeProperty>
    


    <!-- http://www.semanticweb.org/cadex/ontologies/2020/1/untitled-ontology-71#hasStaffEmailAddress -->

    <owl:DatatypeProperty rdf:about="http://www.semanticweb.org/cadex/ontologies/2020/1/untitled-ontology-71#hasStaffEmailAddress">
        <rdfs:subPropertyOf rdf:resource="http://www.semanticweb.org/cadex/ontologies/2020/1/untitled-ontology-71#hasStaffInfo"/>
        <rdfs:domain rdf:resource="http://www.semanticweb.org/cadex/ontologies/2020/1/untitled-ontology-71#Staff"/>
        <rdfs:range rdf:resource="http://www.w3.org/2001/XMLSchema#string"/>
        <rdfs:comment>This property represents a metadata field that indicates the email address of a staff member.</rdfs:comment>
    </owl:DatatypeProperty>
    


    <!-- http://www.semanticweb.org/cadex/ontologies/2020/1/untitled-ontology-71#hasStaffInfo -->

    <owl:DatatypeProperty rdf:about="http://www.semanticweb.org/cadex/ontologies/2020/1/untitled-ontology-71#hasStaffInfo">
        <rdfs:subPropertyOf rdf:resource="http://www.semanticweb.org/cadex/ontologies/2020/1/untitled-ontology-71#hasPersonInfo"/>
        <rdfs:domain rdf:resource="http://www.semanticweb.org/cadex/ontologies/2020/1/untitled-ontology-71#Staff"/>
        <rdfs:comment>This is the parent of a set of properties that represent metadata fields describing a person with a role of staff. This property should not be populated with a value because it does not itself represent a metadata field. Rather, it is used solely to organise the properties representing fields.</rdfs:comment>
    </owl:DatatypeProperty>
    


    <!-- http://www.semanticweb.org/cadex/ontologies/2020/1/untitled-ontology-71#hasTakeInfo -->

    <owl:DatatypeProperty rdf:about="http://www.semanticweb.org/cadex/ontologies/2020/1/untitled-ontology-71#hasTakeInfo">
        <rdfs:domain rdf:resource="http://www.semanticweb.org/cadex/ontologies/2020/1/untitled-ontology-71#Take"/>
        <rdfs:comment>This is the parent of a set of properties that represent metadata fields describing a take. This property should not be populated with a value because it does not itself represent a metadata field. Rather, it is used solely to organise the properties representing fields.</rdfs:comment>
    </owl:DatatypeProperty>
    


    <!-- http://www.semanticweb.org/cadex/ontologies/2020/1/untitled-ontology-71#hasTakeNumber -->

    <owl:DatatypeProperty rdf:about="http://www.semanticweb.org/cadex/ontologies/2020/1/untitled-ontology-71#hasTakeNumber">
        <rdfs:subPropertyOf rdf:resource="http://www.semanticweb.org/cadex/ontologies/2020/1/untitled-ontology-71#hasTakeInfo"/>
        <rdfs:domain rdf:resource="http://www.semanticweb.org/cadex/ontologies/2020/1/untitled-ontology-71#Take"/>
        <rdfs:range rdf:resource="http://www.w3.org/2001/XMLSchema#int"/>
        <rdfs:comment>This property represents a metadata field that indicates the numerical ID of a take.</rdfs:comment>
    </owl:DatatypeProperty>
    


    <!-- http://www.semanticweb.org/cadex/ontologies/2020/1/untitled-ontology-71#hasUnitDescription -->

    <owl:DatatypeProperty rdf:about="http://www.semanticweb.org/cadex/ontologies/2020/1/untitled-ontology-71#hasUnitDescription">
        <rdfs:subPropertyOf rdf:resource="http://www.semanticweb.org/cadex/ontologies/2020/1/untitled-ontology-71#hasUnitInfo"/>
        <rdfs:domain rdf:resource="http://www.semanticweb.org/cadex/ontologies/2020/1/untitled-ontology-71#Unit"/>
        <rdfs:range rdf:resource="http://www.w3.org/2001/XMLSchema#string"/>
        <rdfs:comment>This property represents a metadata field that indicates the description of a unit.</rdfs:comment>
    </owl:DatatypeProperty>
    


    <!-- http://www.semanticweb.org/cadex/ontologies/2020/1/untitled-ontology-71#hasUnitFilmstripThumbnail -->

    <owl:DatatypeProperty rdf:about="http://www.semanticweb.org/cadex/ontologies/2020/1/untitled-ontology-71#hasUnitFilmstripThumbnail">
        <rdfs:subPropertyOf rdf:resource="http://www.semanticweb.org/cadex/ontologies/2020/1/untitled-ontology-71#hasUnitInfo"/>
        <rdfs:domain rdf:resource="http://www.semanticweb.org/cadex/ontologies/2020/1/untitled-ontology-71#Unit"/>
    </owl:DatatypeProperty>
    


    <!-- http://www.semanticweb.org/cadex/ontologies/2020/1/untitled-ontology-71#hasUnitInfo -->

    <owl:DatatypeProperty rdf:about="http://www.semanticweb.org/cadex/ontologies/2020/1/untitled-ontology-71#hasUnitInfo">
        <rdfs:domain rdf:resource="http://www.semanticweb.org/cadex/ontologies/2020/1/untitled-ontology-71#Unit"/>
        <rdfs:comment>This is the parent of a set of properties that represent metadata fields describing a unit. This property should not be populated with a value because it does not itself represent a metadata field. Rather, it is used solely to organise the properties representing fields.</rdfs:comment>
    </owl:DatatypeProperty>
    


    <!-- http://www.semanticweb.org/cadex/ontologies/2020/1/untitled-ontology-71#hasUnitName -->

    <owl:DatatypeProperty rdf:about="http://www.semanticweb.org/cadex/ontologies/2020/1/untitled-ontology-71#hasUnitName">
        <rdfs:subPropertyOf rdf:resource="http://www.semanticweb.org/cadex/ontologies/2020/1/untitled-ontology-71#hasUnitInfo"/>
        <rdfs:domain rdf:resource="http://www.semanticweb.org/cadex/ontologies/2020/1/untitled-ontology-71#Unit"/>
        <rdfs:range rdf:resource="http://www.w3.org/2001/XMLSchema#string"/>
        <rdfs:comment>This property represents a metadata field that indicates the name of a unit.</rdfs:comment>
    </owl:DatatypeProperty>
    


    <!-- http://www.semanticweb.org/cadex/ontologies/2020/1/untitled-ontology-71#hasUnitNameAlternative -->

    <owl:DatatypeProperty rdf:about="http://www.semanticweb.org/cadex/ontologies/2020/1/untitled-ontology-71#hasUnitNameAlternative">
        <rdfs:subPropertyOf rdf:resource="http://www.semanticweb.org/cadex/ontologies/2020/1/untitled-ontology-71#hasUnitInfo"/>
        <rdfs:domain rdf:resource="http://www.semanticweb.org/cadex/ontologies/2020/1/untitled-ontology-71#Unit"/>
        <rdfs:range rdf:resource="http://www.w3.org/2001/XMLSchema#string"/>
        <rdfs:comment>This property represents a metadata field that indicates the alternative name of a unit.</rdfs:comment>
    </owl:DatatypeProperty>
    


    <!-- http://www.semanticweb.org/cadex/ontologies/2020/1/untitled-ontology-71#hasUnitStatus -->

    <owl:DatatypeProperty rdf:about="http://www.semanticweb.org/cadex/ontologies/2020/1/untitled-ontology-71#hasUnitStatus">
        <rdfs:subPropertyOf rdf:resource="http://www.semanticweb.org/cadex/ontologies/2020/1/untitled-ontology-71#hasUnitInfo"/>
        <rdfs:domain rdf:resource="http://www.semanticweb.org/cadex/ontologies/2020/1/untitled-ontology-71#Unit"/>
        <rdfs:range rdf:resource="http://www.w3.org/2001/XMLSchema#string"/>
        <rdfs:comment>This property represents a metadata field that indicates the status of a unit.</rdfs:comment>
    </owl:DatatypeProperty>
    


    <!-- http://www.semanticweb.org/cadex/ontologies/2020/1/untitled-ontology-71#hasUnitTag -->

    <owl:DatatypeProperty rdf:about="http://www.semanticweb.org/cadex/ontologies/2020/1/untitled-ontology-71#hasUnitTag">
        <rdfs:subPropertyOf rdf:resource="http://www.semanticweb.org/cadex/ontologies/2020/1/untitled-ontology-71#hasUnitInfo"/>
        <rdfs:domain rdf:resource="http://www.semanticweb.org/cadex/ontologies/2020/1/untitled-ontology-71#Unit"/>
        <rdfs:range rdf:resource="http://www.w3.org/2001/XMLSchema#string"/>
        <rdfs:comment>This property represents a metadata field that indicates the tags assigned to a unit.</rdfs:comment>
    </owl:DatatypeProperty>
    


    <!-- http://www.semanticweb.org/cadex/ontologies/2020/1/untitled-ontology-71#hasUnitThumbnail -->

    <owl:DatatypeProperty rdf:about="http://www.semanticweb.org/cadex/ontologies/2020/1/untitled-ontology-71#hasUnitThumbnail">
        <rdfs:subPropertyOf rdf:resource="http://www.semanticweb.org/cadex/ontologies/2020/1/untitled-ontology-71#hasUnitInfo"/>
        <rdfs:domain rdf:resource="http://www.semanticweb.org/cadex/ontologies/2020/1/untitled-ontology-71#Unit"/>
    </owl:DatatypeProperty>
    


    <!-- http://www.semanticweb.org/cadex/ontologies/2020/1/untitled-ontology-71#isClipSelected -->

    <owl:DatatypeProperty rdf:about="http://www.semanticweb.org/cadex/ontologies/2020/1/untitled-ontology-71#isClipSelected">
        <rdfs:subPropertyOf rdf:resource="http://www.semanticweb.org/cadex/ontologies/2020/1/untitled-ontology-71#hasClipInfo"/>
        <rdfs:domain rdf:resource="http://www.semanticweb.org/cadex/ontologies/2020/1/untitled-ontology-71#Clip"/>
        <rdfs:range rdf:resource="http://www.w3.org/2001/XMLSchema#boolean"/>
        <rdfs:comment>This property represents a metadata field that indicates whether a clip has been selected.</rdfs:comment>
    </owl:DatatypeProperty>
    


    <!-- http://www.semanticweb.org/cadex/ontologies/2020/1/untitled-ontology-71#isLoggingTagAudioOrVideo -->

    <owl:DatatypeProperty rdf:about="http://www.semanticweb.org/cadex/ontologies/2020/1/untitled-ontology-71#isLoggingTagAudioOrVideo">
        <rdfs:subPropertyOf rdf:resource="http://www.semanticweb.org/cadex/ontologies/2020/1/untitled-ontology-71#hasLoggingTagInfo"/>
        <rdfs:domain rdf:resource="http://www.semanticweb.org/cadex/ontologies/2020/1/untitled-ontology-71#LoggingTag"/>
        <rdfs:range>
            <rdfs:Datatype>
                <owl:oneOf>
                    <rdf:Description>
                        <rdf:type rdf:resource="http://www.w3.org/1999/02/22-rdf-syntax-ns#List"/>
                        <rdf:first>Audio</rdf:first>
                        <rdf:rest>
                            <rdf:Description>
                                <rdf:type rdf:resource="http://www.w3.org/1999/02/22-rdf-syntax-ns#List"/>
                                <rdf:first>Video</rdf:first>
                                <rdf:rest rdf:resource="http://www.w3.org/1999/02/22-rdf-syntax-ns#nil"/>
                            </rdf:Description>
                        </rdf:rest>
                    </rdf:Description>
                </owl:oneOf>
            </rdfs:Datatype>
        </rdfs:range>
        <rdfs:comment>This property represents a metadata field that indicates whether the logging tag refers to audio or video.</rdfs:comment>
    </owl:DatatypeProperty>
    


    <!-- http://www.semanticweb.org/cadex/ontologies/2020/1/untitled-ontology-71#lensCreatedOn -->

    <owl:DatatypeProperty rdf:about="http://www.semanticweb.org/cadex/ontologies/2020/1/untitled-ontology-71#lensCreatedOn">
        <rdfs:subPropertyOf rdf:resource="http://www.semanticweb.org/cadex/ontologies/2020/1/untitled-ontology-71#hasLensInfo"/>
        <rdfs:domain rdf:resource="http://www.semanticweb.org/cadex/ontologies/2020/1/untitled-ontology-71#Lens"/>
        <rdfs:range rdf:resource="http://www.w3.org/2001/XMLSchema#dateTimeStamp"/>
        <rdfs:comment>This property represents a metadata field that indicates the date and time a lens was created.</rdfs:comment>
    </owl:DatatypeProperty>
    


    <!-- http://www.semanticweb.org/cadex/ontologies/2020/1/untitled-ontology-71#lensUpdatedOn -->

    <owl:DatatypeProperty rdf:about="http://www.semanticweb.org/cadex/ontologies/2020/1/untitled-ontology-71#lensUpdatedOn">
        <rdfs:subPropertyOf rdf:resource="http://www.semanticweb.org/cadex/ontologies/2020/1/untitled-ontology-71#hasLensInfo"/>
        <rdfs:domain rdf:resource="http://www.semanticweb.org/cadex/ontologies/2020/1/untitled-ontology-71#Lens"/>
        <rdfs:range rdf:resource="http://www.w3.org/2001/XMLSchema#dateTimeStamp"/>
        <rdfs:comment>This property represents a metadata field that indicates the date and time a len was last updated.</rdfs:comment>
    </owl:DatatypeProperty>
    


    <!-- http://www.semanticweb.org/cadex/ontologies/2020/1/untitled-ontology-71#recordCreatedOn -->

    <owl:DatatypeProperty rdf:about="http://www.semanticweb.org/cadex/ontologies/2020/1/untitled-ontology-71#recordCreatedOn">
        <rdfs:subPropertyOf rdf:resource="http://www.semanticweb.org/cadex/ontologies/2020/1/untitled-ontology-71#hasRecordInfo"/>
        <rdfs:domain rdf:resource="http://www.semanticweb.org/cadex/ontologies/2020/1/untitled-ontology-71#Record"/>
        <rdfs:range rdf:resource="http://www.w3.org/2001/XMLSchema#dateTimeStamp"/>
        <rdfs:comment>This property represents a metadata field that indicates the date and time a record was created. It is used to track the time of creation for a new record, which represents a new version of an instance.</rdfs:comment>
    </owl:DatatypeProperty>
    


    <!-- http://www.semanticweb.org/cadex/ontologies/2020/1/untitled-ontology-71#sceneCreatedOn -->

    <owl:DatatypeProperty rdf:about="http://www.semanticweb.org/cadex/ontologies/2020/1/untitled-ontology-71#sceneCreatedOn">
        <rdfs:subPropertyOf rdf:resource="http://www.semanticweb.org/cadex/ontologies/2020/1/untitled-ontology-71#hasSceneInfo"/>
        <rdfs:domain rdf:resource="http://www.semanticweb.org/cadex/ontologies/2020/1/untitled-ontology-71#Scene"/>
        <rdfs:range rdf:resource="http://www.w3.org/2001/XMLSchema#dateTimeStamp"/>
        <rdfs:comment>This property represents a metadata field that indicates the date and time a scene was created.</rdfs:comment>
    </owl:DatatypeProperty>
    


    <!-- http://www.semanticweb.org/cadex/ontologies/2020/1/untitled-ontology-71#sceneUpdatedOn -->

    <owl:DatatypeProperty rdf:about="http://www.semanticweb.org/cadex/ontologies/2020/1/untitled-ontology-71#sceneUpdatedOn">
        <rdfs:subPropertyOf rdf:resource="http://www.semanticweb.org/cadex/ontologies/2020/1/untitled-ontology-71#hasSceneInfo"/>
        <rdfs:domain rdf:resource="http://www.semanticweb.org/cadex/ontologies/2020/1/untitled-ontology-71#Scene"/>
        <rdfs:range rdf:resource="http://www.w3.org/2001/XMLSchema#dateTimeStamp"/>
        <rdfs:comment>This property represents a metadata field that indicates the date and time a scene was last updated.</rdfs:comment>
    </owl:DatatypeProperty>
    


    <!-- http://www.semanticweb.org/cadex/ontologies/2020/1/untitled-ontology-71#shootCreatedOn -->

    <owl:DatatypeProperty rdf:about="http://www.semanticweb.org/cadex/ontologies/2020/1/untitled-ontology-71#shootCreatedOn">
        <rdfs:subPropertyOf rdf:resource="http://www.semanticweb.org/cadex/ontologies/2020/1/untitled-ontology-71#hasShootInfo"/>
        <rdfs:domain rdf:resource="http://www.semanticweb.org/cadex/ontologies/2020/1/untitled-ontology-71#Shoot"/>
        <rdfs:range rdf:resource="http://www.w3.org/2001/XMLSchema#dateTimeStamp"/>
        <rdfs:comment>This property represents a metadata field that indicates the date and time a shoot was created.</rdfs:comment>
    </owl:DatatypeProperty>
    


    <!-- http://www.semanticweb.org/cadex/ontologies/2020/1/untitled-ontology-71#shootUpdatedOn -->

    <owl:DatatypeProperty rdf:about="http://www.semanticweb.org/cadex/ontologies/2020/1/untitled-ontology-71#shootUpdatedOn">
        <rdfs:subPropertyOf rdf:resource="http://www.semanticweb.org/cadex/ontologies/2020/1/untitled-ontology-71#hasShootInfo"/>
        <rdfs:domain rdf:resource="http://www.semanticweb.org/cadex/ontologies/2020/1/untitled-ontology-71#Shoot"/>
        <rdfs:range rdf:resource="http://www.w3.org/2001/XMLSchema#dateTimeStamp"/>
        <rdfs:comment>This property represents a metadata field that indicates the date and time a shoot was last updated.</rdfs:comment>
    </owl:DatatypeProperty>
    


    <!-- http://www.semanticweb.org/cadex/ontologies/2020/1/untitled-ontology-71#slateCreatedOn -->

    <owl:DatatypeProperty rdf:about="http://www.semanticweb.org/cadex/ontologies/2020/1/untitled-ontology-71#slateCreatedOn">
        <rdfs:subPropertyOf rdf:resource="http://www.semanticweb.org/cadex/ontologies/2020/1/untitled-ontology-71#hasSlateInfo"/>
        <rdfs:domain rdf:resource="http://www.semanticweb.org/cadex/ontologies/2020/1/untitled-ontology-71#Slate"/>
        <rdfs:range rdf:resource="http://www.w3.org/2001/XMLSchema#dateTimeStamp"/>
        <rdfs:comment>This property represents a metadata field that indicates the date and time a slate was created.</rdfs:comment>
    </owl:DatatypeProperty>
    


    <!-- http://www.semanticweb.org/cadex/ontologies/2020/1/untitled-ontology-71#slateHasVFX -->

    <owl:DatatypeProperty rdf:about="http://www.semanticweb.org/cadex/ontologies/2020/1/untitled-ontology-71#slateHasVFX">
        <rdfs:subPropertyOf rdf:resource="http://www.semanticweb.org/cadex/ontologies/2020/1/untitled-ontology-71#hasSlateInfo"/>
        <rdfs:domain rdf:resource="http://www.semanticweb.org/cadex/ontologies/2020/1/untitled-ontology-71#Slate"/>
        <rdfs:range rdf:resource="http://www.w3.org/2001/XMLSchema#boolean"/>
        <rdfs:comment>This property represents a metadata field that indicates whether a slate has VFX.</rdfs:comment>
    </owl:DatatypeProperty>
    


    <!-- http://www.semanticweb.org/cadex/ontologies/2020/1/untitled-ontology-71#slateUpdatedOn -->

    <owl:DatatypeProperty rdf:about="http://www.semanticweb.org/cadex/ontologies/2020/1/untitled-ontology-71#slateUpdatedOn">
        <rdfs:subPropertyOf rdf:resource="http://www.semanticweb.org/cadex/ontologies/2020/1/untitled-ontology-71#hasSlateInfo"/>
        <rdfs:domain rdf:resource="http://www.semanticweb.org/cadex/ontologies/2020/1/untitled-ontology-71#Slate"/>
        <rdfs:range rdf:resource="http://www.w3.org/2001/XMLSchema#dateTimeStamp"/>
        <rdfs:comment>This property represents a metadata field that indicates the date and time a slate was last updated.</rdfs:comment>
    </owl:DatatypeProperty>
    


    <!-- http://www.semanticweb.org/cadex/ontologies/2020/1/untitled-ontology-71#unitCreatedOn -->

    <owl:DatatypeProperty rdf:about="http://www.semanticweb.org/cadex/ontologies/2020/1/untitled-ontology-71#unitCreatedOn">
        <rdfs:subPropertyOf rdf:resource="http://www.semanticweb.org/cadex/ontologies/2020/1/untitled-ontology-71#hasUnitInfo"/>
        <rdfs:domain rdf:resource="http://www.semanticweb.org/cadex/ontologies/2020/1/untitled-ontology-71#Unit"/>
        <rdfs:range rdf:resource="http://www.w3.org/2001/XMLSchema#dateTimeStamp"/>
        <rdfs:comment>This property represents a metadata field that indicates the date and time a unit was created.</rdfs:comment>
    </owl:DatatypeProperty>
    


    <!-- http://www.semanticweb.org/cadex/ontologies/2020/1/untitled-ontology-71#unitUpdatedOn -->

    <owl:DatatypeProperty rdf:about="http://www.semanticweb.org/cadex/ontologies/2020/1/untitled-ontology-71#unitUpdatedOn">
        <rdfs:subPropertyOf rdf:resource="http://www.semanticweb.org/cadex/ontologies/2020/1/untitled-ontology-71#hasUnitInfo"/>
        <rdfs:domain rdf:resource="http://www.semanticweb.org/cadex/ontologies/2020/1/untitled-ontology-71#Unit"/>
        <rdfs:range rdf:resource="http://www.w3.org/2001/XMLSchema#dateTimeStamp"/>
        <rdfs:comment>This property represents a metadata field that indicates the date and time a unit was last updated.</rdfs:comment>
    </owl:DatatypeProperty>
    


    <!-- http://www.semanticweb.org/cadex/ontologies/2020/1/untitled-ontology-71#hasCameraTrackT/O -->

    <owl:DatatypeProperty rdf:about="http://www.semanticweb.org/cadex/ontologies/2020/1/untitled-ontology-71#hasCameraTrackT/O">
        <rdfs:subPropertyOf rdf:resource="http://www.semanticweb.org/cadex/ontologies/2020/1/untitled-ontology-71#hasSlateCameraInfo"/>
        <rdfs:domain rdf:resource="http://www.semanticweb.org/cadex/ontologies/2020/1/untitled-ontology-71#Slate"/>
        <rdfs:range rdf:resource="http://www.w3.org/2001/XMLSchema#string"/>
        <rdfs:comment>This property represents a metadata field that indicates the track T/O of a slate&apos;s camera.</rdfs:comment>
    </owl:DatatypeProperty>
    


    <!-- http://www.w3.org/2002/07/owl#topDataProperty -->

    <rdf:Description rdf:about="http://www.w3.org/2002/07/owl#topDataProperty">
        <rdfs:comment>Every user-defined data property is implicitly a sub-property of owl: topDataProperty in an OWL ontology.</rdfs:comment>
    </rdf:Description>
    


    <!-- 
    ///////////////////////////////////////////////////////////////////////////////////////
    //
    // Classes
    //
    ///////////////////////////////////////////////////////////////////////////////////////
     -->

    


    <!-- http://www.semanticweb.org/cadex/ontologies/2020/1/untitled-ontology-71#Asset -->

    <owl:Class rdf:about="http://www.semanticweb.org/cadex/ontologies/2020/1/untitled-ontology-71#Asset">
        <rdfs:subClassOf rdf:resource="http://www.semanticweb.org/cadex/ontologies/2020/1/untitled-ontology-71#DataItem"/>
        <rdfs:comment>Any data (not metadata) that can be used in the pre-, post-, and production processes. These are usually stored as a File on the file system.</rdfs:comment>
    </owl:Class>
    


    <!-- http://www.semanticweb.org/cadex/ontologies/2020/1/untitled-ontology-71#Budget -->

    <owl:Class rdf:about="http://www.semanticweb.org/cadex/ontologies/2020/1/untitled-ontology-71#Budget">
        <rdfs:subClassOf rdf:resource="http://www.semanticweb.org/cadex/ontologies/2020/1/untitled-ontology-71#TextAssets"/>
        <rdfs:comment>The spreadsheet containing financial information related to the cost of a production.</rdfs:comment>
    </owl:Class>
    


    <!-- http://www.semanticweb.org/cadex/ontologies/2020/1/untitled-ontology-71#Camera -->

    <owl:Class rdf:about="http://www.semanticweb.org/cadex/ontologies/2020/1/untitled-ontology-71#Camera">
        <rdfs:subClassOf rdf:resource="http://www.semanticweb.org/cadex/ontologies/2020/1/untitled-ontology-71#Equipment"/>
        <rdfs:comment>A camera, which creates clips during a shoot.</rdfs:comment>
    </owl:Class>
    


    <!-- http://www.semanticweb.org/cadex/ontologies/2020/1/untitled-ontology-71#CameraRoll -->

    <owl:Class rdf:about="http://www.semanticweb.org/cadex/ontologies/2020/1/untitled-ontology-71#CameraRoll">
        <rdfs:subClassOf rdf:resource="http://www.semanticweb.org/cadex/ontologies/2020/1/untitled-ontology-71#Roll"/>
        <rdfs:comment>This is the video output of a camera after a take.</rdfs:comment>
    </owl:Class>
    


    <!-- http://www.semanticweb.org/cadex/ontologies/2020/1/untitled-ontology-71#Cast -->

    <owl:Class rdf:about="http://www.semanticweb.org/cadex/ontologies/2020/1/untitled-ontology-71#Cast">
        <rdfs:subClassOf rdf:resource="http://www.semanticweb.org/cadex/ontologies/2020/1/untitled-ontology-71#Role"/>
        <rdfs:comment>A person who performed in a shoot.</rdfs:comment>
    </owl:Class>
    


    <!-- http://www.semanticweb.org/cadex/ontologies/2020/1/untitled-ontology-71#Client -->

    <owl:Class rdf:about="http://www.semanticweb.org/cadex/ontologies/2020/1/untitled-ontology-71#Client">
        <rdfs:subClassOf rdf:resource="http://www.semanticweb.org/cadex/ontologies/2020/1/untitled-ontology-71#Role"/>
        <rdfs:comment>A subclass of Role and refers to anyone who works for the project client.</rdfs:comment>
    </owl:Class>
    


    <!-- http://www.semanticweb.org/cadex/ontologies/2020/1/untitled-ontology-71#Clip -->

    <owl:Class rdf:about="http://www.semanticweb.org/cadex/ontologies/2020/1/untitled-ontology-71#Clip">
        <rdfs:subClassOf rdf:resource="http://www.semanticweb.org/cadex/ontologies/2020/1/untitled-ontology-71#MediaAssets"/>
        <rdfs:comment>A single video file.</rdfs:comment>
    </owl:Class>
    


    <!-- http://www.semanticweb.org/cadex/ontologies/2020/1/untitled-ontology-71#Crane -->

    <owl:Class rdf:about="http://www.semanticweb.org/cadex/ontologies/2020/1/untitled-ontology-71#Crane">
        <rdfs:subClassOf rdf:resource="http://www.semanticweb.org/cadex/ontologies/2020/1/untitled-ontology-71#Equipment"/>
        <rdfs:comment>A camera crane, which allows shots to be taken from a height.</rdfs:comment>
    </owl:Class>
    


    <!-- http://www.semanticweb.org/cadex/ontologies/2020/1/untitled-ontology-71#DataItem -->

    <owl:Class rdf:about="http://www.semanticweb.org/cadex/ontologies/2020/1/untitled-ontology-71#DataItem">
        <rdfs:comment>Represents any entity that can have metadata associated with it.</rdfs:comment>
    </owl:Class>
    


    <!-- http://www.semanticweb.org/cadex/ontologies/2020/1/untitled-ontology-71#DataTeamMember -->

    <owl:Class rdf:about="http://www.semanticweb.org/cadex/ontologies/2020/1/untitled-ontology-71#DataTeamMember">
        <rdfs:subClassOf rdf:resource="http://www.semanticweb.org/cadex/ontologies/2020/1/untitled-ontology-71#Staff"/>
        <rdfs:comment>A member of the data team who works for the company using the ontology.</rdfs:comment>
    </owl:Class>
    


    <!-- http://www.semanticweb.org/cadex/ontologies/2020/1/untitled-ontology-71#Deliverable -->

    <owl:Class rdf:about="http://www.semanticweb.org/cadex/ontologies/2020/1/untitled-ontology-71#Deliverable">
        <rdfs:subClassOf rdf:resource="http://www.semanticweb.org/cadex/ontologies/2020/1/untitled-ontology-71#DataItem"/>
        <rdfs:comment>An item delivered as a result of a project.</rdfs:comment>
    </owl:Class>
    


    <!-- http://www.semanticweb.org/cadex/ontologies/2020/1/untitled-ontology-71#Dolly -->

    <owl:Class rdf:about="http://www.semanticweb.org/cadex/ontologies/2020/1/untitled-ontology-71#Dolly">
        <rdfs:subClassOf rdf:resource="http://www.semanticweb.org/cadex/ontologies/2020/1/untitled-ontology-71#Equipment"/>
        <rdfs:comment>A camera dolly, which is a wheeled cart for moving the camera horizontally.</rdfs:comment>
    </owl:Class>
    


    <!-- http://www.semanticweb.org/cadex/ontologies/2020/1/untitled-ontology-71#EditProducer -->

    <owl:Class rdf:about="http://www.semanticweb.org/cadex/ontologies/2020/1/untitled-ontology-71#EditProducer">
        <rdfs:subClassOf rdf:resource="http://www.semanticweb.org/cadex/ontologies/2020/1/untitled-ontology-71#Staff"/>
        <rdfs:comment>An editorial producer who works for the company using the ontology.</rdfs:comment>
    </owl:Class>
    


    <!-- http://www.semanticweb.org/cadex/ontologies/2020/1/untitled-ontology-71#Email -->

    <owl:Class rdf:about="http://www.semanticweb.org/cadex/ontologies/2020/1/untitled-ontology-71#Email">
        <rdfs:subClassOf rdf:resource="http://www.semanticweb.org/cadex/ontologies/2020/1/untitled-ontology-71#TextAssets"/>
        <rdfs:comment>Any email communication, both internal and external, sent in relation to this project.</rdfs:comment>
    </owl:Class>
    


    <!-- http://www.semanticweb.org/cadex/ontologies/2020/1/untitled-ontology-71#EmailReceipt -->

    <owl:Class rdf:about="http://www.semanticweb.org/cadex/ontologies/2020/1/untitled-ontology-71#EmailReceipt">
        <rdfs:subClassOf rdf:resource="http://www.semanticweb.org/cadex/ontologies/2020/1/untitled-ontology-71#Email"/>
        <rdfs:comment>Any email communication, both internal and external, sent in relation to this project that acts as receipt (for example, to confirm the receipt of a drive).</rdfs:comment>
    </owl:Class>
    


    <!-- http://www.semanticweb.org/cadex/ontologies/2020/1/untitled-ontology-71#Equipment -->

    <owl:Class rdf:about="http://www.semanticweb.org/cadex/ontologies/2020/1/untitled-ontology-71#Equipment">
        <rdfs:subClassOf rdf:resource="http://www.semanticweb.org/cadex/ontologies/2020/1/untitled-ontology-71#DataItem"/>
        <rdfs:comment>Any physical equipment (e.g. a camera, etc.) used in a project.</rdfs:comment>
    </owl:Class>
    


    <!-- http://www.semanticweb.org/cadex/ontologies/2020/1/untitled-ontology-71#EquipmentAttachment -->

    <owl:Class rdf:about="http://www.semanticweb.org/cadex/ontologies/2020/1/untitled-ontology-71#EquipmentAttachment">
        <rdfs:subClassOf rdf:resource="http://www.semanticweb.org/cadex/ontologies/2020/1/untitled-ontology-71#DataItem"/>
        <rdfs:comment>Anything that can be attached to piece of equipment (e.g. a lens, etc.) used in a project.</rdfs:comment>
    </owl:Class>
    


    <!-- http://www.semanticweb.org/cadex/ontologies/2020/1/untitled-ontology-71#Event -->

    <owl:Class rdf:about="http://www.semanticweb.org/cadex/ontologies/2020/1/untitled-ontology-71#Event">
        <rdfs:subClassOf rdf:resource="http://www.semanticweb.org/cadex/ontologies/2020/1/untitled-ontology-71#DataItem"/>
        <rdfs:comment>Any action that requires metadata to be stored about.</rdfs:comment>
    </owl:Class>
    


    <!-- http://www.semanticweb.org/cadex/ontologies/2020/1/untitled-ontology-71#File -->

    <owl:Class rdf:about="http://www.semanticweb.org/cadex/ontologies/2020/1/untitled-ontology-71#File">
        <rdfs:subClassOf rdf:resource="http://www.semanticweb.org/cadex/ontologies/2020/1/untitled-ontology-71#DataItem"/>
        <rdfs:comment>A single file stored on the file system which can represent, for instance, a clip.</rdfs:comment>
    </owl:Class>
    


    <!-- http://www.semanticweb.org/cadex/ontologies/2020/1/untitled-ontology-71#FisheyeLens -->

    <owl:Class rdf:about="http://www.semanticweb.org/cadex/ontologies/2020/1/untitled-ontology-71#FisheyeLens">
        <rdfs:subClassOf rdf:resource="http://www.semanticweb.org/cadex/ontologies/2020/1/untitled-ontology-71#Lens"/>
        <rdfs:comment>A fisheye lens used on cameras.</rdfs:comment>
    </owl:Class>
    


    <!-- http://www.semanticweb.org/cadex/ontologies/2020/1/untitled-ontology-71#Folder -->

    <owl:Class rdf:about="http://www.semanticweb.org/cadex/ontologies/2020/1/untitled-ontology-71#Folder">
        <rdfs:subClassOf rdf:resource="http://www.semanticweb.org/cadex/ontologies/2020/1/untitled-ontology-71#DataItem"/>
        <rdfs:comment>A single directory stored in the file system which can represent, for instance, a roll.</rdfs:comment>
    </owl:Class>
    


    <!-- http://www.semanticweb.org/cadex/ontologies/2020/1/untitled-ontology-71#Frame -->

    <owl:Class rdf:about="http://www.semanticweb.org/cadex/ontologies/2020/1/untitled-ontology-71#Frame">
        <rdfs:subClassOf rdf:resource="http://www.semanticweb.org/cadex/ontologies/2020/1/untitled-ontology-71#MediaAssets"/>
        <rdfs:comment>A single frame that, when combined with others, form a clip.</rdfs:comment>
    </owl:Class>
    


    <!-- http://www.semanticweb.org/cadex/ontologies/2020/1/untitled-ontology-71#HardDriveSnapshot -->

    <owl:Class rdf:about="http://www.semanticweb.org/cadex/ontologies/2020/1/untitled-ontology-71#HardDriveSnapshot">
        <rdfs:subClassOf rdf:resource="http://www.semanticweb.org/cadex/ontologies/2020/1/untitled-ontology-71#TextAssets"/>
        <rdfs:comment>A file containing the structure and details of files and folders stored on a hard drive.</rdfs:comment>
    </owl:Class>
    


    <!-- http://www.semanticweb.org/cadex/ontologies/2020/1/untitled-ontology-71#Issue -->

    <owl:Class rdf:about="http://www.semanticweb.org/cadex/ontologies/2020/1/untitled-ontology-71#Issue">
        <rdfs:subClassOf rdf:resource="http://www.semanticweb.org/cadex/ontologies/2020/1/untitled-ontology-71#DataItem"/>
        <rdfs:comment>Stores details of an issue which can be associated with instances of other classes.</rdfs:comment>
    </owl:Class>
    


    <!-- http://www.semanticweb.org/cadex/ontologies/2020/1/untitled-ontology-71#LUT -->

    <owl:Class rdf:about="http://www.semanticweb.org/cadex/ontologies/2020/1/untitled-ontology-71#LUT">
        <rdfs:subClassOf rdf:resource="http://www.semanticweb.org/cadex/ontologies/2020/1/untitled-ontology-71#MediaAssets"/>
        <rdfs:comment>A lookup table which provide a pre-determined colour grading settings for a Clip.</rdfs:comment>
    </owl:Class>
    


    <!-- http://www.semanticweb.org/cadex/ontologies/2020/1/untitled-ontology-71#Lens -->

    <owl:Class rdf:about="http://www.semanticweb.org/cadex/ontologies/2020/1/untitled-ontology-71#Lens">
        <rdfs:subClassOf rdf:resource="http://www.semanticweb.org/cadex/ontologies/2020/1/untitled-ontology-71#EquipmentAttachment"/>
        <rdfs:comment>A lens used on cameras.</rdfs:comment>
    </owl:Class>
    


    <!-- http://www.semanticweb.org/cadex/ontologies/2020/1/untitled-ontology-71#LensGrid -->

    <owl:Class rdf:about="http://www.semanticweb.org/cadex/ontologies/2020/1/untitled-ontology-71#LensGrid">
        <rdfs:subClassOf rdf:resource="http://www.semanticweb.org/cadex/ontologies/2020/1/untitled-ontology-71#MediaAssets"/>
        <rdfs:comment>An image of the checkered grid placed in front of a camera lens to record the physical imperfections that are natural to all camera lenses.</rdfs:comment>
    </owl:Class>
    


    <!-- http://www.semanticweb.org/cadex/ontologies/2020/1/untitled-ontology-71#Location -->

    <owl:Class rdf:about="http://www.semanticweb.org/cadex/ontologies/2020/1/untitled-ontology-71#Location">
        <rdfs:subClassOf rdf:resource="http://www.semanticweb.org/cadex/ontologies/2020/1/untitled-ontology-71#DataItem"/>
        <rdfs:comment>Encapsulates metadata referring to any locations, including shoot locations.</rdfs:comment>
    </owl:Class>
    


    <!-- http://www.semanticweb.org/cadex/ontologies/2020/1/untitled-ontology-71#Logger -->

    <owl:Class rdf:about="http://www.semanticweb.org/cadex/ontologies/2020/1/untitled-ontology-71#Logger">
        <rdfs:subClassOf rdf:resource="http://www.semanticweb.org/cadex/ontologies/2020/1/untitled-ontology-71#Staff"/>
        <rdfs:comment>A member of the live logging team who works for the company using the ontology.</rdfs:comment>
    </owl:Class>
    


    <!-- http://www.semanticweb.org/cadex/ontologies/2020/1/untitled-ontology-71#LoggingTag -->

    <owl:Class rdf:about="http://www.semanticweb.org/cadex/ontologies/2020/1/untitled-ontology-71#LoggingTag">
        <rdfs:subClassOf rdf:resource="http://www.semanticweb.org/cadex/ontologies/2020/1/untitled-ontology-71#DataItem"/>
        <rdfs:comment>A descriptive tag that can be applied to a Clip by the live logging team to enable quick searching of clips.</rdfs:comment>
    </owl:Class>
    


    <!-- http://www.semanticweb.org/cadex/ontologies/2020/1/untitled-ontology-71#MediaAssets -->

    <owl:Class rdf:about="http://www.semanticweb.org/cadex/ontologies/2020/1/untitled-ontology-71#MediaAssets">
        <rdfs:subClassOf rdf:resource="http://www.semanticweb.org/cadex/ontologies/2020/1/untitled-ontology-71#Asset"/>
        <rdfs:comment>Any media-based assets.</rdfs:comment>
    </owl:Class>
    


    <!-- http://www.semanticweb.org/cadex/ontologies/2020/1/untitled-ontology-71#Microphone -->

    <owl:Class rdf:about="http://www.semanticweb.org/cadex/ontologies/2020/1/untitled-ontology-71#Microphone">
        <rdfs:subClassOf rdf:resource="http://www.semanticweb.org/cadex/ontologies/2020/1/untitled-ontology-71#EquipmentAttachment"/>
        <rdfs:comment>A microphone, which adds sound to a clip.</rdfs:comment>
    </owl:Class>
    


    <!-- http://www.semanticweb.org/cadex/ontologies/2020/1/untitled-ontology-71#Note -->

    <owl:Class rdf:about="http://www.semanticweb.org/cadex/ontologies/2020/1/untitled-ontology-71#Note">
        <rdfs:subClassOf rdf:resource="http://www.semanticweb.org/cadex/ontologies/2020/1/untitled-ontology-71#DataItem"/>
        <rdfs:comment>A comment that can be linked to other entities.</rdfs:comment>
    </owl:Class>
    


    <!-- http://www.semanticweb.org/cadex/ontologies/2020/1/untitled-ontology-71#Panoramic -->

    <owl:Class rdf:about="http://www.semanticweb.org/cadex/ontologies/2020/1/untitled-ontology-71#Panoramic">
        <rdfs:subClassOf rdf:resource="http://www.semanticweb.org/cadex/ontologies/2020/1/untitled-ontology-71#MediaAssets"/>
        <rdfs:comment>A panoramic photograph, i.e. a wide-format photo.</rdfs:comment>
    </owl:Class>
    


    <!-- http://www.semanticweb.org/cadex/ontologies/2020/1/untitled-ontology-71#Person -->

    <owl:Class rdf:about="http://www.semanticweb.org/cadex/ontologies/2020/1/untitled-ontology-71#Person">
        <rdfs:subClassOf rdf:resource="http://www.semanticweb.org/cadex/ontologies/2020/1/untitled-ontology-71#DataItem"/>
        <rdfs:comment>Any human entity that requires representation in the ontology.</rdfs:comment>
    </owl:Class>
    


    <!-- http://www.semanticweb.org/cadex/ontologies/2020/1/untitled-ontology-71#Photogrammetry -->

    <owl:Class rdf:about="http://www.semanticweb.org/cadex/ontologies/2020/1/untitled-ontology-71#Photogrammetry">
        <rdfs:subClassOf rdf:resource="http://www.semanticweb.org/cadex/ontologies/2020/1/untitled-ontology-71#MediaAssets"/>
        <rdfs:comment>Photographs used to make a map, drawing or 3D model of a real-world object or scene.</rdfs:comment>
    </owl:Class>
    


    <!-- http://www.semanticweb.org/cadex/ontologies/2020/1/untitled-ontology-71#Project -->

    <owl:Class rdf:about="http://www.semanticweb.org/cadex/ontologies/2020/1/untitled-ontology-71#Project">
        <rdfs:subClassOf rdf:resource="http://www.semanticweb.org/cadex/ontologies/2020/1/untitled-ontology-71#DataItem"/>
        <rdfs:comment>Represents a single project (e.g. a production).</rdfs:comment>
    </owl:Class>
    


    <!-- http://www.semanticweb.org/cadex/ontologies/2020/1/untitled-ontology-71#Prop -->

    <owl:Class rdf:about="http://www.semanticweb.org/cadex/ontologies/2020/1/untitled-ontology-71#Prop">
        <rdfs:subClassOf rdf:resource="http://www.semanticweb.org/cadex/ontologies/2020/1/untitled-ontology-71#Equipment"/>
        <rdfs:comment>An item used by a cast member when being filmed to make the scene more realistic.</rdfs:comment>
    </owl:Class>
    


    <!-- http://www.semanticweb.org/cadex/ontologies/2020/1/untitled-ontology-71#Record -->

    <owl:Class rdf:about="http://www.semanticweb.org/cadex/ontologies/2020/1/untitled-ontology-71#Record">
        <rdfs:comment>Encapsulates versioning metadata, including temporal details, about an entity.</rdfs:comment>
    </owl:Class>
    


    <!-- http://www.semanticweb.org/cadex/ontologies/2020/1/untitled-ontology-71#RectilinearLens -->

    <owl:Class rdf:about="http://www.semanticweb.org/cadex/ontologies/2020/1/untitled-ontology-71#RectilinearLens">
        <rdfs:subClassOf rdf:resource="http://www.semanticweb.org/cadex/ontologies/2020/1/untitled-ontology-71#Lens"/>
        <rdfs:comment>A rectilinear lens used on cameras.</rdfs:comment>
    </owl:Class>
    


    <!-- http://www.semanticweb.org/cadex/ontologies/2020/1/untitled-ontology-71#ReferenceMaterial -->

    <owl:Class rdf:about="http://www.semanticweb.org/cadex/ontologies/2020/1/untitled-ontology-71#ReferenceMaterial">
        <rdfs:subClassOf rdf:resource="http://www.semanticweb.org/cadex/ontologies/2020/1/untitled-ontology-71#TextAssets"/>
        <rdfs:comment>Reference material typically about texture, surface and colour (e.g. Macbeth colour charts).</rdfs:comment>
    </owl:Class>
    


    <!-- http://www.semanticweb.org/cadex/ontologies/2020/1/untitled-ontology-71#Rental -->

    <owl:Class rdf:about="http://www.semanticweb.org/cadex/ontologies/2020/1/untitled-ontology-71#Rental">
        <rdfs:subClassOf rdf:resource="http://www.semanticweb.org/cadex/ontologies/2020/1/untitled-ontology-71#DataItem"/>
        <rdfs:comment>Encapsulates the information regarding the rental of equipment for the purposes of a shoot.</rdfs:comment>
    </owl:Class>
    


    <!-- http://www.semanticweb.org/cadex/ontologies/2020/1/untitled-ontology-71#Rig -->

    <owl:Class rdf:about="http://www.semanticweb.org/cadex/ontologies/2020/1/untitled-ontology-71#Rig">
        <rdfs:subClassOf rdf:resource="http://www.semanticweb.org/cadex/ontologies/2020/1/untitled-ontology-71#Equipment"/>
        <rdfs:comment>A large setup of multiple cameras.</rdfs:comment>
    </owl:Class>
    


    <!-- http://www.semanticweb.org/cadex/ontologies/2020/1/untitled-ontology-71#Role -->

    <owl:Class rdf:about="http://www.semanticweb.org/cadex/ontologies/2020/1/untitled-ontology-71#Role">
        <rdfs:subClassOf rdf:resource="http://www.semanticweb.org/cadex/ontologies/2020/1/untitled-ontology-71#DataItem"/>
        <rdfs:comment>Represents a real-world role that a Person entity can have in a project. This class encapsulates the specific roles in the form of its subclasses.</rdfs:comment>
    </owl:Class>
    


    <!-- http://www.semanticweb.org/cadex/ontologies/2020/1/untitled-ontology-71#Roll -->

    <owl:Class rdf:about="http://www.semanticweb.org/cadex/ontologies/2020/1/untitled-ontology-71#Roll">
        <rdfs:subClassOf rdf:resource="http://www.semanticweb.org/cadex/ontologies/2020/1/untitled-ontology-71#DataItem"/>
        <rdfs:comment>This is the output of a camera after a take. The terminology refers to a pre-digital time period.</rdfs:comment>
    </owl:Class>
    


    <!-- http://www.semanticweb.org/cadex/ontologies/2020/1/untitled-ontology-71#Scene -->

    <owl:Class rdf:about="http://www.semanticweb.org/cadex/ontologies/2020/1/untitled-ontology-71#Scene">
        <rdfs:subClassOf rdf:resource="http://www.semanticweb.org/cadex/ontologies/2020/1/untitled-ontology-71#Event"/>
        <rdfs:comment>The action in a single location and continuous time.</rdfs:comment>
    </owl:Class>
    


    <!-- http://www.semanticweb.org/cadex/ontologies/2020/1/untitled-ontology-71#Script -->

    <owl:Class rdf:about="http://www.semanticweb.org/cadex/ontologies/2020/1/untitled-ontology-71#Script">
        <rdfs:subClassOf rdf:resource="http://www.semanticweb.org/cadex/ontologies/2020/1/untitled-ontology-71#TextAssets"/>
        <rdfs:comment>Represents the physical script which is performed by actors in a production.</rdfs:comment>
    </owl:Class>
    


    <!-- http://www.semanticweb.org/cadex/ontologies/2020/1/untitled-ontology-71#ScriptBreakdown -->

    <owl:Class rdf:about="http://www.semanticweb.org/cadex/ontologies/2020/1/untitled-ontology-71#ScriptBreakdown">
        <rdfs:subClassOf rdf:resource="http://www.semanticweb.org/cadex/ontologies/2020/1/untitled-ontology-71#TextAssets"/>
        <rdfs:comment>Represents a breakdown of the physical script which is performed by actors in a production.</rdfs:comment>
    </owl:Class>
    


    <!-- http://www.semanticweb.org/cadex/ontologies/2020/1/untitled-ontology-71#Shoot -->

    <owl:Class rdf:about="http://www.semanticweb.org/cadex/ontologies/2020/1/untitled-ontology-71#Shoot">
        <rdfs:subClassOf rdf:resource="http://www.semanticweb.org/cadex/ontologies/2020/1/untitled-ontology-71#Event"/>
        <rdfs:comment>Refers to the entire event of producing raw, unedited content.</rdfs:comment>
    </owl:Class>
    


    <!-- http://www.semanticweb.org/cadex/ontologies/2020/1/untitled-ontology-71#ShootDay -->

    <owl:Class rdf:about="http://www.semanticweb.org/cadex/ontologies/2020/1/untitled-ontology-71#ShootDay">
        <rdfs:subClassOf rdf:resource="http://www.semanticweb.org/cadex/ontologies/2020/1/untitled-ontology-71#Event"/>
        <rdfs:comment>Refers to a single day of a shoot.</rdfs:comment>
    </owl:Class>
    


    <!-- http://www.semanticweb.org/cadex/ontologies/2020/1/untitled-ontology-71#ShootingSchedule -->

    <owl:Class rdf:about="http://www.semanticweb.org/cadex/ontologies/2020/1/untitled-ontology-71#ShootingSchedule">
        <rdfs:subClassOf rdf:resource="http://www.semanticweb.org/cadex/ontologies/2020/1/untitled-ontology-71#TextAssets"/>
        <rdfs:comment>Represents a timetable of shoots.</rdfs:comment>
    </owl:Class>
    


    <!-- http://www.semanticweb.org/cadex/ontologies/2020/1/untitled-ontology-71#Shot -->

    <owl:Class rdf:about="http://www.semanticweb.org/cadex/ontologies/2020/1/untitled-ontology-71#Shot">
        <rdfs:subClassOf rdf:resource="http://www.semanticweb.org/cadex/ontologies/2020/1/untitled-ontology-71#DataItem"/>
        <rdfs:comment>The event of shooting one scene. A scene is made up of multiple shots from multiple cameras.</rdfs:comment>
    </owl:Class>
    


    <!-- http://www.semanticweb.org/cadex/ontologies/2020/1/untitled-ontology-71#Slate -->

    <owl:Class rdf:about="http://www.semanticweb.org/cadex/ontologies/2020/1/untitled-ontology-71#Slate">
        <rdfs:subClassOf rdf:resource="http://www.semanticweb.org/cadex/ontologies/2020/1/untitled-ontology-71#DataItem"/>
        <rdfs:comment>The clapperboard used to assist in synchronizing of picture and sound.</rdfs:comment>
    </owl:Class>
    


    <!-- http://www.semanticweb.org/cadex/ontologies/2020/1/untitled-ontology-71#SoundRoll -->

    <owl:Class rdf:about="http://www.semanticweb.org/cadex/ontologies/2020/1/untitled-ontology-71#SoundRoll">
        <rdfs:subClassOf rdf:resource="http://www.semanticweb.org/cadex/ontologies/2020/1/untitled-ontology-71#Roll"/>
        <rdfs:comment>This is the audio output of a camera after a take.</rdfs:comment>
    </owl:Class>
    


    <!-- http://www.semanticweb.org/cadex/ontologies/2020/1/untitled-ontology-71#Staff -->

    <owl:Class rdf:about="http://www.semanticweb.org/cadex/ontologies/2020/1/untitled-ontology-71#Staff">
        <rdfs:subClassOf rdf:resource="http://www.semanticweb.org/cadex/ontologies/2020/1/untitled-ontology-71#Role"/>
        <rdfs:comment>Anyone who works for the company using the ontology.</rdfs:comment>
    </owl:Class>
    


    <!-- http://www.semanticweb.org/cadex/ontologies/2020/1/untitled-ontology-71#StereoLeftEyeLens -->

    <owl:Class rdf:about="http://www.semanticweb.org/cadex/ontologies/2020/1/untitled-ontology-71#StereoLeftEyeLens">
        <rdfs:subClassOf rdf:resource="http://www.semanticweb.org/cadex/ontologies/2020/1/untitled-ontology-71#Lens"/>
        <rdfs:comment>A stereo left eye lens used on cameras.</rdfs:comment>
    </owl:Class>
    


    <!-- http://www.semanticweb.org/cadex/ontologies/2020/1/untitled-ontology-71#StereoRightEyeLens -->

    <owl:Class rdf:about="http://www.semanticweb.org/cadex/ontologies/2020/1/untitled-ontology-71#StereoRightEyeLens">
        <rdfs:subClassOf rdf:resource="http://www.semanticweb.org/cadex/ontologies/2020/1/untitled-ontology-71#Lens"/>
        <rdfs:comment>A stereo right eye lens used on cameras.</rdfs:comment>
    </owl:Class>
    


    <!-- http://www.semanticweb.org/cadex/ontologies/2020/1/untitled-ontology-71#Still -->

    <owl:Class rdf:about="http://www.semanticweb.org/cadex/ontologies/2020/1/untitled-ontology-71#Still">
        <rdfs:subClassOf rdf:resource="http://www.semanticweb.org/cadex/ontologies/2020/1/untitled-ontology-71#MediaAssets"/>
        <rdfs:comment>A still image.</rdfs:comment>
    </owl:Class>
    


    <!-- http://www.semanticweb.org/cadex/ontologies/2020/1/untitled-ontology-71#Storyboard -->

    <owl:Class rdf:about="http://www.semanticweb.org/cadex/ontologies/2020/1/untitled-ontology-71#Storyboard">
        <rdfs:subClassOf rdf:resource="http://www.semanticweb.org/cadex/ontologies/2020/1/untitled-ontology-71#TextAssets"/>
        <rdfs:comment>Represents a visual representation of a script.</rdfs:comment>
    </owl:Class>
    


    <!-- http://www.semanticweb.org/cadex/ontologies/2020/1/untitled-ontology-71#Take -->

    <owl:Class rdf:about="http://www.semanticweb.org/cadex/ontologies/2020/1/untitled-ontology-71#Take">
        <rdfs:subClassOf rdf:resource="http://www.semanticweb.org/cadex/ontologies/2020/1/untitled-ontology-71#Event"/>
        <rdfs:comment>A single version of a shot.</rdfs:comment>
    </owl:Class>
    


    <!-- http://www.semanticweb.org/cadex/ontologies/2020/1/untitled-ontology-71#Task -->

    <owl:Class rdf:about="http://www.semanticweb.org/cadex/ontologies/2020/1/untitled-ontology-71#Task">
        <rdfs:subClassOf rdf:resource="http://www.semanticweb.org/cadex/ontologies/2020/1/untitled-ontology-71#DataItem"/>
        <rdfs:comment>Stores details of a task which can be associated with instances of other classes.</rdfs:comment>
    </owl:Class>
    


    <!-- http://www.semanticweb.org/cadex/ontologies/2020/1/untitled-ontology-71#TextAssets -->

    <owl:Class rdf:about="http://www.semanticweb.org/cadex/ontologies/2020/1/untitled-ontology-71#TextAssets">
        <rdfs:subClassOf rdf:resource="http://www.semanticweb.org/cadex/ontologies/2020/1/untitled-ontology-71#Asset"/>
        <rdfs:comment>Any text-based assets.</rdfs:comment>
    </owl:Class>
    


    <!-- http://www.semanticweb.org/cadex/ontologies/2020/1/untitled-ontology-71#Unit -->

    <owl:Class rdf:about="http://www.semanticweb.org/cadex/ontologies/2020/1/untitled-ontology-71#Unit">
        <rdfs:subClassOf rdf:resource="http://www.semanticweb.org/cadex/ontologies/2020/1/untitled-ontology-71#DataItem"/>
        <rdfs:comment>A shoot unit, which is the crew working at a particular shoot location.</rdfs:comment>
    </owl:Class>
    


    <!-- http://www.semanticweb.org/cadex/ontologies/2020/1/untitled-ontology-71#VideoEditor -->

    <owl:Class rdf:about="http://www.semanticweb.org/cadex/ontologies/2020/1/untitled-ontology-71#VideoEditor">
        <rdfs:subClassOf rdf:resource="http://www.semanticweb.org/cadex/ontologies/2020/1/untitled-ontology-71#Staff"/>
        <rdfs:comment>A video editor who works for the company using the ontology.</rdfs:comment>
    </owl:Class>
    


    <!-- http://www.semanticweb.org/cadex/ontologies/2020/1/untitled-ontology-71#Writer -->

    <owl:Class rdf:about="http://www.semanticweb.org/cadex/ontologies/2020/1/untitled-ontology-71#Writer">
        <rdfs:subClassOf rdf:resource="http://www.semanticweb.org/cadex/ontologies/2020/1/untitled-ontology-71#Role"/>
        <rdfs:comment>A person responsible for writing something (e.g. a script).</rdfs:comment>
    </owl:Class>
    


    <!-- http://www.semanticweb.org/cadex/ontologies/2020/1/untitled-ontology-71#WrittenNote -->

    <owl:Class rdf:about="http://www.semanticweb.org/cadex/ontologies/2020/1/untitled-ontology-71#WrittenNote">
        <rdfs:subClassOf rdf:resource="http://www.semanticweb.org/cadex/ontologies/2020/1/untitled-ontology-71#TextAssets"/>
        <rdfs:comment>A handwritten set of notes that has been scanned and saved on to the file system.</rdfs:comment>
    </owl:Class>
    


    <!-- http://www.semanticweb.org/cadex/ontologies/2020/1/untitled-ontology-71#3DLidarScan -->

    <owl:Class rdf:about="http://www.semanticweb.org/cadex/ontologies/2020/1/untitled-ontology-71#3DLidarScan">
        <rdfs:subClassOf rdf:resource="http://www.semanticweb.org/cadex/ontologies/2020/1/untitled-ontology-71#MediaAssets"/>
        <rdfs:comment>The output of a LIDAR (remote sensing technology) scan, which is then used to create 3D models and maps of objects and scenes.</rdfs:comment>
    </owl:Class>
    


    <!-- http://www.semanticweb.org/cadex/ontologies/2020/1/untitled-ontology-71#3DModel -->

    <owl:Class rdf:about="http://www.semanticweb.org/cadex/ontologies/2020/1/untitled-ontology-71#3DModel">
        <rdfs:subClassOf rdf:resource="http://www.semanticweb.org/cadex/ontologies/2020/1/untitled-ontology-71#MediaAssets"/>
        <rdfs:comment>A computer-generated representation of an object or character in 3D.</rdfs:comment>
    </owl:Class>
    


    <!-- 
    ///////////////////////////////////////////////////////////////////////////////////////
    //
    // Annotations
    //
    ///////////////////////////////////////////////////////////////////////////////////////
     -->

    <rdf:Description rdf:about="http://www.w3.org/2002/07/owl#Thing">
        <rdfs:comment>Every user-defined class is implicitly a subclass of owl:Thing in an OWL ontology.</rdfs:comment>
    </rdf:Description>
    <rdf:Description rdf:about="http://www.w3.org/2002/07/owl#topObjectProperty">
        <rdfs:comment>Every user-defined object property is implicitly a sub-property of owl: topObjectProperty in an OWL ontology.</rdfs:comment>
    </rdf:Description>
</rdf:RDF>



<!-- Generated by the OWL API (version 4.5.9.2019-02-01T07:24:44Z) https://github.com/owlcs/owlapi -->

